@prefix : <https://www.commoncoreontologies.org/ArtifactOntology#> .
@prefix obo: <http://purl.obolibrary.org/obo/> .
@prefix owl: <http://www.w3.org/2002/07/owl#> .
@prefix rdf: <http://www.w3.org/1999/02/22-rdf-syntax-ns#> .
@prefix xml: <http://www.w3.org/XML/1998/namespace> .
@prefix xsd: <http://www.w3.org/2001/XMLSchema#> .
@prefix cco: <https://www.commoncoreontologies.org/> .
@prefix rdfs: <http://www.w3.org/2000/01/rdf-schema#> .
@prefix skos: <http://www.w3.org/2004/02/skos/core#> .
@prefix dcterms: <http://purl.org/dc/terms/> .
@base <https://www.commoncoreontologies.org/ArtifactOntology> .

<https://www.commoncoreontologies.org/ArtifactOntology> rdf:type owl:Ontology ;
                                                                               owl:versionIRI <https://www.commoncoreontologies.org/2024-11-06/ArtifactOntology> ;
                                                                               owl:imports <https://www.commoncoreontologies.org/InformationEntityOntology> ;
                                                                               dcterms:license "BSD 3-Clause: https://github.com/CommonCoreOntology/CommonCoreOntologies/blob/master/LICENSE"@en ;
                                                                               dcterms:rights "CUBRC Inc., see full license."@en ;
                                                                               rdfs:comment "This ontology is designed to represent artifacts that are common to multiple domains along with their models, specifications, and functions."@en ;
                                                                               rdfs:label "Artifact Ontology"@en ;
                                                                               owl:versionInfo "Version 2.0"@en .

#################################################################
#    Annotation properties
#################################################################

###  http://purl.org/dc/terms/rights
dcterms:rights rdf:type owl:AnnotationProperty .


###  https://www.commoncoreontologies.org/ont00001753
cco:ont00001753 rdf:type owl:AnnotationProperty .


###  https://www.commoncoreontologies.org/ont00001754
cco:ont00001754 rdf:type owl:AnnotationProperty .


###  https://www.commoncoreontologies.org/ont00001760
cco:ont00001760 rdf:type owl:AnnotationProperty .


#################################################################
#    Object Properties
#################################################################

###  https://www.commoncoreontologies.org/ont00001855
cco:ont00001855 rdf:type owl:ObjectProperty .


###  https://www.commoncoreontologies.org/ont00001916
cco:ont00001916 rdf:type owl:ObjectProperty .


###  https://www.commoncoreontologies.org/ont00001942
cco:ont00001942 rdf:type owl:ObjectProperty .


###  https://www.commoncoreontologies.org/ont00001944
cco:ont00001944 rdf:type owl:ObjectProperty .


#################################################################
#    Classes
#################################################################

###  https://www.commoncoreontologies.org/ont00000001
cco:ont00000001 rdf:type owl:Class ;
                 rdfs:subClassOf cco:ont00000804 ;
                 rdfs:label "Deflecting Prism"@en ;
                 skos:definition "A Prism designed to deflect a beam of light entering the Prism by a fixed angle."@en ;
                 cco:ont00001760 "https://www.commoncoreontologies.org/ArtifactOntology"^^xsd:anyURI .


###  https://www.commoncoreontologies.org/ont00000002
cco:ont00000002 rdf:type owl:Class ;
                 rdfs:subClassOf cco:ont00000323 ;
                 rdfs:label "Cooling Artifact Function"@en ;
                 skos:definition "An Artifact Function that is realized in a process in which the thermal energy of a system decreases."@en ;
                 cco:ont00001760 "https://www.commoncoreontologies.org/ArtifactOntology"^^xsd:anyURI .


###  https://www.commoncoreontologies.org/ont00000012
cco:ont00000012 rdf:type owl:Class ;
                 rdfs:subClassOf cco:ont00000781 ;
                 rdfs:label "Propulsion Control System"@en ;
                 skos:definition "A Control System that consists of control devices, displays, indicators, or modules designed to control a Propulsion System."@en ;
                 cco:ont00001760 "https://www.commoncoreontologies.org/ArtifactOntology"^^xsd:anyURI .


###  https://www.commoncoreontologies.org/ont00000014
cco:ont00000014 rdf:type owl:Class ;
                 rdfs:subClassOf cco:ont00000241 ;
                 rdfs:label "Aztec Code"@en ;
                 skos:definition "A Two-Dimensional Barcode that is used by the transportation industry to scan tickets."@en ;
                 cco:ont00001760 "https://www.commoncoreontologies.org/ArtifactOntology"^^xsd:anyURI .


###  https://www.commoncoreontologies.org/ont00000015
cco:ont00000015 rdf:type owl:Class ;
                 rdfs:subClassOf cco:ont00001104 ;
                 rdfs:label "Shotgun"@en ;
                 skos:definition "A Long Gun that fires packets of shot, a single slug, a sabot, or a specialty round (such as tear gas, bolo shell, or a breaching round) over shorter ranges than that of Rifles and with less accuracy."@en ;
                 cco:ont00001754 "https://en.wikipedia.org/w/index.php?title=Shotgun&oldid=1062571691"^^xsd:anyURI ;
                 cco:ont00001760 "https://www.commoncoreontologies.org/ArtifactOntology"^^xsd:anyURI .


###  https://www.commoncoreontologies.org/ont00000018
cco:ont00000018 rdf:type owl:Class ;
                 rdfs:subClassOf cco:ont00001346 ;
                 rdfs:label "Title Document"@en ;
                 skos:definition "A Legal Instrument that is designed as evidence of ownership."@en ;
                 cco:ont00001754 "https://en.wikipedia.org/wiki/Title_(property)" ;
                 cco:ont00001760 "https://www.commoncoreontologies.org/ArtifactOntology"^^xsd:anyURI .


###  https://www.commoncoreontologies.org/ont00000019
cco:ont00000019 rdf:type owl:Class ;
                 rdfs:subClassOf cco:ont00000961 ;
                 rdfs:label "Power Inverting Artifact Function"@en ;
                 skos:definition "A Current Conversion Artifact Function that is realized by processes in which some Artifact is used to convert direct current (DC) to alternating current (AC)."@en ;
                 cco:ont00001760 "https://www.commoncoreontologies.org/ArtifactOntology"^^xsd:anyURI .


###  https://www.commoncoreontologies.org/ont00000020
cco:ont00000020 rdf:type owl:Class ;
                 rdfs:subClassOf cco:ont00000995 ;
                 rdfs:label "Container"@en ;
                 skos:definition "A Material Artifact that is designed to contain (wholly or partially) some material entity."@en ;
                 cco:ont00001760 "https://www.commoncoreontologies.org/ArtifactOntology"^^xsd:anyURI .


###  https://www.commoncoreontologies.org/ont00000021
cco:ont00000021 rdf:type owl:Class ;
                 rdfs:subClassOf cco:ont00000995 ;
                 rdfs:label "Sensor Platform"@en ;
                 skos:definition "A Material Artifact that is designed to support, and in some cases transport, a Sensor during its deployment and functioning."@en ;
                 cco:ont00001760 "https://www.commoncoreontologies.org/ArtifactOntology"^^xsd:anyURI .


###  https://www.commoncoreontologies.org/ont00000022
cco:ont00000022 rdf:type owl:Class ;
                 rdfs:subClassOf cco:ont00000422 ;
                 rdfs:label "Radio Communication Reception Artifact Function"@en ;
                 skos:definition "A Communication Reception Artifact Function that is realized during events in which an Artifact receives information transmitted from another Artifact, where the transmission of information occurs using radio waves."@en ;
                 cco:ont00001760 "https://www.commoncoreontologies.org/ArtifactOntology"^^xsd:anyURI .


###  https://www.commoncoreontologies.org/ont00000023
cco:ont00000023 rdf:type owl:Class ;
                 rdfs:subClassOf cco:ont00000323 ;
                 rdfs:label "Sensor Deployment Artifact Function"@en ;
                 skos:definition "An Artifact Function that inheres in Artifacts that are designed to support or convey one or more Sensors while the Sensors are realizing their own Artifact Functions."@en ;
                 cco:ont00001760 "https://www.commoncoreontologies.org/ArtifactOntology"^^xsd:anyURI .


###  https://www.commoncoreontologies.org/ont00000025
cco:ont00000025 rdf:type owl:Class ;
                 rdfs:subClassOf cco:ont00001278 ;
                 rdfs:label "Electronic Stock"@en ;
                 skos:definition "Stock that consists of Bytes."@en ;
                 cco:ont00001760 "https://www.commoncoreontologies.org/ArtifactOntology"^^xsd:anyURI .


###  https://www.commoncoreontologies.org/ont00000028
cco:ont00000028 rdf:type owl:Class ;
                 rdfs:subClassOf cco:ont00000804 ;
                 rdfs:label "Dispersive Prism"@en ;
                 skos:definition "A Prism designed to break up a beam of light entering the Prism into its constituent spectral colors by leveraging the refractive index of light based on its Frequency."@en ;
                 cco:ont00001760 "https://www.commoncoreontologies.org/ArtifactOntology"^^xsd:anyURI .


###  https://www.commoncoreontologies.org/ont00000030
cco:ont00000030 rdf:type owl:Class ;
                 rdfs:subClassOf cco:ont00000288 ;
                 rdfs:label "Nuclear Reactor"@en ;
                 skos:definition "A Power Source that is designed to initiate and control a self-sustained nuclear chain reaction to produce power in the form of heat, which can be transferred to a working fluid for further conversion to mechanical or electrical energy."@en ;
                 cco:ont00001754 "https://en.wikipedia.org/w/index.php?title=Nuclear_reactor&oldid=1063370273"^^xsd:anyURI ;
                 cco:ont00001760 "https://www.commoncoreontologies.org/ArtifactOntology"^^xsd:anyURI .


###  https://www.commoncoreontologies.org/ont00000034
cco:ont00000034 rdf:type owl:Class ;
                 rdfs:subClassOf cco:ont00000448 ;
                 rdfs:label "Conveyance Artifact Function"@en ;
                 skos:definition "A Motion Artifact Function that is realized in a process in which the bearer of the function conveys entities from one location to another."@en ;
                 cco:ont00001754 "https://en.wikipedia.org/w/index.php?title=Vehicle&oldid=1063682179"^^xsd:anyURI ;
                 cco:ont00001760 "https://www.commoncoreontologies.org/ArtifactOntology"^^xsd:anyURI .


###  https://www.commoncoreontologies.org/ont00000036
cco:ont00000036 rdf:type owl:Class ;
                 rdfs:subClassOf cco:ont00001301 ;
                 rdfs:label "Waste Management Artifact Function"@en ;
                 skos:definition "A Service Artifact Function that is realized in processes of collecting transporting processing recycling or disposing and monitoring of waste materials."@en ;
                 cco:ont00001754 "https://en.wikipedia.org/w/index.php?title=Waste_management&oldid=1062844209"^^xsd:anyURI ;
                 cco:ont00001760 "https://www.commoncoreontologies.org/ArtifactOntology"^^xsd:anyURI .


###  https://www.commoncoreontologies.org/ont00000038
cco:ont00000038 rdf:type owl:Class ;
                 rdfs:subClassOf obo:BFO_0000023 ;
                 rdfs:label "System Role"@en ;
                 skos:definition "A Role that inheres in an entity in virtue of its parts or elements being arranged in such a way that they together exhibit behavior or meaning that they do not exhibit individually."@en ;
                 cco:ont00001754 "https://www.incose.org/about-systems-engineering/system-and-se-definition/general-system-definition"^^xsd:anyURI ;
                 cco:ont00001760 "https://www.commoncoreontologies.org/ArtifactOntology"^^xsd:anyURI .


###  https://www.commoncoreontologies.org/ont00000039
cco:ont00000039 rdf:type owl:Class ;
                 rdfs:subClassOf cco:ont00000838 ;
                 rdfs:label "Portion of Solid Fuel"@en ;
                 skos:definition "A Portion of Fuel that is stored in a solid state."@en ;
                 cco:ont00001760 "https://www.commoncoreontologies.org/ArtifactOntology"^^xsd:anyURI .


###  https://www.commoncoreontologies.org/ont00000043
cco:ont00000043 rdf:type owl:Class ;
                 rdfs:subClassOf cco:ont00000593 ;
                 rdfs:label "Portion of Solid Propellant"@en ;
                 skos:definition "A Portion of Propellant that is stored in a solid state."@en ;
                 cco:ont00001760 "https://www.commoncoreontologies.org/ArtifactOntology"^^xsd:anyURI .


###  https://www.commoncoreontologies.org/ont00000047
cco:ont00000047 rdf:type owl:Class ;
                 rdfs:subClassOf cco:ont00000598 ;
                 rdfs:comment "Flow Control Valves are often more complex than a simple Valve and typically include an Actuator that is capable of automatically adjusting the state of the valve in response to signals from a connected Sensor or Controller."@en ;
                 rdfs:label "Flow Control Valve"@en ;
                 skos:definition "A Valve that is designed to regulate the flow or Pressure of a fluid."@en ;
                 cco:ont00001754 "https://en.wikipedia.org/w/index.php?title=Flow_control_valve&oldid=1013438085"^^xsd:anyURI ;
                 cco:ont00001760 "https://www.commoncoreontologies.org/ArtifactOntology"^^xsd:anyURI .


###  https://www.commoncoreontologies.org/ont00000048
cco:ont00000048 rdf:type owl:Class ;
                 rdfs:subClassOf cco:ont00000499 ;
                 rdfs:label "Random Wire Antenna"@en ;
                 skos:definition "A Wire Antenna that consists of a long wire suspended above the ground with a length that does not bear a relation to the wavelength of the radio waves used and which is typically used as a receiving antenna on the long, medium, and short wave bands."@en ;
                 cco:ont00001754 "https://en.wikipedia.org/w/index.php?title=Random_wire_antenna&oldid=1058546356"^^xsd:anyURI ;
                 cco:ont00001760 "https://www.commoncoreontologies.org/ArtifactOntology"^^xsd:anyURI .


###  https://www.commoncoreontologies.org/ont00000049
cco:ont00000049 rdf:type owl:Class ;
                 rdfs:subClassOf cco:ont00000475 ;
                 rdfs:label "Banknote"@en ;
                 skos:definition "A Portion of Cash that consists of a portable slips of paper or fabric designed to bear some specified Financial Value."@en ;
                 cco:ont00001760 "https://www.commoncoreontologies.org/ArtifactOntology"^^xsd:anyURI .


###  https://www.commoncoreontologies.org/ont00000050
cco:ont00000050 rdf:type owl:Class ;
                 rdfs:subClassOf cco:ont00000903 ;
                 rdfs:label "Very High Frequency Communication Instrument"@en ;
                 skos:definition "A Radio Communication Instrument that is designed to participate in some process that has process part some Very High Frequency."@en ;
                 cco:ont00001760 "https://www.commoncoreontologies.org/ArtifactOntology"^^xsd:anyURI .


###  https://www.commoncoreontologies.org/ont00000053
cco:ont00000053 rdf:type owl:Class ;
                 rdfs:subClassOf cco:ont00000618 ;
                 rdfs:label "Ground Motor Vehicle"@en ;
                 skos:definition "A Ground Vehicle that is designed to receive its motive power from an Engine and is not designed to travel on rails."@en ;
                 cco:ont00001754 "https://en.wikipedia.org/w/index.php?title=Motor_vehicle&oldid=1063627395"^^xsd:anyURI ;
                 cco:ont00001760 "https://www.commoncoreontologies.org/ArtifactOntology"^^xsd:anyURI .


###  https://www.commoncoreontologies.org/ont00000054
cco:ont00000054 rdf:type owl:Class ;
                 rdfs:subClassOf cco:ont00000431 ;
                 rdfs:label "Stirling Engine"@en ;
                 skos:definition "An External Combusion Engine that is designed to compress and expand some working fluid at different temperatures, such that there is a net conversion of heat energy to mechanical work."@en ;
                 cco:ont00001754 "https://en.wikipedia.org/w/index.php?title=Stirling_engine&oldid=1061164490"^^xsd:anyURI ;
                 cco:ont00001760 "https://www.commoncoreontologies.org/ArtifactOntology"^^xsd:anyURI .


###  https://www.commoncoreontologies.org/ont00000056
cco:ont00000056 rdf:type owl:Class ;
                 rdfs:subClassOf cco:ont00000210 ;
                 rdfs:label "Reaction Engine"@en ;
                 skos:altLabel "Reaction Motor"@en ;
                 skos:definition "An Engine that provides propulsion by expelling Reaction Mass."@en ;
                 cco:ont00001754 "https://en.wikipedia.org/w/index.php?title=Reaction_engine&oldid=1046981784"^^xsd:anyURI ;
                 cco:ont00001760 "https://www.commoncoreontologies.org/ArtifactOntology"^^xsd:anyURI .


###  https://www.commoncoreontologies.org/ont00000057
cco:ont00000057 rdf:type owl:Class ;
                 rdfs:subClassOf cco:ont00000907 ;
                 rdfs:label "Mobile Telephone"@en ;
                 skos:definition "A Telephone that is connected to a Telephone Network by radio waves."@en ;
                 cco:ont00001754 "https://en.wikipedia.org/w/index.php?title=Mobile_phone&oldid=1061800841"^^xsd:anyURI ;
                 cco:ont00001760 "https://www.commoncoreontologies.org/ArtifactOntology"^^xsd:anyURI .


###  https://www.commoncoreontologies.org/ont00000059
cco:ont00000059 rdf:type owl:Class ;
                 rdfs:subClassOf cco:ont00000825 ;
                 rdfs:label "Telephone Line"@en ;
                 skos:altLabel "Telephone Circuit"@en ;
                 skos:definition "A Telecommunication Network Line that consists of a physical wire or other signaling medium that is designed to be part of a Telephone Network."@en ;
                 cco:ont00001754 "https://en.wikipedia.org/w/index.php?title=Telephone_line&oldid=1063429738"^^xsd:anyURI ;
                 cco:ont00001760 "https://www.commoncoreontologies.org/ArtifactOntology"^^xsd:anyURI .


###  https://www.commoncoreontologies.org/ont00000062
cco:ont00000062 rdf:type owl:Class ;
                 rdfs:subClassOf cco:ont00001100 ;
                 rdfs:label "Frequency Measurement Artifact Function"@en ;
                 skos:definition "A Measurement Artifact Function that is realized during events in which an Artifact is used to measure the Frequency of a specified object or class of objects."@en ;
                 cco:ont00001760 "https://www.commoncoreontologies.org/ArtifactOntology"^^xsd:anyURI .


###  https://www.commoncoreontologies.org/ont00000064
cco:ont00000064 rdf:type owl:Class ;
                 rdfs:subClassOf cco:ont00000798 ;
                 rdfs:label "Book"@en ;
                 skos:definition "An Information Bearing Artifact that is designed to bear some specific Information Content Entity by means of ink, paper, parchment, or other materials fastened together to hinge at one side."@en ;
                 cco:ont00001754 "https://en.wikipedia.org/w/index.php?title=Book&oldid=1063132471"^^xsd:anyURI ;
                 cco:ont00001760 "https://www.commoncoreontologies.org/ArtifactOntology"^^xsd:anyURI .


###  https://www.commoncoreontologies.org/ont00000066
cco:ont00000066 rdf:type owl:Class ;
                 rdfs:subClassOf cco:ont00001301 ;
                 rdfs:label "Military Artifact Function"@en ;
                 skos:definition "A Service Artifact Function that is realized in processes related to the armed services."@en ;
                 cco:ont00001754 "https://en.wikipedia.org/w/index.php?title=Military&oldid=1063431234"^^xsd:anyURI ;
                 cco:ont00001760 "https://www.commoncoreontologies.org/ArtifactOntology"^^xsd:anyURI .


###  https://www.commoncoreontologies.org/ont00000069
cco:ont00000069 rdf:type owl:Class ;
                 rdfs:subClassOf cco:ont00001298 ;
                 rdfs:label "Transcript"@en ;
                 skos:definition "A Document that is designed to bear some specific Information Content Entity that was originally recorded in a different medium."@en ;
                 cco:ont00001754 "https://en.wikipedia.org/w/index.php?title=Transcript&oldid=1038510063"^^xsd:anyURI ;
                 cco:ont00001760 "https://www.commoncoreontologies.org/ArtifactOntology"^^xsd:anyURI .


###  https://www.commoncoreontologies.org/ont00000075
cco:ont00000075 rdf:type owl:Class ;
                 rdfs:subClassOf cco:ont00000304 ;
                 rdfs:label "Optical Microscope"@en ;
                 skos:altLabel "Light Microscope"@en ;
                 skos:definition "A Microscope that is designed to use visible light and a system of Optical Lenses to produce a significantly enlarged image of the Object."@en ;
                 cco:ont00001754 "https://en.wikipedia.org/w/index.php?title=Optical_microscope&oldid=1063131242"^^xsd:anyURI ;
                 cco:ont00001760 "https://www.commoncoreontologies.org/ArtifactOntology"^^xsd:anyURI .


###  https://www.commoncoreontologies.org/ont00000076
cco:ont00000076 rdf:type owl:Class ;
                 rdfs:subClassOf cco:ont00000727 ;
                 rdfs:label "Wired Communication Artifact Function"@en ;
                 skos:definition "A Communication Artifact Function that is realized in a process that conveys meaningful signs by means of a (usually cylindrical) flexible strand or rod of metal."@en ;
                 cco:ont00001754 "https://en.wikipedia.org/w/index.php?title=Telecommunications&oldid=1061143810"^^xsd:anyURI ;
                 cco:ont00001760 "https://www.commoncoreontologies.org/ArtifactOntology"^^xsd:anyURI .


###  https://www.commoncoreontologies.org/ont00000081
cco:ont00000081 rdf:type owl:Class ;
                 rdfs:subClassOf cco:ont00000445 ;
                 rdfs:label "Cutting Weapon"@en ;
                 skos:definition "A Weapon that is designed to inflict harm, damage, or incapacity by means of separating some portion of its target into two or more portions through the application of acutely directed force."@en ;
                 cco:ont00001754 "https://en.wikipedia.org/w/index.php?title=Cutting&oldid=1058846915"^^xsd:anyURI ;
                 cco:ont00001760 "https://www.commoncoreontologies.org/ArtifactOntology"^^xsd:anyURI .


###  https://www.commoncoreontologies.org/ont00000086
cco:ont00000086 rdf:type owl:Class ;
                 rdfs:subClassOf cco:ont00000723 ;
                 rdfs:label "Autopilot System"@en ;
                 skos:altLabel "Autopilot"@en ;
                 skos:definition "A Vehicle Control System that is designed to enable some Agent to control the trajectory of a Vehicle without constant 'hands-on' control."@en ;
                 cco:ont00001754 "https://en.wikipedia.org/w/index.php?title=Autopilot&oldid=1063382206"^^xsd:anyURI ;
                 cco:ont00001760 "https://www.commoncoreontologies.org/ArtifactOntology"^^xsd:anyURI .


###  https://www.commoncoreontologies.org/ont00000088
cco:ont00000088 rdf:type owl:Class ;
                 rdfs:subClassOf cco:ont00001051 ;
                 rdfs:label "Firearm"@en ;
                 skos:definition "A Projectile Launcher that is designed to launch Bullets or Cartridges."@en ;
                 cco:ont00001754 "https://en.wikipedia.org/w/index.php?title=Firearm&oldid=1061216363"^^xsd:anyURI ;
                 cco:ont00001760 "https://www.commoncoreontologies.org/ArtifactOntology"^^xsd:anyURI .


###  https://www.commoncoreontologies.org/ont00000090
cco:ont00000090 rdf:type owl:Class ;
                 rdfs:subClassOf cco:ont00000547 ;
                 rdfs:label "Infrared Telescope"@en ;
                 skos:definition "A Telescope that is designed to aid in the observation of spatially distant Objects by means of collecting and focusing infrared light to form an enhanced image of the Object."@en ;
                 cco:ont00001754 "https://en.wikipedia.org/w/index.php?title=Infrared_telescope&oldid=1062918090"^^xsd:anyURI ;
                 cco:ont00001760 "https://www.commoncoreontologies.org/ArtifactOntology"^^xsd:anyURI .


###  https://www.commoncoreontologies.org/ont00000091
cco:ont00000091 rdf:type owl:Class ;
                 rdfs:subClassOf cco:ont00000457 ;
                 rdfs:label "Portion of Coolant"@en ;
                 skos:definition "A Portion of Material that is designed to be used in a thermal control system to reduce or maintain the temperature of an object to or at a specified level."@en ;
                 cco:ont00001760 "https://www.commoncoreontologies.org/ArtifactOntology"^^xsd:anyURI .


###  https://www.commoncoreontologies.org/ont00000092
cco:ont00000092 rdf:type owl:Class ;
                 rdfs:subClassOf cco:ont00000736 ;
                 rdfs:label "Bidirectional Transducer"@en ;
                 skos:definition "A Transducer that is designed to receive a signal in the form of physical phenomena and convert it into an electrical signal, and vice versa."@en ;
                 cco:ont00001754 "https://en.wikipedia.org/w/index.php?title=Transducer&oldid=1053290948"^^xsd:anyURI ;
                 cco:ont00001760 "https://www.commoncoreontologies.org/ArtifactOntology"^^xsd:anyURI .


###  https://www.commoncoreontologies.org/ont00000093
cco:ont00000093 rdf:type owl:Class ;
                 rdfs:subClassOf cco:ont00001278 ;
                 rdfs:label "Preferred Stock"@en ;
                 skos:definition "Stock that entitles its holder to receive a certain level of dividend payments before any dividends can be issued to other holders."@en ;
                 cco:ont00001760 "https://www.commoncoreontologies.org/ArtifactOntology"^^xsd:anyURI .


###  https://www.commoncoreontologies.org/ont00000095
cco:ont00000095 rdf:type owl:Class ;
                 rdfs:subClassOf cco:ont00000995 ;
                 rdfs:label "Control Surface"@en ;
                 skos:definition "A Material Artifact that is designed to deflect air, water, or another medium around its surface in order to change the Attitude of a Vehicle by rotating the Vehicle on one or more of its Axes of Rotation."@en ;
                 cco:ont00001754 "https://en.wikipedia.org/w/index.php?title=Flight_control_surfaces&oldid=1019271264"^^xsd:anyURI ;
                 cco:ont00001760 "https://www.commoncoreontologies.org/ArtifactOntology"^^xsd:anyURI .


###  https://www.commoncoreontologies.org/ont00000096
cco:ont00000096 rdf:type owl:Class ;
                 rdfs:subClassOf cco:ont00000995 ;
                 rdfs:label "Propulsion System"@en ;
                 skos:definition "A Material Artifact that is designed to facilitate the movement of material entities from one location to another and which consists of a source of mechanical power and a means of converting this power into propulsive force to generate the movement."@en ;
                 cco:ont00001754 "https://en.wikipedia.org/w/index.php?title=Propulsion&oldid=1022034059"^^xsd:anyURI ;
                 cco:ont00001760 "https://www.commoncoreontologies.org/ArtifactOntology"^^xsd:anyURI .


###  https://www.commoncoreontologies.org/ont00000097
cco:ont00000097 rdf:type owl:Class ;
                 rdfs:subClassOf cco:ont00001207 ;
                 rdfs:label "Complex Optical Lens"@en ;
                 skos:altLabel "Lens System"@en ;
                 skos:definition "An Optical Lens consisting of more than one Simple Optical Lenses."@en ;
                 cco:ont00001754 "Hecht, Eugene (1987). Optics (2nd ed.). Addison Wesley. ISBN 978-0-201-11609-0. Chapters 5 & 6."@en ;
                 cco:ont00001760 "https://www.commoncoreontologies.org/ArtifactOntology"^^xsd:anyURI .


###  https://www.commoncoreontologies.org/ont00000098
cco:ont00000098 rdf:type owl:Class ;
                 rdfs:subClassOf cco:ont00000323 ;
                 rdfs:label "Electrical Artifact Function"@en ;
                 skos:definition "An Artifact Function that is realized during events in which an Artifact is used to perform a process involving electrical power."@en ;
                 cco:ont00001760 "https://www.commoncoreontologies.org/ArtifactOntology"^^xsd:anyURI .


###  https://www.commoncoreontologies.org/ont00000101
cco:ont00000101 rdf:type owl:Class ;
                 rdfs:subClassOf cco:ont00000255 ;
                 rdfs:label "Portion of Liquid Oxygen"@en ;
                 skos:definition "A Portion of Cryogenic Material that is composed (almost) entirely of liquid oxygen."@en ;
                 cco:ont00001760 "https://www.commoncoreontologies.org/ArtifactOntology"^^xsd:anyURI .


###  https://www.commoncoreontologies.org/ont00000103
cco:ont00000103 rdf:type owl:Class ;
                 rdfs:subClassOf cco:ont00000995 ;
                 rdfs:label "Vehicle Compartment"@en ;
                 skos:altLabel "Compartment"@en ;
                 skos:definition "A Material Artifact that is designed to partition a Vehicle into subdivisions for various purposes."@en ;
                 cco:ont00001760 "https://www.commoncoreontologies.org/ArtifactOntology"^^xsd:anyURI .


###  https://www.commoncoreontologies.org/ont00000111
cco:ont00000111 rdf:type owl:Class ;
                 rdfs:subClassOf cco:ont00000256 ;
                 rdfs:label "Air Inlet"@en ;
                 skos:altLabel "Air Intake"@en ;
                 skos:definition "A Fluid Control Artifact that consists of an opening that is designed to capture and direct the flow of air into the system it is part of."@en ;
                 cco:ont00001760 "https://www.commoncoreontologies.org/ArtifactOntology"^^xsd:anyURI .


###  https://www.commoncoreontologies.org/ont00000113
cco:ont00000113 rdf:type owl:Class ;
                 rdfs:subClassOf cco:ont00000323 ;
                 rdfs:label "Ventilation Control Artifact Function"@en ;
                 skos:definition "An Artifact Function that is realized in processes in which some Artifact is used to control the quality of air in some space."@en ;
                 cco:ont00001760 "https://www.commoncoreontologies.org/ArtifactOntology"^^xsd:anyURI .


###  https://www.commoncoreontologies.org/ont00000116
cco:ont00000116 rdf:type owl:Class ;
                 rdfs:subClassOf cco:ont00000256 ;
                 rdfs:label "Pump"@en ;
                 skos:definition "A Fluid Control Artifact that is designed to impart motion to a portion of fluid to transport it within a system through the use of mechanical action."@en ;
                 cco:ont00001760 "https://www.commoncoreontologies.org/ArtifactOntology"^^xsd:anyURI .


###  https://www.commoncoreontologies.org/ont00000117
cco:ont00000117 rdf:type owl:Class ;
                 rdfs:subClassOf cco:ont00000995 ;
                 rdfs:label "Information Processing Artifact"@en ;
                 skos:definition "A Material Artifact that is designed to use algorithms to transform some Information Content Entity into another Information Content Entity."@en ;
                 cco:ont00001760 "https://www.commoncoreontologies.org/ArtifactOntology"^^xsd:anyURI .


###  https://www.commoncoreontologies.org/ont00000118
cco:ont00000118 rdf:type owl:Class ;
                 owl:equivalentClass [ owl:intersectionOf ( cco:ont00000965
                                                            [ rdf:type owl:Restriction ;
                                                              owl:onProperty cco:ont00001942 ;
                                                              owl:someValuesFrom cco:ont00000323
                                                            ]
                                                          ) ;
                                       rdf:type owl:Class
                                     ] ;
                 rdfs:subClassOf cco:ont00000965 ;
                 rdfs:label "Artifact Function Specification"@en ;
                 skos:definition "A Directive Information Content Entity that prescribes some Artifact Function and which is part of some Artifact Model."@en ;
                 cco:ont00001760 "https://www.commoncoreontologies.org/ArtifactOntology"^^xsd:anyURI .


###  https://www.commoncoreontologies.org/ont00000122
cco:ont00000122 rdf:type owl:Class ;
                 rdfs:subClassOf cco:ont00000170 ,
                                 [ rdf:type owl:Restriction ;
                                   owl:onProperty cco:ont00001944 ;
                                   owl:someValuesFrom cco:ont00000904
                                 ] ;
                 rdfs:label "Vehicle Track Point"@en ;
                 skos:definition "An Object Track Point that is where a Vehicle is or was located during some motion."@en ;
                 cco:ont00001760 "https://www.commoncoreontologies.org/ArtifactOntology"^^xsd:anyURI .


###  https://www.commoncoreontologies.org/ont00000128
cco:ont00000128 rdf:type owl:Class ;
                 rdfs:subClassOf cco:ont00000255 ;
                 rdfs:label "Portion of Liquid Hydrogen"@en ;
                 skos:definition "A Portion of Cryogenic Material that is composed (almost) entirely of liquid hydrogen."@en ;
                 cco:ont00001760 "https://www.commoncoreontologies.org/ArtifactOntology"^^xsd:anyURI .


###  https://www.commoncoreontologies.org/ont00000130
cco:ont00000130 rdf:type owl:Class ;
                 rdfs:subClassOf cco:ont00000995 ;
                 rdfs:label "Power Transformer"@en ;
                 skos:definition "A Material Artifact that is designed to transfer electrical energy between two or more circuits through electromagnetic induction."@en ;
                 cco:ont00001754 "https://en.wikipedia.org/w/index.php?title=Transformer&oldid=1062163369"^^xsd:anyURI ;
                 cco:ont00001760 "https://www.commoncoreontologies.org/ArtifactOntology"^^xsd:anyURI .


###  https://www.commoncoreontologies.org/ont00000132
cco:ont00000132 rdf:type owl:Class ;
                 rdfs:subClassOf cco:ont00000117 ;
                 rdfs:label "Recording Device"@en ;
                 skos:definition "An Information Processing Artifact that is designed to capture some information and store it in some recording format on some storage medium."@en ;
                 cco:ont00001754 "https://en.wikipedia.org/w/index.php?title=Record&oldid=1062776450"^^xsd:anyURI ;
                 cco:ont00001760 "https://www.commoncoreontologies.org/ArtifactOntology"^^xsd:anyURI .


###  https://www.commoncoreontologies.org/ont00000136
cco:ont00000136 rdf:type owl:Class ;
                 rdfs:subClassOf cco:ont00000995 ;
                 rdfs:comment "Optical Instruments are typically constructed for the purpose of being used to aid in vision or the analysis of light."@en ;
                 rdfs:label "Optical Instrument"@en ;
                 skos:definition "A Material Artifact that is designed to process light waves."@en ;
                 skos:scopeNote "Light waves can be processed in a variety of ways including via reflection, refraction, diffraction, deflection, focusing, collimation, dispersion, and interference."@en ;
                 cco:ont00001754 "https://en.wikipedia.org/w/index.php?title=Optical_instrument&oldid=1061981216"^^xsd:anyURI ;
                 cco:ont00001760 "https://www.commoncoreontologies.org/ArtifactOntology"^^xsd:anyURI .


###  https://www.commoncoreontologies.org/ont00000143
cco:ont00000143 rdf:type owl:Class ;
                 rdfs:subClassOf cco:ont00000103 ;
                 rdfs:label "Cargo Cabin"@en ;
                 skos:definition "A Vehicle Compartment that is used to store goods or materials during transportation."@en ;
                 cco:ont00001760 "https://www.commoncoreontologies.org/ArtifactOntology"^^xsd:anyURI .


###  https://www.commoncoreontologies.org/ont00000145
cco:ont00000145 rdf:type owl:Class ;
                 rdfs:subClassOf cco:ont00000445 ;
                 rdfs:label "Incendiary Weapon"@en ;
                 skos:definition "A Weapon that is designed to inflict harm, damage, or incapacity by means of starting a fire."@en ;
                 cco:ont00001754 "https://en.wikipedia.org/w/index.php?title=Incendiary_device&oldid=1055642422"^^xsd:anyURI ;
                 cco:ont00001760 "https://www.commoncoreontologies.org/ArtifactOntology"^^xsd:anyURI .


###  https://www.commoncoreontologies.org/ont00000147
cco:ont00000147 rdf:type owl:Class ;
                 rdfs:subClassOf cco:ont00000325 ;
                 rdfs:label "Flight Transponder"@en ;
                 skos:definition "A Radio Transponder that is designed to produce a specified response (typically for identification, location, or status update purposes) when it receives a radio-frequency interrogation."@en ;
                 cco:ont00001754 "https://en.wikipedia.org/w/index.php?title=Transponder_(aeronautics)&oldid=1052688836"^^xsd:anyURI ;
                 cco:ont00001760 "https://www.commoncoreontologies.org/ArtifactOntology"^^xsd:anyURI .


###  https://www.commoncoreontologies.org/ont00000152
cco:ont00000152 rdf:type owl:Class ;
                 rdfs:subClassOf cco:ont00000998 ;
                 rdfs:label "Telephone Network"@en ;
                 skos:definition "A Telecommunication Network that is designed to allow telephone calls to be made between two or more parties connected to the network."@en ;
                 cco:ont00001754 "https://en.wikipedia.org/w/index.php?title=Telephone_network&oldid=1046265527"^^xsd:anyURI ;
                 cco:ont00001760 "https://www.commoncoreontologies.org/ArtifactOntology"^^xsd:anyURI .


###  https://www.commoncoreontologies.org/ont00000153
cco:ont00000153 rdf:type owl:Class ;
                 rdfs:subClassOf cco:ont00000781 ;
                 rdfs:label "Generator Control Unit"@en ;
                 skos:definition "A Control System that is designed to regulate the voltage of some Electrical Power Source."@en ;
                 cco:ont00001760 "https://www.commoncoreontologies.org/ArtifactOntology"^^xsd:anyURI .


###  https://www.commoncoreontologies.org/ont00000156
cco:ont00000156 rdf:type owl:Class ;
                 rdfs:subClassOf cco:ont00000088 ;
                 rdfs:label "Hand Gun"@en ;
                 skos:definition "A Firearm that is designed to have a relatively short barrel and to be held in one or two hands and to be fired without being braced against the shoulder."@en ;
                 cco:ont00001754 "https://en.wikipedia.org/w/index.php?title=Handgun&oldid=1060570395"^^xsd:anyURI ;
                 cco:ont00001760 "https://www.commoncoreontologies.org/ArtifactOntology"^^xsd:anyURI .


###  https://www.commoncoreontologies.org/ont00000158
cco:ont00000158 rdf:type owl:Class ;
                 rdfs:subClassOf cco:ont00001105 ;
                 rdfs:label "Lithium-ion Electric Battery"@en ;
                 skos:definition "A Secondary Cell Electric Battery that produces electricity when lithium ions move from anode to cathode."@en ;
                 cco:ont00001754 "https://en.wikipedia.org/w/index.php?title=Lithium-ion_battery&oldid=1064099588"^^xsd:anyURI ;
                 cco:ont00001760 "https://www.commoncoreontologies.org/ArtifactOntology"^^xsd:anyURI .


###  https://www.commoncoreontologies.org/ont00000159
cco:ont00000159 rdf:type owl:Class ;
                 rdfs:subClassOf cco:ont00000798 ;
                 rdfs:label "Timekeeping Instrument"@en ;
                 skos:definition "An Information Bearing Artifact that is designed to bear some specific Information Content Entity that is about some temporal region."@en ;
                 cco:ont00001754 "https://en.wikipedia.org/w/index.php?title=Timekeeper&oldid=1061681902"^^xsd:anyURI ;
                 cco:ont00001760 "https://www.commoncoreontologies.org/ArtifactOntology"^^xsd:anyURI .


###  https://www.commoncoreontologies.org/ont00000160
cco:ont00000160 rdf:type owl:Class ;
                 rdfs:subClassOf cco:ont00000581 ;
                 rdfs:label "Manual Tool"@en ;
                 skos:altLabel "Hand Tool"@en ;
                 skos:definition "A Tool that is designed to be powered by manual labor rather than by an engine."@en ;
                 cco:ont00001754 "https://en.wikipedia.org/w/index.php?title=Hand_tool&oldid=1060741381"^^xsd:anyURI ;
                 cco:ont00001760 "https://www.commoncoreontologies.org/ArtifactOntology"^^xsd:anyURI .


###  https://www.commoncoreontologies.org/ont00000162
cco:ont00000162 rdf:type owl:Class ;
                 rdfs:subClassOf cco:ont00000795 ;
                 rdfs:label "Electrical Connector Artifact Function"@en ;
                 skos:definition "An Electrical Conduction Artifact Function that is realized by processes in which some Artifact is used to join electrical terminations to create an electrical circuit."@en ;
                 cco:ont00001760 "https://www.commoncoreontologies.org/ArtifactOntology"^^xsd:anyURI .


###  https://www.commoncoreontologies.org/ont00000167
cco:ont00000167 rdf:type owl:Class ;
                 rdfs:subClassOf cco:ont00001173 ;
                 rdfs:label "Large-Scale Rocket Launcher"@en ;
                 skos:definition "A Rocket Launcher that is designed to contain multiple Rocket Launchers."@en ;
                 cco:ont00001760 "https://www.commoncoreontologies.org/ArtifactOntology"^^xsd:anyURI .


###  https://www.commoncoreontologies.org/ont00000170
cco:ont00000170 rdf:type owl:Class .


###  https://www.commoncoreontologies.org/ont00000171
cco:ont00000171 rdf:type owl:Class ;
                 rdfs:subClassOf cco:ont00000344 ;
                 rdfs:label "Detergent Artifact Function"@en ;
                 skos:definition "A Surfactant Artifact Function that is realized in a process that cleans substances in dilute solutions."@en ;
                 cco:ont00001754 "https://en.wikipedia.org/w/index.php?title=Detergent&oldid=1064079329"^^xsd:anyURI ;
                 cco:ont00001760 "https://www.commoncoreontologies.org/ArtifactOntology"^^xsd:anyURI .


###  https://www.commoncoreontologies.org/ont00000174
cco:ont00000174 rdf:type owl:Class ;
                 rdfs:subClassOf cco:ont00000547 ;
                 rdfs:label "Ultraviolet Telescope"@en ;
                 skos:altLabel "UV Telescope"@en ;
                 skos:definition "A Telescope that is designed to aid in the observation of spatially distant Objects by means of collecting and focusing ultraviolet light to form an enhanced image of the Object."@en ;
                 cco:ont00001760 "https://www.commoncoreontologies.org/ArtifactOntology"^^xsd:anyURI .


###  https://www.commoncoreontologies.org/ont00000178
cco:ont00000178 rdf:type owl:Class ;
                 rdfs:subClassOf cco:ont00001150 ;
                 rdfs:label "Arrow"@en ;
                 skos:definition "A Portion of Ammunition that is designed to be fired from a Bow and consists of a long straight stiff shaft with stabilizers (fletchings) and a slot (the nock) on one end and a weighted tip (the arrowhead) on the other end."@en ;
                 cco:ont00001754 "https://en.wikipedia.org/w/index.php?title=Arrow&oldid=1058445874"^^xsd:anyURI ;
                 cco:ont00001760 "https://www.commoncoreontologies.org/ArtifactOntology"^^xsd:anyURI .


###  https://www.commoncoreontologies.org/ont00000183
cco:ont00000183 rdf:type owl:Class ;
                 rdfs:subClassOf cco:ont00000323 ;
                 rdfs:label "Fragrance Artifact Function"@en ;
                 skos:definition "An Artifact Function that is realized in processes of perceiving a pleasant or sweet odor."@en ;
                 cco:ont00001754 "https://en.wikipedia.org/w/index.php?title=Perfume&oldid=1062785740"^^xsd:anyURI ;
                 cco:ont00001760 "https://www.commoncoreontologies.org/ArtifactOntology"^^xsd:anyURI .


###  https://www.commoncoreontologies.org/ont00000189
cco:ont00000189 rdf:type owl:Class ;
                 rdfs:subClassOf cco:ont00000798 ;
                 rdfs:label "Certificate"@en ;
                 skos:definition "An Information Bearing Artifact that bears an Information Content Entity which attests to certain demonstrated characteristics of an Object, Person, or Organization."@en ;
                 cco:ont00001754 "http://www.dictionary.com/browse/degree" ;
                 cco:ont00001760 "https://www.commoncoreontologies.org/ArtifactOntology"^^xsd:anyURI .


###  https://www.commoncoreontologies.org/ont00000190
cco:ont00000190 rdf:type owl:Class ;
                 rdfs:subClassOf cco:ont00001353 ;
                 rdfs:label "Minimum Speed Artifact Function"@en ;
                 skos:definition "A Speed Artifact Function that is realized in some process in which the Artifact bearing the Artifact Function attains the lowest speed at which that Artifact is designed to operate."@en ;
                 cco:ont00001760 "https://www.commoncoreontologies.org/ArtifactOntology"^^xsd:anyURI .


###  https://www.commoncoreontologies.org/ont00000192
cco:ont00000192 rdf:type owl:Class ;
                 rdfs:subClassOf cco:ont00000995 ,
                                 [ rdf:type owl:Restriction ;
                                   owl:onProperty obo:BFO_0000171 ;
                                   owl:someValuesFrom cco:ont00001341
                                 ] ;
                 rdfs:label "Facility"@en ;
                 skos:definition "A Material Artifact that is designed as a building or campus dedicated to some specific purpose."@en ;
                 cco:ont00001760 "https://www.commoncoreontologies.org/ArtifactOntology"^^xsd:anyURI .


###  https://www.commoncoreontologies.org/ont00000193
cco:ont00000193 rdf:type owl:Class ;
                 rdfs:subClassOf cco:ont00000059 ;
                 rdfs:label "Telephone Subscriber Line"@en ;
                 skos:definition "A Telephone Line that connects a Communication Endpoint to another node in a Telecommunication Network to enable service to a user's Telephone."@en ;
                 cco:ont00001754 "https://en.wikipedia.org/w/index.php?title=Telephone_line&oldid=1063429738"^^xsd:anyURI ;
                 cco:ont00001760 "https://www.commoncoreontologies.org/ArtifactOntology"^^xsd:anyURI .


###  https://www.commoncoreontologies.org/ont00000194
cco:ont00000194 rdf:type owl:Class ;
                 rdfs:subClassOf cco:ont00000795 ;
                 rdfs:label "Electrical Contact Artifact Function"@en ;
                 skos:definition "An Electrical Conduction Artifact Function that is realized by processes in which some Artifact is used as an endpoint of an electrical circuit from which an electrical current is passed via physical contact with the endpoint."@en ;
                 cco:ont00001760 "https://www.commoncoreontologies.org/ArtifactOntology"^^xsd:anyURI .


###  https://www.commoncoreontologies.org/ont00000199
cco:ont00000199 rdf:type owl:Class ;
                 rdfs:subClassOf cco:ont00000771 ;
                 rdfs:label "Camera"@en ;
                 skos:definition "An Imaging Instrument that is designed to form and digitally or physically record an image of an entity."@en ;
                 cco:ont00001754 "http://www.dictionary.com/browse/camera" ;
                 cco:ont00001760 "https://www.commoncoreontologies.org/ArtifactOntology"^^xsd:anyURI .


###  https://www.commoncoreontologies.org/ont00000204
cco:ont00000204 rdf:type owl:Class ;
                 rdfs:subClassOf cco:ont00001104 ;
                 rdfs:label "Rifle"@en ;
                 skos:definition "A Long Gun that is designed to have a rifled barrel and to fire single Bullets over long ranges with high accuracy."@en ;
                 cco:ont00001754 "https://en.wikipedia.org/w/index.php?title=Rifle&oldid=1056172452"^^xsd:anyURI ;
                 cco:ont00001760 "https://www.commoncoreontologies.org/ArtifactOntology"^^xsd:anyURI .


###  https://www.commoncoreontologies.org/ont00000205
cco:ont00000205 rdf:type owl:Class .


###  https://www.commoncoreontologies.org/ont00000206
cco:ont00000206 rdf:type owl:Class ;
                 rdfs:subClassOf cco:ont00000323 ;
                 rdfs:label "Friction Reduction Artifact Function"@en ;
                 skos:definition "An Artifact Function that is realized in processes of reducing the force resisting the relative motion of surfaces in contact."@en ;
                 cco:ont00001754 "https://en.wikipedia.org/w/index.php?title=Friction&oldid=1061569068"^^xsd:anyURI ;
                 cco:ont00001760 "https://www.commoncoreontologies.org/ArtifactOntology"^^xsd:anyURI .


###  https://www.commoncoreontologies.org/ont00000210
cco:ont00000210 rdf:type owl:Class ;
                 rdfs:subClassOf cco:ont00000995 ;
                 rdfs:label "Engine"@en ;
                 skos:altLabel "Motor"@en ;
                 skos:definition "A Material Artifact that is designed to convert one form of energy into mechanical energy."@en ;
                 cco:ont00001754 "https://en.wikipedia.org/w/index.php?title=Engine&oldid=1063879193"^^xsd:anyURI ;
                 cco:ont00001760 "https://www.commoncoreontologies.org/ArtifactOntology"^^xsd:anyURI .


###  https://www.commoncoreontologies.org/ont00000212
cco:ont00000212 rdf:type owl:Class ;
                 rdfs:subClassOf cco:ont00000445 ;
                 rdfs:label "Chemical Weapon"@en ;
                 skos:definition "A Weapon that is designed to inflict harm, damage, or incapacity by means of releasing toxic chemicals."@en ;
                 cco:ont00001754 "https://en.wikipedia.org/w/index.php?title=Chemical_weapon&oldid=1054342645"^^xsd:anyURI ;
                 cco:ont00001760 "https://www.commoncoreontologies.org/ArtifactOntology"^^xsd:anyURI .


###  https://www.commoncoreontologies.org/ont00000214
cco:ont00000214 rdf:type owl:Class ;
                 rdfs:subClassOf cco:ont00000289 ;
                 rdfs:label "Moving Target Indication Artifact Function"@en ;
                 skos:definition "A Radar Imaging Artifact Function that inheres in Artifacts that are designed to identify and produce visual representations of moving entities by using a radar to emit successive phase coherent pulses, which are sampled and added to the subsequent pulse to cancel out signals from non-moving entities such that only signals from moving entities remain and are displayed."@en ;
                 cco:ont00001760 "https://www.commoncoreontologies.org/ArtifactOntology"^^xsd:anyURI .


###  https://www.commoncoreontologies.org/ont00000215
cco:ont00000215 rdf:type owl:Class ;
                 rdfs:subClassOf cco:ont00000547 ;
                 rdfs:comment "A Radio Telescope consists of a specialized Antenna and a Radio Receiver and is typically used to receive radio waves from sources in outer space."@en ;
                 rdfs:label "Radio Telescope"@en ;
                 skos:definition "A Telescope that is designed to aid in the observation of spatially distant Objects by means of collecting and focusing radio waves to form an enhanced image of the Object."@en ;
                 cco:ont00001754 "https://en.wikipedia.org/w/index.php?title=Radio_telescope&oldid=1052819190"^^xsd:anyURI ;
                 cco:ont00001760 "https://www.commoncoreontologies.org/ArtifactOntology"^^xsd:anyURI .


###  https://www.commoncoreontologies.org/ont00000216
cco:ont00000216 rdf:type owl:Class ;
                 rdfs:subClassOf cco:ont00001150 ;
                 rdfs:label "Shell"@en ;
                 skos:definition "A Portion of Ammunition that is designed to be a non-self-propelled projectile and to carry a payload (explosive or other) over a relatively short distance."@en ;
                 cco:ont00001754 "https://en.wikipedia.org/wiki/Shell_(projectile)" ;
                 cco:ont00001760 "https://www.commoncoreontologies.org/ArtifactOntology"^^xsd:anyURI .


###  https://www.commoncoreontologies.org/ont00000219
cco:ont00000219 rdf:type owl:Class ;
                 rdfs:subClassOf cco:ont00001009 ;
                 rdfs:label "Reflecting Optical Telescope"@en ;
                 skos:altLabel "Reflecting Telescope"@en ,
                               "Reflector"@en ;
                 skos:definition "An Optical Telescope that is designed to aid in the observation of spatially distant Objects by means of collecting and focusing visible light via reflection through the use of one or more curved Mirrors to form an enhanced image of the Object."@en ;
                 cco:ont00001754 "https://en.wikipedia.org/w/index.php?title=Reflecting_telescope&oldid=1062982683"^^xsd:anyURI ;
                 cco:ont00001760 "https://www.commoncoreontologies.org/ArtifactOntology"^^xsd:anyURI .


###  https://www.commoncoreontologies.org/ont00000230
cco:ont00000230 rdf:type owl:Class ;
                 rdfs:subClassOf cco:ont00000136 ;
                 rdfs:label "Diffraction Grating"@en ;
                 skos:definition "An Optical Instrument with a periodic structure that is designed to split and defract a beam of light into several beams travelling in different directions."@en ;
                 cco:ont00001754 "https://en.wikipedia.org/w/index.php?title=Diffraction_grating&oldid=1060463366"^^xsd:anyURI ;
                 cco:ont00001760 "https://www.commoncoreontologies.org/ArtifactOntology"^^xsd:anyURI .


###  https://www.commoncoreontologies.org/ont00000231
cco:ont00000231 rdf:type owl:Class ;
                 rdfs:subClassOf cco:ont00001051 ;
                 rdfs:label "Torpedo Tube"@en ;
                 skos:definition "A Projectile Launcher that is designed to launch Torpedoes."@en ;
                 cco:ont00001754 "https://en.wikipedia.org/w/index.php?title=Torpedo_tube&oldid=1063672665"^^xsd:anyURI ;
                 cco:ont00001760 "https://www.commoncoreontologies.org/ArtifactOntology"^^xsd:anyURI .


###  https://www.commoncoreontologies.org/ont00000233
cco:ont00000233 rdf:type owl:Class ;
                 rdfs:subClassOf cco:ont00001278 ;
                 rdfs:label "Stock Certificate"@en ;
                 skos:definition "Stock that consists of a Certificate."@en ;
                 cco:ont00001760 "https://www.commoncoreontologies.org/ArtifactOntology"^^xsd:anyURI .


###  https://www.commoncoreontologies.org/ont00000236
cco:ont00000236 rdf:type owl:Class ;
                 rdfs:subClassOf cco:ont00000995 ;
                 rdfs:label "Lighting System"@en ;
                 skos:definition "A Material Artifact that is designed to emit light within some area."@en ;
                 cco:ont00001760 "https://www.commoncoreontologies.org/ArtifactOntology"^^xsd:anyURI .


###  https://www.commoncoreontologies.org/ont00000238
cco:ont00000238 rdf:type owl:Class ;
                 rdfs:subClassOf cco:ont00000995 ;
                 rdfs:label "Propeller"@en ;
                 skos:altLabel "Propelling Screw"@en ;
                 skos:definition "A Material Artifact that is designed to convert rotary motion from an Engine or other mechanical Power Source into propulsive Force."@en ;
                 cco:ont00001754 "https://en.wikipedia.org/wiki/Propeller_(aeronautics)" ;
                 cco:ont00001760 "https://www.commoncoreontologies.org/ArtifactOntology"^^xsd:anyURI .


###  https://www.commoncoreontologies.org/ont00000241
cco:ont00000241 rdf:type owl:Class ;
                 rdfs:subClassOf cco:ont00001064 ;
                 rdfs:label "Two-Dimensional Barcode"@en ;
                 skos:definition "A Barcode that is designed to bear lines of varying widths, spacing, height, and color that concretize some Directive Information Content Entity."@en ;
                 cco:ont00001760 "https://www.commoncoreontologies.org/ArtifactOntology"^^xsd:anyURI .


###  https://www.commoncoreontologies.org/ont00000242
cco:ont00000242 rdf:type owl:Class ;
                 rdfs:subClassOf cco:ont00000241 ;
                 rdfs:label "Data Matrix Code"@en ;
                 skos:definition "A Two-Dimensional Barcode that consists of cells arranged in rectangular patterns and is used for marking small items in logistics and operations."@en ;
                 cco:ont00001760 "https://www.commoncoreontologies.org/ArtifactOntology"^^xsd:anyURI .


###  https://www.commoncoreontologies.org/ont00000243
cco:ont00000243 rdf:type owl:Class ;
                 rdfs:subClassOf cco:ont00000995 ;
                 rdfs:label "Heat Sink"@en ;
                 skos:definition "A Material Artifact that is designed to regulate the temperature of a computer by the passive transfer of heat away from other components in the computer."@en ;
                 cco:ont00001754 "https://en.wikipedia.org/w/index.php?title=Heat_sink&oldid=1062822080"^^xsd:anyURI ;
                 cco:ont00001760 "https://www.commoncoreontologies.org/ArtifactOntology"^^xsd:anyURI .


###  https://www.commoncoreontologies.org/ont00000244
cco:ont00000244 rdf:type owl:Class ;
                 rdfs:subClassOf cco:ont00001153 ;
                 rdfs:label "Fragmentation Artifact Function"@en ;
                 skos:definition "A Damaging Artifact Function that is realized in a process in which the structural integrity of an entity is impaired because of a detonation which causes fragmentation."@en ;
                 cco:ont00001754 "http://www.dictionary.com/browse/fragmentation" ;
                 cco:ont00001760 "https://www.commoncoreontologies.org/ArtifactOntology"^^xsd:anyURI .


###  https://www.commoncoreontologies.org/ont00000247
cco:ont00000247 rdf:type owl:Class ;
                 rdfs:subClassOf cco:ont00001326 ;
                 rdfs:label "Road"@en ;
                 skos:definition "A Land Transportation Artifact that is designed to enable Ground Vehicles to travel from one location to another."@en ;
                 cco:ont00001754 "https://en.wikipedia.org/w/index.php?title=Road&oldid=1063402841" ;
                 cco:ont00001760 "https://www.commoncoreontologies.org/ArtifactOntology"^^xsd:anyURI .


###  https://www.commoncoreontologies.org/ont00000249
cco:ont00000249 rdf:type owl:Class ;
                 rdfs:subClassOf cco:ont00000995 ;
                 rdfs:comment "A Shaft is usually used to connect other components of a drive train that cannot be connected directly either because of the distance between them or the need to allow for relative movement between those components."@en ;
                 rdfs:label "Shaft"@en ;
                 skos:definition "A Material Artifact that is designed to rotate and transmit Torque, Power, or Rotational Motion from one machine element to another."@en ;
                 cco:ont00001754 "https://en.wikipedia.org/w/index.php?title=Shaft&oldid=1023963656"^^xsd:anyURI ;
                 cco:ont00001760 "https://www.commoncoreontologies.org/ArtifactOntology"^^xsd:anyURI .


###  https://www.commoncoreontologies.org/ont00000252
cco:ont00000252 rdf:type owl:Class ;
                 rdfs:subClassOf cco:ont00000256 ;
                 rdfs:label "Nozzle"@en ;
                 skos:definition "A Fluid Control Artifact that is designed to control the speed, direction, rate, shape, or pressure of the flow of fluid exiting it."@en ;
                 cco:ont00001760 "https://www.commoncoreontologies.org/ArtifactOntology"^^xsd:anyURI .


###  https://www.commoncoreontologies.org/ont00000253
cco:ont00000253 rdf:type owl:Class .


###  https://www.commoncoreontologies.org/ont00000254
cco:ont00000254 rdf:type owl:Class ;
                 rdfs:subClassOf cco:ont00000995 ;
                 rdfs:label "Transportation Artifact"@en ;
                 skos:definition "A Material Artifact that is fixed in place and designed to bear a Function, the realization of which is sometimes part of a process moving Vehicles and Agents from one location to another."@en ;
                 cco:ont00001760 "https://www.commoncoreontologies.org/ArtifactOntology"^^xsd:anyURI .


###  https://www.commoncoreontologies.org/ont00000255
cco:ont00000255 rdf:type owl:Class ;
                 rdfs:subClassOf cco:ont00000457 ;
                 rdfs:label "Portion of Cryogenic Material"@en ;
                 skos:definition "A Portion of Material that has been reduced to a very low temperature (below -180 degrees Celcius)."@en ;
                 cco:ont00001760 "https://www.commoncoreontologies.org/ArtifactOntology"^^xsd:anyURI .


###  https://www.commoncoreontologies.org/ont00000256
cco:ont00000256 rdf:type owl:Class ;
                 rdfs:subClassOf cco:ont00000995 ;
                 rdfs:label "Fluid Control Artifact"@en ;
                 skos:definition "A Material Artifact that is designed to manipulate the flow of a fluid (i.e. a liquid or a gas)."@en ;
                 cco:ont00001760 "https://www.commoncoreontologies.org/ArtifactOntology"^^xsd:anyURI .


###  https://www.commoncoreontologies.org/ont00000258
cco:ont00000258 rdf:type owl:Class ;
                 rdfs:subClassOf cco:ont00001064 ;
                 rdfs:label "One-Dimensional Barcode"@en ;
                 skos:definition "A Barcode that is designed to bear parallel lines of varying widths and spacing that concretize some Directive Information Content Entity."@en ;
                 cco:ont00001760 "https://www.commoncoreontologies.org/ArtifactOntology"^^xsd:anyURI .


###  https://www.commoncoreontologies.org/ont00000264
cco:ont00000264 rdf:type owl:Class ;
                 rdfs:subClassOf cco:ont00000020 ;
                 rdfs:label "Hydraulic Fluid Reservoir"@en ;
                 skos:definition "A Container that is designed to store some hydraulic fluid for use in some Hyrdraulic Power Source."@en ;
                 cco:ont00001760 "https://www.commoncoreontologies.org/ArtifactOntology"^^xsd:anyURI .


###  https://www.commoncoreontologies.org/ont00000266
cco:ont00000266 rdf:type owl:Class ;
                 rdfs:subClassOf cco:ont00001381 ;
                 rdfs:label "Hearing Aid"@en ;
                 skos:definition "A Medical Artifact that is designed to improve hearing for its user."@en ;
                 cco:ont00001754 "https://en.wikipedia.org/w/index.php?title=Hearing_aid&oldid=1062688647"^^xsd:anyURI ;
                 cco:ont00001760 "https://www.commoncoreontologies.org/ArtifactOntology"^^xsd:anyURI .


###  https://www.commoncoreontologies.org/ont00000267
cco:ont00000267 rdf:type owl:Class ;
                 rdfs:subClassOf cco:ont00000791 ;
                 rdfs:label "Catalyst Artifact Function"@en ;
                 skos:definition "A Chemical Reaction Artifact Function that is realized in a process in which the rate of a chemical reaction is increased due to the participation of an additional substance, without that substance being consumed in the reaction."@en ;
                 cco:ont00001754 "https://en.wikipedia.org/w/index.php?title=Catalysis&oldid=1063864001"^^xsd:anyURI ;
                 cco:ont00001760 "https://www.commoncoreontologies.org/ArtifactOntology"^^xsd:anyURI .


###  https://www.commoncoreontologies.org/ont00000268
cco:ont00000268 rdf:type owl:Class ;
                 rdfs:subClassOf cco:ont00001051 ;
                 rdfs:label "Cannon"@en ;
                 skos:definition "A Projectile Launcher that is designed to use a controlled explosion to launch a relatively large Portion of Ammunition, such as a Round Shot or a Shell, at a significant Velocity."@en ;
                 cco:ont00001754 "https://en.wikipedia.org/w/index.php?title=Cannon&oldid=1063792906"^^xsd:anyURI ;
                 cco:ont00001760 "https://www.commoncoreontologies.org/ArtifactOntology"^^xsd:anyURI .


###  https://www.commoncoreontologies.org/ont00000269
cco:ont00000269 rdf:type owl:Class ;
                 rdfs:subClassOf cco:ont00000903 ;
                 rdfs:label "Radio Transmitter"@en ;
                 skos:definition "A Radio Communication Instrument that is an electronic device that is designed to generate a radio frequency alternating current, which can be applied to a Radio Antenna to be transmitted as radio waves."@en ;
                 cco:ont00001754 "https://en.wikipedia.org/w/index.php?title=Transmitter&oldid=1061735586"^^xsd:anyURI ;
                 cco:ont00001760 "https://www.commoncoreontologies.org/ArtifactOntology"^^xsd:anyURI .


###  https://www.commoncoreontologies.org/ont00000273
cco:ont00000273 rdf:type owl:Class ;
                 rdfs:subClassOf cco:ont00000323 ;
                 rdfs:label "Communication Interference Artifact Function"@en ;
                 skos:definition "An Artifact Function that is realized during events in which an Artifact is used to interfere with the transmission of information for the purpose of preventing communication."@en ;
                 cco:ont00001760 "https://www.commoncoreontologies.org/ArtifactOntology"^^xsd:anyURI .


###  https://www.commoncoreontologies.org/ont00000277
cco:ont00000277 rdf:type owl:Class ;
                 rdfs:subClassOf cco:ont00000445 ;
                 rdfs:label "Nuclear Weapon"@en ;
                 skos:definition "A Weapon that is designed to inflict harm, damage, or incapacity by means of a destructive nuclear reaction, either through fission or through a combination of fission and fusion."@en ;
                 cco:ont00001754 "https://en.wikipedia.org/w/index.php?title=Nuclear_weapon&oldid=1060854171"^^xsd:anyURI ;
                 cco:ont00001760 "https://www.commoncoreontologies.org/ArtifactOntology"^^xsd:anyURI .


###  https://www.commoncoreontologies.org/ont00000280
cco:ont00000280 rdf:type owl:Class ;
                 rdfs:subClassOf cco:ont00001124 ;
                 rdfs:label "Torpedo"@en ;
                 skos:definition "A Precision-Guided Missile that is designed to be fired into a body of water, be self-propelled through the water, and carry an explosive payload."@en ;
                 cco:ont00001754 "https://en.wikipedia.org/w/index.php?title=Torpedo&oldid=1062609830"^^xsd:anyURI ;
                 cco:ont00001760 "https://www.commoncoreontologies.org/ArtifactOntology"^^xsd:anyURI .


###  https://www.commoncoreontologies.org/ont00000282
cco:ont00000282 rdf:type owl:Class ;
                 rdfs:subClassOf cco:ont00000719 ;
                 rdfs:label "Counterfeit Financial Instrument"@en ;
                 skos:definition "A Counterfeit Instrument that is designed to be a fake replica of some legally sanctioned Financial Instrument."@en ;
                 cco:ont00001754 "https://en.wikipedia.org/w/index.php?title=Counterfeit_money&oldid=1064052318"^^xsd:anyURI ;
                 cco:ont00001760 "https://www.commoncoreontologies.org/ArtifactOntology"^^xsd:anyURI .


###  https://www.commoncoreontologies.org/ont00000285
cco:ont00000285 rdf:type owl:Class ;
                 rdfs:subClassOf cco:ont00000269 ;
                 rdfs:label "Emergency Locator Transmitter"@en ;
                 skos:definition "A Radio Transmitter that is designed to signal distress and provide positional data for the entity it is located on."@en ;
                 cco:ont00001754 "https://en.wikipedia.org/w/index.php?title=Emergency_position-indicating_radiobeacon&oldid=1063407242"^^xsd:anyURI ;
                 cco:ont00001760 "https://www.commoncoreontologies.org/ArtifactOntology"^^xsd:anyURI .


###  https://www.commoncoreontologies.org/ont00000287
cco:ont00000287 rdf:type owl:Class ;
                 rdfs:subClassOf cco:ont00001187 ;
                 rdfs:label "Inertial Navigation System"@en ;
                 skos:altLabel "INS"@en ;
                 skos:definition "A Navigation System that is designed to continuously calculate via dead reckoning the position, orientation, and velocity of a moving object without the need for external references."@en ;
                 cco:ont00001754 "https://en.wikipedia.org/w/index.php?title=Inertial_navigation_system&oldid=1063682725"^^xsd:anyURI ;
                 cco:ont00001760 "https://www.commoncoreontologies.org/ArtifactOntology"^^xsd:anyURI .


###  https://www.commoncoreontologies.org/ont00000288
cco:ont00000288 rdf:type owl:Class ;
                 rdfs:subClassOf cco:ont00000995 ;
                 rdfs:label "Power Source"@en ;
                 skos:definition "A Material Artifact that is designed to supply power to some other Artifact."@en ;
                 cco:ont00001754 "https://en.wikipedia.org/w/index.php?title=Power_source&oldid=1032888635"^^xsd:anyURI ;
                 cco:ont00001760 "https://www.commoncoreontologies.org/ArtifactOntology"^^xsd:anyURI .


###  https://www.commoncoreontologies.org/ont00000289
cco:ont00000289 rdf:type owl:Class ;
                 rdfs:subClassOf cco:ont00000601 ;
                 rdfs:label "Radar Imaging Artifact Function"@en ;
                 skos:definition "An Imaging Artifact Function that inheres in Artifacts that are designed to produce visual representations of entities using radio waves."@en ;
                 cco:ont00001760 "https://www.commoncoreontologies.org/ArtifactOntology"^^xsd:anyURI .


###  https://www.commoncoreontologies.org/ont00000292
cco:ont00000292 rdf:type owl:Class ;
                 owl:equivalentClass [ owl:intersectionOf ( cco:ont00000686
                                                            [ rdf:type owl:Restriction ;
                                                              owl:onProperty cco:ont00001916 ;
                                                              owl:someValuesFrom cco:ont00000995
                                                            ]
                                                          ) ;
                                       rdf:type owl:Class
                                     ] ;
                 rdfs:subClassOf cco:ont00000686 ;
                 rdfs:label "Artifact Identifier"@en ;
                 skos:definition "A Designative Information Content Entity which designates some Artifact."@en ;
                 cco:ont00001760 "https://www.commoncoreontologies.org/ArtifactOntology"^^xsd:anyURI .


###  https://www.commoncoreontologies.org/ont00000294
cco:ont00000294 rdf:type owl:Class ;
                 rdfs:subClassOf cco:ont00000533 ;
                 rdfs:label "Air-Breathing Jet Engine"@en ;
                 skos:altLabel "Ducted Jet Engine"@en ;
                 skos:definition "A Jet Engine that is propelled by a jet of hot exhaust gases formed from air that is drawn into the Engine via an Air Inlet."@en ;
                 cco:ont00001754 "https://en.wikipedia.org/w/index.php?title=Airbreathing_jet_engine&oldid=1062364308"^^xsd:anyURI ;
                 cco:ont00001760 "https://www.commoncoreontologies.org/ArtifactOntology"^^xsd:anyURI .


###  https://www.commoncoreontologies.org/ont00000298
cco:ont00000298 rdf:type owl:Class ;
                 rdfs:subClassOf cco:ont00001173 ;
                 rdfs:label "Shoulder-Fired Rocket Launcher"@en ;
                 skos:definition "A Rocket Launcher that is designed to be small enough to be carried by a single person and fired while supported on the person's shoulder."@en ;
                 cco:ont00001760 "https://www.commoncoreontologies.org/ArtifactOntology"^^xsd:anyURI .


###  https://www.commoncoreontologies.org/ont00000299
cco:ont00000299 rdf:type owl:Class ;
                 rdfs:subClassOf cco:ont00000715 ;
                 rdfs:label "Prosthetic Leg"@en ;
                 skos:definition "A Prosthesis that is designed to replace a missing leg."@en ;
                 cco:ont00001754 "https://en.wikipedia.org/w/index.php?title=Prosthesis&oldid=1063749698"^^xsd:anyURI ;
                 cco:ont00001760 "https://www.commoncoreontologies.org/ArtifactOntology"^^xsd:anyURI .


###  https://www.commoncoreontologies.org/ont00000301
cco:ont00000301 rdf:type owl:Class ;
                 rdfs:subClassOf cco:ont00000663 ;
                 rdfs:label "Vehicle Transmission"@en ;
                 skos:altLabel "Gearbox"@en ,
                               "Transmission"@en ;
                 skos:definition "A Power Transmission Artifact that is designed to vary the output speed and torque in a rotating power transfer system."@en ;
                 cco:ont00001754 "https://en.wikipedia.org/wiki/Transmission_(mechanics)"^^xsd:anyURI ;
                 cco:ont00001760 "https://www.commoncoreontologies.org/ArtifactOntology"^^xsd:anyURI .


###  https://www.commoncoreontologies.org/ont00000302
cco:ont00000302 rdf:type owl:Class ;
                 rdfs:subClassOf cco:ont00001049 ;
                 rdfs:label "Alternating Current Power Source"@en ;
                 skos:definition "An Electrical Power Source that is designed to transfer electrical power in the form of alternating current."@en ;
                 cco:ont00001760 "https://www.commoncoreontologies.org/ArtifactOntology"^^xsd:anyURI .


###  https://www.commoncoreontologies.org/ont00000303
cco:ont00000303 rdf:type owl:Class ;
                 rdfs:subClassOf cco:ont00001036 ;
                 rdfs:label "Intercommunication System"@en ;
                 skos:definition "A Communication System that is designed to enable some Act of Communication between end points within a building, small collection of buildings, or within a small area of service."@en ;
                 cco:ont00001754 "https://en.wikipedia.org/w/index.php?title=Intercom&oldid=1055934442"^^xsd:anyURI ;
                 cco:ont00001760 "https://www.commoncoreontologies.org/ArtifactOntology"^^xsd:anyURI .


###  https://www.commoncoreontologies.org/ont00000304
cco:ont00000304 rdf:type owl:Class ;
                 rdfs:subClassOf cco:ont00000771 ;
                 rdfs:label "Microscope"@en ;
                 skos:definition "An Imaging Instrument that is designed to enable users to see Objects that are otherwise too small to be seen by the naked eye by producing a significantly enlarged image of the Object."@en ;
                 cco:ont00001754 "https://en.wikipedia.org/w/index.php?title=Microscope&oldid=1059024357"^^xsd:anyURI ;
                 cco:ont00001760 "https://www.commoncoreontologies.org/ArtifactOntology"^^xsd:anyURI .


###  https://www.commoncoreontologies.org/ont00000306
cco:ont00000306 rdf:type owl:Class ;
                 rdfs:subClassOf cco:ont00001370 ;
                 rdfs:label "Hinge"@en ;
                 skos:definition "A Machine Bearing that is designed to limit the angle of Rotation between two solid objects."@en ;
                 cco:ont00001754 "https://en.wikipedia.org/w/index.php?title=Hinge&oldid=1059935559"^^xsd:anyURI ;
                 cco:ont00001760 "https://www.commoncoreontologies.org/ArtifactOntology"^^xsd:anyURI .


###  https://www.commoncoreontologies.org/ont00000307
cco:ont00000307 rdf:type owl:Class ;
                 rdfs:subClassOf cco:ont00001084 ;
                 rdfs:label "Portion of Food"@en ;
                 skos:definition "A Portion of Processed Material that is designed to be consumed and ingested for nutrition or taste."@en ;
                 cco:ont00001754 "https://en.wikipedia.org/w/index.php?title=Food&oldid=1062824590"^^xsd:anyURI ;
                 cco:ont00001760 "https://www.commoncoreontologies.org/ArtifactOntology"^^xsd:anyURI .


###  https://www.commoncoreontologies.org/ont00000309
cco:ont00000309 rdf:type owl:Class ;
                 rdfs:subClassOf cco:ont00001301 ;
                 rdfs:label "Healthcare Artifact Function"@en ;
                 skos:definition "A Service Artifact Function that is realized in processes of treating and preventing illness."@en ;
                 cco:ont00001754 "https://en.wikipedia.org/w/index.php?title=Health_care&oldid=1064015344"^^xsd:anyURI ;
                 cco:ont00001760 "https://www.commoncoreontologies.org/ArtifactOntology"^^xsd:anyURI .


###  https://www.commoncoreontologies.org/ont00000310
cco:ont00000310 rdf:type owl:Class ;
                 rdfs:subClassOf cco:ont00000552 ;
                 rdfs:label "Grenade"@en ;
                 skos:altLabel "Hand Grenade"@en ;
                 skos:definition "An Explosive Weapon that is designed to be relatively small and to be thrown by hand."@en ;
                 cco:ont00001754 "https://en.wikipedia.org/w/index.php?title=Grenade&oldid=1060366148"^^xsd:anyURI ;
                 cco:ont00001760 "https://www.commoncoreontologies.org/ArtifactOntology"^^xsd:anyURI .


###  https://www.commoncoreontologies.org/ont00000311
cco:ont00000311 rdf:type owl:Class ;
                 rdfs:subClassOf cco:ont00001999 ;
                 rdfs:label "Filtration Artifact Function"@en ;
                 skos:definition "A Filter Function that is realized in a process in which some solid entity is prevented from moving along with some quantity of liquid."@en ;
                 cco:ont00001754 "https://en.wikipedia.org/w/index.php?title=Filtration&oldid=1061655528"^^xsd:anyURI ;
                 cco:ont00001760 "https://www.commoncoreontologies.org/ArtifactOntology"^^xsd:anyURI .


###  https://www.commoncoreontologies.org/ont00000315
cco:ont00000315 rdf:type owl:Class ;
                 rdfs:subClassOf cco:ont00000918 ;
                 rdfs:label "Telecommunication Switching Node"@en ;
                 skos:definition "A Telecommunication Network Node that is capable of redirecting a communication transmission to another Telecommunication Network Node."@en ;
                 cco:ont00001754 "https://en.wikipedia.org/w/index.php?title=Telecommunications_network&oldid=1063347482"^^xsd:anyURI ;
                 cco:ont00001760 "https://www.commoncoreontologies.org/ArtifactOntology"^^xsd:anyURI .


###  https://www.commoncoreontologies.org/ont00000316
cco:ont00000316 rdf:type owl:Class ;
                 rdfs:subClassOf cco:ont00000255 ;
                 rdfs:label "Portion of Liquid Helium"@en ;
                 skos:definition "A Portion of Cryogenic Material that is composed (almost) entirely of liquid helium."@en ;
                 cco:ont00001760 "https://www.commoncoreontologies.org/ArtifactOntology"^^xsd:anyURI .


###  https://www.commoncoreontologies.org/ont00000317
cco:ont00000317 rdf:type owl:Class ;
                 rdfs:subClassOf cco:ont00001218 ;
                 rdfs:label "Electronic Signal Processing Artifact Function"@en ;
                 skos:definition "A Signal Processing Artifact Function that inheres in Artifacts that are designed to process or transfer information contained in electronic signals."@en ;
                 cco:ont00001760 "https://www.commoncoreontologies.org/ArtifactOntology"^^xsd:anyURI .


###  https://www.commoncoreontologies.org/ont00000319
cco:ont00000319 rdf:type owl:Class ;
                 rdfs:subClassOf cco:ont00000965 ,
                                 [ rdf:type owl:Restriction ;
                                   owl:onProperty cco:ont00001942 ;
                                   owl:someValuesFrom cco:ont00000995
                                 ] ;
                 rdfs:label "Artifact Design"@en ;
                 skos:definition "A Directive Information Content Entity that is a specification of an object, manifested by an agent, intended to accomplish goals, in a particular environment, using a set of primitive components, satisfying a set of requirements, subject to constraints."@en ;
                 cco:ont00001754 "https://en.wikipedia.org/w/index.php?title=Design&oldid=1063941625"^^xsd:anyURI ;
                 cco:ont00001760 "https://www.commoncoreontologies.org/ArtifactOntology"^^xsd:anyURI .


###  https://www.commoncoreontologies.org/ont00000321
cco:ont00000321 rdf:type owl:Class ;
                 rdfs:subClassOf cco:ont00001301 ;
                 rdfs:label "Residential Artifact Function"@en ;
                 skos:definition "A Service Artifact Function that is realized in processes of residing in a dwelling or home."@en ;
                 cco:ont00001754 "https://en.wikipedia.org/w/index.php?title=Residence&oldid=1019728937"^^xsd:anyURI ;
                 cco:ont00001760 "https://www.commoncoreontologies.org/ArtifactOntology"^^xsd:anyURI .


###  https://www.commoncoreontologies.org/ont00000323
cco:ont00000323 rdf:type owl:Class ;
                 rdfs:subClassOf obo:BFO_0000034 ,
                                 [ rdf:type owl:Restriction ;
                                   owl:onProperty obo:BFO_0000197 ;
                                   owl:someValuesFrom cco:ont00000995
                                 ] ;
                 rdfs:label "Artifact Function"@en ;
                 skos:definition "A Function that inheres in some Artifact in virtue of that Artifact being designed to be used in processes that require that Function to be realized."@en ;
                 cco:ont00001760 "https://www.commoncoreontologies.org/ArtifactOntology"^^xsd:anyURI .


###  https://www.commoncoreontologies.org/ont00000325
cco:ont00000325 rdf:type owl:Class ;
                 rdfs:subClassOf cco:ont00000903 ;
                 rdfs:label "Radio Transponder"@en ;
                 skos:altLabel "Transmitter-Responder"@en ;
                 skos:definition "A Radio Communication Instrument that is an electronic device that acts as both a Radio Transmitter and responder and is used to wirelessly receive and transmit electrical signals."@en ;
                 cco:ont00001760 "https://www.commoncoreontologies.org/ArtifactOntology"^^xsd:anyURI .


###  https://www.commoncoreontologies.org/ont00000326
cco:ont00000326 rdf:type owl:Class ;
                 rdfs:subClassOf cco:ont00000258 ;
                 rdfs:label "UPC Barcode"@en ;
                 skos:definition "A One-Dimensional Barcode that consists of 6 or 12 numerical digits and is used to scan consumer goods."@en ;
                 cco:ont00001760 "https://www.commoncoreontologies.org/ArtifactOntology"^^xsd:anyURI .


###  https://www.commoncoreontologies.org/ont00000328
cco:ont00000328 rdf:type owl:Class ;
                 rdfs:subClassOf cco:ont00000870 ;
                 rdfs:label "Transportation Infrastructure"@en ;
                 skos:definition "An Infrastructure System that is designed to facilitate the movement of material entities from one location to another by providing the necessary structures for Persons to travel or for Vehicles to transport material entities."@en ;
                 cco:ont00001754 "http://www.cfr.org/infrastructure/transportation-infrastructure-moving-america/p18611" ;
                 cco:ont00001760 "https://www.commoncoreontologies.org/ArtifactOntology"^^xsd:anyURI .


###  https://www.commoncoreontologies.org/ont00000333
cco:ont00000333 rdf:type owl:Class ;
                 rdfs:subClassOf cco:ont00000394 ;
                 rdfs:label "Gas Turbine"@en ;
                 skos:altLabel "Combustion Turbine"@en ;
                 skos:definition "An Internal Combustion Engine that has a rotating compressor and a turbine and is designed to operate utilizing continous Combustion to produce Thrust, either directly via exhaust or indirectly via a prop."@en ;
                 cco:ont00001754 "https://en.wikipedia.org/w/index.php?title=Gas_turbine&oldid=1062398125"^^xsd:anyURI ;
                 cco:ont00001760 "https://www.commoncoreontologies.org/ArtifactOntology"^^xsd:anyURI .


###  https://www.commoncoreontologies.org/ont00000334
cco:ont00000334 rdf:type owl:Class ;
                 rdfs:subClassOf cco:ont00000303 ;
                 rdfs:label "Interphone"@en ;
                 skos:definition "An Intercommunication System that that is designed to facilitate some Act of Communication between agents by means of audio messages."@en ;
                 cco:ont00001760 "https://www.commoncoreontologies.org/ArtifactOntology"^^xsd:anyURI .


###  https://www.commoncoreontologies.org/ont00000337
cco:ont00000337 rdf:type owl:Class ;
                 rdfs:subClassOf cco:ont00001029 ;
                 rdfs:label "Rocket-Propelled Grenade"@en ;
                 skos:definition "An Unguided Rocket that is designed to contain an explosive warhead, be fired from a Shoulder-Fired Rocket Launcher, and be used against Tanks."@en ;
                 cco:ont00001753 "RPG" ;
                 cco:ont00001754 "https://en.wikipedia.org/w/index.php?title=Rocket-propelled_grenade&oldid=1063641548"^^xsd:anyURI ;
                 cco:ont00001760 "https://www.commoncoreontologies.org/ArtifactOntology"^^xsd:anyURI .


###  https://www.commoncoreontologies.org/ont00000338
cco:ont00000338 rdf:type owl:Class ;
                 rdfs:subClassOf cco:ont00000256 ;
                 rdfs:label "Fan"@en ;
                 skos:definition "A Fluid Control Artifact that consists of a rotating arrangement of vanes or blades that are designed to act on a portion of fluid to create flow within it."@en ;
                 cco:ont00001754 "https://en.wikipedia.org/wiki/Fan_(machine)" ;
                 cco:ont00001760 "https://www.commoncoreontologies.org/ArtifactOntology"^^xsd:anyURI .


###  https://www.commoncoreontologies.org/ont00000340
cco:ont00000340 rdf:type owl:Class ;
                 rdfs:subClassOf cco:ont00000268 ;
                 rdfs:label "Mortar"@en ;
                 skos:definition "A Cannon that is designed to fire projectiles at relatively low velocities over relatively short ranges."@en ;
                 cco:ont00001754 "https://en.wikipedia.org/wiki/Mortar_(weapon)" ;
                 cco:ont00001760 "https://www.commoncoreontologies.org/ArtifactOntology"^^xsd:anyURI .


###  https://www.commoncoreontologies.org/ont00000341
cco:ont00000341 rdf:type owl:Class ;
                 rdfs:subClassOf cco:ont00000715 ;
                 rdfs:label "Prosthetic Arm"@en ;
                 skos:definition "A Prosthesis that is designed to replace a missing arm."@en ;
                 cco:ont00001754 "https://en.wikipedia.org/w/index.php?title=Prosthesis&oldid=1063749698"^^xsd:anyURI ;
                 cco:ont00001760 "https://www.commoncoreontologies.org/ArtifactOntology"^^xsd:anyURI .


###  https://www.commoncoreontologies.org/ont00000342
cco:ont00000342 rdf:type owl:Class ;
                 rdfs:subClassOf cco:ont00000995 ;
                 rdfs:label "Brake"@en ;
                 skos:definition "A Material Artifact that is designed to inhibit the Vehicle's Motion by absorbing energy from a moving system."@en ;
                 cco:ont00001754 "https://en.wikipedia.org/w/index.php?title=Brake&oldid=1047693009"^^xsd:anyURI ;
                 cco:ont00001760 "https://www.commoncoreontologies.org/ArtifactOntology"^^xsd:anyURI .


###  https://www.commoncoreontologies.org/ont00000343
cco:ont00000343 rdf:type owl:Class ;
                 rdfs:subClassOf cco:ont00000634 ;
                 rdfs:label "Reciprocating Steam Engine"@en ;
                 skos:definition "A Steam Engine that is designed to use one or more reciprocating pistons to convert pressure into a rotating motion."@en ;
                 cco:ont00001754 "https://en.wikipedia.org/w/index.php?title=Reciprocating_engine&oldid=1057783145"^^xsd:anyURI ;
                 cco:ont00001760 "https://www.commoncoreontologies.org/ArtifactOntology"^^xsd:anyURI .


###  https://www.commoncoreontologies.org/ont00000344
cco:ont00000344 rdf:type owl:Class ;
                 rdfs:subClassOf cco:ont00001281 ;
                 rdfs:label "Surfactant Artifact Function"@en ;
                 skos:definition "An Emulsifier Artifact Function that is realized in a process that lowers the surface tension between two liquids or between a liquid and a solid."@en ;
                 cco:ont00001754 "https://en.wikipedia.org/w/index.php?title=Surfactant&oldid=1063693411"^^xsd:anyURI ;
                 cco:ont00001760 "https://www.commoncoreontologies.org/ArtifactOntology"^^xsd:anyURI .


###  https://www.commoncoreontologies.org/ont00000346
cco:ont00000346 rdf:type owl:Class ;
                 rdfs:subClassOf cco:ont00000995 ;
                 rdfs:label "Communication Instrument"@en ;
                 skos:definition "A Material Artifact that is designed to facilitate communication between at least two entities."@en ;
                 cco:ont00001760 "https://www.commoncoreontologies.org/ArtifactOntology"^^xsd:anyURI .


###  https://www.commoncoreontologies.org/ont00000347
cco:ont00000347 rdf:type owl:Class ;
                 rdfs:subClassOf cco:ont00001159 ;
                 rdfs:label "Electronic Bond"@en ;
                 skos:definition "A Bond that consists of Bytes."@en ;
                 cco:ont00001760 "https://www.commoncoreontologies.org/ArtifactOntology"^^xsd:anyURI .


###  https://www.commoncoreontologies.org/ont00000348
cco:ont00000348 rdf:type owl:Class ;
                 owl:equivalentClass [ owl:intersectionOf ( cco:ont00000995
                                                            [ rdf:type owl:Restriction ;
                                                              owl:onProperty obo:BFO_0000196 ;
                                                              owl:someValuesFrom cco:ont00001999
                                                            ]
                                                          ) ;
                                       rdf:type owl:Class
                                     ] ;
                 rdfs:subClassOf cco:ont00000995 ;
                 rdfs:label "Filter"@en ;
                 skos:definition "A Material Artifact that bears a Filter Function."@en ;
                 cco:ont00001760 "https://www.commoncoreontologies.org/ArtifactOntology"^^xsd:anyURI .


###  https://www.commoncoreontologies.org/ont00000350
cco:ont00000350 rdf:type owl:Class ;
                 rdfs:subClassOf cco:ont00000453 ;
                 rdfs:label "Cooling System"@en ;
                 skos:definition "An Environment Control System that is designed to cool the air or objects in a Site."@en ;
                 cco:ont00001760 "https://www.commoncoreontologies.org/ArtifactOntology"^^xsd:anyURI .


###  https://www.commoncoreontologies.org/ont00000352
cco:ont00000352 rdf:type owl:Class ;
                 rdfs:subClassOf cco:ont00001139 ;
                 rdfs:label "Satellite Artifact"@en ;
                 skos:definition "A Spacecraft that is designed to Orbit a Space Object (typically Earth)."@en ;
                 cco:ont00001760 "https://www.commoncoreontologies.org/ArtifactOntology"^^xsd:anyURI .


###  https://www.commoncoreontologies.org/ont00000353
cco:ont00000353 rdf:type owl:Class ;
                 rdfs:subClassOf cco:ont00000323 ;
                 rdfs:label "Research Artifact Function"@en ;
                 skos:definition "An Artifact Function that is realized during events in which an Artifact is used to perform research on a specified entity or class of entities."@en ;
                 cco:ont00001760 "https://www.commoncoreontologies.org/ArtifactOntology"^^xsd:anyURI .


###  https://www.commoncoreontologies.org/ont00000355
cco:ont00000355 rdf:type owl:Class ;
                 rdfs:subClassOf cco:ont00001009 ;
                 rdfs:label "Refracting Optical Telescope"@en ;
                 skos:altLabel "Refracting Telescope"@en ,
                               "Refractor"@en ;
                 skos:definition "An Optical Telescope that is designed to aid in the observation of spatially distant Objects by means of collecting and focusing visible light via refraction through the use of one or more Lenses to form an enhanced image of the Object."@en ;
                 cco:ont00001754 "https://en.wikipedia.org/w/index.php?title=Refracting_telescope&oldid=1059975066"^^xsd:anyURI ;
                 cco:ont00001760 "https://www.commoncoreontologies.org/ArtifactOntology"^^xsd:anyURI .


###  https://www.commoncoreontologies.org/ont00000362
cco:ont00000362 rdf:type owl:Class ;
                 rdfs:subClassOf cco:ont00000533 ;
                 rdfs:comment "Most rocket engines are also Internal Combustion Engines, however non-combusting forms also exist. For example, an untied balloon full of air that is released and allowed to zoom around the room may be both a Rocket Engine and a Physically Powered Engine."@en ;
                 rdfs:label "Rocket Engine"@en ;
                 skos:altLabel "Thruster"@en ;
                 skos:definition "A Jet Engine that is designed to use only stored Rocket Propellant to form a high speed propulsive jet in order to generate Thrust."@en ;
                 cco:ont00001754 "https://en.wikipedia.org/w/index.php?title=Rocket_engine&oldid=1063879464"^^xsd:anyURI ;
                 cco:ont00001760 "https://www.commoncoreontologies.org/ArtifactOntology"^^xsd:anyURI .


###  https://www.commoncoreontologies.org/ont00000363
cco:ont00000363 rdf:type owl:Class ;
                 rdfs:subClassOf cco:ont00000998 ;
                 rdfs:label "Wireless Telecommunication Network"@en ;
                 skos:altLabel "Wireless Network"@en ;
                 skos:definition "A Telecommunication Network that uses wireless connections to connect Telecommunication Network Nodes."@en ;
                 cco:ont00001754 "https://en.wikipedia.org/w/index.php?title=Wireless_network&oldid=1060257041"^^xsd:anyURI ;
                 cco:ont00001760 "https://www.commoncoreontologies.org/ArtifactOntology"^^xsd:anyURI .


###  https://www.commoncoreontologies.org/ont00000364
cco:ont00000364 rdf:type owl:Class ;
                 rdfs:subClassOf cco:ont00001221 ;
                 rdfs:label "Pneumatic Motor"@en ;
                 skos:altLabel "Air Motor"@en ,
                               "Compressed Air Engine"@en ;
                 skos:definition "A Physically Powered Engine that converts potential energy stored in a portion of compressed air into mechanical energy."@en ;
                 cco:ont00001760 "https://www.commoncoreontologies.org/ArtifactOntology"^^xsd:anyURI .


###  https://www.commoncoreontologies.org/ont00000372
cco:ont00000372 rdf:type owl:Class ;
                 rdfs:subClassOf cco:ont00000995 ;
                 rdfs:label "Power Transformer Rectifier Unit"@en ;
                 skos:altLabel "TRU"@en ;
                 skos:definition "A Material Artifact that is designed to perform the functions of both a Rectifier and a Transformer."@en ;
                 cco:ont00001754 "http://www.skybrary.aero/index.php/Transformer_Rectifier_Unit_(TRU)" ;
                 cco:ont00001760 "https://www.commoncoreontologies.org/ArtifactOntology"^^xsd:anyURI .


###  https://www.commoncoreontologies.org/ont00000376
cco:ont00000376 rdf:type owl:Class ;
                 rdfs:subClassOf cco:ont00000457 ;
                 rdfs:label "Portion of Gallium Arsenide"@en ;
                 skos:altLabel "Portion of GaAs"@en ;
                 skos:definition "A Portion of Material that is composed of a compound of the elements gallium and arsenic."@en ;
                 cco:ont00001760 "https://www.commoncoreontologies.org/ArtifactOntology"^^xsd:anyURI .


###  https://www.commoncoreontologies.org/ont00000382
cco:ont00000382 rdf:type owl:Class ;
                 rdfs:subClassOf cco:ont00000798 ;
                 rdfs:label "Spreadsheet"@en ;
                 skos:definition "An Information Bearing Artifact that is designed to bear some Information Content Entity in an interactive, tabular form."@en ;
                 cco:ont00001754 "https://en.wikipedia.org/w/index.php?title=Spreadsheet&oldid=1064060503"^^xsd:anyURI ;
                 cco:ont00001760 "https://www.commoncoreontologies.org/ArtifactOntology"^^xsd:anyURI .


###  https://www.commoncoreontologies.org/ont00000394
cco:ont00000394 rdf:type owl:Class ;
                 rdfs:subClassOf cco:ont00000746 ;
                 rdfs:label "Internal Combustion Engine"@en ;
                 skos:definition "A Combustion Engine that is designed to have an internal Combustion Chamber where portions of Fuel and Oxidizer mixture are burned to generate thermal energy that is then converted into mechanical energy."@en ;
                 cco:ont00001754 "https://en.wikipedia.org/w/index.php?title=Internal_combustion_engine&oldid=1063281505"^^xsd:anyURI ;
                 cco:ont00001760 "https://www.commoncoreontologies.org/ArtifactOntology"^^xsd:anyURI .


###  https://www.commoncoreontologies.org/ont00000397
cco:ont00000397 rdf:type owl:Class ;
                 rdfs:subClassOf cco:ont00000995 ;
                 rdfs:label "Combustion Chamber"@en ;
                 skos:altLabel "Burner"@en ,
                               "Combustor"@en ,
                               "Flame Holder"@en ;
                 skos:definition "A Material Artifact that is designed to wholly or partially bound an internal Site where a Combustion process is intended to occur."@en ;
                 cco:ont00001760 "https://www.commoncoreontologies.org/ArtifactOntology"^^xsd:anyURI .


###  https://www.commoncoreontologies.org/ont00000403
cco:ont00000403 rdf:type owl:Class ;
                 rdfs:subClassOf cco:ont00000323 ;
                 rdfs:label "Diffraction Artifact Function"@en ;
                 skos:definition "An Artifact Function that is realized by an Artifact participating in a diffraction event in which the Artifact forces a wave to bend around the corners of an obstacle or aperture into the region of geometrical shadow of the obstacle."@en ;
                 cco:ont00001760 "https://www.commoncoreontologies.org/ArtifactOntology"^^xsd:anyURI .


###  https://www.commoncoreontologies.org/ont00000407
cco:ont00000407 rdf:type owl:Class ;
                 rdfs:subClassOf cco:ont00000098 ;
                 rdfs:label "Electrical Resistance Artifact Function"@en ;
                 skos:definition "An Electrical Artifact Function that is realized in processes in which an Artifact opposes the flow of an electric current."@en ;
                 cco:ont00001754 "https://en.wikipedia.org/w/index.php?title=Electrical_resistivity_and_conductivity&oldid=1063749049"^^xsd:anyURI ;
                 cco:ont00001760 "https://www.commoncoreontologies.org/ArtifactOntology"^^xsd:anyURI .


###  https://www.commoncoreontologies.org/ont00000409
cco:ont00000409 rdf:type owl:Class ;
                 rdfs:subClassOf cco:ont00000742 ;
                 rdfs:label "Spark Ignition System"@en ;
                 skos:definition "An Ignition System that is designed to produce a spark in order to initiate an Ignition process."@en ;
                 cco:ont00001760 "https://www.commoncoreontologies.org/ArtifactOntology"^^xsd:anyURI .


###  https://www.commoncoreontologies.org/ont00000411
cco:ont00000411 rdf:type owl:Class ;
                 rdfs:subClassOf cco:ont00001100 ;
                 rdfs:label "Speed Measurement Artifact Function"@en ;
                 skos:definition "A Measurement Artifact Function that is realized during events in which an Artifact is used to measure the Speed of a specified object's or class of objects' Motion."@en ;
                 cco:ont00001760 "https://www.commoncoreontologies.org/ArtifactOntology"^^xsd:anyURI .


###  https://www.commoncoreontologies.org/ont00000412
cco:ont00000412 rdf:type owl:Class ;
                 rdfs:subClassOf cco:ont00000791 ;
                 rdfs:label "Oxidizer Artifact Function"@en ;
                 skos:definition "A Chemical Reaction Artifact Function that is realized in a process in which electrons are removed from a reactant in a redox reaction."@en ;
                 cco:ont00001754 "https://en.wikipedia.org/w/index.php?title=Redox&oldid=1063866348"^^xsd:anyURI ;
                 cco:ont00001760 "https://www.commoncoreontologies.org/ArtifactOntology"^^xsd:anyURI .


###  https://www.commoncoreontologies.org/ont00000413
cco:ont00000413 rdf:type owl:Class ;
                 rdfs:subClassOf cco:ont00000304 ;
                 rdfs:label "Electron Microscope"@en ;
                 skos:definition "A Microscope that is designed to use a beam of accelerated electrons to illuminate the target and produce a significantly enlarged image of the Object."@en ;
                 cco:ont00001754 "https://en.wikipedia.org/w/index.php?title=Electron_microscope&oldid=1060512240"^^xsd:anyURI ;
                 cco:ont00001760 "https://www.commoncoreontologies.org/ArtifactOntology"^^xsd:anyURI .


###  https://www.commoncoreontologies.org/ont00000415
cco:ont00000415 rdf:type owl:Class ;
                 rdfs:subClassOf cco:ont00000828 ;
                 rdfs:label "Anti-Microbial Artifact Function"@en ;
                 skos:definition "A Pesticide Artifact Function that is realized in a process which causes illness in, or the death of, a microorganism."@en ;
                 cco:ont00001754 "https://en.wikipedia.org/w/index.php?title=Antimicrobial&oldid=1064100151"^^xsd:anyURI ;
                 cco:ont00001760 "https://www.commoncoreontologies.org/ArtifactOntology"^^xsd:anyURI .


###  https://www.commoncoreontologies.org/ont00000417
cco:ont00000417 rdf:type owl:Class ;
                 rdfs:subClassOf cco:ont00000715 ;
                 rdfs:label "Prosthetic Hand"@en ;
                 skos:definition "A Prosthesis that is designed to replace a missing hand."@en ;
                 cco:ont00001754 "https://en.wikipedia.org/w/index.php?title=Prosthesis&oldid=1063749698"^^xsd:anyURI ;
                 cco:ont00001760 "https://www.commoncoreontologies.org/ArtifactOntology"^^xsd:anyURI .


###  https://www.commoncoreontologies.org/ont00000420
cco:ont00000420 rdf:type owl:Class ;
                 rdfs:subClassOf cco:ont00000117 ;
                 rdfs:label "Computer"@en ;
                 skos:definition "An Information Processing Artifact that is designed to execute an arbitrary set of arithmetic or logical operations automatically."@en ;
                 cco:ont00001754 "https://en.wikipedia.org/w/index.php?title=Computer&oldid=1061553332"^^xsd:anyURI ;
                 cco:ont00001760 "https://www.commoncoreontologies.org/ArtifactOntology"^^xsd:anyURI .


###  https://www.commoncoreontologies.org/ont00000422
cco:ont00000422 rdf:type owl:Class ;
                 rdfs:subClassOf cco:ont00000323 ;
                 rdfs:label "Communication Reception Artifact Function"@en ;
                 skos:definition "An Artifact Function that is realized during events in which an Artifact is used to receive information that has been transmitted for the purpose of communiction."@en ;
                 cco:ont00001760 "https://www.commoncoreontologies.org/ArtifactOntology"^^xsd:anyURI .


###  https://www.commoncoreontologies.org/ont00000427
cco:ont00000427 rdf:type owl:Class ;
                 rdfs:subClassOf cco:ont00000053 ;
                 rdfs:label "Armored Fighting Vehicle"@en ;
                 skos:definition "A Ground Motor Vehicle that is designed to be armored and used to transport and support military personal in combat missions."@en ;
                 cco:ont00001754 "https://en.wikipedia.org/w/index.php?title=Armoured_fighting_vehicle&oldid=1063212018"^^xsd:anyURI ;
                 cco:ont00001760 "https://www.commoncoreontologies.org/ArtifactOntology"^^xsd:anyURI .


###  https://www.commoncoreontologies.org/ont00000428
cco:ont00000428 rdf:type owl:Class ;
                 rdfs:subClassOf cco:ont00001326 ;
                 rdfs:label "Railway Junction"@en ;
                 skos:definition "A Land Transportation Artifact that is designed to enable a Train to switch between the tracks of two routes."@en ;
                 cco:ont00001754 "https://en.wikipedia.org/wiki/Junction_(rail)" ;
                 cco:ont00001760 "https://www.commoncoreontologies.org/ArtifactOntology"^^xsd:anyURI .


###  https://www.commoncoreontologies.org/ont00000429
cco:ont00000429 rdf:type owl:Class ;
                 rdfs:subClassOf cco:ont00000258 ;
                 rdfs:label "Codabar Barcode"@en ;
                 skos:definition "A One-Dimensional Barcode that consists of numbers 0-9 and the characters -$:/.+ and is used by logistics and healthcare professionals."@en ;
                 cco:ont00001760 "https://www.commoncoreontologies.org/ArtifactOntology"^^xsd:anyURI .


###  https://www.commoncoreontologies.org/ont00000431
cco:ont00000431 rdf:type owl:Class ;
                 rdfs:subClassOf cco:ont00000746 ;
                 rdfs:label "External Combustion Engine"@en ;
                 skos:definition "A Combustion Engine that is designed to have an external Combustion Chamber where portions of Fuel and Oxidizer mixture are burned to generate thermal energy to heat the working fluid, which transfers energy to the Engine where it is converted into mechanical energy."@en ;
                 cco:ont00001754 "https://en.wikipedia.org/w/index.php?title=External_combustion_engine&oldid=1063941809"^^xsd:anyURI ;
                 cco:ont00001760 "https://www.commoncoreontologies.org/ArtifactOntology"^^xsd:anyURI .


###  https://www.commoncoreontologies.org/ont00000434
cco:ont00000434 rdf:type owl:Class ;
                 rdfs:subClassOf cco:ont00001207 ;
                 rdfs:label "Simple Optical Lens"@en ;
                 skos:definition "An Optical Lens consisting of a single piece of transparent material."@en ;
                 cco:ont00001760 "https://www.commoncoreontologies.org/ArtifactOntology"^^xsd:anyURI .


###  https://www.commoncoreontologies.org/ont00000436
cco:ont00000436 rdf:type owl:Class ;
                 rdfs:subClassOf cco:ont00000304 ;
                 rdfs:label "X-ray Microscope"@en ;
                 skos:definition "A Microscope that is designed to use Electromagnetic Radiation in the soft X-ray band to produce a significantly enlarged image of the Object."@en ;
                 cco:ont00001754 "https://en.wikipedia.org/w/index.php?title=X-ray_microscope&oldid=1046169107"^^xsd:anyURI ;
                 cco:ont00001760 "https://www.commoncoreontologies.org/ArtifactOntology"^^xsd:anyURI .


###  https://www.commoncoreontologies.org/ont00000437
cco:ont00000437 rdf:type owl:Class ;
                 rdfs:subClassOf cco:ont00000323 ;
                 rdfs:label "Enhancing Artifact Function"@en ;
                 skos:definition "An Artifact Function that is realized in processes of intensifying, increainsg, or further improving the quality, value, or extent of some entity."@en ;
                 cco:ont00001754 "https://en.wikipedia.org/w/index.php?title=Enhancement&oldid=1003326590"^^xsd:anyURI ;
                 cco:ont00001760 "https://www.commoncoreontologies.org/ArtifactOntology"^^xsd:anyURI .


###  https://www.commoncoreontologies.org/ont00000440
cco:ont00000440 rdf:type owl:Class ;
                 rdfs:subClassOf cco:ont00000713 ;
                 rdfs:label "Watercraft"@en ;
                 skos:definition "A Vehicle that is designed to convey passengers, cargo, or equipment from one location to another by water travel."@en ;
                 cco:ont00001754 "https://en.wikipedia.org/w/index.php?title=Watercraft&oldid=1054071067"^^xsd:anyURI ;
                 cco:ont00001760 "https://www.commoncoreontologies.org/ArtifactOntology"^^xsd:anyURI .


###  https://www.commoncoreontologies.org/ont00000445
cco:ont00000445 rdf:type owl:Class ;
                 rdfs:subClassOf cco:ont00000995 ;
                 rdfs:label "Weapon"@en ;
                 skos:definition "A Material Artifact that is designed to destroy or inflict damage to structures or systems, or to kill or wound living things by creating specific lethal or nonlethal effects."@en ;
                 skos:scopeNote "Nonlethal effects include all outcomes short of death or destruction. This is captured by the fact that Damaged Stasis and Wounded Stasis are defined in terms of impairment of the Independent Continuant that participates in them."@en ;
                 cco:ont00001754 "https://en.wikipedia.org/w/index.php?title=Weapon&oldid=1143263715"^^xsd:anyURI ;
                 cco:ont00001760 "https://www.commoncoreontologies.org/ArtifactOntology"^^xsd:anyURI .


###  https://www.commoncoreontologies.org/ont00000448
cco:ont00000448 rdf:type owl:Class ;
                 rdfs:subClassOf cco:ont00000323 ;
                 rdfs:label "Motion Artifact Function"@en ;
                 skos:definition "An Artifact Function that is realized in a process in which an entity changes its position with respect to time."@en ;
                 cco:ont00001754 "https://en.wikipedia.org/wiki/Motion_(physics)" ;
                 cco:ont00001760 "https://www.commoncoreontologies.org/ArtifactOntology"^^xsd:anyURI .


###  https://www.commoncoreontologies.org/ont00000451
cco:ont00000451 rdf:type owl:Class ;
                 rdfs:subClassOf cco:ont00000323 ;
                 rdfs:label "Collimation Artifact Function"@en ;
                 skos:definition "An Artifact Function that is realized by an Artifact participating in a collimation event in which the Artifact narrows a beam of particles or waves by either causing the spatial cross-section of the beam to become smaller or by causing the directions of motion of the beam's constituents to be aligned in a specifc direction of Motion."@en ;
                 cco:ont00001760 "https://www.commoncoreontologies.org/ArtifactOntology"^^xsd:anyURI .


###  https://www.commoncoreontologies.org/ont00000452
cco:ont00000452 rdf:type owl:Class ;
                 rdfs:subClassOf cco:ont00000323 ;
                 rdfs:label "Timekeeping Artifact Function"@en ;
                 skos:definition "An Artifact Function that is realized during events in which an Artifact is used to keep track of and report the current time."@en ;
                 cco:ont00001760 "https://www.commoncoreontologies.org/ArtifactOntology"^^xsd:anyURI .


###  https://www.commoncoreontologies.org/ont00000453
cco:ont00000453 rdf:type owl:Class ;
                 rdfs:subClassOf cco:ont00000995 ;
                 rdfs:comment "Controlling air quality typically involves temperature control, oxygen replenishment, and removal of moisture, odor, smoke, heat, dust, airborne bacteria, carbon dioxide, and other undesired gases or particulates."@en ;
                 rdfs:label "Environment Control System"@en ;
                 skos:definition "A Material Artifact that is designed to control the temperature, air quality, or other feature of a Site that is relevant to the comfort or operation of entities located within that Site."@en ;
                 cco:ont00001760 "https://www.commoncoreontologies.org/ArtifactOntology"^^xsd:anyURI .


###  https://www.commoncoreontologies.org/ont00000454
cco:ont00000454 rdf:type owl:Class ;
                 rdfs:subClassOf cco:ont00000742 ;
                 rdfs:label "Compression Ignition System"@en ;
                 skos:definition "An Ignition System that is designed to generate heat by compressing a portion of fuel and oxidizer mixture in order to initiate an Ignition process."@en ;
                 cco:ont00001760 "https://www.commoncoreontologies.org/ArtifactOntology"^^xsd:anyURI .


###  https://www.commoncoreontologies.org/ont00000456
cco:ont00000456 rdf:type owl:Class ;
                 rdfs:subClassOf cco:ont00001326 ;
                 rdfs:label "Railway"@en ;
                 skos:definition "A Land Transportation Artifact that is designed to enable Trains to transport passengers and goods."@en ;
                 cco:ont00001754 "https://en.wikipedia.org/w/index.php?title=Rail_transport&oldid=1063793805" ;
                 cco:ont00001760 "https://www.commoncoreontologies.org/ArtifactOntology"^^xsd:anyURI .


###  https://www.commoncoreontologies.org/ont00000457
cco:ont00000457 rdf:type owl:Class ;
                 rdfs:subClassOf cco:ont00001084 ;
                 rdfs:label "Portion of Material"@en ;
                 skos:definition "A Portion of Processed Material that was produced to be used as the input for another Act of Artifact Processing."@en ;
                 cco:ont00001760 "https://www.commoncoreontologies.org/ArtifactOntology"^^xsd:anyURI .


###  https://www.commoncoreontologies.org/ont00000458
cco:ont00000458 rdf:type owl:Class ;
                 rdfs:subClassOf cco:ont00000995 ;
                 rdfs:label "Coupling"@en ;
                 skos:definition "A Material Artifact that is designed to connect two Shafts together at their ends for the purpose of transmitting power."@en ;
                 cco:ont00001754 "https://en.wikipedia.org/w/index.php?title=Coupling&oldid=1055718683"^^xsd:anyURI ;
                 cco:ont00001760 "https://www.commoncoreontologies.org/ArtifactOntology"^^xsd:anyURI .


###  https://www.commoncoreontologies.org/ont00000461
cco:ont00000461 rdf:type owl:Class ;
                 rdfs:subClassOf cco:ont00000966 ;
                 rdfs:label "ISSN Barcode"@en ;
                 skos:definition "An EAN Barcode that is used to designate periodicals."@en ;
                 cco:ont00001760 "https://www.commoncoreontologies.org/ArtifactOntology"^^xsd:anyURI .


###  https://www.commoncoreontologies.org/ont00000466
cco:ont00000466 rdf:type owl:Class ;
                 rdfs:subClassOf cco:ont00000323 ;
                 rdfs:label "Orientation Control Artifact Function"@en ;
                 skos:definition "An Artifact Function that is realized by processes in which some Artifact is used to control the Orientation of some object."@en ;
                 cco:ont00001760 "https://www.commoncoreontologies.org/ArtifactOntology"^^xsd:anyURI .


###  https://www.commoncoreontologies.org/ont00000467
cco:ont00000467 rdf:type owl:Class ;
                 rdfs:subClassOf cco:ont00000427 ;
                 rdfs:label "Armored Personnel Carrier"@en ;
                 skos:definition "An Armored Fighting Vehicle that is designed to transport infantry to the battlefield but which are not usually designed to take part in a direct-fire battle."@en ;
                 cco:ont00001753 "APC" ;
                 cco:ont00001754 "https://en.wikipedia.org/w/index.php?title=Armoured_personnel_carrier&oldid=1061608326"^^xsd:anyURI ;
                 cco:ont00001760 "https://www.commoncoreontologies.org/ArtifactOntology"^^xsd:anyURI .


###  https://www.commoncoreontologies.org/ont00000470
cco:ont00000470 rdf:type owl:Class ;
                 rdfs:subClassOf cco:ont00000189 ;
                 rdfs:label "Academic Degree"@en ;
                 skos:definition "A Certificate issued by an Educational Organization to a Person to indicate that the Person has satisfactorily completed a course of study, or as an honorary recognition of the Person's achievement."@en ;
                 cco:ont00001754 "http://www.dictionary.com/browse/degree" ;
                 cco:ont00001760 "https://www.commoncoreontologies.org/ArtifactOntology"^^xsd:anyURI .


###  https://www.commoncoreontologies.org/ont00000471
cco:ont00000471 rdf:type owl:Class ;
                 rdfs:subClassOf cco:ont00001046 ;
                 rdfs:label "Warning Message"@en ;
                 skos:definition "A Notification Message that is designed to bear an Information Content Entity that describes a possible or impending threat."@en ;
                 cco:ont00001760 "https://www.commoncoreontologies.org/ArtifactOntology"^^xsd:anyURI .


###  https://www.commoncoreontologies.org/ont00000475
cco:ont00000475 rdf:type owl:Class ;
                 rdfs:subClassOf cco:ont00000537 ;
                 rdfs:label "Portion of Cash"@en ;
                 skos:definition "A Financial Instrument that is designed to be a ready medium of exchange."@en ;
                 cco:ont00001760 "https://www.commoncoreontologies.org/ArtifactOntology"^^xsd:anyURI .


###  https://www.commoncoreontologies.org/ont00000477
cco:ont00000477 rdf:type owl:Class ;
                 rdfs:subClassOf cco:ont00001049 ;
                 rdfs:label "Fuel Cell"@en ;
                 skos:definition "An Electrical Power Source that consists in part of an anode, a cathode, and an electrolyte; converts chemical energy from a fuel into electricity through a chemical reaction of positively charged hydrogen ions with an oxidizing agent (typically oxygen); and, if given a continuous source of fuel and oxidizing agent, can continuously produce electricity."@en ;
                 skos:scopeNote "A Fuel Cell differs from a Battery in that it requires a continuous source of fuel and oxygen to sustain the chemical reaction, whereas a Battery only uses chemicals already stored inside it."@en ;
                 cco:ont00001754 "https://en.wikipedia.org/w/index.php?title=Fuel_cell&oldid=1063586731"^^xsd:anyURI ;
                 cco:ont00001760 "https://www.commoncoreontologies.org/ArtifactOntology"^^xsd:anyURI .


###  https://www.commoncoreontologies.org/ont00000480
cco:ont00000480 rdf:type owl:Class ;
                 rdfs:subClassOf cco:ont00000323 ;
                 rdfs:label "Life Support Artifact Function"@en ;
                 skos:definition "An Artifact Function that is realized during events in which an Artifact materially affects an organism, where this causes that organism to continue living in a situation where death would otherwise occur."@en ;
                 cco:ont00001760 "https://www.commoncoreontologies.org/ArtifactOntology"^^xsd:anyURI .


###  https://www.commoncoreontologies.org/ont00000481
cco:ont00000481 rdf:type owl:Class ;
                 rdfs:subClassOf cco:ont00001301 ;
                 rdfs:label "Research and Development Artifact Function"@en ;
                 skos:definition "A Service Artifact Function that is realized in processes of producing new knowledge or of devising new applications of existing knowledge."@en ;
                 cco:ont00001754 "https://en.wikipedia.org/w/index.php?title=Research_and_development&oldid=1062181110"^^xsd:anyURI ;
                 cco:ont00001760 "https://www.commoncoreontologies.org/ArtifactOntology"^^xsd:anyURI .


###  https://www.commoncoreontologies.org/ont00000482
cco:ont00000482 rdf:type owl:Class ;
                 rdfs:subClassOf cco:ont00000289 ;
                 rdfs:label "Synthetic Aperture Radar Imaging Artifact Function"@en ;
                 skos:definition "A Radar Imaging Artifact Function that inheres in Artifacts that are designed to produce visual representations of entities using the motion of a radar antenna over a targeted region to create a synthetic aperture."@en ;
                 cco:ont00001760 "https://www.commoncoreontologies.org/ArtifactOntology"^^xsd:anyURI .


###  https://www.commoncoreontologies.org/ont00000488
cco:ont00000488 rdf:type owl:Class ;
                 rdfs:subClassOf cco:ont00000995 ;
                 rdfs:label "Tripod"@en ;
                 skos:definition "A Material Artifact that consists of three legs and a platform that joins them and which is designed to support the weight and maintain the stability of objects that are attached to or rested on the platform."@en ;
                 cco:ont00001754 "https://en.wikipedia.org/w/index.php?title=Tripod&oldid=1063988190"^^xsd:anyURI ;
                 cco:ont00001760 "https://www.commoncoreontologies.org/ArtifactOntology"^^xsd:anyURI .


###  https://www.commoncoreontologies.org/ont00000491
cco:ont00000491 rdf:type owl:Class ;
                 rdfs:subClassOf cco:ont00000323 ;
                 rdfs:label "Detonating Artifact Function"@en ;
                 skos:definition "An Artifact Function that is realized in processes of combustion involving a supersonic exothermic front accelerating through a medium that eventually drives a shock front propagating directly in front of it."@en ;
                 cco:ont00001754 "https://en.wikipedia.org/w/index.php?title=Detonation&oldid=1061553336"^^xsd:anyURI ;
                 cco:ont00001760 "https://www.commoncoreontologies.org/ArtifactOntology"^^xsd:anyURI .


###  https://www.commoncoreontologies.org/ont00000493
cco:ont00000493 rdf:type owl:Class ;
                 rdfs:subClassOf cco:ont00000799 ;
                 rdfs:label "Code List"@en ;
                 skos:definition "A List that contains an ordered sequence of Information Bearing Entities that carry Code Identifiers."@en ;
                 cco:ont00001760 "https://www.commoncoreontologies.org/ArtifactOntology"^^xsd:anyURI .


###  https://www.commoncoreontologies.org/ont00000495
cco:ont00000495 rdf:type owl:Class ;
                 rdfs:subClassOf cco:ont00000273 ;
                 rdfs:label "Radio Communication Interference Artifact Function"@en ;
                 skos:definition "A Communication Interference Artifact Function that is realized during events in which an Artifact is used to interfere with the transmission of information via radio waves."@en ;
                 cco:ont00001760 "https://www.commoncoreontologies.org/ArtifactOntology"^^xsd:anyURI .


###  https://www.commoncoreontologies.org/ont00000499
cco:ont00000499 rdf:type owl:Class ;
                 rdfs:subClassOf cco:ont00001192 ;
                 rdfs:label "Wire Antenna"@en ;
                 skos:definition "A Radio Antenna that consists primarily of a length of wire."@en ;
                 cco:ont00001760 "https://www.commoncoreontologies.org/ArtifactOntology"^^xsd:anyURI .


###  https://www.commoncoreontologies.org/ont00000504
cco:ont00000504 rdf:type owl:Class ;
                 rdfs:subClassOf cco:ont00000323 ;
                 rdfs:label "Optical Processing Artifact Function"@en ;
                 skos:definition "An Artifact Function that is realized by an Artifact participating in a visible light processing event."@en ;
                 cco:ont00001760 "https://www.commoncoreontologies.org/ArtifactOntology"^^xsd:anyURI .


###  https://www.commoncoreontologies.org/ont00000516
cco:ont00000516 rdf:type owl:Class ;
                 rdfs:subClassOf cco:ont00000288 ;
                 rdfs:label "Pneumatic Power Source"@en ;
                 skos:definition "A Power Source that is designed to generate, control, or transmit power by means of compressed air or compressed inert gases."@en ;
                 cco:ont00001760 "https://www.commoncoreontologies.org/ArtifactOntology"^^xsd:anyURI .


###  https://www.commoncoreontologies.org/ont00000522
cco:ont00000522 rdf:type owl:Class ;
                 rdfs:subClassOf cco:ont00000294 ;
                 rdfs:label "Pulsejet Engine"@en ;
                 skos:altLabel "Pulse Jet"@en ,
                               "Pulsejet"@en ;
                 skos:definition "An Air-Breathing Jet Engine that is capable of operating statically and uses intermittent (pulsing) Combustion of the fuel-oxidizer mixture before expelling the exhaust out through the rear Propelling Nozzle to generate Thrust."@en ;
                 cco:ont00001754 "https://en.wikipedia.org/w/index.php?title=Pulsejet&oldid=1050473545"^^xsd:anyURI ;
                 cco:ont00001760 "https://www.commoncoreontologies.org/ArtifactOntology"^^xsd:anyURI .


###  https://www.commoncoreontologies.org/ont00000524
cco:ont00000524 rdf:type owl:Class ;
                 rdfs:subClassOf cco:ont00000350 ;
                 rdfs:label "Air Conditioning Unit"@en ;
                 skos:altLabel "AC Unit"@en ;
                 skos:definition "A Cooling System that is designed to remove excess heat and humidity from the air in an enclosed space."@en ;
                 cco:ont00001754 "https://en.wikipedia.org/w/index.php?title=Air_conditioning&oldid=1063494896"^^xsd:anyURI ;
                 cco:ont00001760 "https://www.commoncoreontologies.org/ArtifactOntology"^^xsd:anyURI .


###  https://www.commoncoreontologies.org/ont00000526
cco:ont00000526 rdf:type owl:Class ;
                 rdfs:subClassOf cco:ont00000547 ;
                 rdfs:label "Gamma-ray Telescope"@en ;
                 skos:definition "A Telescope that is designed to aid in the observation of spatially distant Objects by means of collecting and focusing Gamma-rays to form an enhanced image of the Object."@en ;
                 cco:ont00001754 "https://en.wikipedia.org/w/index.php?title=Telescope&oldid=1057722342"^^xsd:anyURI ;
                 cco:ont00001760 "https://www.commoncoreontologies.org/ArtifactOntology"^^xsd:anyURI .


###  https://www.commoncoreontologies.org/ont00000533
cco:ont00000533 rdf:type owl:Class ;
                 rdfs:subClassOf cco:ont00000056 ;
                 rdfs:comment "Some (most) jet engines utilize turbines, but some do not. Most rocket engines do not utilize turbines, but some do."@en ;
                 rdfs:label "Jet Engine"@en ;
                 skos:definition "A Reaction Engine that discharges a fast moving jet that generates Thrust by jet propulsion."@en ;
                 cco:ont00001754 "https://en.wikipedia.org/w/index.php?title=Jet_engine&oldid=1060157063"^^xsd:anyURI ;
                 cco:ont00001760 "https://www.commoncoreontologies.org/ArtifactOntology"^^xsd:anyURI .


###  https://www.commoncoreontologies.org/ont00000534
cco:ont00000534 rdf:type owl:Class ;
                 rdfs:subClassOf cco:ont00001153 ;
                 rdfs:label "Cutting Artifact Function"@en ;
                 skos:definition "A Damaging Artifact Function that is realized in a process in which the structural integrity of an entity is impaired by being opened or divided."@en ;
                 cco:ont00001754 "http://www.dictionary.com/browse/cutting" ;
                 cco:ont00001760 "https://www.commoncoreontologies.org/ArtifactOntology"^^xsd:anyURI .


###  https://www.commoncoreontologies.org/ont00000536
cco:ont00000536 rdf:type owl:Class ;
                 rdfs:subClassOf cco:ont00001159 ;
                 rdfs:label "Bond Certificate"@en ;
                 skos:definition "A Bond that consists of a Certificate."@en ;
                 cco:ont00001760 "https://www.commoncoreontologies.org/ArtifactOntology"^^xsd:anyURI .


###  https://www.commoncoreontologies.org/ont00000537
cco:ont00000537 rdf:type owl:Class ;
                 rdfs:subClassOf cco:ont00000995 ;
                 rdfs:label "Financial Instrument"@en ;
                 skos:definition "A Material Artifact that is designed to be a tradeable asset and that is legally sanctioned."@en ;
                 cco:ont00001754 "https://en.wikipedia.org/w/index.php?title=Finance&oldid=1062402926"^^xsd:anyURI ;
                 cco:ont00001760 "https://www.commoncoreontologies.org/ArtifactOntology"^^xsd:anyURI .


###  https://www.commoncoreontologies.org/ont00000538
cco:ont00000538 rdf:type owl:Class ;
                 rdfs:subClassOf cco:ont00000831 ;
                 rdfs:label "Defoliant Artifact Function"@en ;
                 skos:definition "An Herbicide Artifact Function that is realized in a process that causes a plant to lose its leaves."@en ;
                 cco:ont00001754 "https://en.wikipedia.org/w/index.php?title=Defoliant&oldid=1059494225"^^xsd:anyURI ;
                 cco:ont00001760 "https://www.commoncoreontologies.org/ArtifactOntology"^^xsd:anyURI .


###  https://www.commoncoreontologies.org/ont00000547
cco:ont00000547 rdf:type owl:Class ;
                 rdfs:subClassOf cco:ont00000771 ;
                 rdfs:label "Telescope"@en ;
                 skos:definition "An Imaging Instrument that is designed to aid in the observation of spatially distant Objects by means of collecting and focusing Electromagnetic Radiation to form an enhanced image of the Object."@en ;
                 cco:ont00001754 "https://en.wikipedia.org/w/index.php?title=Telescope&oldid=1057722342"^^xsd:anyURI ;
                 cco:ont00001760 "https://www.commoncoreontologies.org/ArtifactOntology"^^xsd:anyURI .


###  https://www.commoncoreontologies.org/ont00000549
cco:ont00000549 rdf:type owl:Class ;
                 rdfs:subClassOf cco:ont00000254 ;
                 rdfs:label "Water Transportation Artifact"@en ;
                 skos:definition "A Transportation Artifact that is fixed in place and designed to bear a Function, the realization of which is sometimes part of a process of moving Vehicles and Agents from one location to another via water."@en ;
                 cco:ont00001760 "https://www.commoncoreontologies.org/ArtifactOntology"^^xsd:anyURI .


###  https://www.commoncoreontologies.org/ont00000552
cco:ont00000552 rdf:type owl:Class ;
                 rdfs:subClassOf cco:ont00000445 ;
                 rdfs:label "Explosive Weapon"@en ;
                 skos:altLabel "Bomb"@en ;
                 skos:definition "A Weapon that is designed to inflict harm, damage, or incapacity by means of a violent release of energy caused by the exothermic reaction of an explosive material."@en ;
                 cco:ont00001754 "https://en.wikipedia.org/w/index.php?title=Explosive_weapon&oldid=1062481268"^^xsd:anyURI ;
                 cco:ont00001760 "https://www.commoncoreontologies.org/ArtifactOntology"^^xsd:anyURI .


###  https://www.commoncoreontologies.org/ont00000556
cco:ont00000556 rdf:type owl:Class ;
                 rdfs:subClassOf obo:BFO_0000040 ;
                 rdfs:comment "Depending on the nature of the Flight or Mission, the Payload of a Vehicle may include cargo, passengers, flight crew, munitions, scientific instruments or experiments, or other equipment. Extra fuel, when optionally carried, is also considered part of the payload."@en ;
                 rdfs:label "Payload"@en ;
                 skos:definition "A Material Entity that is transported by a Vehicle during an Act of Location Change for the purpose of being delivered to or performing one or more functions at a predefined location."@en ;
                 skos:scopeNote "In each case, the Payload is what provides the immediate reason for performing the Act of Location Change (e.g. transporting the passengers of a commercial airline flight to their destination; transporting food, fuel, oxygen, research equipment, and spare parts to the International Space Station; or conveying an array of sensors, cameras, and communications systems so they can operate during a Sun-Synchronous Earth Orbit)."@en ;
                 cco:ont00001754 "https://en.wikipedia.org/w/index.php?title=Payload&oldid=1035953573"^^xsd:anyURI ;
                 cco:ont00001760 "https://www.commoncoreontologies.org/ArtifactOntology"^^xsd:anyURI .


###  https://www.commoncoreontologies.org/ont00000559
cco:ont00000559 rdf:type owl:Class ;
                 rdfs:subClassOf cco:ont00000241 ;
                 rdfs:label "QR Code"@en ;
                 skos:definition "A Two-Dimensional Barcode that consists of numeric, alphanumeric, binary, or kanji information and is used primarily for tracking and marketing."@en ;
                 cco:ont00001760 "https://www.commoncoreontologies.org/ArtifactOntology"^^xsd:anyURI .


###  https://www.commoncoreontologies.org/ont00000561
cco:ont00000561 rdf:type owl:Class ;
                 rdfs:subClassOf cco:ont00000995 ;
                 rdfs:label "Dam"@en ;
                 skos:definition "A Material Artifact that is designed to impound surface water or underground streams."@en ;
                 cco:ont00001754 "https://en.wikipedia.org/w/index.php?title=Dam&oldid=1053601756" ;
                 cco:ont00001760 "https://www.commoncoreontologies.org/ArtifactOntology"^^xsd:anyURI .


###  https://www.commoncoreontologies.org/ont00000569
cco:ont00000569 rdf:type owl:Class ;
                 rdfs:subClassOf cco:ont00000736 ;
                 rdfs:label "Sensor"@en ;
                 skos:definition "A Transducer that is designed to convert incoming energy into a output signal which reliably corresponds to changes in that energy."@en ;
                 cco:ont00001754 "https://en.wikipedia.org/w/index.php?title=Sensor&oldid=1059883466"^^xsd:anyURI ;
                 cco:ont00001760 "https://www.commoncoreontologies.org/ArtifactOntology"^^xsd:anyURI .


###  https://www.commoncoreontologies.org/ont00000571
cco:ont00000571 rdf:type owl:Class ;
                 rdfs:subClassOf cco:ont00000980 ;
                 rdfs:label "Article of Solid Waste"@en ;
                 skos:definition "A Portion of Waste Material that has a low liquid content."@en ;
                 cco:ont00001754 "https://stats.oecd.org/glossary/detail.asp?ID=2508" ;
                 cco:ont00001760 "https://www.commoncoreontologies.org/ArtifactOntology"^^xsd:anyURI .


###  https://www.commoncoreontologies.org/ont00000575
cco:ont00000575 rdf:type owl:Class ;
                 owl:equivalentClass [ owl:intersectionOf ( cco:ont00000965
                                                            [ rdf:type owl:Restriction ;
                                                              owl:onProperty cco:ont00001942 ;
                                                              owl:someValuesFrom obo:BFO_0000019
                                                            ]
                                                          ) ;
                                       rdf:type owl:Class
                                     ] ;
                 rdfs:subClassOf cco:ont00000965 ;
                 rdfs:label "Quality Specification"@en ;
                 skos:definition "A Directive Information Content Entity that prescribes some Quality."@en ;
                 cco:ont00001760 "https://www.commoncoreontologies.org/ArtifactOntology"^^xsd:anyURI .


###  https://www.commoncoreontologies.org/ont00000577
cco:ont00000577 rdf:type owl:Class ;
                 rdfs:subClassOf cco:ont00000995 ;
                 rdfs:label "Power Rectifier"@en ;
                 skos:definition "A Material Artifact that is designed to convert alternating current (AC) to direct current (DC)."@en ;
                 cco:ont00001754 "https://en.wikipedia.org/w/index.php?title=Rectifier&oldid=1049943028"^^xsd:anyURI ;
                 cco:ont00001760 "https://www.commoncoreontologies.org/ArtifactOntology"^^xsd:anyURI .


###  https://www.commoncoreontologies.org/ont00000581
cco:ont00000581 rdf:type owl:Class ;
                 rdfs:subClassOf cco:ont00000995 ;
                 rdfs:label "Tool"@en ;
                 skos:definition "A Material Artifact that is designed to assist in the performance of manual or mechanical work and not to be consumed in that process."@en ;
                 cco:ont00001754 "https://en.wikipedia.org/w/index.php?title=Tool&oldid=1061967184"^^xsd:anyURI ;
                 cco:ont00001760 "https://www.commoncoreontologies.org/ArtifactOntology"^^xsd:anyURI .


###  https://www.commoncoreontologies.org/ont00000582
cco:ont00000582 rdf:type owl:Class ;
                 rdfs:subClassOf cco:ont00000258 ;
                 rdfs:label "Code 93 Barcode"@en ;
                 skos:definition "A One-Dimensional Barcode that consists of up to 93 ASCII characters and is used in logistics to identify packages in retail inventory, lable electornic components, and provide supplementary delivery information."@en ;
                 cco:ont00001760 "https://www.commoncoreontologies.org/ArtifactOntology"^^xsd:anyURI .


###  https://www.commoncoreontologies.org/ont00000586
cco:ont00000586 rdf:type owl:Class ;
                 rdfs:subClassOf cco:ont00000238 ;
                 rdfs:label "Controllable Pitch Propeller"@en ;
                 skos:altLabel "Variable-Pitch Propeller"@en ;
                 skos:definition "A Propeller whose blades are designed to be alterable by rotating the blades about their vertical axis by means of mechanical or hydraulic arrangement."@en ;
                 cco:ont00001754 "https://en.wikipedia.org/w/index.php?title=Variable-pitch_propeller&oldid=1041375492"^^xsd:anyURI ;
                 cco:ont00001760 "https://www.commoncoreontologies.org/ArtifactOntology"^^xsd:anyURI .


###  https://www.commoncoreontologies.org/ont00000591
cco:ont00000591 rdf:type owl:Class ;
                 owl:equivalentClass [ owl:intersectionOf ( obo:BFO_0000029
                                                            [ rdf:type owl:Restriction ;
                                                              owl:onProperty obo:BFO_0000124 ;
                                                              owl:someValuesFrom cco:ont00000995
                                                            ]
                                                          ) ;
                                       rdf:type owl:Class
                                     ] ;
                 rdfs:subClassOf obo:BFO_0000029 ;
                 rdfs:label "Artifact Location"@en ;
                 skos:definition "A Site that is the location of some Artifact."@en ;
                 cco:ont00001760 "https://www.commoncoreontologies.org/ArtifactOntology"^^xsd:anyURI .


###  https://www.commoncoreontologies.org/ont00000593
cco:ont00000593 rdf:type owl:Class ;
                 rdfs:subClassOf cco:ont00000457 ;
                 rdfs:label "Portion of Propellant"@en ;
                 skos:definition "A Portion of Material that is designed to be used as an input in a Propulsion Process to produce Thrust."@en ;
                 cco:ont00001760 "https://www.commoncoreontologies.org/ArtifactOntology"^^xsd:anyURI .


###  https://www.commoncoreontologies.org/ont00000596
cco:ont00000596 rdf:type owl:Class ;
                 rdfs:subClassOf cco:ont00000966 ;
                 rdfs:label "JAN-13 Barcode"@en ;
                 skos:definition "An EAN Barcode that consists of 13 numerical digits and is used primarily in Japan to designate products at the point of sale."@en ;
                 cco:ont00001760 "https://www.commoncoreontologies.org/ArtifactOntology"^^xsd:anyURI .


###  https://www.commoncoreontologies.org/ont00000597
cco:ont00000597 rdf:type owl:Class ;
                 rdfs:subClassOf cco:ont00000798 ;
                 rdfs:label "Instrument Display Panel"@en ;
                 skos:definition "An Information Bearing Artifact that is designed to bear information about some Artifact that is derived by the instrumentation Sensors of that Artifact."@en ;
                 cco:ont00001754 "https://en.wikipedia.org/w/index.php?title=Flight_instruments&oldid=1062972990"^^xsd:anyURI ;
                 cco:ont00001760 "https://www.commoncoreontologies.org/ArtifactOntology"^^xsd:anyURI .


###  https://www.commoncoreontologies.org/ont00000598
cco:ont00000598 rdf:type owl:Class ;
                 rdfs:subClassOf cco:ont00000256 ;
                 rdfs:label "Valve"@en ;
                 skos:definition "A Fluid Control Artifact that is designed to regulate, direct, or control the flow of fluid by opening, closing, or partially obstructing the fluid from moving along a passageway."@en ;
                 cco:ont00001754 "https://en.wikipedia.org/w/index.php?title=Valve&oldid=1048906126"^^xsd:anyURI ;
                 cco:ont00001760 "https://www.commoncoreontologies.org/ArtifactOntology"^^xsd:anyURI .


###  https://www.commoncoreontologies.org/ont00000600
cco:ont00000600 rdf:type owl:Class ;
                 rdfs:subClassOf cco:ont00001301 ;
                 rdfs:label "Legal Artifact Function"@en ;
                 skos:definition "A Service Artifact Function that is realized in processes of giving legal advice to clients drafting legal documents for clients and representing clients in legal negotiations and court proceedings such as lawsuits."@en ;
                 cco:ont00001754 "https://en.wikipedia.org/w/index.php?title=Law&oldid=1060821734"^^xsd:anyURI ;
                 cco:ont00001760 "https://www.commoncoreontologies.org/ArtifactOntology"^^xsd:anyURI .


###  https://www.commoncoreontologies.org/ont00000601
cco:ont00000601 rdf:type owl:Class ;
                 rdfs:subClassOf cco:ont00000323 ;
                 rdfs:label "Imaging Artifact Function"@en ;
                 skos:definition "An Artifact Function that inheres in Artifacts that are designed to produce visual representations of entities."@en ;
                 cco:ont00001760 "https://www.commoncoreontologies.org/ArtifactOntology"^^xsd:anyURI .


###  https://www.commoncoreontologies.org/ont00000602
cco:ont00000602 rdf:type owl:Class ;
                 rdfs:subClassOf cco:ont00000258 ;
                 rdfs:label "ITF Barcode"@en ;
                 skos:definition "A One-Dimensional Barcode that consists of an even number of numerical characters and is used primarily in packaging and distribution."@en ;
                 cco:ont00001760 "https://www.commoncoreontologies.org/ArtifactOntology"^^xsd:anyURI .


###  https://www.commoncoreontologies.org/ont00000603
cco:ont00000603 rdf:type owl:Class ;
                 rdfs:subClassOf cco:ont00000323 ;
                 rdfs:label "Navigation Artifact Function"@en ;
                 skos:definition "An Artifact Function that is realized during events in which an Artifact is used to determine the precise location of itself or another object and plan a route to a specified destination."@en ;
                 cco:ont00001760 "https://www.commoncoreontologies.org/ArtifactOntology"^^xsd:anyURI .


###  https://www.commoncoreontologies.org/ont00000606
cco:ont00000606 rdf:type owl:Class ;
                 rdfs:subClassOf cco:ont00000053 ;
                 rdfs:comment "Trucks vary greatly in their size and power -- ranging from small ultra-light trucks to enormous heavy trucks. Trucks also vary greatly in their configurations -- ranging from very basic flatbeds or box trucks to highly specialized cargo carriers. Trucks may also be configured to mount specialized equipment, such as in the case of fire trucks, concrete mixers, and suction excavators."@en ;
                 rdfs:label "Truck"@en ;
                 skos:definition "A Ground Motor Vehicle that is designed to be used to transport cargo."@en ;
                 cco:ont00001754 "https://en.wikipedia.org/w/index.php?title=Truck&oldid=1060924486"^^xsd:anyURI ;
                 cco:ont00001760 "https://www.commoncoreontologies.org/ArtifactOntology"^^xsd:anyURI .


###  https://www.commoncoreontologies.org/ont00000617
cco:ont00000617 rdf:type owl:Class ;
                 rdfs:subClassOf cco:ont00000199 ;
                 rdfs:label "Infrared Camera"@en ;
                 skos:altLabel "Thermal Imaging Camera"@en ,
                               "Thermographic Camera"@en ;
                 skos:definition "A Camera that is designed to form and record an image generated from infrared radiation."@en ;
                 cco:ont00001754 "https://en.wikipedia.org/w/index.php?title=Thermographic_camera&oldid=1063916009"^^xsd:anyURI ;
                 cco:ont00001760 "https://www.commoncoreontologies.org/ArtifactOntology"^^xsd:anyURI .


###  https://www.commoncoreontologies.org/ont00000618
cco:ont00000618 rdf:type owl:Class ;
                 rdfs:subClassOf cco:ont00000713 ;
                 rdfs:label "Ground Vehicle"@en ;
                 skos:definition "A Vehicle that is designed to convey passengers, cargo, or equipment from one location to another by some form of ground travel."@en ;
                 cco:ont00001754 "https://en.wikipedia.org/w/index.php?title=Category:Land_vehicles&oldid=546083623"^^xsd:anyURI ;
                 cco:ont00001760 "https://www.commoncoreontologies.org/ArtifactOntology"^^xsd:anyURI .


###  https://www.commoncoreontologies.org/ont00000623
cco:ont00000623 rdf:type owl:Class ;
                 rdfs:subClassOf cco:ont00000323 ;
                 rdfs:label "Impact Shielding Artifact Function"@en ;
                 skos:definition "An Artifact Function that is realized during events in which an Artifact reduces the damage caused to the shielded object by an impact with another object."@en ;
                 cco:ont00001760 "https://www.commoncoreontologies.org/ArtifactOntology"^^xsd:anyURI .


###  https://www.commoncoreontologies.org/ont00000624
cco:ont00000624 rdf:type owl:Class ;
                 rdfs:subClassOf cco:ont00001298 ;
                 rdfs:label "Report"@en ;
                 skos:definition "A Document that is designed to bear some specific Information Content Entity that conveys an account of some event, situation, or the result of some observation or inquiry."@en ;
                 cco:ont00001754 "https://en.wikipedia.org/w/index.php?title=Report&oldid=1063765657"^^xsd:anyURI ;
                 cco:ont00001760 "https://www.commoncoreontologies.org/ArtifactOntology"^^xsd:anyURI .


###  https://www.commoncoreontologies.org/ont00000625
cco:ont00000625 rdf:type owl:Class ;
                 rdfs:subClassOf cco:ont00000256 ;
                 rdfs:label "Nozzle Throat"@en ;
                 skos:definition "A Fluid Control Artifact that consists of the narrowest portion of a Nozzle that is designed to converge the flow of fluid in order to increase the Velocity of the flow."@en ;
                 cco:ont00001760 "https://www.commoncoreontologies.org/ArtifactOntology"^^xsd:anyURI .


###  https://www.commoncoreontologies.org/ont00000627
cco:ont00000627 rdf:type owl:Class ;
                 owl:equivalentClass [ owl:intersectionOf ( obo:BFO_0000040
                                                            [ rdf:type owl:Restriction ;
                                                              owl:onProperty obo:BFO_0000196 ;
                                                              owl:someValuesFrom cco:ont00001141
                                                            ]
                                                          ) ;
                                       rdf:type owl:Class
                                     ] ;
                 rdfs:subClassOf obo:BFO_0000040 ;
                 rdfs:label "Infrastructure Element"@en ;
                 skos:definition "A Material Entity that bears an Infrastructure Role."@en ;
                 cco:ont00001760 "https://www.commoncoreontologies.org/ArtifactOntology"^^xsd:anyURI .


###  https://www.commoncoreontologies.org/ont00000629
cco:ont00000629 rdf:type owl:Class ;
                 rdfs:subClassOf cco:ont00000323 ;
                 rdfs:label "Deception Artifact Function"@en ;
                 skos:definition "An Artifact Function that is realized in processes which misinform or mislead some other entity."@en ;
                 cco:ont00001754 "https://en.wikipedia.org/w/index.php?title=Deception&oldid=1061346984"^^xsd:anyURI ;
                 cco:ont00001760 "https://www.commoncoreontologies.org/ArtifactOntology"^^xsd:anyURI .


###  https://www.commoncoreontologies.org/ont00000634
cco:ont00000634 rdf:type owl:Class ;
                 rdfs:subClassOf cco:ont00000431 ;
                 rdfs:label "Steam Engine"@en ;
                 skos:definition "An External Combustion Engine that is designed to use steam as its working fluid."@en ;
                 cco:ont00001754 "https://en.wikipedia.org/w/index.php?title=Steam_engine&oldid=1064097686"^^xsd:anyURI ;
                 cco:ont00001760 "https://www.commoncoreontologies.org/ArtifactOntology"^^xsd:anyURI .


###  https://www.commoncoreontologies.org/ont00000635
cco:ont00000635 rdf:type owl:Class ;
                 rdfs:subClassOf cco:ont00000323 ;
                 rdfs:label "Refraction Artifact Function"@en ;
                 skos:definition "An Artifact Function that is realized by an Artifact participating in a refraction event in which the Artifact causes a change in direction of wave propagation due to a change in its transmission medium."@en ;
                 cco:ont00001760 "https://www.commoncoreontologies.org/ArtifactOntology"^^xsd:anyURI .


###  https://www.commoncoreontologies.org/ont00000637
cco:ont00000637 rdf:type owl:Class ;
                 rdfs:subClassOf cco:ont00000593 ;
                 rdfs:label "Portion of Gaseous Propellant"@en ;
                 skos:definition "A Portion of Propellant that is stored in a gaseous state."@en ;
                 cco:ont00001760 "https://www.commoncoreontologies.org/ArtifactOntology"^^xsd:anyURI .


###  https://www.commoncoreontologies.org/ont00000638
cco:ont00000638 rdf:type owl:Class ;
                 rdfs:subClassOf cco:ont00000210 ;
                 rdfs:label "Heat Engine"@en ;
                 skos:definition "An Engine that is designed to convert thermal energy into mechanical energy."@en ;
                 cco:ont00001760 "https://www.commoncoreontologies.org/ArtifactOntology"^^xsd:anyURI .


###  https://www.commoncoreontologies.org/ont00000640
cco:ont00000640 rdf:type owl:Class ;
                 rdfs:subClassOf cco:ont00001002 ;
                 rdfs:label "Email Message"@en ;
                 skos:definition "A Message that is transmitted to the recipient's Email Box."@en ;
                 cco:ont00001754 "https://en.wikipedia.org/w/index.php?title=Email&oldid=1063646749"^^xsd:anyURI ;
                 cco:ont00001760 "https://www.commoncoreontologies.org/ArtifactOntology"^^xsd:anyURI .


###  https://www.commoncoreontologies.org/ont00000646
cco:ont00000646 rdf:type owl:Class ;
                 rdfs:subClassOf cco:ont00000247 ;
                 rdfs:label "Highway"@en ;
                 skos:definition "A Road that is designed to enable Ground Vehicles to travel between relatively major destinations."@en ;
                 cco:ont00001754 "https://en.wikipedia.org/w/index.php?title=Highway&oldid=1063985949"^^xsd:anyURI ;
                 cco:ont00001760 "https://www.commoncoreontologies.org/ArtifactOntology"^^xsd:anyURI .


###  https://www.commoncoreontologies.org/ont00000650
cco:ont00000650 rdf:type owl:Class ;
                 rdfs:subClassOf cco:ont00000214 ;
                 rdfs:label "Ground Moving Target Indication Artifact Function"@en ;
                 skos:definition "A Moving Target Indication Artifact Function that inheres in Artifacts that are designed to identify and track entities moving on or near the ground."@en ;
                 cco:ont00001760 "https://www.commoncoreontologies.org/ArtifactOntology"^^xsd:anyURI .


###  https://www.commoncoreontologies.org/ont00000651
cco:ont00000651 rdf:type owl:Class ;
                 rdfs:subClassOf cco:ont00000323 ;
                 rdfs:label "Containing Artifact Function"@en ;
                 skos:definition "An Artifact Function that is realized in a process in which one entity contains another."@en ;
                 cco:ont00001754 "http://www.dictionary.com/browse/containing" ;
                 cco:ont00001760 "https://www.commoncoreontologies.org/ArtifactOntology"^^xsd:anyURI .


###  https://www.commoncoreontologies.org/ont00000652
cco:ont00000652 rdf:type owl:Class ;
                 rdfs:subClassOf cco:ont00000995 ;
                 rdfs:label "Decoy"@en ;
                 skos:definition "A Material Artifact that is designed to distract or conceal what an individual or group might be looking for."@en ;
                 cco:ont00001754 "https://en.wikipedia.org/w/index.php?title=Decoy&oldid=1058455081"^^xsd:anyURI ;
                 cco:ont00001760 "https://www.commoncoreontologies.org/ArtifactOntology"^^xsd:anyURI .


###  https://www.commoncoreontologies.org/ont00000656
cco:ont00000656 rdf:type owl:Class ;
                 rdfs:subClassOf cco:ont00000445 ;
                 rdfs:label "Radiological Weapon"@en ;
                 skos:definition "A Weapon that is designed to inflict harm, damage, or incapacity by means of releasing radioactive material."@en ;
                 cco:ont00001754 "https://en.wikipedia.org/w/index.php?title=Radiological_warfare&oldid=1060817328"^^xsd:anyURI ;
                 cco:ont00001760 "https://www.commoncoreontologies.org/ArtifactOntology"^^xsd:anyURI .


###  https://www.commoncoreontologies.org/ont00000657
cco:ont00000657 rdf:type owl:Class ;
                 rdfs:subClassOf cco:ont00001100 ;
                 rdfs:label "Distance Measurement Artifact Function"@en ;
                 skos:definition "A Measurement Artifact Function that is realized during events in which an Artifact is used to measure the spatial Distance to a specified object or class of objects."@en ;
                 cco:ont00001760 "https://www.commoncoreontologies.org/ArtifactOntology"^^xsd:anyURI .


###  https://www.commoncoreontologies.org/ont00000658
cco:ont00000658 rdf:type owl:Class ;
                 rdfs:subClassOf cco:ont00001051 ;
                 rdfs:label "Missile Launcher"@en ;
                 skos:definition "A Projectile Launcher that is designed to launch one or more Precision-Guided Missiles."@en ;
                 cco:ont00001760 "https://www.commoncoreontologies.org/ArtifactOntology"^^xsd:anyURI .


###  https://www.commoncoreontologies.org/ont00000661
cco:ont00000661 rdf:type owl:Class ;
                 rdfs:subClassOf cco:ont00001301 ;
                 rdfs:label "Government Artifact Function"@en ;
                 skos:definition "A Service Artifact Function that is realized in processes in which a Government administers public policy or directs the actions of the Populace of its Domain, or in which one or more of its members or parts does so while acting in their official capacity."@en ;
                 cco:ont00001754 "https://en.wikipedia.org/w/index.php?title=Government&oldid=1063736308"^^xsd:anyURI ;
                 cco:ont00001760 "https://www.commoncoreontologies.org/ArtifactOntology"^^xsd:anyURI .


###  https://www.commoncoreontologies.org/ont00000663
cco:ont00000663 rdf:type owl:Class ;
                 rdfs:subClassOf cco:ont00000995 ;
                 rdfs:label "Power Transmission Artifact"@en ;
                 skos:definition "A Material Artifact that is designed to transfer and regulate Power flow from a Power Source to an application point."@en ;
                 cco:ont00001760 "https://www.commoncoreontologies.org/ArtifactOntology"^^xsd:anyURI .


###  https://www.commoncoreontologies.org/ont00000665
cco:ont00000665 rdf:type owl:Class ;
                 rdfs:subClassOf cco:ont00000323 ;
                 rdfs:label "Cleaning Artifact Function"@en ;
                 skos:definition "An Artifact Function that is realized in processes in which some Artifact is used to remove foreign objects from another object."@en ;
                 cco:ont00001760 "https://www.commoncoreontologies.org/ArtifactOntology"^^xsd:anyURI .


###  https://www.commoncoreontologies.org/ont00000668
cco:ont00000668 rdf:type owl:Class ;
                 rdfs:subClassOf cco:ont00000995 ;
                 rdfs:label "Battery Terminal"@en ;
                 skos:definition "A Material Artifact that is designed to connect a load or charger to a single or multiple-cell Battery."@en ;
                 cco:ont00001754 "https://en.wikipedia.org/w/index.php?title=Battery_terminal&oldid=1059455659"^^xsd:anyURI ;
                 cco:ont00001760 "https://www.commoncoreontologies.org/ArtifactOntology"^^xsd:anyURI .


###  https://www.commoncoreontologies.org/ont00000671
cco:ont00000671 rdf:type owl:Class ;
                 rdfs:subClassOf cco:ont00000415 ;
                 rdfs:label "Anti-Bacterial Artifact Function"@en ;
                 skos:definition "An Anti-Microbial Artifact Function that is realized in a process which causes harm to, or the death of, some bacterium."@en ;
                 cco:ont00001754 "https://en.wikipedia.org/w/index.php?title=Antibiotic&oldid=1063633090"^^xsd:anyURI ;
                 cco:ont00001760 "https://www.commoncoreontologies.org/ArtifactOntology"^^xsd:anyURI .


###  https://www.commoncoreontologies.org/ont00000673
cco:ont00000673 rdf:type owl:Class ;
                 rdfs:subClassOf cco:ont00000715 ;
                 rdfs:label "Prosthetic Foot"@en ;
                 skos:definition "A Prosthesis that is designed to replace a missing foot."@en ;
                 cco:ont00001754 "https://en.wikipedia.org/w/index.php?title=Prosthesis&oldid=1063749698"^^xsd:anyURI ;
                 cco:ont00001760 "https://www.commoncoreontologies.org/ArtifactOntology"^^xsd:anyURI .


###  https://www.commoncoreontologies.org/ont00000678
cco:ont00000678 rdf:type owl:Class ;
                 rdfs:subClassOf cco:ont00000098 ;
                 rdfs:label "Voltage Regulating Artifact Function"@en ;
                 skos:definition "An Artifact Function that is realized by processes in which some Artifact is used to cause a change in the voltage magnitude between the sending and receiving end of an electrical component."@en ;
                 cco:ont00001754 "https://en.wikipedia.org/w/index.php?title=Voltage_regulation&oldid=1045628774"^^xsd:anyURI ;
                 cco:ont00001760 "https://www.commoncoreontologies.org/ArtifactOntology"^^xsd:anyURI .


###  https://www.commoncoreontologies.org/ont00000679
cco:ont00000679 rdf:type owl:Class ;
                 rdfs:subClassOf cco:ont00000323 ;
                 rdfs:label "Attitude Control Artifact Function"@en ;
                 skos:altLabel "Orientation Control Artifact Function"@en ;
                 skos:definition "An Artifact Function that is realized by an Artifact participating in an attitude control process."@en ;
                 cco:ont00001760 "https://www.commoncoreontologies.org/ArtifactOntology"^^xsd:anyURI .


###  https://www.commoncoreontologies.org/ont00000681
cco:ont00000681 rdf:type owl:Class ;
                 rdfs:subClassOf cco:ont00000236 ;
                 rdfs:label "External Navigation Lighting System"@en ;
                 skos:definition "A Lighting System that is designed to be attached to some Vehicle and to emit colored light in order to signal that Vehicle's position, heading, and status."@en ;
                 cco:ont00001754 "https://en.wikipedia.org/w/index.php?title=Navigation_light&oldid=1034200601"^^xsd:anyURI ;
                 cco:ont00001760 "https://www.commoncoreontologies.org/ArtifactOntology"^^xsd:anyURI .


###  https://www.commoncoreontologies.org/ont00000682
cco:ont00000682 rdf:type owl:Class ;
                 rdfs:subClassOf cco:ont00000136 ;
                 rdfs:label "Mirror"@en ;
                 skos:definition "An Optical Instrument that is designed to reflect light that has a wavelength within a given range and is incident on its relflecting surface such that the reflected light maintains most of the characteristics of the original light."@en ;
                 cco:ont00001754 "https://en.wikipedia.org/w/index.php?title=Mirror&oldid=1063296474"^^xsd:anyURI ;
                 cco:ont00001760 "https://www.commoncoreontologies.org/ArtifactOntology"^^xsd:anyURI .


###  https://www.commoncoreontologies.org/ont00000686
cco:ont00000686 rdf:type owl:Class .


###  https://www.commoncoreontologies.org/ont00000688
cco:ont00000688 rdf:type owl:Class ;
                 rdfs:subClassOf cco:ont00000294 ;
                 rdfs:label "Turbofan Air-Breathing Jet Engine"@en ;
                 skos:definition "An Air-Breathing Jet Engine that uses a Turbofan, which consists of a Turbine and a Fan."@en ;
                 cco:ont00001754 "https://en.wikipedia.org/w/index.php?title=Turbofan&oldid=1063724215"^^xsd:anyURI ;
                 cco:ont00001760 "https://www.commoncoreontologies.org/ArtifactOntology"^^xsd:anyURI .


###  https://www.commoncoreontologies.org/ont00000689
cco:ont00000689 rdf:type owl:Class ;
                 rdfs:subClassOf cco:ont00000323 ;
                 rdfs:label "Switch Artifact Function"@en ;
                 skos:definition "An Artifact Function that is realized in a process of breaking an electric circuit by interrupting the current or diverting it from one conductor to another."@en ;
                 cco:ont00001754 "https://en.wikipedia.org/w/index.php?title=Switch&oldid=1059685800"^^xsd:anyURI ;
                 cco:ont00001760 "https://www.commoncoreontologies.org/ArtifactOntology"^^xsd:anyURI .


###  https://www.commoncoreontologies.org/ont00000690
cco:ont00000690 rdf:type owl:Class ;
                 rdfs:subClassOf cco:ont00000346 ;
                 rdfs:label "Telecommunication Instrument"@en ;
                 skos:definition "A Communication Instrument that is designed for use by some Agent in some Act of Communication where the recipient of that communication is potentially a significant distance away from the Agent."@en ;
                 cco:ont00001760 "https://www.commoncoreontologies.org/ArtifactOntology"^^xsd:anyURI .


###  https://www.commoncoreontologies.org/ont00000691
cco:ont00000691 rdf:type owl:Class ;
                 rdfs:subClassOf cco:ont00000020 ;
                 rdfs:label "Fuel Tank"@en ;
                 skos:definition "A Container that is designed to store a Portion of Fuel."@en ;
                 cco:ont00001760 "https://www.commoncoreontologies.org/ArtifactOntology"^^xsd:anyURI .


###  https://www.commoncoreontologies.org/ont00000693
cco:ont00000693 rdf:type owl:Class ;
                 rdfs:subClassOf cco:ont00000575 ;
                 rdfs:label "Mass Specification"@en ;
                 skos:definition "A Quality Specification that prescribes the Amount of Mass that a Material Entity should have."@en ;
                 cco:ont00001760 "https://www.commoncoreontologies.org/ArtifactOntology"^^xsd:anyURI .


###  https://www.commoncoreontologies.org/ont00000694
cco:ont00000694 rdf:type owl:Class ;
                 rdfs:subClassOf cco:ont00000256 ;
                 rdfs:label "Nozzle Mouth"@en ;
                 skos:definition "A Fluid Control Artifact that consists of the portion of a Nozzle at the end that is designed to be where the flow of fluid exits the Nozzle."@en ;
                 cco:ont00001760 "https://www.commoncoreontologies.org/ArtifactOntology"^^xsd:anyURI .


###  https://www.commoncoreontologies.org/ont00000698
cco:ont00000698 rdf:type owl:Class ;
                 rdfs:subClassOf cco:ont00000252 ;
                 rdfs:comment "By increasing the Exhaust Velocity of the gas, the Nozzle increases the Thrust generated."@en ;
                 rdfs:label "Convergent-Divergent Nozzle"@en ;
                 skos:altLabel "CD Nozzle"@en ,
                               "de Laval Nozzle"@en ;
                 skos:definition "A Nozzle that consists of a tube with an asymmetric hourglass shape that is designed to accelerate hot pressurized gas by converting the heat energy of the gas flow into kinetic energy as it passes through the Nozzle Throat to generate increased Exhaust Velocity of the gas as it exits the Nozzle."@en ;
                 cco:ont00001754 "https://en.wikipedia.org/w/index.php?title=De_Laval_nozzle&oldid=1062746288"^^xsd:anyURI ;
                 cco:ont00001760 "https://www.commoncoreontologies.org/ArtifactOntology"^^xsd:anyURI .


###  https://www.commoncoreontologies.org/ont00000700
cco:ont00000700 rdf:type owl:Class ;
                 rdfs:subClassOf cco:ont00000998 ;
                 rdfs:label "Computer Network"@en ;
                 skos:altLabel "Data Network"@en ;
                 skos:definition "A Telecommunication Network that is designed to allow the exchange of data between two or more computers connected to the network."@en ;
                 cco:ont00001754 "https://en.wikipedia.org/w/index.php?title=Computer_network&oldid=1061571662"^^xsd:anyURI ;
                 cco:ont00001760 "https://www.commoncoreontologies.org/ArtifactOntology"^^xsd:anyURI .


###  https://www.commoncoreontologies.org/ont00000701
cco:ont00000701 rdf:type owl:Class ;
                 rdfs:subClassOf cco:ont00001145 ;
                 rdfs:label "Wire Receiver"@en ;
                 skos:definition "A Radio Receiver that uses a Wire Antenna to intercept radio signals."@en ;
                 cco:ont00001760 "https://www.commoncoreontologies.org/ArtifactOntology"^^xsd:anyURI .


###  https://www.commoncoreontologies.org/ont00000702
cco:ont00000702 rdf:type owl:Class ;
                 rdfs:subClassOf cco:ont00000798 ;
                 rdfs:label "Image"@en ;
                 skos:definition "An Information Bearing Artifact that is designed to carry an Information Content Entity that represents some entity owing to a visual isomorphism between the carrying artifact and the entity."@en ;
                 cco:ont00001754 "https://en.wikipedia.org/w/index.php?title=Image&oldid=1062709732"^^xsd:anyURI ;
                 cco:ont00001760 "https://www.commoncoreontologies.org/ArtifactOntology"^^xsd:anyURI .


###  https://www.commoncoreontologies.org/ont00000703
cco:ont00000703 rdf:type owl:Class ;
                 rdfs:subClassOf cco:ont00000159 ;
                 rdfs:label "System Clock"@en ;
                 skos:definition "A Timekeeping Instrument that is part of a computer an is designed to issue a steady high-frequency signal that is used to synchronize all of the computer's internal components."@en ;
                 cco:ont00001754 "http://www.thefreedictionary.com/system+clock" ;
                 cco:ont00001760 "https://www.commoncoreontologies.org/ArtifactOntology"^^xsd:anyURI .


###  https://www.commoncoreontologies.org/ont00000704
cco:ont00000704 rdf:type owl:Class ;
                 rdfs:subClassOf cco:ont00001326 ;
                 rdfs:label "Tunnel"@en ;
                 skos:definition "A Land Transportation Artifact that is designed to enable Ground Vehicles to travel underneath a surrounding soil, earth, or rock formation."@en ;
                 cco:ont00001754 "https://en.wikipedia.org/w/index.php?title=Tunnel&oldid=1062456881"^^xsd:anyURI ;
                 cco:ont00001760 "https://www.commoncoreontologies.org/ArtifactOntology"^^xsd:anyURI .


###  https://www.commoncoreontologies.org/ont00000706
cco:ont00000706 rdf:type owl:Class ;
                 rdfs:subClassOf cco:ont00000995 ;
                 rdfs:label "Terminal Board"@en ;
                 skos:definition "A Material Artifact that is designed to join electrical terminations and create an electrical circuit by means of a block which connects individual wires without a splice or physically joining the ends."@en ;
                 cco:ont00001754 "https://en.wikipedia.org/w/index.php?title=Electrical_connector&oldid=1061247409"^^xsd:anyURI ;
                 cco:ont00001760 "https://www.commoncoreontologies.org/ArtifactOntology"^^xsd:anyURI .


###  https://www.commoncoreontologies.org/ont00000709
cco:ont00000709 rdf:type owl:Class ;
                 rdfs:subClassOf cco:ont00001248 ;
                 rdfs:label "Visual Prosthesis"@en ;
                 skos:altLabel "Bionic Eye"@en ;
                 skos:definition "An Artificial Eye that is designed to replace a missing eye, which performs the function of an eye."@en ;
                 cco:ont00001754 "https://en.wikipedia.org/w/index.php?title=Visual_prosthesis&oldid=1059269261"^^xsd:anyURI ;
                 cco:ont00001760 "https://www.commoncoreontologies.org/ArtifactOntology"^^xsd:anyURI .


###  https://www.commoncoreontologies.org/ont00000711
cco:ont00000711 rdf:type owl:Class ;
                 rdfs:subClassOf cco:ont00000156 ;
                 rdfs:label "Semi-automatic Pistol"@en ;
                 skos:definition "A Hand Gun that has a single fixed firing chamber machined into the rear of the barrel and an ammunition magazine capable of holding multiple Cartridges such that the Hand Gun is designed to automatically reload each time it is fired and to fire a Bullet with each successive pull of the trigger until the stored ammunition is depleted."@en ;
                 cco:ont00001754 "https://en.wikipedia.org/w/index.php?title=Semi-automatic_pistol&oldid=1058568715"^^xsd:anyURI ;
                 cco:ont00001760 "https://www.commoncoreontologies.org/ArtifactOntology"^^xsd:anyURI .


###  https://www.commoncoreontologies.org/ont00000713
cco:ont00000713 rdf:type owl:Class ;
                 rdfs:subClassOf cco:ont00000995 ;
                 rdfs:label "Vehicle"@en ;
                 skos:definition "A Material Artifact that is designed to facilitate the movement of material entities from one location to another by conveying them there."@en ;
                 cco:ont00001754 "https://en.wikipedia.org/w/index.php?title=Vehicle&oldid=1063682179"^^xsd:anyURI ;
                 cco:ont00001760 "https://www.commoncoreontologies.org/ArtifactOntology"^^xsd:anyURI .


###  https://www.commoncoreontologies.org/ont00000714
cco:ont00000714 rdf:type owl:Class ;
                 rdfs:subClassOf cco:ont00001192 ;
                 rdfs:label "Horn Antenna"@en ;
                 skos:altLabel "Microwave Horn"@en ;
                 skos:definition "A Radio Antenna that consists of a flaring metal waveguide shaped like a horn to direct radio waves in a beam and can be used on its own or as a feeder for larger antenna structures, such as Parabolic Antennas."@en ;
                 cco:ont00001754 "https://en.wikipedia.org/w/index.php?title=Horn_antenna&oldid=1050375403"^^xsd:anyURI ;
                 cco:ont00001760 "https://www.commoncoreontologies.org/ArtifactOntology"^^xsd:anyURI .


###  https://www.commoncoreontologies.org/ont00000715
cco:ont00000715 rdf:type owl:Class ;
                 rdfs:subClassOf cco:ont00001381 ;
                 rdfs:label "Prosthesis"@en ;
                 skos:definition "A Medical Artifact that is designed to replace a missing body part."@en ;
                 cco:ont00001754 "https://en.wikipedia.org/w/index.php?title=Prosthesis&oldid=1063749698"^^xsd:anyURI ;
                 cco:ont00001760 "https://www.commoncoreontologies.org/ArtifactOntology"^^xsd:anyURI .


###  https://www.commoncoreontologies.org/ont00000716
cco:ont00000716 rdf:type owl:Class ;
                 rdfs:subClassOf cco:ont00001049 ;
                 rdfs:label "Electric Battery"@en ;
                 skos:altLabel "Battery"@en ;
                 skos:definition "An Electrical Power Source that is designed to produce electric power by converting chemical energy to electrical energy."@en ;
                 cco:ont00001754 "https://en.wikipedia.org/wiki/Battery_(electricity)" ;
                 cco:ont00001760 "https://www.commoncoreontologies.org/ArtifactOntology"^^xsd:anyURI .


###  https://www.commoncoreontologies.org/ont00000719
cco:ont00000719 rdf:type owl:Class ;
                 rdfs:subClassOf cco:ont00000995 ;
                 rdfs:label "Counterfeit Instrument"@en ;
                 skos:definition "A Material Artifact that is designed to be a fake replica of some genuine Artifact."@en ;
                 cco:ont00001754 "https://en.wikipedia.org/w/index.php?title=Counterfeit&oldid=1063493600"^^xsd:anyURI ;
                 cco:ont00001760 "https://www.commoncoreontologies.org/ArtifactOntology"^^xsd:anyURI .


###  https://www.commoncoreontologies.org/ont00000720
cco:ont00000720 rdf:type owl:Class ;
                 rdfs:subClassOf cco:ont00000020 ;
                 rdfs:label "Cryogenic Storage Dewar"@en ;
                 skos:definition "A Container that is designed to store a Portion of Cryogenic Material (such as liquid helium or liquid oxygen) and which consists of, minimally, walls that are constructed from two or more layers that are separated by a high vacuum to provide thermal insulation between the interior and exterior of the dewar."@en ;
                 cco:ont00001754 "https://en.wikipedia.org/w/index.php?title=Cryogenic_storage_dewar&oldid=1021282649"^^xsd:anyURI ;
                 cco:ont00001760 "https://www.commoncoreontologies.org/ArtifactOntology"^^xsd:anyURI .


###  https://www.commoncoreontologies.org/ont00000721
cco:ont00000721 rdf:type owl:Class ;
                 rdfs:subClassOf cco:ont00000804 ;
                 rdfs:label "Polarizing Prism"@en ;
                 skos:definition "A Prism designed to split a beam of light entering the Prism into components of varying polarization."@en ;
                 cco:ont00001760 "https://www.commoncoreontologies.org/ArtifactOntology"^^xsd:anyURI .


###  https://www.commoncoreontologies.org/ont00000723
cco:ont00000723 rdf:type owl:Class ;
                 rdfs:subClassOf cco:ont00000781 ;
                 rdfs:label "Vehicle Control System"@en ;
                 skos:definition "A Control System that is designed to enable some Agent to control some Vehicle."@en ;
                 cco:ont00001760 "https://www.commoncoreontologies.org/ArtifactOntology"^^xsd:anyURI .


###  https://www.commoncoreontologies.org/ont00000724
cco:ont00000724 rdf:type owl:Class ;
                 rdfs:subClassOf cco:ont00001192 ;
                 rdfs:label "Parabolic Antenna"@en ;
                 skos:altLabel "Dish Antenna"@en ,
                               "Parabolic Dish"@en ;
                 skos:definition "A Radio Antenna that uses a parabolic reflector to direct or receive radio waves and has a very high gain."@en ;
                 cco:ont00001754 "https://en.wikipedia.org/w/index.php?title=Parabolic_antenna&oldid=1057213241"^^xsd:anyURI ;
                 cco:ont00001760 "https://www.commoncoreontologies.org/ArtifactOntology"^^xsd:anyURI .


###  https://www.commoncoreontologies.org/ont00000727
cco:ont00000727 rdf:type owl:Class ;
                 rdfs:subClassOf cco:ont00000323 ;
                 rdfs:label "Communication Artifact Function"@en ;
                 skos:definition "An Artifact Function that is realized in a process in which meaningful signs are conveyed from one entity to another."@en ;
                 cco:ont00001760 "https://www.commoncoreontologies.org/ArtifactOntology"^^xsd:anyURI .


###  https://www.commoncoreontologies.org/ont00000728
cco:ont00000728 rdf:type owl:Class ;
                 rdfs:subClassOf cco:ont00000215 ;
                 rdfs:comment "The submillimeter waveband is between the far-infrared and microwave wavebands and is typically taken to have a wavelength of between a few hundred micrometers and a millimeter."@en ;
                 rdfs:label "Submillimeter Wavelength Radio Telescope"@en ;
                 skos:altLabel "Microwave Telescope"@en ;
                 skos:definition "A Radio Telescope that is designed to aid in the observation of spatially distant Objects by means of collecting and focusing radio waves from the submillimeter waveband (i.e. microwaves) to form an enhanced image of the Object."@en ;
                 cco:ont00001754 "http://kp12m.as.arizona.edu/docs/what_is_submillimeter.htm, https://en.wikipedia.org/wiki/Submillimetre_astronomy" ;
                 cco:ont00001760 "https://www.commoncoreontologies.org/ArtifactOntology"^^xsd:anyURI .


###  https://www.commoncoreontologies.org/ont00000730
cco:ont00000730 rdf:type owl:Class ;
                 rdfs:subClassOf cco:ont00000995 ;
                 rdfs:label "Hydraulic Power Transfer Unit"@en ;
                 skos:definition "A Material Artifact that is designed to transfer hydraulic power from one of an Aircraft's hydraulic systems to another in the event that a system has failed or been turned off."@en ;
                 cco:ont00001754 "https://en.wikipedia.org/w/index.php?title=Power_transfer_unit&oldid=1002682083"^^xsd:anyURI ;
                 cco:ont00001760 "https://www.commoncoreontologies.org/ArtifactOntology"^^xsd:anyURI .


###  https://www.commoncoreontologies.org/ont00000734
cco:ont00000734 rdf:type owl:Class ;
                 rdfs:subClassOf cco:ont00000552 ;
                 rdfs:label "Land Mine"@en ;
                 skos:definition "An Explosive Weapon that is designed to be concealed under or on the ground and to detonate as its target passes over or near it."@en ;
                 cco:ont00001754 "https://en.wikipedia.org/w/index.php?title=Land_mine&oldid=1060289159"^^xsd:anyURI ;
                 cco:ont00001760 "https://www.commoncoreontologies.org/ArtifactOntology"^^xsd:anyURI .


###  https://www.commoncoreontologies.org/ont00000736
cco:ont00000736 rdf:type owl:Class ;
                 rdfs:subClassOf cco:ont00000995 ;
                 rdfs:label "Transducer"@en ;
                 skos:definition "A Material Artifact that is designed to convert one form of energy to another."@en ;
                 cco:ont00001754 "https://en.wikipedia.org/w/index.php?title=Transducer&oldid=1053290948"^^xsd:anyURI ;
                 cco:ont00001760 "https://www.commoncoreontologies.org/ArtifactOntology"^^xsd:anyURI .


###  https://www.commoncoreontologies.org/ont00000740
cco:ont00000740 rdf:type owl:Class ;
                 rdfs:subClassOf obo:BFO_0000002 ;
                 rdfs:comment "This class is designed to group continuants according to a very broad criterion and is not intended to be used as a parent class for entities that can be more specifically represented under another class. Hence, Natural Resource may be an appropriate subtype but Money, Oil, and Gold Mine are not."@en ;
                 rdfs:label "Resource"@en ;
                 skos:definition "A Continuant that is owned by, in the possession of, or is otherwise controlled by an Agent such that it could be used by that Agent."@en ;
                 skos:example "a group of interns" ,
                              "a knowledge base" ,
                              "a plot of land" ,
                              "a software program" ,
                              "a sum of money" ,
                              "a vehicle" ;
                 skos:scopeNote "Resources are Resources for some Agent. If no instance of Agent existed, no instance of Resource would exist either. It is not a requirement that something be valuable in order for it to be a Resource. Thus the value of something can drastically change without altering whether that thing is a Resource."@en ;
                 cco:ont00001760 "https://www.commoncoreontologies.org/ArtifactOntology"^^xsd:anyURI .


###  https://www.commoncoreontologies.org/ont00000742
cco:ont00000742 rdf:type owl:Class ;
                 rdfs:subClassOf cco:ont00000995 ;
                 rdfs:label "Ignition System"@en ;
                 skos:definition "A Material Artifact that is designed to produce an Ignition process."@en ;
                 cco:ont00001760 "https://www.commoncoreontologies.org/ArtifactOntology"^^xsd:anyURI .


###  https://www.commoncoreontologies.org/ont00000743
cco:ont00000743 rdf:type owl:Class ;
                 rdfs:subClassOf cco:ont00000702 ;
                 rdfs:label "Chart"@en ;
                 skos:definition "An Image that is designed to carry some Representational Information Content Entity that is prescribed by some canonical visual format."@en ;
                 cco:ont00001754 "Adapted from “Chart.” Merriam-Webster.com Dictionary, Merriam-Webster, https://www.merriam-webster.com/dictionary/chart. Accessed 4 Aug. 2024." ;
                 cco:ont00001760 "https://www.commoncoreontologies.org/ArtifactOntology"^^xsd:anyURI .


###  https://www.commoncoreontologies.org/ont00000746
cco:ont00000746 rdf:type owl:Class ;
                 rdfs:subClassOf cco:ont00000638 ;
                 rdfs:label "Combustion Engine"@en ;
                 skos:definition "A Heat Engine that is designed to convert thermal energy that is generated through a local Combustion process into mechanical energy."@en ;
                 cco:ont00001760 "https://www.commoncoreontologies.org/ArtifactOntology"^^xsd:anyURI .


###  https://www.commoncoreontologies.org/ont00000747
cco:ont00000747 rdf:type owl:Class ;
                 rdfs:subClassOf cco:ont00000549 ;
                 rdfs:label "Canal"@en ;
                 skos:definition "A Water Transportation Artifact that is an artificial Hydrographic Feature designed to convey water or enable Watercraft to travel inland."@en ;
                 cco:ont00001754 "https://en.wikipedia.org/w/index.php?title=Canal&oldid=1059514223" ;
                 cco:ont00001760 "https://www.commoncoreontologies.org/ArtifactOntology"^^xsd:anyURI .


###  https://www.commoncoreontologies.org/ont00000748
cco:ont00000748 rdf:type owl:Class ;
                 rdfs:subClassOf cco:ont00001150 ;
                 rdfs:label "Bullet"@en ;
                 skos:definition "A Portion of Ammunition that is designed to be projected by a Firearm, Sling, Slingshot, or Air Gun, but which does not (typically) contain explosives."@en ;
                 cco:ont00001754 "https://en.wikipedia.org/w/index.php?title=Bullet&oldid=1062391591"^^xsd:anyURI ;
                 cco:ont00001760 "https://www.commoncoreontologies.org/ArtifactOntology"^^xsd:anyURI .


###  https://www.commoncoreontologies.org/ont00000756
cco:ont00000756 rdf:type owl:Class ;
                 rdfs:subClassOf cco:ont00000798 ;
                 rdfs:label "Database"@en ;
                 skos:definition "An Information Bearing Artifact that is designed to bear some set of specific Information Content Entities and to be rapidly searchable and retrievable."@en ;
                 cco:ont00001754 "https://en.wikipedia.org/w/index.php?title=Database&oldid=1057024641"^^xsd:anyURI ;
                 cco:ont00001760 "https://www.commoncoreontologies.org/ArtifactOntology"^^xsd:anyURI .


###  https://www.commoncoreontologies.org/ont00000758
cco:ont00000758 rdf:type owl:Class ;
                 rdfs:subClassOf obo:BFO_0000023 ;
                 rdfs:label "Component Role"@en ;
                 skos:definition "A Role that inheres in an entity having a discrete structure in virtue of that entity being part of a system considered at a particular level of analysis."@en ;
                 cco:ont00001754 "ISO/IEC. 1998. Information Technology ― System and Software Integrity Levels Geneva, Switzerland: International Organization for Standardization (ISO)/International Electrotechnical Commission (IEC). ISO/IEC. 15026:1998. : 3.1"@en ;
                 cco:ont00001760 "https://www.commoncoreontologies.org/ArtifactOntology"^^xsd:anyURI .


###  https://www.commoncoreontologies.org/ont00000762
cco:ont00000762 rdf:type owl:Class ;
                 rdfs:subClassOf cco:ont00000415 ;
                 rdfs:label "Fungicide Artifact Function"@en ;
                 skos:definition "An Anti-Microbial Artifact Function that is realized in a process which causes harm to, or the death of, some fungus or fungal spore."@en ;
                 cco:ont00001754 "https://en.wikipedia.org/w/index.php?title=Fungicide&oldid=1056769271"^^xsd:anyURI ;
                 cco:ont00001760 "https://www.commoncoreontologies.org/ArtifactOntology"^^xsd:anyURI .


###  https://www.commoncoreontologies.org/ont00000764
cco:ont00000764 rdf:type owl:Class ;
                 rdfs:subClassOf cco:ont00000504 ;
                 rdfs:label "Optical Focusing Artifact Function"@en ;
                 skos:definition "An Optical Processing Artifact Function that is realized by an Artifact participating in a light focusing event in which the Artifact causes the light beam to converge on a target spatial point."@en ;
                 cco:ont00001760 "https://www.commoncoreontologies.org/ArtifactOntology"^^xsd:anyURI .


###  https://www.commoncoreontologies.org/ont00000767
cco:ont00000767 rdf:type owl:Class ;
                 rdfs:subClassOf cco:ont00000995 ;
                 rdfs:comment "A Lubrication System typical consists of a reservoir, pump, heat exchanger, filter, regulator, valves, sensors, pipes, and hoses. In some cases it also includes the passageways and openings within the artifact it is designed to lubricate. For example, the oil holes in a bearing and crankshaft."@en ;
                 rdfs:label "Lubrication System"@en ;
                 skos:definition "A Material Artifact that is designed to contain, transfer, and regulate the flow of lubricant to multiple locations in an Artifact."@en ;
                 cco:ont00001760 "https://www.commoncoreontologies.org/ArtifactOntology"^^xsd:anyURI .


###  https://www.commoncoreontologies.org/ont00000771
cco:ont00000771 rdf:type owl:Class ;
                 rdfs:subClassOf cco:ont00000995 ;
                 rdfs:label "Imaging Instrument"@en ;
                 skos:definition "A Material Artifact that is designed to produce images (visual representations) of an entity."@en ;
                 cco:ont00001760 "https://www.commoncoreontologies.org/ArtifactOntology"^^xsd:anyURI .


###  https://www.commoncoreontologies.org/ont00000774
cco:ont00000774 rdf:type owl:Class ;
                 rdfs:subClassOf cco:ont00000199 ;
                 rdfs:label "Video Camera"@en ;
                 skos:definition "A Camera that is designed to form and digitally or physically record a continuous stream of subsequent images of an entity or scene such that the images can be played back in succession as a video."@en ;
                 cco:ont00001760 "https://www.commoncoreontologies.org/ArtifactOntology"^^xsd:anyURI .


###  https://www.commoncoreontologies.org/ont00000775
cco:ont00000775 rdf:type owl:Class ;
                 rdfs:subClassOf cco:ont00000796 ;
                 rdfs:label "Locomotive"@en ;
                 skos:definition "A Rail Transport Vehicle that is designed to provide the motive power for a Train."@en ;
                 cco:ont00001754 "https://en.wikipedia.org/w/index.php?title=Locomotive&oldid=1062802629"^^xsd:anyURI ;
                 cco:ont00001760 "https://www.commoncoreontologies.org/ArtifactOntology"^^xsd:anyURI .


###  https://www.commoncoreontologies.org/ont00000776
cco:ont00000776 rdf:type owl:Class ;
                 rdfs:subClassOf cco:ont00000323 ;
                 rdfs:label "Signal Detection Artifact Function"@en ;
                 skos:definition "An Artifact Function that is realized in the process of discerning between information-bearing patterns and random patterns, or noise, that distract from the information."@en ;
                 cco:ont00001754 "https://en.wikipedia.org/w/index.php?title=Detection_theory&oldid=1049765804"^^xsd:anyURI ;
                 cco:ont00001760 "https://www.commoncoreontologies.org/ArtifactOntology"^^xsd:anyURI .


###  https://www.commoncoreontologies.org/ont00000777
cco:ont00000777 rdf:type owl:Class ;
                 rdfs:subClassOf cco:ont00001221 ;
                 rdfs:label "Hydraulic Motor"@en ;
                 skos:definition "A Physically Powered Engine that converts hydraulic pressure and flow into torque and angular displacement."@en ;
                 cco:ont00001754 "https://en.wikipedia.org/w/index.php?title=Hydraulic_motor&oldid=1027427666"^^xsd:anyURI ;
                 cco:ont00001760 "https://www.commoncoreontologies.org/ArtifactOntology"^^xsd:anyURI .


###  https://www.commoncoreontologies.org/ont00000781
cco:ont00000781 rdf:type owl:Class ;
                 rdfs:subClassOf cco:ont00000995 ;
                 rdfs:label "Control System"@en ;
                 skos:definition "A Material Artifact that is designed to manage, command, direct, or regulate the behavior of at least one other Artifact."@en ;
                 cco:ont00001754 "https://en.wikipedia.org/w/index.php?title=Control_system&oldid=1061817176"^^xsd:anyURI ;
                 cco:ont00001760 "https://www.commoncoreontologies.org/ArtifactOntology"^^xsd:anyURI .


###  https://www.commoncoreontologies.org/ont00000785
cco:ont00000785 rdf:type owl:Class ;
                 rdfs:subClassOf cco:ont00001320 ;
                 rdfs:label "Radio Repeater"@en ;
                 skos:definition "A Radio Transceiver that is designed to receive a radio signal, amplify it, and retransmit it (often on another frequency)."@en ;
                 cco:ont00001754 "https://en.wikipedia.org/w/index.php?title=Repeater&oldid=1040047439"^^xsd:anyURI ;
                 cco:ont00001760 "https://www.commoncoreontologies.org/ArtifactOntology"^^xsd:anyURI .


###  https://www.commoncoreontologies.org/ont00000788
cco:ont00000788 rdf:type owl:Class ;
                 rdfs:subClassOf cco:ont00000634 ;
                 rdfs:label "Turbine Steam Engine"@en ;
                 skos:altLabel "Steam Turbine"@en ;
                 skos:definition "A Steam Engine that is designed to extract thermal energy from pressurized steam and use it to do mechanical work on a rotating output shaft."@en ;
                 cco:ont00001754 "https://en.wikipedia.org/w/index.php?title=Steam_turbine&oldid=1060224962"^^xsd:anyURI ;
                 cco:ont00001760 "https://www.commoncoreontologies.org/ArtifactOntology"^^xsd:anyURI .


###  https://www.commoncoreontologies.org/ont00000790
cco:ont00000790 rdf:type owl:Class ;
                 rdfs:subClassOf cco:ont00001049 ;
                 rdfs:label "Direct Current Power Source"@en ;
                 skos:definition "An Electrical Power Source that is designed to transfer electrical power in the form of direct current."@en ;
                 cco:ont00001760 "https://www.commoncoreontologies.org/ArtifactOntology"^^xsd:anyURI .


###  https://www.commoncoreontologies.org/ont00000791
cco:ont00000791 rdf:type owl:Class ;
                 rdfs:subClassOf cco:ont00000323 ;
                 rdfs:label "Chemical Reaction Artifact Function"@en ;
                 skos:definition "An Artifact Function that is realized in a process that leads to the transformation of one set of chemical substances to another."@en ;
                 cco:ont00001754 "https://en.wikipedia.org/w/index.php?title=Chemical_reaction&oldid=1063262412"^^xsd:anyURI ;
                 cco:ont00001760 "https://www.commoncoreontologies.org/ArtifactOntology"^^xsd:anyURI .


###  https://www.commoncoreontologies.org/ont00000792
cco:ont00000792 rdf:type owl:Class ;
                 rdfs:subClassOf cco:ont00001009 ;
                 rdfs:label "Catadioptric Optical Telescope"@en ;
                 skos:altLabel "Catadioptric Telescope"@en ;
                 skos:definition "An Optical Telescope that is designed to aid in the observation of spatially distant Objects by means of collecting and focusing visible light through the use of a combination of Lenses and Mirrors to form an enhanced image of the Object."@en ;
                 cco:ont00001754 "https://en.wikipedia.org/w/index.php?title=Catadioptric_system&oldid=1017210114"^^xsd:anyURI ;
                 cco:ont00001760 "https://www.commoncoreontologies.org/ArtifactOntology"^^xsd:anyURI .


###  https://www.commoncoreontologies.org/ont00000793
cco:ont00000793 rdf:type owl:Class ;
                 rdfs:subClassOf cco:ont00000256 ;
                 rdfs:label "Fuel Ventilation System"@en ;
                 skos:definition "A Fluid Control Artifact that is designed to allow air into the Fuel Tank to take the place of burned fuel."@en ;
                 cco:ont00001754 "https://en.wikipedia.org/w/index.php?title=Aircraft_fuel_system&oldid=1003132173"^^xsd:anyURI ;
                 cco:ont00001760 "https://www.commoncoreontologies.org/ArtifactOntology"^^xsd:anyURI .


###  https://www.commoncoreontologies.org/ont00000795
cco:ont00000795 rdf:type owl:Class ;
                 rdfs:subClassOf cco:ont00000098 ;
                 rdfs:label "Electrical Conduction Artifact Function"@en ;
                 skos:definition "An Electrical Artifact Function that is realized by an Artifact being used to conduct an electric current."@en ;
                 cco:ont00001760 "https://www.commoncoreontologies.org/ArtifactOntology"^^xsd:anyURI .


###  https://www.commoncoreontologies.org/ont00000796
cco:ont00000796 rdf:type owl:Class ;
                 rdfs:subClassOf cco:ont00000618 ;
                 rdfs:label "Rail Transport Vehicle"@en ;
                 skos:definition "A Ground Vehicle that is designed to convey cargo, passengers, or equipment by Railway."@en ;
                 cco:ont00001754 "https://en.wikipedia.org/w/index.php?title=Rail_transport&oldid=1063793805"^^xsd:anyURI ;
                 cco:ont00001760 "https://www.commoncoreontologies.org/ArtifactOntology"^^xsd:anyURI .


###  https://www.commoncoreontologies.org/ont00000798
cco:ont00000798 rdf:type owl:Class ;
                 rdfs:subClassOf cco:ont00000995 ,
                                 [ rdf:type owl:Restriction ;
                                   owl:onProperty obo:BFO_0000101 ;
                                   owl:someValuesFrom cco:ont00000958
                                 ] ,
                                 [ rdf:type owl:Restriction ;
                                   owl:onProperty obo:BFO_0000176 ;
                                   owl:someValuesFrom cco:ont00000893
                                 ] ;
                 rdfs:label "Information Bearing Artifact"@en ;
                 skos:definition "A Material Artifact that carries an Information Content Entity and is designed to do so using a particular format or structure."@en ;
                 cco:ont00001760 "https://www.commoncoreontologies.org/ArtifactOntology"^^xsd:anyURI .


###  https://www.commoncoreontologies.org/ont00000799
cco:ont00000799 rdf:type owl:Class ;
                 rdfs:subClassOf cco:ont00000798 ;
                 rdfs:label "List"@en ;
                 skos:definition "An Information Bearing Artifact that consists of one or more Information Bearing Artifacts that carry Information Content Entities and are the subjects of some Sequence Position Ordinality."@en ;
                 cco:ont00001754 "https://en.wikipedia.org/w/index.php?title=List_(abstract_data_type)&oldid=1041588680"^^xsd:anyURI ;
                 cco:ont00001760 "https://www.commoncoreontologies.org/ArtifactOntology"^^xsd:anyURI .


###  https://www.commoncoreontologies.org/ont00000804
cco:ont00000804 rdf:type owl:Class ;
                 rdfs:subClassOf cco:ont00000136 ;
                 rdfs:label "Prism"@en ;
                 skos:definition "An Optical Instrument that is designed to refract light and which consists of a transparent material with flat polished surfaces where at least two of these surfaces have an angle between them."@en ;
                 cco:ont00001754 "https://en.wikipedia.org/w/index.php?title=Prism&oldid=1060221124"^^xsd:anyURI ;
                 cco:ont00001760 "https://www.commoncoreontologies.org/ArtifactOntology"^^xsd:anyURI .


###  https://www.commoncoreontologies.org/ont00000806
cco:ont00000806 rdf:type owl:Class ;
                 rdfs:subClassOf cco:ont00000581 ;
                 rdfs:label "Power Tool"@en ;
                 skos:definition "A Tool that is designed to be actuated by a Power Source and mechanism other than or in addition to manual labor."@en ;
                 cco:ont00001754 "https://en.wikipedia.org/w/index.php?title=Power_tool&oldid=1057147715"^^xsd:anyURI ;
                 cco:ont00001760 "https://www.commoncoreontologies.org/ArtifactOntology"^^xsd:anyURI .


###  https://www.commoncoreontologies.org/ont00000807
cco:ont00000807 rdf:type owl:Class ;
                 rdfs:subClassOf cco:ont00000394 ;
                 rdfs:label "Compression Ignition Engine"@en ;
                 skos:definition "An Internal Combustion Engine that is designed to operate by igniting a portion of Fuel and Oxidizer mixture using heat generated via compression of the mixture."@en ;
                 cco:ont00001760 "https://www.commoncoreontologies.org/ArtifactOntology"^^xsd:anyURI .


###  https://www.commoncoreontologies.org/ont00000808
cco:ont00000808 rdf:type owl:Class ;
                 rdfs:subClassOf cco:ont00000791 ;
                 rdfs:label "Reactant Artifact Function"@en ;
                 skos:definition "A Chemical Reaction Artifact Function that is realized in a process in which a substance or compound is added to a system in order to bring about a chemical reaction and is consumed in the course of the reaction."@en ;
                 cco:ont00001754 "https://en.wikipedia.org/w/index.php?title=Reagent&oldid=1017651471"^^xsd:anyURI ;
                 cco:ont00001760 "https://www.commoncoreontologies.org/ArtifactOntology"^^xsd:anyURI .


###  https://www.commoncoreontologies.org/ont00000809
cco:ont00000809 rdf:type owl:Class ;
                 rdfs:subClassOf cco:ont00000323 ;
                 rdfs:label "Submersible Artifact Function"@en ;
                 skos:definition "An Artifact Function that is realized in processes of operating while submerged in water."@en ;
                 cco:ont00001754 "https://en.wikipedia.org/w/index.php?title=Submersible&oldid=1062994844"^^xsd:anyURI ;
                 cco:ont00001760 "https://www.commoncoreontologies.org/ArtifactOntology"^^xsd:anyURI .


###  https://www.commoncoreontologies.org/ont00000811
cco:ont00000811 rdf:type owl:Class ;
                 rdfs:subClassOf cco:ont00000323 ;
                 rdfs:label "Radio Wave Conversion Artifact Function"@en ;
                 skos:definition "An Artifact Function that is realized by an Artifact being used to convert electric power into radio waves or radio waves into electric power."@en ;
                 cco:ont00001760 "https://www.commoncoreontologies.org/ArtifactOntology"^^xsd:anyURI .


###  https://www.commoncoreontologies.org/ont00000813
cco:ont00000813 rdf:type owl:Class ;
                 rdfs:subClassOf cco:ont00000457 ;
                 rdfs:label "Portion of Nuclear Fuel"@en ;
                 skos:definition "A Portion of Material that is designed to be used in a nuclear fission process to produce energy."@en ;
                 cco:ont00001760 "https://www.commoncoreontologies.org/ArtifactOntology"^^xsd:anyURI .


###  https://www.commoncoreontologies.org/ont00000816
cco:ont00000816 rdf:type owl:Class ;
                 rdfs:subClassOf cco:ont00000255 ;
                 rdfs:label "Portion of Liquid Nitrogen"@en ;
                 skos:definition "A Portion of Cryogenic Material that is composed (almost) entirely of liquid nitrogen."@en ;
                 cco:ont00001760 "https://www.commoncoreontologies.org/ArtifactOntology"^^xsd:anyURI .


###  https://www.commoncoreontologies.org/ont00000823
cco:ont00000823 rdf:type owl:Class ;
                 rdfs:subClassOf cco:ont00001148 ;
                 rdfs:label "Optical Communication Artifact Function"@en ;
                 skos:definition "An Electromagnetic Communication Artifact Function that is realized in a process that conveys meaningful signs by means of visible light."@en ;
                 cco:ont00001754 "https://en.wikipedia.org/w/index.php?title=Telecommunications&oldid=1061143810"^^xsd:anyURI ;
                 cco:ont00001760 "https://www.commoncoreontologies.org/ArtifactOntology"^^xsd:anyURI .


###  https://www.commoncoreontologies.org/ont00000825
cco:ont00000825 rdf:type owl:Class ;
                 rdfs:subClassOf cco:ont00000346 ;
                 rdfs:label "Telecommunication Network Line"@en ;
                 skos:definition "A Communication Artifact that is designed to be the physical transmission medium that connects two or more Telecommunication Network Nodes within a Telecommunication Network to facilitate communication between the Nodes."@en ;
                 cco:ont00001754 "https://en.wikipedia.org/w/index.php?title=Telecommunications_link&oldid=1062252217"^^xsd:anyURI ;
                 cco:ont00001760 "https://www.commoncoreontologies.org/ArtifactOntology"^^xsd:anyURI .


###  https://www.commoncoreontologies.org/ont00000828
cco:ont00000828 rdf:type owl:Class ;
                 rdfs:subClassOf cco:ont00001123 ;
                 rdfs:label "Pesticide Artifact Function"@en ;
                 skos:definition "A Poison Artifact Function that is realized in a process which causes illness in, or the death of, a living thing that is detrimental to humans or human concerns."@en ;
                 cco:ont00001754 "http://www.dictionary.com/browse/pesticide" ;
                 cco:ont00001760 "https://www.commoncoreontologies.org/ArtifactOntology"^^xsd:anyURI .


###  https://www.commoncoreontologies.org/ont00000831
cco:ont00000831 rdf:type owl:Class ;
                 rdfs:subClassOf cco:ont00000828 ;
                 rdfs:label "Herbicide Artifact Function"@en ;
                 skos:definition "A Pesticide Artifact Function that is realized in a process which causes harm to, or the death to, unwanted plants."@en ;
                 cco:ont00001754 "https://en.wikipedia.org/w/index.php?title=Herbicide&oldid=1061228045"^^xsd:anyURI ;
                 cco:ont00001760 "https://www.commoncoreontologies.org/ArtifactOntology"^^xsd:anyURI .


###  https://www.commoncoreontologies.org/ont00000838
cco:ont00000838 rdf:type owl:Class ;
                 rdfs:subClassOf cco:ont00000457 ;
                 rdfs:label "Portion of Fuel"@en ;
                 skos:definition "A Portion of Material that is designed to release thermal energy when reacted with other substances."@en ;
                 cco:ont00001760 "https://www.commoncoreontologies.org/ArtifactOntology"^^xsd:anyURI .


###  https://www.commoncoreontologies.org/ont00000840
cco:ont00000840 rdf:type owl:Class ;
                 rdfs:subClassOf cco:ont00000618 ;
                 rdfs:label "Bicycle"@en ;
                 skos:definition "A Ground Vehicle that consists of two wheels, one in front of the other, attached to a frame along with handlebars and pedals such that it is designed to receive its motive power from pedaling."@en ;
                 cco:ont00001754 "https://en.wikipedia.org/w/index.php?title=Bicycle&oldid=1063761124"^^xsd:anyURI ;
                 cco:ont00001760 "https://www.commoncoreontologies.org/ArtifactOntology"^^xsd:anyURI .


###  https://www.commoncoreontologies.org/ont00000841
cco:ont00000841 rdf:type owl:Class ;
                 rdfs:subClassOf cco:ont00001153 ;
                 rdfs:label "Explosive Artifact Function"@en ;
                 skos:definition "A Damaging Artifact Function that is realized in a process in which the structural integrity of an entity is impaired beucase of the rapid increase in volume and release of energy in an extreme manner."@en ;
                 cco:ont00001754 "http://www.dictionary.com/browse/explosive" ;
                 cco:ont00001760 "https://www.commoncoreontologies.org/ArtifactOntology"^^xsd:anyURI .


###  https://www.commoncoreontologies.org/ont00000843
cco:ont00000843 rdf:type owl:Class ;
                 rdfs:subClassOf cco:ont00001049 ;
                 rdfs:label "Solar Panel"@en ;
                 skos:definition "An Electrical Power Source that consists in part of one or more photovoltaic (i.e. solar) cells that convert light energy (photons) directly into electricity by means of the photovoltaic effect."@en ;
                 cco:ont00001754 "https://en.wikipedia.org/w/index.php?title=Solar_cell&oldid=1063439932"^^xsd:anyURI ,
                                  "https://en.wikipedia.org/w/index.php?title=Solar_panel&oldid=1064397496"^^xsd:anyURI ;
                 cco:ont00001760 "https://www.commoncoreontologies.org/ArtifactOntology"^^xsd:anyURI .


###  https://www.commoncoreontologies.org/ont00000848
cco:ont00000848 rdf:type owl:Class ;
                 rdfs:subClassOf cco:ont00000088 ;
                 rdfs:label "Mounted Gun"@en ;
                 skos:definition "A Firearm that is designed to be fired while mounted."@en ;
                 cco:ont00001760 "https://www.commoncoreontologies.org/ArtifactOntology"^^xsd:anyURI .


###  https://www.commoncoreontologies.org/ont00000849
cco:ont00000849 rdf:type owl:Class ;
                 rdfs:subClassOf cco:ont00000453 ;
                 rdfs:label "Heating System"@en ;
                 skos:definition "An Environment Control System that is designed to heat the air or objects in a Site."@en ;
                 cco:ont00001760 "https://www.commoncoreontologies.org/ArtifactOntology"^^xsd:anyURI .


###  https://www.commoncoreontologies.org/ont00000851
cco:ont00000851 rdf:type owl:Class ;
                 rdfs:subClassOf cco:ont00001104 ;
                 rdfs:label "Light Machine Gun"@en ;
                 skos:definition "A Long Gun that is designed to fire bullets in quick succession from an ammunition belt or magazine and to be employed by an individual soldier, with or without assistance, and typically weighing 9-22 lbs."@en ;
                 cco:ont00001754 "https://en.wikipedia.org/w/index.php?title=Light_machine_gun&oldid=1063598801"^^xsd:anyURI ;
                 cco:ont00001760 "https://www.commoncoreontologies.org/ArtifactOntology"^^xsd:anyURI .


###  https://www.commoncoreontologies.org/ont00000856
cco:ont00000856 rdf:type owl:Class ;
                 rdfs:subClassOf obo:BFO_0000182 ;
                 rdfs:label "Artifact History"@en ;
                 skos:definition "A History of an Artifact."@en ;
                 cco:ont00001760 "https://www.commoncoreontologies.org/ArtifactOntology"^^xsd:anyURI .


###  https://www.commoncoreontologies.org/ont00000857
cco:ont00000857 rdf:type owl:Class ;
                 rdfs:subClassOf cco:ont00000903 ;
                 rdfs:label "Ultra High Frequency Communication Instrument"@en ;
                 skos:definition "A Radio Communication Instrument that is designed to participate in some process that has process part some Ultra High Frequency."@en ;
                 cco:ont00001760 "https://www.commoncoreontologies.org/ArtifactOntology"^^xsd:anyURI .


###  https://www.commoncoreontologies.org/ont00000858
cco:ont00000858 rdf:type owl:Class ;
                 rdfs:subClassOf cco:ont00000552 ;
                 rdfs:label "Improvised Explosive Device"@en ;
                 skos:definition "An Explosive Weapon that is designed to be used in non-conventional military action."@en ;
                 cco:ont00001753 "IED" ;
                 cco:ont00001754 "https://en.wikipedia.org/w/index.php?title=Improvised_explosive_device&oldid=1063432318"^^xsd:anyURI ;
                 cco:ont00001760 "https://www.commoncoreontologies.org/ArtifactOntology"^^xsd:anyURI .


###  https://www.commoncoreontologies.org/ont00000864
cco:ont00000864 rdf:type owl:Class ;
                 rdfs:subClassOf cco:ont00001301 ;
                 rdfs:label "Public Safety Artifact Function"@en ;
                 skos:definition "A Service Artifact Function that is realized in processes of preventing and responding to events that could endanger the safety of the general public from significant danger, injury/harm, or damage, such as crimes or disasters (natural or man-made)."@en ;
                 cco:ont00001754 "https://en.wikipedia.org/w/index.php?title=Public_security&oldid=1058257389"^^xsd:anyURI ;
                 cco:ont00001760 "https://www.commoncoreontologies.org/ArtifactOntology"^^xsd:anyURI .


###  https://www.commoncoreontologies.org/ont00000868
cco:ont00000868 rdf:type owl:Class ;
                 rdfs:subClassOf cco:ont00001173 ;
                 rdfs:label "Rocket Pod"@en ;
                 skos:definition "A Rocket Launcher that is designed to contain several Unguided Rockets held in individual tubes and to be used by Aircraft or Helicopters for close air support."@en ;
                 cco:ont00001760 "https://www.commoncoreontologies.org/ArtifactOntology"^^xsd:anyURI .


###  https://www.commoncoreontologies.org/ont00000869
cco:ont00000869 rdf:type owl:Class ;
                 rdfs:subClassOf cco:ont00000199 ;
                 rdfs:label "Optical Camera"@en ;
                 skos:definition "A Camera that is designed to form and record an image generated from visible light."@en ;
                 cco:ont00001754 "https://en.wikipedia.org/w/index.php?title=Camera&oldid=1063931551"^^xsd:anyURI ;
                 cco:ont00001760 "https://www.commoncoreontologies.org/ArtifactOntology"^^xsd:anyURI .


###  https://www.commoncoreontologies.org/ont00000870
cco:ont00000870 rdf:type owl:Class ;
                 rdfs:subClassOf obo:BFO_0000040 ;
                 rdfs:label "Infrastructure System"@en ;
                 skos:altLabel "Infrastructure"@en ;
                 skos:definition "A Material Entity that is composed of elements bearing Infrastructure Roles and is by itself sufficient to provide a planned service or benefit to some organization that maintains its elements."@en ;
                 cco:ont00001760 "https://www.commoncoreontologies.org/ArtifactOntology"^^xsd:anyURI .


###  https://www.commoncoreontologies.org/ont00000874
cco:ont00000874 rdf:type owl:Class ;
                 rdfs:subClassOf cco:ont00000798 ;
                 rdfs:label "Video"@en ;
                 skos:definition "An Information Bearing Artifact that is designed to bear some specific Information Content Entity in the form of a sequence of representations that are presented sufficiently rapidly to create the appearance of motion and continuity."@en ;
                 cco:ont00001754 "https://en.wikipedia.org/w/index.php?title=Video&oldid=1049376249"^^xsd:anyURI ;
                 cco:ont00001760 "https://www.commoncoreontologies.org/ArtifactOntology"^^xsd:anyURI .


###  https://www.commoncoreontologies.org/ont00000877
cco:ont00000877 rdf:type owl:Class ;
                 rdfs:subClassOf cco:ont00000723 ;
                 rdfs:label "Brake Control System"@en ;
                 skos:definition "A Vehicle Control System that is designed to control the process of braking with the aim of preventing rolling, skidding, and hydroplaning."@en ;
                 cco:ont00001760 "https://www.commoncoreontologies.org/ArtifactOntology"^^xsd:anyURI .


###  https://www.commoncoreontologies.org/ont00000878
cco:ont00000878 rdf:type owl:Class ;
                 rdfs:subClassOf cco:ont00000325 ;
                 rdfs:label "Identification Friend or Foe Transponder"@en ;
                 skos:altLabel "IFF"@en ;
                 skos:definition "A Radio Transponder that is designed to automatically transmit a predefined signal in response to receiving an appropriate interrogation signal such that the entity it is located on can be positively identified as friendly."@en ;
                 cco:ont00001754 "https://en.wikipedia.org/w/index.php?title=Identification_friend_or_foe&oldid=1055168718"^^xsd:anyURI ;
                 cco:ont00001760 "https://www.commoncoreontologies.org/ArtifactOntology"^^xsd:anyURI .


###  https://www.commoncoreontologies.org/ont00000880
cco:ont00000880 rdf:type owl:Class ;
                 rdfs:subClassOf cco:ont00001301 ;
                 rdfs:label "Religious Artifact Function"@en ;
                 skos:definition "A Service Artifact Function that is realized in processes related to worship and prayer."@en ;
                 cco:ont00001754 "https://en.wikipedia.org/w/index.php?title=Religion&oldid=1063431202"^^xsd:anyURI ;
                 cco:ont00001760 "https://www.commoncoreontologies.org/ArtifactOntology"^^xsd:anyURI .


###  https://www.commoncoreontologies.org/ont00000886
cco:ont00000886 rdf:type owl:Class ;
                 rdfs:subClassOf cco:ont00000422 ;
                 rdfs:label "Wired Communication Reception Artifact Function"@en ;
                 skos:definition "A Communication Reception Artifact Function that is realized during events in which an Artifact receives information transmitted from another Artifact, where the transmission of information occurs via a direct connection using an electrical conductor."@en ;
                 cco:ont00001760 "https://www.commoncoreontologies.org/ArtifactOntology"^^xsd:anyURI .


###  https://www.commoncoreontologies.org/ont00000888
cco:ont00000888 rdf:type owl:Class ;
                 rdfs:subClassOf cco:ont00000903 ;
                 rdfs:label "High Frequency Communication Instrument"@en ;
                 skos:definition "A Radio Communication Instrument that is designed to participate in some process that has process part some High Frequency."@en ;
                 cco:ont00001760 "https://www.commoncoreontologies.org/ArtifactOntology"^^xsd:anyURI .


###  https://www.commoncoreontologies.org/ont00000893
cco:ont00000893 rdf:type owl:Class ;
                 rdfs:subClassOf cco:ont00000995 ;
                 rdfs:comment "An empty notebook, when manufactured, is a medium but not yet a carrier of information content. However, a book, in the sense of a novel or collection of philosophical essays or poems, depends necessarily on it carrying some information content. Thus, there are no empty books. Likewise, there are no empty databases, only portions of digital storage that have not yet been configured to carry some information content according to a database software application."@en ;
                 rdfs:label "Information Medium Artifact"@en ;
                 skos:definition "A Material Artifact that is designed to have some Information Bearing Artifact as part."@en ;
                 skos:example "A magnetic hard drive" ,
                              "A notebook" ;
                 cco:ont00001760 "https://www.commoncoreontologies.org/ArtifactOntology"^^xsd:anyURI .


###  https://www.commoncoreontologies.org/ont00000897
cco:ont00000897 rdf:type owl:Class ;
                 rdfs:subClassOf cco:ont00000457 ;
                 rdfs:comment "Oxidizers are essential participants in many processes including combustion and rusting. Hence, a portion of oxidizer must always be present along with a portion of fuel in order for combustion to occur."@en ;
                 rdfs:label "Portion of Oxidizer"@en ;
                 skos:altLabel "Portion of Oxidant"@en ,
                               "Portion of Oxidizing Agent"@en ;
                 skos:definition "A Portion of Material that is disposed to steal electrons from other substances (i.e. to oxidize other substances) as a participant in a reduction-oxidation process."@en ;
                 skos:example "oxygen, hydrogen peroxide, chlorine, sulfiric acid, potassium nitrate" ;
                 cco:ont00001760 "https://www.commoncoreontologies.org/ArtifactOntology"^^xsd:anyURI .


###  https://www.commoncoreontologies.org/ont00000899
cco:ont00000899 rdf:type owl:Class ;
                 rdfs:subClassOf cco:ont00000258 ;
                 rdfs:label "MSI Plessey Barcode"@en ;
                 skos:definition "A One-Dimensional Barcode that consists of an indefinite number of numerical characters and is used for inventory control and marking storage containers and shelves in warehouse environments."@en ;
                 cco:ont00001760 "https://www.commoncoreontologies.org/ArtifactOntology"^^xsd:anyURI .


###  https://www.commoncoreontologies.org/ont00000900
cco:ont00000900 rdf:type owl:Class ;
                 rdfs:subClassOf cco:ont00001169 ;
                 rdfs:label "Radio Communication Relay Artifact Function"@en ;
                 skos:definition "A Communication Relay Artifact Function that is realized during events in which an Artifact is used to first receive and then transmit information without the use of wires from one Artifact to another for the purpose of communiction."@en ;
                 cco:ont00001760 "https://www.commoncoreontologies.org/ArtifactOntology"^^xsd:anyURI .


###  https://www.commoncoreontologies.org/ont00000903
cco:ont00000903 rdf:type owl:Class ;
                 rdfs:subClassOf cco:ont00000346 ;
                 rdfs:label "Radio Communication Instrument"@en ;
                 skos:definition "A Communication Instrument that is designed to enable communication between two or more entities via the use of radio waves."@en ;
                 cco:ont00001760 "https://www.commoncoreontologies.org/ArtifactOntology"^^xsd:anyURI .


###  https://www.commoncoreontologies.org/ont00000904
cco:ont00000904 rdf:type owl:Class ;
                 rdfs:subClassOf cco:ont00000205 ,
                                 [ rdf:type owl:Restriction ;
                                   owl:onProperty cco:ont00001855 ;
                                   owl:someValuesFrom cco:ont00000122
                                 ] ;
                 rdfs:label "Vehicle Track"@en ;
                 skos:definition "An Object Track for a Vehicle during some motion."@en ;
                 cco:ont00001760 "https://www.commoncoreontologies.org/ArtifactOntology"^^xsd:anyURI .


###  https://www.commoncoreontologies.org/ont00000906
cco:ont00000906 rdf:type owl:Class ;
                 rdfs:subClassOf cco:ont00000690 ;
                 rdfs:label "Email Box"@en ;
                 skos:definition "A Telecommunication Instrument that is designed to be the delivery destination of Email Messages that are addressed to the corresponding Email Address."@en ;
                 cco:ont00001754 "https://en.wikipedia.org/w/index.php?title=Email_box&oldid=1061295368"^^xsd:anyURI ;
                 cco:ont00001760 "https://www.commoncoreontologies.org/ArtifactOntology"^^xsd:anyURI .


###  https://www.commoncoreontologies.org/ont00000907
cco:ont00000907 rdf:type owl:Class ;
                 rdfs:subClassOf cco:ont00000690 ;
                 rdfs:label "Telephone"@en ;
                 skos:altLabel "Phone"@en ;
                 skos:definition "A Telecommunication Instrument that is designed to provide point-to-point communication between agents by means of audio messages."@en ;
                 cco:ont00001754 "https://en.wikipedia.org/w/index.php?title=Telephone&oldid=1060006278"^^xsd:anyURI ;
                 cco:ont00001760 "https://www.commoncoreontologies.org/ArtifactOntology"^^xsd:anyURI .


###  https://www.commoncoreontologies.org/ont00000909
cco:ont00000909 rdf:type owl:Class ;
                 rdfs:subClassOf cco:ont00001049 ;
                 rdfs:label "Emergency AC/DC Power Source"@en ;
                 skos:definition "An Electrical Power Source that is designed to provide electrical power in an emergency situation by means of both alternating current and direct current."@en ;
                 cco:ont00001760 "https://www.commoncoreontologies.org/ArtifactOntology"^^xsd:anyURI .


###  https://www.commoncoreontologies.org/ont00000918
cco:ont00000918 rdf:type owl:Class ;
                 rdfs:subClassOf cco:ont00000346 ,
                                 [ rdf:type owl:Restriction ;
                                   owl:onProperty obo:BFO_0000176 ;
                                   owl:someValuesFrom cco:ont00000998
                                 ] ;
                 rdfs:label "Telecommunication Network Node"@en ;
                 skos:definition "A Communication Artifact that consists of a connection point, redistribution point, or endpoint that is designed to be part of a Telecommunication Network and can be either active or passive."@en ;
                 cco:ont00001754 "https://en.wikipedia.org/wiki/Node_(networking)" ;
                 cco:ont00001760 "https://www.commoncoreontologies.org/ArtifactOntology"^^xsd:anyURI .


###  https://www.commoncoreontologies.org/ont00000919
cco:ont00000919 rdf:type owl:Class ;
                 rdfs:subClassOf cco:ont00000575 ;
                 rdfs:label "Parts List"@en ;
                 skos:definition "A Quality Specification that prescribes the Amount of some type of Artifact that are part of or located on another Artifact."@en ;
                 cco:ont00001760 "https://www.commoncoreontologies.org/ArtifactOntology"^^xsd:anyURI .


###  https://www.commoncoreontologies.org/ont00000928
cco:ont00000928 rdf:type owl:Class ;
                 rdfs:subClassOf cco:ont00000796 ;
                 rdfs:label "Train Car"@en ;
                 skos:altLabel "Railroad Car"@en ;
                 skos:definition "A Rail Transport Vehicle that consists of a single Vehicle that is not a Train but is designed to be connected to other Train Cars along with at least one Locomotive to form a Train."@en ;
                 cco:ont00001754 "https://en.wikipedia.org/w/index.php?title=Railroad_car&oldid=1063802472"^^xsd:anyURI ;
                 cco:ont00001760 "https://www.commoncoreontologies.org/ArtifactOntology"^^xsd:anyURI .


###  https://www.commoncoreontologies.org/ont00000929
cco:ont00000929 rdf:type owl:Class ;
                 rdfs:subClassOf obo:BFO_0000023 ;
                 rdfs:label "Part Role"@en ;
                 skos:definition "A Role that inheres in an entity in virtue of it being part of some other entity without being subject to further subdivision or disassembly without destruction of its designated use."@en ;
                 cco:ont00001754 "http://origins.sese.asu.edu/ses405/Class%20Notes/Sys-Hier-WBS_Module_V1.0_PAS.pdf"^^xsd:anyURI ;
                 cco:ont00001760 "https://www.commoncoreontologies.org/ArtifactOntology"^^xsd:anyURI .


###  https://www.commoncoreontologies.org/ont00000930
cco:ont00000930 rdf:type owl:Class ;
                 rdfs:subClassOf cco:ont00001105 ;
                 rdfs:label "Nickel-metal Hydride Electric Battery"@en ;
                 skos:altLabel "NiMH Battery"@en ;
                 skos:definition "A Secondary Cell Electric Battery that has a metal-hydride anode and nickel oxide hydroxide cathode."@en ;
                 cco:ont00001754 "https://en.wikipedia.org/w/index.php?title=Nickel%E2%80%93metal_hydride_battery&oldid=1061626676"^^xsd:anyURI ;
                 cco:ont00001760 "https://www.commoncoreontologies.org/ArtifactOntology"^^xsd:anyURI .


###  https://www.commoncoreontologies.org/ont00000931
cco:ont00000931 rdf:type owl:Class ;
                 rdfs:subClassOf cco:ont00000326 ;
                 rdfs:label "UPC-A Barcode"@en ;
                 skos:definition "A UPC Barcode that consists of 12 numerical digits."@en ;
                 cco:ont00001760 "https://www.commoncoreontologies.org/ArtifactOntology"^^xsd:anyURI .


###  https://www.commoncoreontologies.org/ont00000932
cco:ont00000932 rdf:type owl:Class ;
                 rdfs:subClassOf cco:ont00000323 ;
                 rdfs:label "Computing Artifact Function"@en ;
                 skos:definition "An Artifact Function that is realized by an Artifact participating in a computation process."@en ;
                 cco:ont00001760 "https://www.commoncoreontologies.org/ArtifactOntology"^^xsd:anyURI .


###  https://www.commoncoreontologies.org/ont00000933
cco:ont00000933 rdf:type owl:Class ;
                 rdfs:subClassOf cco:ont00000907 ;
                 rdfs:label "Landline Telephone"@en ;
                 skos:definition "A Telephone that is connected to a Telephone Network through a pair of wires."@en ;
                 cco:ont00001754 "https://en.wikipedia.org/w/index.php?title=Telephone&oldid=1060006278"^^xsd:anyURI ;
                 cco:ont00001760 "https://www.commoncoreontologies.org/ArtifactOntology"^^xsd:anyURI .


###  https://www.commoncoreontologies.org/ont00000937
cco:ont00000937 rdf:type owl:Class ;
                 rdfs:subClassOf cco:ont00000323 ;
                 rdfs:label "Inhibiting Motion Artifact Function"@en ;
                 skos:definition "An Artifact Function that is realized by processes in which some Artifact is used to inhibit the motion of some object."@en ;
                 cco:ont00001760 "https://www.commoncoreontologies.org/ArtifactOntology"^^xsd:anyURI .


###  https://www.commoncoreontologies.org/ont00000938
cco:ont00000938 rdf:type owl:Class ;
                 rdfs:subClassOf cco:ont00001301 ;
                 rdfs:label "Financial Artifact Function"@en ;
                 skos:definition "A Service Artifact Function that is realized in processes of managing money."@en ;
                 cco:ont00001754 "https://en.wikipedia.org/w/index.php?title=Finance&oldid=1062402926"^^xsd:anyURI ;
                 cco:ont00001760 "https://www.commoncoreontologies.org/ArtifactOntology"^^xsd:anyURI .


###  https://www.commoncoreontologies.org/ont00000942
cco:ont00000942 rdf:type owl:Class ;
                 rdfs:subClassOf cco:ont00000204 ;
                 rdfs:label "Sniper Rifle"@en ;
                 skos:definition "A Rifle that is designed to be highly accurate for long-range precision tactical shooting."@en ;
                 cco:ont00001754 "https://en.wikipedia.org/w/index.php?title=Sniper_rifle&oldid=1061592308"^^xsd:anyURI ;
                 cco:ont00001760 "https://www.commoncoreontologies.org/ArtifactOntology"^^xsd:anyURI .


###  https://www.commoncoreontologies.org/ont00000943
cco:ont00000943 rdf:type owl:Class ;
                 rdfs:subClassOf cco:ont00001248 ;
                 rdfs:label "Ocular Prosthesis"@en ;
                 skos:definition "An Artificial Eye that is designed to replace a missing eye, but which does not function as an eye."@en ;
                 cco:ont00001754 "https://en.wikipedia.org/w/index.php?title=Ocular_prosthesis&oldid=1061336760"^^xsd:anyURI ;
                 cco:ont00001760 "https://www.commoncoreontologies.org/ArtifactOntology"^^xsd:anyURI .


###  https://www.commoncoreontologies.org/ont00000944
cco:ont00000944 rdf:type owl:Class ;
                 rdfs:subClassOf cco:ont00000601 ;
                 rdfs:label "Thermal Imaging Artifact Function"@en ;
                 skos:definition "An Imaging Artifact Function that is realized during events in which an Artifact is used to create a visual representation of an entity using radiation from the far infrared region of the electromagnetic spectrum that the entity emits"@en ;
                 cco:ont00001760 "https://www.commoncoreontologies.org/ArtifactOntology"^^xsd:anyURI .


###  https://www.commoncoreontologies.org/ont00000945
cco:ont00000945 rdf:type owl:Class ;
                 rdfs:subClassOf cco:ont00000547 ;
                 rdfs:label "X-ray Telescope"@en ;
                 skos:definition "A Telescope that is designed to aid in the observation of spatially distant Objects by means of collecting and focusing X-rays to form an enhanced image of the Object."@en ;
                 cco:ont00001754 "https://en.wikipedia.org/w/index.php?title=X-ray_telescope&oldid=1035025593"^^xsd:anyURI ;
                 cco:ont00001760 "https://www.commoncoreontologies.org/ArtifactOntology"^^xsd:anyURI .


###  https://www.commoncoreontologies.org/ont00000947
cco:ont00000947 rdf:type owl:Class ;
                 rdfs:subClassOf cco:ont00001100 ;
                 rdfs:label "Temperature Measurement Artifact Function"@en ;
                 skos:definition "A Measurement Artifact Function that is realized during events in which an Artifact is used to measure the Temperature of a specified object or class of objects."@en ;
                 cco:ont00001760 "https://www.commoncoreontologies.org/ArtifactOntology"^^xsd:anyURI .


###  https://www.commoncoreontologies.org/ont00000952
cco:ont00000952 rdf:type owl:Class ;
                 rdfs:subClassOf cco:ont00000210 ;
                 rdfs:label "Electric Motor"@en ;
                 skos:altLabel "Electric Engine"@en ;
                 skos:definition "An Engine that is designed to convert electrical energy into mechanical energy."@en ;
                 cco:ont00001754 "https://en.wikipedia.org/w/index.php?title=Electric_motor&oldid=1063829856"^^xsd:anyURI ;
                 cco:ont00001760 "https://www.commoncoreontologies.org/ArtifactOntology"^^xsd:anyURI .


###  https://www.commoncoreontologies.org/ont00000954
cco:ont00000954 rdf:type owl:Class ;
                 rdfs:subClassOf cco:ont00000870 ;
                 rdfs:label "Telecommunication Infrastructure"@en ;
                 skos:definition "An Infrastructure System that is designed to support the use of Telecommunication Instruments to communicate."@en ;
                 cco:ont00001754 "https://en.wikipedia.org/w/index.php?title=Category:Telecommunications_infrastructure&oldid=989151314"^^xsd:anyURI ;
                 cco:ont00001760 "https://www.commoncoreontologies.org/ArtifactOntology"^^xsd:anyURI .


###  https://www.commoncoreontologies.org/ont00000956
cco:ont00000956 rdf:type owl:Class ;
                 rdfs:subClassOf cco:ont00001086 ;
                 rdfs:label "Highway Interchange"@en ;
                 skos:definition "A Road Junction that is designed to enable Ground Vehicles to exit one or more Highways and enter another Highway without directly crossing any other traffic stream."@en ;
                 cco:ont00001754 "https://en.wikipedia.org/wiki/Interchange_(road)" ;
                 cco:ont00001760 "https://www.commoncoreontologies.org/ArtifactOntology"^^xsd:anyURI .


###  https://www.commoncoreontologies.org/ont00000958
cco:ont00000958 rdf:type owl:Class .


###  https://www.commoncoreontologies.org/ont00000961
cco:ont00000961 rdf:type owl:Class ;
                 rdfs:subClassOf cco:ont00000098 ;
                 rdfs:label "Current Conversion Artifact Function"@en ;
                 skos:definition "An Electrical Artifact Function that is realized by processes in which some Artifact is used to convert some electrical current."@en ;
                 cco:ont00001760 "https://www.commoncoreontologies.org/ArtifactOntology"^^xsd:anyURI .


###  https://www.commoncoreontologies.org/ont00000962
cco:ont00000962 rdf:type owl:Class ;
                 rdfs:subClassOf cco:ont00000593 ;
                 rdfs:label "Portion of Liquid Propellant"@en ;
                 skos:definition "A Portion of Propellant that is stored in a liquid state."@en ;
                 cco:ont00001760 "https://www.commoncoreontologies.org/ArtifactOntology"^^xsd:anyURI .


###  https://www.commoncoreontologies.org/ont00000963
cco:ont00000963 rdf:type owl:Class ;
                 rdfs:subClassOf cco:ont00000256 ;
                 rdfs:label "Fuel Transfer System"@en ;
                 skos:definition "A Fluid Control Artifact that is designed to facilitate the transfer of some Portion of Fuel from the Fuel Tank for use in some Engine."@en ;
                 cco:ont00001760 "https://www.commoncoreontologies.org/ArtifactOntology"^^xsd:anyURI .


###  https://www.commoncoreontologies.org/ont00000965
cco:ont00000965 rdf:type owl:Class .


###  https://www.commoncoreontologies.org/ont00000966
cco:ont00000966 rdf:type owl:Class ;
                 rdfs:subClassOf cco:ont00000258 ;
                 rdfs:label "EAN Barcode"@en ;
                 skos:definition "A One-Dimensional Barcode that consists of 8 or 13 numerical digits and is used to scan consumer goods."@en ;
                 cco:ont00001760 "https://www.commoncoreontologies.org/ArtifactOntology"^^xsd:anyURI .


###  https://www.commoncoreontologies.org/ont00000968
cco:ont00000968 rdf:type owl:Class ;
                 rdfs:subClassOf cco:ont00000204 ;
                 rdfs:label "Assault Rifle"@en ;
                 skos:definition "A Rifle that is designed to have selective-fire functionality and use an intermediate Cartridge and a detachable magazine."@en ;
                 cco:ont00001754 "https://en.wikipedia.org/w/index.php?title=Assault_rifle&oldid=1063774380"^^xsd:anyURI ;
                 cco:ont00001760 "https://www.commoncoreontologies.org/ArtifactOntology"^^xsd:anyURI .


###  https://www.commoncoreontologies.org/ont00000972
cco:ont00000972 rdf:type owl:Class ;
                 rdfs:subClassOf cco:ont00000966 ;
                 rdfs:label "EAN-13 Barcode"@en ;
                 skos:definition "An EAN Barcode that consists of 13 numerical digits and is used to designate products at the point of sale."@en ;
                 cco:ont00001760 "https://www.commoncoreontologies.org/ArtifactOntology"^^xsd:anyURI .


###  https://www.commoncoreontologies.org/ont00000980
cco:ont00000980 rdf:type owl:Class ;
                 rdfs:subClassOf cco:ont00001084 ;
                 rdfs:label "Portion of Waste Material"@en ;
                 skos:definition "A Portion of Processed Material that serves no further use in terms of the initial user's own purposes of production, transformation, or consumption such that the Agent wants to dispose of it."@en ;
                 cco:ont00001760 "https://www.commoncoreontologies.org/ArtifactOntology"^^xsd:anyURI .


###  https://www.commoncoreontologies.org/ont00000985
cco:ont00000985 rdf:type owl:Class ;
                 rdfs:subClassOf cco:ont00001350 ;
                 rdfs:label "Thermal Insulation Artifact Function"@en ;
                 skos:definition "A Thermal Control Artifact Function that is realized during events in which an Artifact prevents or reduces the transfer of heat between objects that are in thermal contact or in range of radiative influence."@en ;
                 cco:ont00001754 "https://en.wikipedia.org/w/index.php?title=Thermal_insulation&oldid=1059273300"^^xsd:anyURI ;
                 cco:ont00001760 "https://www.commoncoreontologies.org/ArtifactOntology"^^xsd:anyURI .


###  https://www.commoncoreontologies.org/ont00000988
cco:ont00000988 rdf:type owl:Class ;
                 rdfs:subClassOf cco:ont00000804 ;
                 rdfs:label "Reflective Prism"@en ;
                 skos:definition "A Prism designed to reflect light in order to flip, invert, rotate, deviate, or displace a beam of light entering the Prism."@en ;
                 cco:ont00001760 "https://www.commoncoreontologies.org/ArtifactOntology"^^xsd:anyURI .


###  https://www.commoncoreontologies.org/ont00000993
cco:ont00000993 rdf:type owl:Class ;
                 rdfs:subClassOf cco:ont00000961 ;
                 rdfs:label "Power Rectifying Artifact Function"@en ;
                 skos:definition "A Current Conversion Artifact Function that is realized by processes in which some Artifact is used to convert alternating current (AC) to direct current (DC)."@en ;
                 cco:ont00001760 "https://www.commoncoreontologies.org/ArtifactOntology"^^xsd:anyURI .


###  https://www.commoncoreontologies.org/ont00000994
cco:ont00000994 rdf:type owl:Class ;
                 rdfs:subClassOf cco:ont00000098 ;
                 rdfs:label "Electrical Power Production Artifact Function"@en ;
                 skos:definition "An Electrical Artifact Function that is realized during events in which an Artifact is used to generate electrical power."@en ;
                 cco:ont00001760 "https://www.commoncoreontologies.org/ArtifactOntology"^^xsd:anyURI .


###  https://www.commoncoreontologies.org/ont00000995
cco:ont00000995 rdf:type owl:Class ;
                 rdfs:subClassOf obo:BFO_0000040 ;
                 rdfs:label "Material Artifact"@en ;
                 skos:definition "A Material Entity that was designed by some Agent to realize a certain Function."@en ;
                 cco:ont00001760 "https://www.commoncoreontologies.org/ArtifactOntology"^^xsd:anyURI .


###  https://www.commoncoreontologies.org/ont00000996
cco:ont00000996 rdf:type owl:Class ;
                 rdfs:subClassOf cco:ont00000294 ;
                 rdfs:label "Ramjet Engine"@en ;
                 skos:altLabel "Ramjet"@en ;
                 skos:definition "An Air-Breathing Jet Engine that uses the forward motion of the Engine to compress incoming air (without the use of an axial compressor) and decelerate it to subsonic speeds before adding the fuel and constantly combusting the mixture then expelling the exhaust out through the rear Propelling Nozzle to generate Thrust."@en ;
                 cco:ont00001754 "https://en.wikipedia.org/w/index.php?title=Ramjet&oldid=1062836331"^^xsd:anyURI ;
                 cco:ont00001760 "https://www.commoncoreontologies.org/ArtifactOntology"^^xsd:anyURI .


###  https://www.commoncoreontologies.org/ont00000998
cco:ont00000998 rdf:type owl:Class ;
                 rdfs:subClassOf cco:ont00001036 ;
                 rdfs:label "Telecommunication Network"@en ;
                 skos:definition "A Communication System that is designed to enable the transmission of information over significant distances between Telecommunication Endpoints via Telecommunication Network Nodes and Lines."@en ;
                 cco:ont00001754 "https://en.wikipedia.org/w/index.php?title=Telecommunications_network&oldid=1063347482"^^xsd:anyURI ;
                 cco:ont00001760 "https://www.commoncoreontologies.org/ArtifactOntology"^^xsd:anyURI .


###  https://www.commoncoreontologies.org/ont00001000
cco:ont00001000 rdf:type owl:Class ;
                 rdfs:subClassOf cco:ont00000252 ;
                 rdfs:label "Spray Nozzle"@en ;
                 skos:definition "A Nozzle that is designed to facilitate a conversion of the flow of a portion of liquid into a dynamic collection of drops dispersed in a portion of gas."@en ;
                 cco:ont00001760 "https://www.commoncoreontologies.org/ArtifactOntology"^^xsd:anyURI .


###  https://www.commoncoreontologies.org/ont00001002
cco:ont00001002 rdf:type owl:Class ;
                 rdfs:subClassOf cco:ont00000798 ;
                 rdfs:label "Message"@en ;
                 skos:definition "An Information Bearing Artifact that is designed to bear some specific Information Content Entity that is relatively brief and to be transmitted from a sender to a recipient."@en ;
                 cco:ont00001754 "https://en.wikipedia.org/w/index.php?title=Message&oldid=1060098631"^^xsd:anyURI ;
                 cco:ont00001760 "https://www.commoncoreontologies.org/ArtifactOntology"^^xsd:anyURI .


###  https://www.commoncoreontologies.org/ont00001003
cco:ont00001003 rdf:type owl:Class ;
                 rdfs:subClassOf cco:ont00001150 ;
                 rdfs:label "Cartridge"@en ;
                 skos:definition "A Portion of Ammunition that is designed to package a Bullet, a propellant substance, and a primer within a case that is designed to fit within the firing chamber of a Firearm."@en ;
                 cco:ont00001754 "https://en.wikipedia.org/wiki/Cartridge_(firearms)" ;
                 cco:ont00001760 "https://www.commoncoreontologies.org/ArtifactOntology"^^xsd:anyURI .


###  https://www.commoncoreontologies.org/ont00001005
cco:ont00001005 rdf:type owl:Class ;
                 rdfs:subClassOf cco:ont00000294 ;
                 rdfs:label "Turbojet Air-Breathing Jet Engine"@en ;
                 skos:definition "An Air-Breathing Jet Engine that uses a Turbojet, which consists of a Turbine with a Propelling Nozzle."@en ;
                 cco:ont00001754 "https://en.wikipedia.org/w/index.php?title=Turbojet&oldid=1060948529"^^xsd:anyURI ;
                 cco:ont00001760 "https://www.commoncoreontologies.org/ArtifactOntology"^^xsd:anyURI .


###  https://www.commoncoreontologies.org/ont00001007
cco:ont00001007 rdf:type owl:Class ;
                 rdfs:subClassOf cco:ont00000928 ;
                 rdfs:label "Passenger Train Car"@en ;
                 skos:definition "A Train Car that is designed to transport passengers."@en ;
                 cco:ont00001754 "https://en.wikipedia.org/wiki/Passenger_car_(rail)" ;
                 cco:ont00001760 "https://www.commoncoreontologies.org/ArtifactOntology"^^xsd:anyURI .


###  https://www.commoncoreontologies.org/ont00001008
cco:ont00001008 rdf:type owl:Class ;
                 rdfs:subClassOf cco:ont00000445 ;
                 rdfs:label "Biological Weapon"@en ;
                 skos:definition "A Weapon that is designed to inflict harm, incapacity, or death by means of releasing disease-producing agents—such as bacteria, viruses, or fungi."@en ;
                 cco:ont00001754 "https://en.wikipedia.org/w/index.php?title=Biological_warfare&oldid=1062972883"^^xsd:anyURI ;
                 cco:ont00001760 "https://www.commoncoreontologies.org/ArtifactOntology"^^xsd:anyURI .


###  https://www.commoncoreontologies.org/ont00001009
cco:ont00001009 rdf:type owl:Class ;
                 rdfs:subClassOf cco:ont00000547 ;
                 rdfs:label "Optical Telescope"@en ;
                 skos:definition "A Telescope that is designed to aid in the observation of spatially distant Objects by means of collecting and focusing visible light to form an enhanced image of the Object."@en ;
                 cco:ont00001754 "https://en.wikipedia.org/w/index.php?title=Optical_telescope&oldid=1062201329"^^xsd:anyURI ;
                 cco:ont00001760 "https://www.commoncoreontologies.org/ArtifactOntology"^^xsd:anyURI .


###  https://www.commoncoreontologies.org/ont00001011
cco:ont00001011 rdf:type owl:Class ;
                 rdfs:subClassOf cco:ont00000053 ;
                 rdfs:label "Automobile"@en ;
                 skos:definition "A Ground Motor Vehicle that is designed to transport a small number of passengers while traveling on four tired wheels."@en ;
                 cco:ont00001754 "https://en.wikipedia.org/w/index.php?title=Car&oldid=1064116950"^^xsd:anyURI ;
                 cco:ont00001760 "https://www.commoncoreontologies.org/ArtifactOntology"^^xsd:anyURI .


###  https://www.commoncoreontologies.org/ont00001012
cco:ont00001012 rdf:type owl:Class ;
                 rdfs:subClassOf cco:ont00000258 ;
                 rdfs:comment "Further variants of GS1 DataBar have not been defined here."@en ;
                 rdfs:label "GS1 DataBar Barcode"@en ;
                 skos:definition "A One-Dimensional Barcode that consists of 12-14 numerical digits and is used in retail and healthcare."@en ;
                 cco:ont00001760 "https://www.commoncoreontologies.org/ArtifactOntology"^^xsd:anyURI .


###  https://www.commoncoreontologies.org/ont00001013
cco:ont00001013 rdf:type owl:Class ;
                 rdfs:subClassOf cco:ont00000323 ;
                 rdfs:label "Heating Artifact Function"@en ;
                 skos:definition "An Artifact Function that is realized in a process in which the thermal energy of a system increases."@en ;
                 cco:ont00001760 "https://www.commoncoreontologies.org/ArtifactOntology"^^xsd:anyURI .


###  https://www.commoncoreontologies.org/ont00001015
cco:ont00001015 rdf:type owl:Class ;
                 rdfs:subClassOf cco:ont00000646 ;
                 rdfs:label "Controlled-Access Highway"@en ;
                 skos:altLabel "Expressway"@en ,
                               "Freeway"@en ,
                               "Motorway"@en ;
                 skos:definition "A Highway that is designed for high-speed vehicular traffic, with all traffic flow and ingress/egress regulated."@en ;
                 cco:ont00001754 "https://en.wikipedia.org/w/index.php?title=Controlled-access_highway&oldid=1063655601"^^xsd:anyURI ;
                 cco:ont00001760 "https://www.commoncoreontologies.org/ArtifactOntology"^^xsd:anyURI .


###  https://www.commoncoreontologies.org/ont00001018
cco:ont00001018 rdf:type owl:Class ;
                 rdfs:subClassOf cco:ont00000350 ;
                 rdfs:label "Equipment Cooling System"@en ;
                 skos:definition "A Cooling System that is designed to cool some piece of equipment."@en ;
                 cco:ont00001760 "https://www.commoncoreontologies.org/ArtifactOntology"^^xsd:anyURI .


###  https://www.commoncoreontologies.org/ont00001019
cco:ont00001019 rdf:type owl:Class ;
                 rdfs:subClassOf cco:ont00000723 ;
                 rdfs:label "Steering Control System"@en ;
                 skos:definition "A Vehicle Control System that is designed to control the direction some Vehicle is traveling."@en ;
                 cco:ont00001760 "https://www.commoncoreontologies.org/ArtifactOntology"^^xsd:anyURI .


###  https://www.commoncoreontologies.org/ont00001020
cco:ont00001020 rdf:type owl:Class ;
                 rdfs:subClassOf cco:ont00000838 ;
                 rdfs:label "Portion of Gaseous Fuel"@en ;
                 skos:definition "A Portion of Fuel that is stored in a gaseous state."@en ;
                 cco:ont00001760 "https://www.commoncoreontologies.org/ArtifactOntology"^^xsd:anyURI .


###  https://www.commoncoreontologies.org/ont00001024
cco:ont00001024 rdf:type owl:Class ;
                 rdfs:subClassOf cco:ont00000394 ;
                 rdfs:label "Spark Ignition Engine"@en ;
                 skos:definition "An Internal Combustion Engine that is designed to operate by generating a spark to ignite a portion of Fuel and Oxidizer mixture."@en ;
                 cco:ont00001760 "https://www.commoncoreontologies.org/ArtifactOntology"^^xsd:anyURI .


###  https://www.commoncoreontologies.org/ont00001025
cco:ont00001025 rdf:type owl:Class ;
                 rdfs:subClassOf cco:ont00001049 ;
                 rdfs:label "Electric Generator"@en ;
                 skos:definition "An Electrical Power Source that is designed to convert mechanical energy to electrical energy for use in an external circuit."@en ;
                 cco:ont00001754 "https://en.wikipedia.org/w/index.php?title=Electric_generator&oldid=1057805035"^^xsd:anyURI ;
                 cco:ont00001760 "https://www.commoncoreontologies.org/ArtifactOntology"^^xsd:anyURI .


###  https://www.commoncoreontologies.org/ont00001027
cco:ont00001027 rdf:type owl:Class ;
                 rdfs:subClassOf cco:ont00000095 ;
                 rdfs:label "Trim Tab"@en ;
                 skos:definition "A Control Surface that is designed to counteract hydro-, aerodynamic, or other forces in order to stabilize the Vehicle it is part of in the desired Attitude."@en ;
                 cco:ont00001754 "https://en.wikipedia.org/w/index.php?title=Trim_tab&oldid=1054550485"^^xsd:anyURI ;
                 cco:ont00001760 "https://www.commoncoreontologies.org/ArtifactOntology"^^xsd:anyURI .


###  https://www.commoncoreontologies.org/ont00001029
cco:ont00001029 rdf:type owl:Class ;
                 rdfs:subClassOf cco:ont00001150 ;
                 rdfs:label "Unguided Rocket"@en ;
                 skos:altLabel "Rocket"@en ;
                 skos:definition "A Portion of Ammunition that is designed to be a self-propelled, but unguided, projectile that delivers some payload (explosive or other) over relatively long distances through the use of a Rocket Engine."@en ;
                 cco:ont00001754 "https://en.wikipedia.org/wiki/Rocket_(weapon)" ;
                 cco:ont00001760 "https://www.commoncoreontologies.org/ArtifactOntology"^^xsd:anyURI .


###  https://www.commoncoreontologies.org/ont00001030
cco:ont00001030 rdf:type owl:Class ;
                 rdfs:subClassOf cco:ont00000796 ;
                 rdfs:label "Train"@en ;
                 skos:altLabel "Railroad Train"@en ,
                               "Railway Train"@en ;
                 skos:definition "A Rail Transport Vehicle that consists of a series of connected Train Cars or Railcars."@en ;
                 cco:ont00001754 "https://en.wikipedia.org/w/index.php?title=Train&oldid=1064071492"^^xsd:anyURI ;
                 cco:ont00001760 "https://www.commoncoreontologies.org/ArtifactOntology"^^xsd:anyURI .


###  https://www.commoncoreontologies.org/ont00001034
cco:ont00001034 rdf:type owl:Class ;
                 rdfs:subClassOf cco:ont00000774 ;
                 rdfs:label "Full Motion Video Camera"@en ;
                 skos:definition "A Video Camera that is designed to capture and record images of sufficiently high quality and in rapid enough succession that the resulting video supports smooth playback."@en ;
                 cco:ont00001760 "https://www.commoncoreontologies.org/ArtifactOntology"^^xsd:anyURI .


###  https://www.commoncoreontologies.org/ont00001036
cco:ont00001036 rdf:type owl:Class ;
                 rdfs:subClassOf cco:ont00000995 ;
                 rdfs:label "Communication System"@en ;
                 skos:definition "A Material Artifact that is designed to enable some Act of Communication by means of transmission systems, relay stations, tributary stations, and data terminal equipment, usually capable of interconnection and interoperation to form an integrated whole."@en ;
                 cco:ont00001754 "https://en.wikipedia.org/w/index.php?title=Communications_system&oldid=1058600948"^^xsd:anyURI ;
                 cco:ont00001760 "https://www.commoncoreontologies.org/ArtifactOntology"^^xsd:anyURI .


###  https://www.commoncoreontologies.org/ont00001038
cco:ont00001038 rdf:type owl:Class ;
                 rdfs:subClassOf cco:ont00001105 ;
                 rdfs:label "Nickel Cadmium Electric Battery"@en ;
                 skos:altLabel "NiCad Battery"@en ;
                 skos:definition "A Secondary Cell Electric Battery that has a cadmium anode and nickel oxide hydroxide cathode."@en ;
                 cco:ont00001754 "https://en.wikipedia.org/w/index.php?title=Nickel%E2%80%93cadmium_battery&oldid=1061809659"^^xsd:anyURI ;
                 cco:ont00001760 "https://www.commoncoreontologies.org/ArtifactOntology"^^xsd:anyURI .


###  https://www.commoncoreontologies.org/ont00001042
cco:ont00001042 rdf:type owl:Class ;
                 rdfs:subClassOf cco:ont00000995 ;
                 rdfs:label "Equipment Mount"@en ;
                 skos:definition "A Material Artifact that is designed to support an Artifact."@en ;
                 cco:ont00001760 "https://www.commoncoreontologies.org/ArtifactOntology"^^xsd:anyURI .


###  https://www.commoncoreontologies.org/ont00001043
cco:ont00001043 rdf:type owl:Class ;
                 rdfs:subClassOf cco:ont00000713 ;
                 rdfs:label "Aircraft"@en ;
                 skos:definition "A Vehicle that is designed to convey passengers, cargo, or equipment from one location to another by air travel."@en ;
                 cco:ont00001754 "https://en.wikipedia.org/w/index.php?title=Aircraft&oldid=1063924562"^^xsd:anyURI ;
                 cco:ont00001760 "https://www.commoncoreontologies.org/ArtifactOntology"^^xsd:anyURI .


###  https://www.commoncoreontologies.org/ont00001044
cco:ont00001044 rdf:type owl:Class ;
                 rdfs:subClassOf cco:ont00000323 ;
                 rdfs:label "Nuclear Radiation Detection Artifact Function"@en ;
                 skos:definition "An Artifact Function that is realized during events in which an Artifact is used to detect the presence of nuclear radiation particles."@en ;
                 cco:ont00001760 "https://www.commoncoreontologies.org/ArtifactOntology"^^xsd:anyURI .


###  https://www.commoncoreontologies.org/ont00001045
cco:ont00001045 rdf:type owl:Class ;
                 rdfs:subClassOf cco:ont00000319 ;
                 rdfs:label "Artifact Model"@en ;
                 skos:definition "A Directive Information Content Entity that prescribes a common set of Functions and Qualities to inhere in a set of artifact instances."@en ;
                 cco:ont00001760 "https://www.commoncoreontologies.org/ArtifactOntology"^^xsd:anyURI .


###  https://www.commoncoreontologies.org/ont00001046
cco:ont00001046 rdf:type owl:Class ;
                 rdfs:subClassOf cco:ont00001002 ;
                 rdfs:label "Notification Message"@en ;
                 skos:definition "A Message that is designed to bear an Information Content Entity that describes a scenario that has been determined to merit attention by the recipient."@en ;
                 cco:ont00001760 "https://www.commoncoreontologies.org/ArtifactOntology"^^xsd:anyURI .


###  https://www.commoncoreontologies.org/ont00001049
cco:ont00001049 rdf:type owl:Class ;
                 rdfs:subClassOf cco:ont00000288 ;
                 rdfs:label "Electrical Power Source"@en ;
                 skos:definition "A Power Source that is designed to generate, control, and transfer power in the form of electrical energy."@en ;
                 cco:ont00001760 "https://www.commoncoreontologies.org/ArtifactOntology"^^xsd:anyURI .


###  https://www.commoncoreontologies.org/ont00001050
cco:ont00001050 rdf:type owl:Class ;
                 rdfs:subClassOf cco:ont00000716 ;
                 rdfs:label "Primary Cell Electric Battery"@en ;
                 skos:altLabel "Primary Cell Battery"@en ;
                 skos:definition "A Electric Battery that is designed for one-time use and not to be recharged."@en ;
                 cco:ont00001754 "https://en.wikipedia.org/w/index.php?title=Primary_cell&oldid=1047226932"^^xsd:anyURI ;
                 cco:ont00001760 "https://www.commoncoreontologies.org/ArtifactOntology"^^xsd:anyURI .


###  https://www.commoncoreontologies.org/ont00001051
cco:ont00001051 rdf:type owl:Class ;
                 rdfs:subClassOf cco:ont00000445 ;
                 rdfs:label "Projectile Launcher"@en ;
                 skos:definition "A Weapon that is designed to inflict damage or harm by means of launching a high-velocity projectile at a target."@en ;
                 cco:ont00001754 "https://en.wikipedia.org/w/index.php?title=Projectile&oldid=1062048285"^^xsd:anyURI ;
                 cco:ont00001760 "https://www.commoncoreontologies.org/ArtifactOntology"^^xsd:anyURI .


###  https://www.commoncoreontologies.org/ont00001054
cco:ont00001054 rdf:type owl:Class ;
                 rdfs:subClassOf cco:ont00000499 ;
                 rdfs:label "Helical Antenna"@en ;
                 skos:definition "A Wire Antenna that consists of a conducting wire wound in the form of a helix that is typically mounted over a ground plane with a feed line connected between the bottom of the helix and the ground plane."@en ;
                 cco:ont00001754 "https://en.wikipedia.org/w/index.php?title=Helical_antenna&oldid=1062343033"^^xsd:anyURI ;
                 cco:ont00001760 "https://www.commoncoreontologies.org/ArtifactOntology"^^xsd:anyURI .


###  https://www.commoncoreontologies.org/ont00001060
cco:ont00001060 rdf:type owl:Class ;
                 rdfs:subClassOf cco:ont00000995 ;
                 rdfs:label "Fuel System"@en ;
                 skos:definition "A Material Artifact that is designed to pump, manage, and deliver some Portion of Fuel to the Propulsion System and Auxiliary Power Unit of some Vehicle."@en ;
                 cco:ont00001754 "https://en.wikipedia.org/w/index.php?title=Aircraft_fuel_system&oldid=1003132173"^^xsd:anyURI ;
                 cco:ont00001760 "https://www.commoncoreontologies.org/ArtifactOntology"^^xsd:anyURI .


###  https://www.commoncoreontologies.org/ont00001061
cco:ont00001061 rdf:type owl:Class ;
                 rdfs:subClassOf cco:ont00000053 ;
                 rdfs:label "Motorcycle"@en ;
                 skos:altLabel "Motorbike"@en ;
                 skos:definition "A Ground Motor Vehicle that is designed to transport a very small number of passengers (usually 1 or 2) while traveling on two or three tired wheels."@en ;
                 cco:ont00001754 "https://en.wikipedia.org/w/index.php?title=Motorcycle&oldid=1063743553"^^xsd:anyURI ;
                 cco:ont00001760 "https://www.commoncoreontologies.org/ArtifactOntology"^^xsd:anyURI .


###  https://www.commoncoreontologies.org/ont00001064
cco:ont00001064 rdf:type owl:Class ;
                 rdfs:subClassOf cco:ont00000798 ;
                 rdfs:comment "For information on types of barcodes, see: https://www.scandit.com/types-barcodes-choosing-right-barcode/"@en ;
                 rdfs:label "Barcode"@en ;
                 skos:definition "An Information Bearing Artifact that is designed to bear one or more geometric shapes that concretize some Directive Information Content Entity."@en ;
                 cco:ont00001754 "https://en.wikipedia.org/w/index.php?title=Barcode&oldid=1059844765"^^xsd:anyURI ;
                 cco:ont00001760 "https://www.commoncoreontologies.org/ArtifactOntology"^^xsd:anyURI .


###  https://www.commoncoreontologies.org/ont00001067
cco:ont00001067 rdf:type owl:Class ;
                 rdfs:subClassOf cco:ont00000995 ;
                 rdfs:label "Laser"@en ;
                 skos:definition "A Material Artifact that is designed to emit light coherently through a process of optical amplification based on the stimulated emission of electromagnetic radiation."@en ;
                 cco:ont00001754 "https://en.wikipedia.org/w/index.php?title=Laser&oldid=1059215159"^^xsd:anyURI ;
                 cco:ont00001760 "https://www.commoncoreontologies.org/ArtifactOntology"^^xsd:anyURI .


###  https://www.commoncoreontologies.org/ont00001070
cco:ont00001070 rdf:type owl:Class ;
                 rdfs:subClassOf cco:ont00000323 ;
                 rdfs:label "Fluid Control Artifact Function"@en ;
                 skos:definition "An Artifact Function that is realized in processes in which some Artifact is used to control the direction or flow of some fluid."@en ;
                 cco:ont00001760 "https://www.commoncoreontologies.org/ArtifactOntology"^^xsd:anyURI .


###  https://www.commoncoreontologies.org/ont00001071
cco:ont00001071 rdf:type owl:Class ;
                 rdfs:subClassOf cco:ont00000323 ,
                                 [ rdf:type owl:Restriction ;
                                   owl:onProperty obo:BFO_0000197 ;
                                   owl:someValuesFrom cco:ont00000713
                                 ] ;
                 rdfs:label "Payload Capacity"@en ;
                 skos:definition "An Artifact Function that inheres in a Vehicle that is designed to transport Payload, and which is typically characterized by the maximum Weight, Mass, or Volume of Payload that the Vehicle can transport."@en ;
                 cco:ont00001754 "https://en.wikipedia.org/w/index.php?title=Payload&oldid=1035953573"^^xsd:anyURI ;
                 cco:ont00001760 "https://www.commoncoreontologies.org/ArtifactOntology"^^xsd:anyURI .


###  https://www.commoncoreontologies.org/ont00001077
cco:ont00001077 rdf:type owl:Class ;
                 rdfs:subClassOf cco:ont00000848 ;
                 rdfs:label "Heavy Machine Gun"@en ;
                 skos:definition "A Mounted Gun that is designed to fire ammunition greater than .50 caliber or 12.7mm ammunition in quick succession from an ammunition belt, and which typically weighs more than 30lbs."@en ;
                 cco:ont00001754 "https://en.wikipedia.org/w/index.php?title=Heavy_machine_gun&oldid=1047303735"^^xsd:anyURI ;
                 cco:ont00001760 "https://www.commoncoreontologies.org/ArtifactOntology"^^xsd:anyURI .


###  https://www.commoncoreontologies.org/ont00001082
cco:ont00001082 rdf:type owl:Class ;
                 rdfs:subClassOf cco:ont00001145 ;
                 rdfs:label "Patch Receiver"@en ;
                 skos:definition "A Radio Receiver that uses a Patch Antenna to intercept radio signals."@en ;
                 cco:ont00001760 "https://www.commoncoreontologies.org/ArtifactOntology"^^xsd:anyURI .


###  https://www.commoncoreontologies.org/ont00001083
cco:ont00001083 rdf:type owl:Class ;
                 rdfs:subClassOf cco:ont00000056 ;
                 rdfs:label "Air-Breathing Combustion Engine"@en ;
                 skos:definition "A Reaction Engine that functions by drawing a continuous stream of air into and through the Engine where it is compressed, mixed with a Portion of Fuel, ignited, and then expelled as exhaust gas."@en ;
                 cco:ont00001754 "https://en.wikipedia.org/w/index.php?title=Engine&oldid=1063879193"^^xsd:anyURI ;
                 cco:ont00001760 "https://www.commoncoreontologies.org/ArtifactOntology"^^xsd:anyURI .


###  https://www.commoncoreontologies.org/ont00001084
cco:ont00001084 rdf:type owl:Class ;
                 rdfs:subClassOf cco:ont00000995 ;
                 rdfs:label "Portion of Processed Material"@en ;
                 skos:definition "A Material Artifact that is the output of an Act of Artifact Processing."@en ;
                 cco:ont00001760 "https://www.commoncoreontologies.org/ArtifactOntology"^^xsd:anyURI .


###  https://www.commoncoreontologies.org/ont00001085
cco:ont00001085 rdf:type owl:Class ;
                 rdfs:subClassOf cco:ont00000323 ;
                 rdfs:label "Reflection Artifact Function"@en ;
                 skos:definition "An Artifact Function that is realized by an Artifact participating in a reflection event in which the Artifact causes a change in a wavefront at an interface between the reflecting medium and the transmission medium such that the wavefront returns into the transmission medium."@en ;
                 cco:ont00001760 "https://www.commoncoreontologies.org/ArtifactOntology"^^xsd:anyURI .


###  https://www.commoncoreontologies.org/ont00001086
cco:ont00001086 rdf:type owl:Class ;
                 rdfs:subClassOf cco:ont00001326 ;
                 rdfs:label "Road Junction"@en ;
                 skos:definition "A Land Transportation Artifact that is designed to enable Ground Vehicles to exit one Road and enter another."@en ;
                 cco:ont00001754 "https://en.wikipedia.org/wiki/Junction_(road)" ;
                 cco:ont00001760 "https://www.commoncoreontologies.org/ArtifactOntology"^^xsd:anyURI .


###  https://www.commoncoreontologies.org/ont00001087
cco:ont00001087 rdf:type owl:Class ;
                 rdfs:subClassOf cco:ont00001306 ;
                 rdfs:label "Orientation Observation Artifact Function"@en ;
                 skos:altLabel "Attitude Observation Artifact Function"@en ;
                 skos:definition "An Observation Artifact Function that is realized during events in which an Artifact is used to collect information about the Orientation of a specified object or class of objects."@en ;
                 cco:ont00001760 "https://www.commoncoreontologies.org/ArtifactOntology"^^xsd:anyURI .


###  https://www.commoncoreontologies.org/ont00001092
cco:ont00001092 rdf:type owl:Class ;
                 rdfs:subClassOf cco:ont00000098 ;
                 rdfs:label "Electrical Power Storage Artifact Function"@en ;
                 skos:altLabel "Capacitance"@en ;
                 skos:definition "An Electrical Artifact Function that is realized during events in which an Artifact is used to store electrical power to be released at a later time."@en ;
                 cco:ont00001760 "https://www.commoncoreontologies.org/ArtifactOntology"^^xsd:anyURI .


###  https://www.commoncoreontologies.org/ont00001093
cco:ont00001093 rdf:type owl:Class ;
                 rdfs:subClassOf cco:ont00000475 ;
                 rdfs:label "Coin"@en ;
                 skos:definition "A Portion of Cash that consists of a flat, portable, round pieces of metal designed to bear some specified Financial Value."@en ;
                 cco:ont00001760 "https://www.commoncoreontologies.org/ArtifactOntology"^^xsd:anyURI .


###  https://www.commoncoreontologies.org/ont00001095
cco:ont00001095 rdf:type owl:Class ;
                 rdfs:subClassOf cco:ont00000363 ;
                 rdfs:label "Cellular Telecommunication Network"@en ;
                 skos:altLabel "Cellular Network"@en ,
                               "Mobile Telecommunication Network"@en ;
                 skos:definition "A Wireless Telecommunication Network where the last link between the network and the end user is wireless and is distributed over service areas called cells."@en ;
                 cco:ont00001754 "https://en.wikipedia.org/w/index.php?title=Cellular_network&oldid=1061429562"^^xsd:anyURI ;
                 cco:ont00001760 "https://www.commoncoreontologies.org/ArtifactOntology"^^xsd:anyURI .


###  https://www.commoncoreontologies.org/ont00001096
cco:ont00001096 rdf:type owl:Class ;
                 rdfs:subClassOf cco:ont00001104 ;
                 rdfs:label "Submachine Gun"@en ;
                 skos:definition "An Long Gun that is designed to be have automatic-fire functionality, fire pistol-caliber ammunition that is magazine-fed, and which is usually smaller than other automatic firearms."@en ;
                 cco:ont00001754 "https://en.wikipedia.org/w/index.php?title=Submachine_gun&oldid=1063939013"^^xsd:anyURI ;
                 cco:ont00001760 "https://www.commoncoreontologies.org/ArtifactOntology"^^xsd:anyURI .


###  https://www.commoncoreontologies.org/ont00001097
cco:ont00001097 rdf:type owl:Class ;
                 rdfs:subClassOf cco:ont00001278 ;
                 rdfs:label "Common Stock"@en ;
                 skos:definition "Stock that entitles its holder to voting on corporate decisions."@en ;
                 cco:ont00001760 "https://www.commoncoreontologies.org/ArtifactOntology"^^xsd:anyURI .


###  https://www.commoncoreontologies.org/ont00001099
cco:ont00001099 rdf:type owl:Class ;
                 rdfs:subClassOf cco:ont00001326 ;
                 rdfs:label "Bridge"@en ;
                 skos:definition "A Land Transportation Artifact that is designed to span physical obstacles without closing the way underneath to enable Persons or Ground Vehicles to pass over the obstacles."@en ;
                 cco:ont00001754 "https://en.wikipedia.org/w/index.php?title=Bridge&oldid=1061858310" ;
                 cco:ont00001760 "https://www.commoncoreontologies.org/ArtifactOntology"^^xsd:anyURI .


###  https://www.commoncoreontologies.org/ont00001100
cco:ont00001100 rdf:type owl:Class ;
                 rdfs:subClassOf cco:ont00000323 ;
                 rdfs:label "Measurement Artifact Function"@en ;
                 skos:definition "An Artifact Function that is realized during events in which an Artifact is used to measure one or more features of a specified object or class of objects."@en ;
                 cco:ont00001760 "https://www.commoncoreontologies.org/ArtifactOntology"^^xsd:anyURI .


###  https://www.commoncoreontologies.org/ont00001103
cco:ont00001103 rdf:type owl:Class ;
                 owl:equivalentClass [ owl:intersectionOf ( cco:ont00000686
                                                            [ rdf:type owl:Restriction ;
                                                              owl:onProperty cco:ont00001916 ;
                                                              owl:someValuesFrom cco:ont00001045
                                                            ]
                                                          ) ;
                                       rdf:type owl:Class
                                     ] ;
                 rdfs:subClassOf cco:ont00000686 ;
                 rdfs:label "Artifact Model Name"@en ;
                 skos:definition "A Designative Information Content Entity that designates some Artifact Model."@en ;
                 cco:ont00001760 "https://www.commoncoreontologies.org/ArtifactOntology"^^xsd:anyURI .


###  https://www.commoncoreontologies.org/ont00001104
cco:ont00001104 rdf:type owl:Class ;
                 rdfs:subClassOf cco:ont00000088 ;
                 rdfs:label "Long Gun"@en ;
                 skos:definition "A Firearm that is designed to have a longer barrel than a Hand Gun and to be fired while braced against the shoulder."@en ;
                 cco:ont00001754 "https://en.wikipedia.org/w/index.php?title=Long_gun&oldid=1063715506"^^xsd:anyURI ;
                 cco:ont00001760 "https://www.commoncoreontologies.org/ArtifactOntology"^^xsd:anyURI .


###  https://www.commoncoreontologies.org/ont00001105
cco:ont00001105 rdf:type owl:Class ;
                 rdfs:subClassOf cco:ont00000716 ;
                 rdfs:label "Secondary Cell Electric Battery"@en ;
                 skos:altLabel "Rechargeable Battery"@en ,
                               "Secondary Cell Battery"@en ;
                 skos:definition "An Electric Battery that is designed to be recharged."@en ;
                 cco:ont00001754 "https://en.wikipedia.org/w/index.php?title=Rechargeable_battery&oldid=1064096406"^^xsd:anyURI ;
                 cco:ont00001760 "https://www.commoncoreontologies.org/ArtifactOntology"^^xsd:anyURI .


###  https://www.commoncoreontologies.org/ont00001117
cco:ont00001117 rdf:type owl:Class ;
                 rdfs:subClassOf cco:ont00000252 ;
                 rdfs:label "Propelling Nozzle"@en ;
                 skos:altLabel "Jet Nozzle"@en ;
                 skos:definition "A Nozzle that is used to convert a propulsion Engine into a Jet Engine and functions by using its narrowest part, the throat, to increase Pressure within the Engine by constricting flow, usually until the flow chokes, then expanding the exhaust stream to, or near to, atmospheric pressure, while forming it into a high speed jet to propel the Vehicle."@en ;
                 cco:ont00001754 "https://en.wikipedia.org/w/index.php?title=Propelling_nozzle&oldid=1061239812"^^xsd:anyURI ;
                 cco:ont00001760 "https://www.commoncoreontologies.org/ArtifactOntology"^^xsd:anyURI .


###  https://www.commoncoreontologies.org/ont00001119
cco:ont00001119 rdf:type owl:Class ;
                 rdfs:subClassOf cco:ont00001298 ;
                 rdfs:label "Document Form"@en ;
                 skos:definition "A Document having Document Fields as parts in which to write or select prescribed content."@en ;
                 cco:ont00001754 "https://en.wikipedia.org/wiki/Form_(document)" ;
                 cco:ont00001760 "https://www.commoncoreontologies.org/ArtifactOntology"^^xsd:anyURI .


###  https://www.commoncoreontologies.org/ont00001121
cco:ont00001121 rdf:type owl:Class ;
                 rdfs:subClassOf cco:ont00000294 ;
                 rdfs:label "Scramjet Engine"@en ;
                 skos:altLabel "Scramjet"@en ,
                               "Supersonic Combusting Ramjet"@en ;
                 skos:definition "An Air-Breathing Jet Engine that uses the forward motion of the Engine to compress incoming air at supersonic speeds before adding the fuel and constantly combusting the mixture then expelling the exhaust out through the rear Propelling Nozzle to generate Thrust."@en ;
                 cco:ont00001754 "https://en.wikipedia.org/w/index.php?title=Scramjet&oldid=1062429697"^^xsd:anyURI ;
                 cco:ont00001760 "https://www.commoncoreontologies.org/ArtifactOntology"^^xsd:anyURI .


###  https://www.commoncoreontologies.org/ont00001123
cco:ont00001123 rdf:type owl:Class ;
                 rdfs:subClassOf cco:ont00001153 ;
                 rdfs:label "Poison Artifact Function"@en ;
                 skos:definition "A Damaging Artifact Function that is realized in a process which causes illness in, or the death of, a living thing."@en ;
                 cco:ont00001754 "http://www.dictionary.com/browse/poison" ;
                 cco:ont00001760 "https://www.commoncoreontologies.org/ArtifactOntology"^^xsd:anyURI .


###  https://www.commoncoreontologies.org/ont00001124
cco:ont00001124 rdf:type owl:Class ;
                 rdfs:subClassOf cco:ont00001150 ;
                 rdfs:label "Precision-Guided Missile"@en ;
                 skos:altLabel "Missile"@en ;
                 skos:definition "A Portion of Ammunition that is designed to be a self-propelled and precision-guided projectile that delivers some payload (explosive or other) over relatively long distances."@en ;
                 cco:ont00001754 "https://en.wikipedia.org/w/index.php?title=Missile&oldid=1062028589"^^xsd:anyURI ;
                 cco:ont00001760 "https://www.commoncoreontologies.org/ArtifactOntology"^^xsd:anyURI .


###  https://www.commoncoreontologies.org/ont00001129
cco:ont00001129 rdf:type owl:Class ;
                 rdfs:subClassOf cco:ont00000113 ;
                 rdfs:label "Pressurization Control Artifact Function"@en ;
                 skos:definition "A Ventilation Control Artifact Function that is realized by processes in which some Artifact is used to control the partial pressure of air in some space."@en ;
                 cco:ont00001760 "https://www.commoncoreontologies.org/ArtifactOntology"^^xsd:anyURI .


###  https://www.commoncoreontologies.org/ont00001131
cco:ont00001131 rdf:type owl:Class ;
                 rdfs:subClassOf cco:ont00000966 ;
                 rdfs:label "EAN-8 Barcode"@en ;
                 skos:definition "An EAN Barcode that consists of 8 numerical digits and is used to designate products at the point of sale."@en ;
                 cco:ont00001760 "https://www.commoncoreontologies.org/ArtifactOntology"^^xsd:anyURI .


###  https://www.commoncoreontologies.org/ont00001134
cco:ont00001134 rdf:type owl:Class ;
                 rdfs:subClassOf cco:ont00000995 ;
                 rdfs:label "Vehicle Frame"@en ;
                 skos:definition "A Material Artifact that is designed to be the main supporting structure of some Vehicle."@en ;
                 cco:ont00001754 "https://en.wikipedia.org/w/index.php?title=Vehicle_frame&oldid=1054003530"^^xsd:anyURI ;
                 cco:ont00001760 "https://www.commoncoreontologies.org/ArtifactOntology"^^xsd:anyURI .


###  https://www.commoncoreontologies.org/ont00001135
cco:ont00001135 rdf:type owl:Class ;
                 rdfs:subClassOf cco:ont00000838 ;
                 rdfs:label "Portion of Liquid Fuel"@en ;
                 skos:definition "A Portion of Fuel that is stored in a liquid state."@en ;
                 cco:ont00001760 "https://www.commoncoreontologies.org/ArtifactOntology"^^xsd:anyURI .


###  https://www.commoncoreontologies.org/ont00001138
cco:ont00001138 rdf:type owl:Class ;
                 rdfs:subClassOf cco:ont00000499 ;
                 rdfs:label "Beverage Antenna"@en ;
                 skos:definition "A Wire Antenna that consists of a horizontal wire one-half to two wavelengths long that is suspended above the ground with one end attached to the receiver feedline and the other grounded and which is typically used in the low and medium frequency radio bands."@en ;
                 cco:ont00001754 "Adapted from: https://en.wikipedia.org/wiki/Beverage_antenna" ;
                 cco:ont00001760 "https://www.commoncoreontologies.org/ArtifactOntology"^^xsd:anyURI .


###  https://www.commoncoreontologies.org/ont00001139
cco:ont00001139 rdf:type owl:Class ;
                 rdfs:subClassOf cco:ont00000713 ;
                 rdfs:label "Spacecraft"@en ;
                 skos:definition "A Vehicle that is designed to convey passengers, cargo, or equipment from one location to another by Spaceflight."@en ;
                 cco:ont00001754 "https://en.wikipedia.org/w/index.php?title=Spacecraft&oldid=1062102614"^^xsd:anyURI ;
                 cco:ont00001760 "https://www.commoncoreontologies.org/ArtifactOntology"^^xsd:anyURI .


###  https://www.commoncoreontologies.org/ont00001140
cco:ont00001140 rdf:type owl:Class ;
                 rdfs:subClassOf cco:ont00000995 ;
                 rdfs:label "Flywheel"@en ;
                 skos:definition "A Material Artifact that is designed to store rotational energy such that it has a significant moment of inertia which enables it to resist changes in rotational speed."@en ;
                 cco:ont00001754 "https://en.wikipedia.org/w/index.php?title=Flywheel&oldid=1061360783"^^xsd:anyURI ;
                 cco:ont00001760 "https://www.commoncoreontologies.org/ArtifactOntology"^^xsd:anyURI .


###  https://www.commoncoreontologies.org/ont00001141
cco:ont00001141 rdf:type owl:Class ;
                 rdfs:subClassOf obo:BFO_0000023 ;
                 rdfs:comment "The disposition will typically be a function of an artifact, which is often designed to be part of some Infrastructure system. But not always. In some cases an entity may be repurposed to be an element of some Infrastructure. In those cases it is a capability of that entity that supports the functioning of the system."@en ;
                 rdfs:label "Infrastructure Role"@en ;
                 skos:definition "A Role that inheres in the bearer of a Disposition and has been assigned to an Infrastructure System such that the realization of that Disposition is sometimes part of the functioning of the Infrastructure System."@en ;
                 cco:ont00001754 "https://archive.org/details/economicsprincip00osul/page/n489/mode/2up"^^xsd:anyURI ;
                 cco:ont00001760 "https://www.commoncoreontologies.org/ArtifactOntology"^^xsd:anyURI .


###  https://www.commoncoreontologies.org/ont00001145
cco:ont00001145 rdf:type owl:Class ;
                 rdfs:subClassOf cco:ont00000903 ;
                 rdfs:label "Radio Receiver"@en ;
                 skos:definition "A Radio Communication Instrument that is an electronic device that is designed to extract information from radio waves intercepted by a Radio Antenna by using electronic filters to separate the desired radio frequency signal from other signals, an electronic amplifier to increase the power of the signal, and demodulation to recover the desired information."@en ;
                 cco:ont00001754 "https://en.wikipedia.org/w/index.php?title=Radio_receiver&oldid=1060111342"^^xsd:anyURI ;
                 cco:ont00001760 "https://www.commoncoreontologies.org/ArtifactOntology"^^xsd:anyURI .


###  https://www.commoncoreontologies.org/ont00001148
cco:ont00001148 rdf:type owl:Class ;
                 rdfs:subClassOf cco:ont00000727 ;
                 rdfs:label "Electromagnetic Communication Artifact Function"@en ;
                 skos:definition "A Communication Artifact Function that is realized in a process that conveys meaningful signs by means of electromagnetic radiation."@en ;
                 cco:ont00001754 "https://en.wikipedia.org/w/index.php?title=Telecommunications&oldid=1061143810"^^xsd:anyURI ;
                 cco:ont00001760 "https://www.commoncoreontologies.org/ArtifactOntology"^^xsd:anyURI .


###  https://www.commoncoreontologies.org/ont00001150
cco:ont00001150 rdf:type owl:Class ;
                 rdfs:subClassOf cco:ont00000445 ;
                 rdfs:label "Portion of Ammunition"@en ;
                 skos:definition "A Weapon that is designed to inflict harm, damage, or incapacity by being projected toward its target at a significant Velocity."@en ;
                 cco:ont00001754 "https://en.wikipedia.org/w/index.php?title=Ammunition&oldid=1062875850"^^xsd:anyURI ;
                 cco:ont00001760 "https://www.commoncoreontologies.org/ArtifactOntology"^^xsd:anyURI .


###  https://www.commoncoreontologies.org/ont00001151
cco:ont00001151 rdf:type owl:Class ;
                 rdfs:subClassOf cco:ont00000893 ;
                 rdfs:label "Portion of Paper"@en ;
                 skos:definition "An Information Medium Artifact that is designed to bear some Information Content Entity by means of pressing together moist fibres of cellulose pulp derived from wood, rags, or grasses, and drying them into flexible sheets."@en ;
                 cco:ont00001754 "https://en.wikipedia.org/w/index.php?title=Paper&oldid=1057624743"^^xsd:anyURI ;
                 cco:ont00001760 "https://www.commoncoreontologies.org/ArtifactOntology"^^xsd:anyURI .


###  https://www.commoncoreontologies.org/ont00001153
cco:ont00001153 rdf:type owl:Class ;
                 rdfs:subClassOf cco:ont00000323 ;
                 rdfs:label "Damaging Artifact Function"@en ;
                 skos:definition "An Artifact Function that is realized in a process in which the structural integrity of an entity is impaired."@en ;
                 cco:ont00001760 "https://www.commoncoreontologies.org/ArtifactOntology"^^xsd:anyURI .


###  https://www.commoncoreontologies.org/ont00001155
cco:ont00001155 rdf:type owl:Class ;
                 rdfs:subClassOf cco:ont00000601 ;
                 rdfs:label "Full Motion Video Imaging Artifact Function"@en ;
                 skos:definition "An Imaging Artifact Function that inheres in Artifacts that are designed to produce video of entities that is of high enough quality to make the represented motion appear continuous to human viewers."@en ;
                 cco:ont00001760 "https://www.commoncoreontologies.org/ArtifactOntology"^^xsd:anyURI .


###  https://www.commoncoreontologies.org/ont00001156
cco:ont00001156 rdf:type owl:Class ;
                 rdfs:subClassOf cco:ont00000798 ;
                 rdfs:label "Information Line"@en ;
                 skos:definition "An Information Bearing Artifact that consists of a single line or row of some larger Information Bearing Artifact of which it is a part."@en ;
                 skos:example "a line in a computer file that bears a portion of code for some computer program" ,
                              "a line of data in a database" ,
                              "a line of text in a book" ;
                 cco:ont00001760 "https://www.commoncoreontologies.org/ArtifactOntology"^^xsd:anyURI .


###  https://www.commoncoreontologies.org/ont00001157
cco:ont00001157 rdf:type owl:Class ;
                 rdfs:subClassOf cco:ont00000288 ;
                 rdfs:label "Hydraulic Power Source"@en ;
                 skos:definition "A Power Source that is designed to generate, control, or transmit power by means of pressurized liquid."@en ;
                 cco:ont00001760 "https://www.commoncoreontologies.org/ArtifactOntology"^^xsd:anyURI .


###  https://www.commoncoreontologies.org/ont00001159
cco:ont00001159 rdf:type owl:Class ;
                 rdfs:subClassOf cco:ont00000537 ;
                 rdfs:label "Bond"@en ;
                 skos:definition "A Financial Instrument that is designed to secure an Agent's debt for the holders of that debt."@en ;
                 cco:ont00001754 "https://en.wikipedia.org/wiki/Bond_(finance)" ;
                 cco:ont00001760 "https://www.commoncoreontologies.org/ArtifactOntology"^^xsd:anyURI .


###  https://www.commoncoreontologies.org/ont00001160
cco:ont00001160 rdf:type owl:Class ;
                 rdfs:subClassOf cco:ont00000791 ;
                 rdfs:label "Solvent Artifact Function"@en ;
                 skos:definition "A Chemical Reaction Artifact Function that is realized in the dissolving of other substances (namely, solutes) without change in the former's chemical structure."@en ;
                 cco:ont00001754 "https://en.wikipedia.org/w/index.php?title=Solvent&oldid=1062572314"^^xsd:anyURI ;
                 cco:ont00001760 "https://www.commoncoreontologies.org/ArtifactOntology"^^xsd:anyURI .


###  https://www.commoncoreontologies.org/ont00001161
cco:ont00001161 rdf:type owl:Class ;
                 rdfs:subClassOf cco:ont00000719 ;
                 rdfs:label "Counterfeit Legal Instrument"@en ;
                 skos:definition "A Counterfeit Instrument that is designed to be a fake replica of some genuine Legal Instrument."@en ;
                 cco:ont00001754 "https://en.wikipedia.org/w/index.php?title=Counterfeit&oldid=1063493600"^^xsd:anyURI ;
                 cco:ont00001760 "https://www.commoncoreontologies.org/ArtifactOntology"^^xsd:anyURI .


###  https://www.commoncoreontologies.org/ont00001168
cco:ont00001168 rdf:type owl:Class ;
                 rdfs:subClassOf obo:BFO_0000040 ;
                 rdfs:label "Reaction Mass"@en ;
                 skos:altLabel "Working Mass"@en ;
                 skos:definition "A Material Entity against which a Propulsion System operates in order to produce Acceleration."@en ;
                 cco:ont00001754 "https://en.wikipedia.org/w/index.php?title=Working_mass&oldid=1057126114"^^xsd:anyURI ;
                 cco:ont00001760 "https://www.commoncoreontologies.org/ArtifactOntology"^^xsd:anyURI .


###  https://www.commoncoreontologies.org/ont00001169
cco:ont00001169 rdf:type owl:Class ;
                 rdfs:subClassOf cco:ont00000323 ;
                 rdfs:label "Communication Relay Artifact Function"@en ;
                 skos:definition "An Artifact Function that is realized during events in which an Artifact is used to first receive and then transmit information from one Artifact to another for the purpose of communiction."@en ;
                 cco:ont00001760 "https://www.commoncoreontologies.org/ArtifactOntology"^^xsd:anyURI .


###  https://www.commoncoreontologies.org/ont00001172
cco:ont00001172 rdf:type owl:Class ;
                 rdfs:subClassOf cco:ont00000593 ;
                 rdfs:label "Portion of Gelatinous Propellant"@en ;
                 skos:definition "A Portion of Propellant that is stored in a gelatinous state."@en ;
                 cco:ont00001760 "https://www.commoncoreontologies.org/ArtifactOntology"^^xsd:anyURI .


###  https://www.commoncoreontologies.org/ont00001173
cco:ont00001173 rdf:type owl:Class ;
                 rdfs:subClassOf cco:ont00001051 ;
                 rdfs:label "Rocket Launcher"@en ;
                 skos:definition "A Projectile Launcher that is designed to launch one or more Unguided Rockets."@en ;
                 cco:ont00001754 "https://en.wikipedia.org/w/index.php?title=Rocket_launcher&oldid=1049900727"^^xsd:anyURI ;
                 cco:ont00001760 "https://www.commoncoreontologies.org/ArtifactOntology"^^xsd:anyURI .


###  https://www.commoncoreontologies.org/ont00001174
cco:ont00001174 rdf:type owl:Class ;
                 rdfs:subClassOf cco:ont00000323 ;
                 rdfs:label "Electromagnetic Shielding Artifact Function"@en ;
                 skos:definition "An Artifact Function that is realized in a process in which an electromagnetic field is blocked by barriers made of conductive or magnetic materials."@en ;
                 cco:ont00001754 "https://en.wikipedia.org/w/index.php?title=Electromagnetic_shielding&oldid=1063432544"^^xsd:anyURI ;
                 cco:ont00001760 "https://www.commoncoreontologies.org/ArtifactOntology"^^xsd:anyURI .


###  https://www.commoncoreontologies.org/ont00001178
cco:ont00001178 rdf:type owl:Class ;
                 rdfs:subClassOf cco:ont00001326 ;
                 rdfs:label "Railway Crossing"@en ;
                 skos:altLabel "Level Crossing"@en ;
                 skos:definition "A Land Transportation Artifact that is designed to enable Persons or Ground Vehicles to cross a Railway when traveling along a road or path that is perpendicular to and at the same elevation as the Railway at the point where they overlap."@en ;
                 cco:ont00001760 "https://www.commoncoreontologies.org/ArtifactOntology"^^xsd:anyURI .


###  https://www.commoncoreontologies.org/ont00001179
cco:ont00001179 rdf:type owl:Class ;
                 rdfs:subClassOf cco:ont00000893 ;
                 rdfs:label "Digital Storage Device"@en ;
                 skos:definition "An Information Medium Artifact that is designed to bear some Information Content Entity by means of recording that information in digital (binary) format."@en ;
                 skos:example "A computer's Hard Disk Drive" ,
                              "A portable USB Drive" ;
                 cco:ont00001754 "https://en.wikipedia.org/w/index.php?title=Data_storage&oldid=1060116427"^^xsd:anyURI ;
                 cco:ont00001760 "https://www.commoncoreontologies.org/ArtifactOntology"^^xsd:anyURI .


###  https://www.commoncoreontologies.org/ont00001181
cco:ont00001181 rdf:type owl:Class ;
                 rdfs:subClassOf cco:ont00000287 ;
                 rdfs:label "Triple Inertial Navigation System"@en ;
                 skos:altLabel "Triple INS"@en ;
                 skos:definition "An Inertial Navigation System that is designed to use three redundant computers to continuously calculate via dead reckoning the position, orientation, and velocity of a moving object without the need for external references, in such a way that eliminates the need for a navigator."@en ;
                 cco:ont00001760 "https://www.commoncoreontologies.org/ArtifactOntology"^^xsd:anyURI .


###  https://www.commoncoreontologies.org/ont00001185
cco:ont00001185 rdf:type owl:Class ;
                 rdfs:subClassOf cco:ont00000713 ;
                 rdfs:label "Rocket"@en ;
                 skos:definition "A Vehicle that is designed to travel through air or space and which obtains Thrust from a Rocket Engine."@en ;
                 cco:ont00001754 "https://en.wikipedia.org/w/index.php?title=Rocket&oldid=1063307477"^^xsd:anyURI ;
                 cco:ont00001760 "https://www.commoncoreontologies.org/ArtifactOntology"^^xsd:anyURI .


###  https://www.commoncoreontologies.org/ont00001187
cco:ont00001187 rdf:type owl:Class ;
                 rdfs:subClassOf cco:ont00000995 ;
                 rdfs:label "Navigation System"@en ;
                 skos:definition "A Material Artifact that is designed to enable an Agent or Artifact to determine the position or direction of some object, usually for the purpose of monitoring or controlling the movement of some Vehicle from one place to another."@en ;
                 cco:ont00001754 "https://en.wikipedia.org/w/index.php?title=Navigation&oldid=1064122463"^^xsd:anyURI ;
                 cco:ont00001760 "https://www.commoncoreontologies.org/ArtifactOntology"^^xsd:anyURI .


###  https://www.commoncoreontologies.org/ont00001188
cco:ont00001188 rdf:type owl:Class ;
                 rdfs:subClassOf cco:ont00000715 ;
                 rdfs:label "Denture"@en ;
                 skos:definition "A Prosthesis that is designed to replace missing teeth."@en ;
                 cco:ont00001754 "https://en.wikipedia.org/w/index.php?title=Dentures&oldid=1056527226"^^xsd:anyURI ;
                 cco:ont00001760 "https://www.commoncoreontologies.org/ArtifactOntology"^^xsd:anyURI .


###  https://www.commoncoreontologies.org/ont00001192
cco:ont00001192 rdf:type owl:Class ;
                 rdfs:subClassOf cco:ont00000092 ;
                 rdfs:label "Radio Antenna"@en ;
                 skos:definition "A Bidirectional Transducer that is designed to convert electric power into radio waves, and radio waves into electric power."@en ;
                 cco:ont00001754 "https://en.wikipedia.org/wiki/Antenna_(radio)" ;
                 cco:ont00001760 "https://www.commoncoreontologies.org/ArtifactOntology"^^xsd:anyURI .


###  https://www.commoncoreontologies.org/ont00001198
cco:ont00001198 rdf:type owl:Class ;
                 rdfs:subClassOf cco:ont00000796 ;
                 rdfs:comment "In American-English, the term 'Railcar' is often used in a broader sense that is interchangeable with 'Railroad Car'."@en ;
                 rdfs:label "Railcar"@en ;
                 skos:definition "A Rail Transport Vehicle that consists of a single self-propelled Vehicle that is not a Train, is designed to transport passengers, and which may also be designed to connect to other Railcars to form a Train."@en ;
                 cco:ont00001754 "https://en.wikipedia.org/w/index.php?title=Railcar&oldid=1063519348"^^xsd:anyURI ;
                 cco:ont00001760 "https://www.commoncoreontologies.org/ArtifactOntology"^^xsd:anyURI .


###  https://www.commoncoreontologies.org/ont00001200
cco:ont00001200 rdf:type owl:Class ;
                 rdfs:subClassOf cco:ont00000323 ;
                 rdfs:label "Structural Support Artifact Function"@en ;
                 skos:definition "An Artifact Function that is realized by an Artifact providing physical support to another object."@en ;
                 cco:ont00001760 "https://www.commoncoreontologies.org/ArtifactOntology"^^xsd:anyURI .


###  https://www.commoncoreontologies.org/ont00001201
cco:ont00001201 rdf:type owl:Class ;
                 rdfs:subClassOf cco:ont00001326 ;
                 rdfs:label "Trail"@en ;
                 skos:definition "A Land Transportation Artifact that is designed to enable transport through rough country, such as a forest or moor."@en ;
                 cco:ont00001754 "https://en.wikipedia.org/w/index.php?title=Trail&oldid=1056047142"^^xsd:anyURI ;
                 cco:ont00001760 "https://www.commoncoreontologies.org/ArtifactOntology"^^xsd:anyURI .


###  https://www.commoncoreontologies.org/ont00001207
cco:ont00001207 rdf:type owl:Class ;
                 rdfs:subClassOf cco:ont00000136 ;
                 rdfs:label "Optical Lens"@en ;
                 skos:altLabel "Lens"@en ;
                 skos:definition "An Optical Instrument that is designed to focus or disperse a beam of light entering the lens by means of refraction."@en ;
                 cco:ont00001754 "https://en.wikipedia.org/wiki/Lens_(optics)" ;
                 cco:ont00001760 "https://www.commoncoreontologies.org/ArtifactOntology"^^xsd:anyURI .


###  https://www.commoncoreontologies.org/ont00001209
cco:ont00001209 rdf:type owl:Class ;
                 rdfs:subClassOf cco:ont00000326 ;
                 rdfs:label "UPC-E Barcode"@en ;
                 skos:definition "A UPC Barcode that consists of 6 numerical digits."@en ;
                 cco:ont00001760 "https://www.commoncoreontologies.org/ArtifactOntology"^^xsd:anyURI .


###  https://www.commoncoreontologies.org/ont00001210
cco:ont00001210 rdf:type owl:Class ;
                 rdfs:subClassOf cco:ont00001301 ;
                 rdfs:label "Retail Artifact Function"@en ;
                 skos:definition "A Service Artifact Function that is realized in processes of selling goods or merchandise in small or individual lots for direct consumption by persons or organizations."@en ;
                 cco:ont00001754 "https://en.wikipedia.org/w/index.php?title=Retail&oldid=1061431295"^^xsd:anyURI ;
                 cco:ont00001760 "https://www.commoncoreontologies.org/ArtifactOntology"^^xsd:anyURI .


###  https://www.commoncoreontologies.org/ont00001211
cco:ont00001211 rdf:type owl:Class ;
                 rdfs:subClassOf cco:ont00000323 ;
                 rdfs:label "Lifting Artifact Function"@en ;
                 skos:definition "An Artifact Function that is realized by processes in which some Artifact is used to lift some object."@en ;
                 cco:ont00001760 "https://www.commoncoreontologies.org/ArtifactOntology"^^xsd:anyURI .


###  https://www.commoncoreontologies.org/ont00001216
cco:ont00001216 rdf:type owl:Class ;
                 rdfs:subClassOf cco:ont00000136 ;
                 rdfs:label "Periscope"@en ;
                 skos:definition "An Optical Instrument that is designed to enable observation of an object that is located over, around, or through another object, obstacle, or condition that prevents direct line-of-sight observation from the observer's current position."@en ;
                 cco:ont00001754 "https://en.wikipedia.org/w/index.php?title=Periscope&oldid=1030400442"^^xsd:anyURI ;
                 cco:ont00001760 "https://www.commoncoreontologies.org/ArtifactOntology"^^xsd:anyURI .


###  https://www.commoncoreontologies.org/ont00001217
cco:ont00001217 rdf:type owl:Class ;
                 rdfs:subClassOf cco:ont00000848 ;
                 rdfs:label "Medium Machine Gun"@en ;
                 skos:definition "A Mounted Gun that is designed to fire full-power rifle Cartridges (less than .50 caliber or 12.7mm) in quick succession from an ammunition belt, and which typically weighs 22-30 lbs."@en ;
                 cco:ont00001754 "https://en.wikipedia.org/w/index.php?title=Medium_machine_gun&oldid=1063571269"^^xsd:anyURI ;
                 cco:ont00001760 "https://www.commoncoreontologies.org/ArtifactOntology"^^xsd:anyURI .


###  https://www.commoncoreontologies.org/ont00001218
cco:ont00001218 rdf:type owl:Class ;
                 rdfs:subClassOf cco:ont00000323 ;
                 rdfs:label "Signal Processing Artifact Function"@en ;
                 skos:definition "An Artifact Function that is realized in the process of transferring or processing information contained in signals."@en ;
                 cco:ont00001754 "https://en.wikipedia.org/w/index.php?title=Signal_processing&oldid=1062720685"^^xsd:anyURI ;
                 cco:ont00001760 "https://www.commoncoreontologies.org/ArtifactOntology"^^xsd:anyURI .


###  https://www.commoncoreontologies.org/ont00001221
cco:ont00001221 rdf:type owl:Class ;
                 rdfs:subClassOf cco:ont00000210 ;
                 rdfs:label "Physically Powered Engine"@en ;
                 skos:altLabel "Physical Engine"@en ;
                 skos:definition "An Engine that is designed to convert potential or kinetic energy into mechanical energy."@en ;
                 cco:ont00001760 "https://www.commoncoreontologies.org/ArtifactOntology"^^xsd:anyURI .


###  https://www.commoncoreontologies.org/ont00001222
cco:ont00001222 rdf:type owl:Class ;
                 rdfs:subClassOf cco:ont00001049 ;
                 rdfs:label "Solar Panel System"@en ;
                 skos:altLabel "Photovoltaic System"@en ,
                               "Solar Array"@en ;
                 skos:definition "An Electrical Power Source that consists in part of one or more Solar Panels, a power inverter, electrical wiring between the components, a mounting and support structure, and may also include a battery and/or a solar tracking system and is the bearer of functions realized in processes of deriving, transferring, and storing electrical energy derived from light energy."@en ;
                 cco:ont00001754 "https://en.wikipedia.org/w/index.php?title=Photovoltaic_system&oldid=1063366598"^^xsd:anyURI ;
                 cco:ont00001760 "https://www.commoncoreontologies.org/ArtifactOntology"^^xsd:anyURI .


###  https://www.commoncoreontologies.org/ont00001223
cco:ont00001223 rdf:type owl:Class ;
                 rdfs:subClassOf cco:ont00001145 ;
                 rdfs:label "Dish Receiver"@en ;
                 skos:definition "A Radio Receiver that uses a Parabolic (or Dish) Antenna to intercept radio signals."@en ;
                 cco:ont00001760 "https://www.commoncoreontologies.org/ArtifactOntology"^^xsd:anyURI .


###  https://www.commoncoreontologies.org/ont00001228
cco:ont00001228 rdf:type owl:Class ;
                 rdfs:subClassOf cco:ont00000798 ;
                 rdfs:label "Journal Article"@en ;
                 skos:definition "An Information Bearing Artifact that is designed to bear a specific brief composition on a specific topic as part of a Journal Issue."@en ;
                 cco:ont00001754 "https://en.wikipedia.org/w/index.php?title=Academic_journal&oldid=1059723283"^^xsd:anyURI ;
                 cco:ont00001760 "https://www.commoncoreontologies.org/ArtifactOntology"^^xsd:anyURI .


###  https://www.commoncoreontologies.org/ont00001229
cco:ont00001229 rdf:type owl:Class ;
                 rdfs:subClassOf cco:ont00001050 ;
                 rdfs:label "Alkaline Electric Battery"@en ;
                 skos:definition "A Primary Cell Electric Battery that has a Zinc anode and Manganese (IV) oxide cathode."@en ;
                 cco:ont00001754 "https://en.wikipedia.org/w/index.php?title=Alkaline_battery&oldid=1055652562"^^xsd:anyURI ;
                 cco:ont00001760 "https://www.commoncoreontologies.org/ArtifactOntology"^^xsd:anyURI .


###  https://www.commoncoreontologies.org/ont00001230
cco:ont00001230 rdf:type owl:Class ;
                 rdfs:subClassOf cco:ont00000499 ;
                 rdfs:label "Rhombic Antenna"@en ;
                 skos:definition "A Wire Antenna that consists of one to three parallel wires suspended above the ground by poles or towers at each vertex in a rhombic shape with each of the four sides being the same length (typically at least one wavelength or longer)."@en ;
                 cco:ont00001754 "https://en.wikipedia.org/w/index.php?title=Rhombic_antenna&oldid=1057114456"^^xsd:anyURI ;
                 cco:ont00001760 "https://www.commoncoreontologies.org/ArtifactOntology"^^xsd:anyURI .


###  https://www.commoncoreontologies.org/ont00001233
cco:ont00001233 rdf:type owl:Class ;
                 rdfs:subClassOf cco:ont00001153 ;
                 rdfs:label "Crushing Artifact Function"@en ;
                 skos:definition "A Damaging Artifact Function that is realized in a process in which the structural integrity of an entity is impaired because of significant pressure."@en ;
                 cco:ont00001754 "http://www.dictionary.com/browse/crushing" ;
                 cco:ont00001760 "https://www.commoncoreontologies.org/ArtifactOntology"^^xsd:anyURI .


###  https://www.commoncoreontologies.org/ont00001234
cco:ont00001234 rdf:type owl:Class ;
                 rdfs:subClassOf cco:ont00000791 ;
                 rdfs:label "Neutralization Artifact Function"@en ;
                 skos:definition "A Chemical Reaction Artifact Function that is realized in a process in which an acid and a base react quantitatively with each other."@en ;
                 cco:ont00001754 "https://en.wikipedia.org/wiki/Neutralization_(chemistry)" ;
                 cco:ont00001760 "https://www.commoncoreontologies.org/ArtifactOntology"^^xsd:anyURI .


###  https://www.commoncoreontologies.org/ont00001240
cco:ont00001240 rdf:type owl:Class ;
                 rdfs:subClassOf cco:ont00001148 ;
                 rdfs:label "Radio Communication Artifact Function"@en ;
                 skos:definition "An Electromagnetic Communication Artifact Function that is realized in a process that conveys meaningful signs by means of radio waves."@en ;
                 cco:ont00001754 "https://en.wikipedia.org/w/index.php?title=Telecommunications&oldid=1061143810"^^xsd:anyURI ;
                 cco:ont00001760 "https://www.commoncoreontologies.org/ArtifactOntology"^^xsd:anyURI .


###  https://www.commoncoreontologies.org/ont00001241
cco:ont00001241 rdf:type owl:Class ;
                 rdfs:subClassOf cco:ont00000323 ;
                 rdfs:label "Sensor Artifact Function"@en ;
                 skos:definition "An Artifact Function that is realized in processes wherein its bearer is used to produce an output signal which reliably corresponds to changes in the artifact's environment."@en ;
                 cco:ont00001754 "https://en.wikipedia.org/w/index.php?title=Sensor&oldid=1059883466"^^xsd:anyURI ;
                 cco:ont00001760 "https://www.commoncoreontologies.org/ArtifactOntology"^^xsd:anyURI .


###  https://www.commoncoreontologies.org/ont00001242
cco:ont00001242 rdf:type owl:Class ;
                 rdfs:subClassOf cco:ont00000736 ;
                 rdfs:label "Actuator"@en ;
                 skos:definition "A Transducer that is designed to convert some control signal into mechanical motion."@en ;
                 cco:ont00001754 "https://en.wikipedia.org/w/index.php?title=Actuator&oldid=1064000375"^^xsd:anyURI ;
                 cco:ont00001760 "https://www.commoncoreontologies.org/ArtifactOntology"^^xsd:anyURI .


###  https://www.commoncoreontologies.org/ont00001243
cco:ont00001243 rdf:type owl:Class ;
                 rdfs:subClassOf cco:ont00000253 ;
                 rdfs:label "Document Field"@en ;
                 skos:definition "An Information Bearing Entity that is a part of some document into which bearers of prescribed information can be written or selected."@en ;
                 cco:ont00001760 "https://www.commoncoreontologies.org/ArtifactOntology"^^xsd:anyURI .


###  https://www.commoncoreontologies.org/ont00001245
cco:ont00001245 rdf:type owl:Class ;
                 rdfs:subClassOf cco:ont00000241 ;
                 rdfs:label "PDF417 Code"@en ;
                 skos:definition "A Two-Dimensional Barcode that is used in applications that require the storage of huge amounts of data."@en ;
                 cco:ont00001760 "https://www.commoncoreontologies.org/ArtifactOntology"^^xsd:anyURI .


###  https://www.commoncoreontologies.org/ont00001247
cco:ont00001247 rdf:type owl:Class ;
                 rdfs:subClassOf cco:ont00000918 ;
                 rdfs:label "Telecommunication Endpoint"@en ;
                 skos:definition "A Telecommunication Network Node that connects a Telecommunication Terminal to a Telecommunication Network."@en ;
                 skos:scopeNote "A Telecommunication Terminal is an end user device such as a Telephone, fax machine, or Computer."@en ;
                 cco:ont00001754 "https://en.wikipedia.org/w/index.php?title=Communication_endpoint&oldid=1020569501"^^xsd:anyURI ;
                 cco:ont00001760 "https://www.commoncoreontologies.org/ArtifactOntology"^^xsd:anyURI .


###  https://www.commoncoreontologies.org/ont00001248
cco:ont00001248 rdf:type owl:Class ;
                 rdfs:subClassOf cco:ont00000715 ;
                 rdfs:label "Artificial Eye"@en ;
                 skos:definition "A Prosthesis that is designed to replace a missing eye."@en ;
                 cco:ont00001754 "https://en.wikipedia.org/w/index.php?title=Artificial_eye&oldid=1046672400"^^xsd:anyURI ;
                 cco:ont00001760 "https://www.commoncoreontologies.org/ArtifactOntology"^^xsd:anyURI .


###  https://www.commoncoreontologies.org/ont00001249
cco:ont00001249 rdf:type owl:Class ;
                 rdfs:subClassOf cco:ont00000453 ;
                 rdfs:label "Cabin Pressurization Control System"@en ;
                 skos:definition "An Environment Control System that is designed to control the process in which conditioned air is pumped into the Cabin of some Aircraft or Spacecraft in order to create a safe and comfortable environment for passengers and crew flying at high altitudes."@en ;
                 cco:ont00001754 "https://en.wikipedia.org/w/index.php?title=Cabin_pressurization&oldid=1062243955"^^xsd:anyURI ;
                 cco:ont00001760 "https://www.commoncoreontologies.org/ArtifactOntology"^^xsd:anyURI .


###  https://www.commoncoreontologies.org/ont00001250
cco:ont00001250 rdf:type owl:Class ;
                 rdfs:subClassOf cco:ont00000236 ;
                 rdfs:label "Interior Lighting System"@en ;
                 skos:definition "A Lighting System that is designed to emit light within the interior of some area."@en ;
                 cco:ont00001760 "https://www.commoncoreontologies.org/ArtifactOntology"^^xsd:anyURI .


###  https://www.commoncoreontologies.org/ont00001252
cco:ont00001252 rdf:type owl:Class ;
                 rdfs:subClassOf cco:ont00000448 ;
                 rdfs:label "Propulsion Artifact Function"@en ;
                 skos:definition "A Motion Artifact Function that is realized in a process in which the bearer of the function creates force leading to an entity's movement."@en ;
                 cco:ont00001754 "https://en.wikipedia.org/w/index.php?title=Propulsion&oldid=1022034059"^^xsd:anyURI ;
                 cco:ont00001760 "https://www.commoncoreontologies.org/ArtifactOntology"^^xsd:anyURI .


###  https://www.commoncoreontologies.org/ont00001253
cco:ont00001253 rdf:type owl:Class ;
                 rdfs:subClassOf cco:ont00000323 ;
                 rdfs:label "Fuel Artifact Function"@en ;
                 skos:definition "An Artifact Function that is realized in processes in which a Portion of Fuel is reacted with other substances in order to release chemical or nuclear energy to be used for heat or for work."@en ;
                 cco:ont00001754 "https://en.wikipedia.org/w/index.php?title=Fuel&oldid=1063590518"^^xsd:anyURI ;
                 cco:ont00001760 "https://www.commoncoreontologies.org/ArtifactOntology"^^xsd:anyURI .


###  https://www.commoncoreontologies.org/ont00001254
cco:ont00001254 rdf:type owl:Class ;
                 rdfs:subClassOf cco:ont00000156 ;
                 rdfs:label "Revolver"@en ;
                 skos:definition "A Hand Gun having a number of firing chambers in a revolving cylinder, where each chamber in the cylinder can be loaded with a single Cartridge."@en ;
                 cco:ont00001754 "https://en.wikipedia.org/w/index.php?title=Revolver&oldid=1060461644"^^xsd:anyURI ;
                 cco:ont00001760 "https://www.commoncoreontologies.org/ArtifactOntology"^^xsd:anyURI .


###  https://www.commoncoreontologies.org/ont00001255
cco:ont00001255 rdf:type owl:Class ;
                 rdfs:subClassOf cco:ont00000828 ;
                 rdfs:label "Insecticide Artifact Function"@en ;
                 skos:definition "A Pesticide Artifact Function that is realized in a process that causes harm to, or the death of, an insect."@en ;
                 cco:ont00001754 "https://en.wikipedia.org/w/index.php?title=Insecticide&oldid=1063322558"^^xsd:anyURI ;
                 cco:ont00001760 "https://www.commoncoreontologies.org/ArtifactOntology"^^xsd:anyURI .


###  https://www.commoncoreontologies.org/ont00001260
cco:ont00001260 rdf:type owl:Class ;
                 rdfs:subClassOf cco:ont00000258 ;
                 rdfs:label "Code 39 Barcode"@en ;
                 skos:definition "A One-Dimensional Barcode that consists of 39 characters that are numbers 0-9, capital letters A-Z, or the symbols -.$/+% and space and is used primarily in automotive and defense industries."@en ;
                 cco:ont00001760 "https://www.commoncoreontologies.org/ArtifactOntology"^^xsd:anyURI .


###  https://www.commoncoreontologies.org/ont00001264
cco:ont00001264 rdf:type owl:Class ;
                 rdfs:subClassOf cco:ont00000258 ;
                 rdfs:label "Code 128 Barcode"@en ;
                 skos:definition "A One-Dimensional Barcode that consists of up to 128 ASCII characters and is used primarily in supply chains."@en ;
                 cco:ont00001760 "https://www.commoncoreontologies.org/ArtifactOntology"^^xsd:anyURI .


###  https://www.commoncoreontologies.org/ont00001265
cco:ont00001265 rdf:type owl:Class ;
                 rdfs:subClassOf cco:ont00001036 ;
                 rdfs:label "Public Address System"@en ;
                 skos:altLabel "PA System"@en ;
                 skos:definition "A Communication System that is designed to allow a Person to speak to a large audience."@en ;
                 cco:ont00001754 "https://en.wikipedia.org/w/index.php?title=Public_address_system&oldid=1059177344"^^xsd:anyURI ;
                 cco:ont00001760 "https://www.commoncoreontologies.org/ArtifactOntology"^^xsd:anyURI .


###  https://www.commoncoreontologies.org/ont00001268
cco:ont00001268 rdf:type owl:Class ;
                 rdfs:subClassOf cco:ont00000966 ;
                 rdfs:label "ISBN Barcode"@en ;
                 skos:definition "An EAN Barcode that is used to designate books."@en ;
                 cco:ont00001760 "https://www.commoncoreontologies.org/ArtifactOntology"^^xsd:anyURI .


###  https://www.commoncoreontologies.org/ont00001270
cco:ont00001270 rdf:type owl:Class ;
                 rdfs:subClassOf cco:ont00000268 ;
                 rdfs:label "Howitzer"@en ;
                 skos:definition "A Cannon that is designed to have a relatively short barrel and to use relatively small propellant charges to propel projectiles in relatively high trajectories with a steep angle of descent."@en ;
                 cco:ont00001754 "https://en.wikipedia.org/w/index.php?title=Howitzer&oldid=1059576383"^^xsd:anyURI ;
                 cco:ont00001760 "https://www.commoncoreontologies.org/ArtifactOntology"^^xsd:anyURI .


###  https://www.commoncoreontologies.org/ont00001271
cco:ont00001271 rdf:type owl:Class ;
                 rdfs:subClassOf cco:ont00001169 ;
                 rdfs:label "Wired Communication Relay Artifact Function"@en ;
                 skos:definition "A Communication Relay Artifact Function that is realized during events in which an Artifact is used to first receive and then transmit information by means of wires from one Artifact to another for the purpose of communiction."@en ;
                 cco:ont00001760 "https://www.commoncoreontologies.org/ArtifactOntology"^^xsd:anyURI .


###  https://www.commoncoreontologies.org/ont00001273
cco:ont00001273 rdf:type owl:Class ;
                 rdfs:subClassOf cco:ont00001241 ,
                                 [ rdf:type owl:Restriction ;
                                   owl:onProperty obo:BFO_0000197 ;
                                   owl:someValuesFrom cco:ont00000569
                                 ] ;
                 rdfs:label "Sensor Modality Function"@en ;
                 skos:definition "A Sensor Artifact Function that inheres in some Sensor in virtue of the type of energy the Sensor is capable of converting into an output signal."@en ;
                 cco:ont00001760 "https://www.commoncoreontologies.org/ArtifactOntology"^^xsd:anyURI .


###  https://www.commoncoreontologies.org/ont00001275
cco:ont00001275 rdf:type owl:Class ;
                 rdfs:subClassOf cco:ont00001353 ;
                 rdfs:label "Nominal Speed Artifact Function"@en ;
                 skos:definition "A Speed Artifact Function that is realized in some process in which the Artifact bearing the Artifact Function attains a speed that does not exceed some specified tolerance of that Artifact."@en ;
                 cco:ont00001760 "https://www.commoncoreontologies.org/ArtifactOntology"^^xsd:anyURI .


###  https://www.commoncoreontologies.org/ont00001278
cco:ont00001278 rdf:type owl:Class ;
                 rdfs:subClassOf cco:ont00000537 ;
                 rdfs:label "Stock"@en ;
                 skos:definition "A Financial Instrument that entitles holders to an ownership interest (equity) in the specified Incorporated Organization."@en ;
                 cco:ont00001754 "https://en.wikipedia.org/w/index.php?title=Stock&oldid=1064040249"^^xsd:anyURI ;
                 cco:ont00001760 "https://www.commoncoreontologies.org/ArtifactOntology"^^xsd:anyURI .


###  https://www.commoncoreontologies.org/ont00001281
cco:ont00001281 rdf:type owl:Class ;
                 rdfs:subClassOf cco:ont00000791 ;
                 rdfs:label "Emulsifier Artifact Function"@en ;
                 skos:definition "A Chemical Reaction Artifact Function that is realized in a process in which two or more liquids that are normally immiscible are mixed."@en ;
                 cco:ont00001754 "https://en.wikipedia.org/w/index.php?title=Emulsion&oldid=1056901580"^^xsd:anyURI ;
                 cco:ont00001760 "https://www.commoncoreontologies.org/ArtifactOntology"^^xsd:anyURI .


###  https://www.commoncoreontologies.org/ont00001282
cco:ont00001282 rdf:type owl:Class ;
                 rdfs:subClassOf cco:ont00000598 ;
                 rdfs:label "Hydraulic Valve"@en ;
                 skos:definition "A Valve that is designed to regulate, direct, or control the flow of a liquid by opening, closing, or partially obstructing various passageways."@en ;
                 cco:ont00001754 "https://en.wikipedia.org/w/index.php?title=Power_transfer_unit&oldid=1002682083"^^xsd:anyURI ;
                 cco:ont00001760 "https://www.commoncoreontologies.org/ArtifactOntology"^^xsd:anyURI .


###  https://www.commoncoreontologies.org/ont00001288
cco:ont00001288 rdf:type owl:Class ;
                 rdfs:subClassOf cco:ont00001150 ;
                 rdfs:label "Round Shot"@en ;
                 skos:definition "A Portion of Ammunition that is designed to be a solid projectile without explosive charge and to be fired from a cannon."@en ;
                 cco:ont00001754 "https://en.wikipedia.org/w/index.php?title=Round_shot&oldid=1062790260"^^xsd:anyURI ;
                 cco:ont00001760 "https://www.commoncoreontologies.org/ArtifactOntology"^^xsd:anyURI .


###  https://www.commoncoreontologies.org/ont00001292
cco:ont00001292 rdf:type owl:Class ;
                 rdfs:subClassOf cco:ont00000053 ;
                 rdfs:label "Bus"@en ;
                 skos:definition "A Ground Motor Vehicle that is designed to transport a large number of people and to travel on six or more tired wheels."@en ;
                 cco:ont00001754 "https://en.wikipedia.org/w/index.php?title=Bus&oldid=1055341487"^^xsd:anyURI ;
                 cco:ont00001760 "https://www.commoncoreontologies.org/ArtifactOntology"^^xsd:anyURI .


###  https://www.commoncoreontologies.org/ont00001298
cco:ont00001298 rdf:type owl:Class ;
                 rdfs:subClassOf cco:ont00000798 ;
                 rdfs:label "Document"@en ;
                 skos:definition "An Information Bearing Artifact that is designed to bear some specific Information Content Entity in a series of paragraphs of text or diagrams in the form of physical pieces of paper or an electronic word processor file."@en ;
                 cco:ont00001754 "https://en.wikipedia.org/w/index.php?title=Document&oldid=1057829688"^^xsd:anyURI ;
                 cco:ont00001760 "https://www.commoncoreontologies.org/ArtifactOntology"^^xsd:anyURI .


###  https://www.commoncoreontologies.org/ont00001299
cco:ont00001299 rdf:type owl:Class ;
                 rdfs:subClassOf cco:ont00000344 ;
                 rdfs:label "Wetting Agent Artifact Function"@en ;
                 skos:definition "A Surfactant Artifact Function that is realized in a process that reduces the water repellent tendency of a substance thereby allowing it to become wet."@en ;
                 cco:ont00001754 "https://en.wikipedia.org/w/index.php?title=Wetting&oldid=1062806793"^^xsd:anyURI ;
                 cco:ont00001760 "https://www.commoncoreontologies.org/ArtifactOntology"^^xsd:anyURI .


###  https://www.commoncoreontologies.org/ont00001300
cco:ont00001300 rdf:type owl:Class ;
                 rdfs:subClassOf cco:ont00001192 ;
                 rdfs:label "Patch Antenna"@en ;
                 skos:altLabel "Microstrip Patch Antenna"@en ,
                               "Rectangular Microstrip Antenna"@en ;
                 skos:definition "A Radio Antenna that consists of a flat rectangular sheet (or patch) of metal mounted over a larger sheet of metal called a ground plane which is typically contained inside a plastic radome for protection and is small enough that it can be mounted on a flat surface."@en ;
                 cco:ont00001754 "https://en.wikipedia.org/w/index.php?title=Patch_antenna&oldid=1016658507"^^xsd:anyURI ;
                 cco:ont00001760 "https://www.commoncoreontologies.org/ArtifactOntology"^^xsd:anyURI .


###  https://www.commoncoreontologies.org/ont00001301
cco:ont00001301 rdf:type owl:Class ;
                 rdfs:subClassOf cco:ont00000323 ;
                 rdfs:label "Service Artifact Function"@en ;
                 skos:definition "An Artifact Function that is realized in a process of providing intangible goods to consumers."@en ;
                 cco:ont00001754 "https://en.wikipedia.org/w/index.php?title=Goods_and_services&oldid=1063137197"^^xsd:anyURI ;
                 cco:ont00001760 "https://www.commoncoreontologies.org/ArtifactOntology"^^xsd:anyURI .


###  https://www.commoncoreontologies.org/ont00001303
cco:ont00001303 rdf:type owl:Class ;
                 rdfs:subClassOf cco:ont00001306 ;
                 rdfs:label "Position Observation Artifact Function"@en ;
                 skos:definition "An Observation Artifact Function that is realized during events in which an Artifact is used to collect information about the position of a specified object or class of objects."@en ;
                 cco:ont00001760 "https://www.commoncoreontologies.org/ArtifactOntology"^^xsd:anyURI .


###  https://www.commoncoreontologies.org/ont00001304
cco:ont00001304 rdf:type owl:Class ;
                 rdfs:subClassOf cco:ont00000575 ;
                 rdfs:label "Dimension Specification"@en ;
                 skos:definition "An Quality Specification that prescribes some Size Quality."@en ;
                 cco:ont00001760 "https://www.commoncoreontologies.org/ArtifactOntology"^^xsd:anyURI .


###  https://www.commoncoreontologies.org/ont00001306
cco:ont00001306 rdf:type owl:Class ;
                 rdfs:subClassOf cco:ont00000323 ;
                 rdfs:label "Observation Artifact Function"@en ;
                 skos:definition "An Artifact Function that is realized during events in which an Artifact is used to collect information about a specified object or class of objects."@en ;
                 cco:ont00001760 "https://www.commoncoreontologies.org/ArtifactOntology"^^xsd:anyURI .


###  https://www.commoncoreontologies.org/ont00001310
cco:ont00001310 rdf:type owl:Class ;
                 rdfs:subClassOf cco:ont00000323 ;
                 rdfs:label "Covering Artifact Function"@en ;
                 skos:definition "An Artifact Function that is realized in a process in which an entity is covered."@en ;
                 cco:ont00001754 "http://www.dictionary.com/browse/covering" ;
                 cco:ont00001760 "https://www.commoncoreontologies.org/ArtifactOntology"^^xsd:anyURI .


###  https://www.commoncoreontologies.org/ont00001313
cco:ont00001313 rdf:type owl:Class ;
                 rdfs:subClassOf cco:ont00000995 ;
                 rdfs:label "Article of Clothing"@en ;
                 skos:definition "A Material Artifact that is designed to cover some portion of a body."@en ;
                 cco:ont00001754 "https://en.wikipedia.org/w/index.php?title=Clothing&oldid=1063505718"^^xsd:anyURI ;
                 cco:ont00001760 "https://www.commoncoreontologies.org/ArtifactOntology"^^xsd:anyURI .


###  https://www.commoncoreontologies.org/ont00001316
cco:ont00001316 rdf:type owl:Class ;
                 rdfs:subClassOf cco:ont00001042 ;
                 rdfs:label "Gimbal"@en ;
                 skos:definition "An Equipment Mount that consists of a pivoted support that allows an Artifact to Rotate about one or more Axes."@en ;
                 cco:ont00001754 "https://en.wikipedia.org/w/index.php?title=Gimbal&oldid=1053306885"^^xsd:anyURI ;
                 cco:ont00001760 "https://www.commoncoreontologies.org/ArtifactOntology"^^xsd:anyURI .


###  https://www.commoncoreontologies.org/ont00001319
cco:ont00001319 rdf:type owl:Class ;
                 rdfs:subClassOf cco:ont00000427 ;
                 rdfs:comment "Tank firepower is normally provided by a large-caliber main gun mounted in a rotating turret, which is supported by secondary machine guns. A tank's heavy armour and all-terrain mobility provide protection for both the tank and its crew, allowing it to perform all primary tasks of the armoured troops on the battlefield."@en ;
                 rdfs:label "Tank"@en ;
                 skos:definition "An Armored Fighting Vehicle that is designed to carry heavy firepower, have a powerful Engine, and travel on one or more continuous tracks such that it is suitable for front-line combat and can provide operational maneuverability as well as tactical offensive and defensive capabilities."@en ;
                 cco:ont00001754 "https://en.wikipedia.org/w/index.php?title=Tank&oldid=1060527612"^^xsd:anyURI ;
                 cco:ont00001760 "https://www.commoncoreontologies.org/ArtifactOntology"^^xsd:anyURI .


###  https://www.commoncoreontologies.org/ont00001320
cco:ont00001320 rdf:type owl:Class ;
                 rdfs:subClassOf cco:ont00000903 ;
                 rdfs:label "Radio Transceiver"@en ;
                 skos:definition "A Radio Communication Instrument that is an electronic device composed of both a Radio Transmitter and a Radio Receiver that share common circuitry or a single housing."@en ;
                 cco:ont00001754 "https://en.wikipedia.org/w/index.php?title=Transceiver&oldid=1058453736"^^xsd:anyURI ;
                 cco:ont00001760 "https://www.commoncoreontologies.org/ArtifactOntology"^^xsd:anyURI .


###  https://www.commoncoreontologies.org/ont00001321
cco:ont00001321 rdf:type owl:Class ;
                 rdfs:subClassOf cco:ont00001105 ;
                 rdfs:label "Lead Acid Electric Battery"@en ;
                 skos:definition "A Secondary Cell Electric Battery that has a lead anode and lead oxide cathode."@en ;
                 cco:ont00001754 "https://en.wikipedia.org/w/index.php?title=Lead%E2%80%93acid_battery&oldid=1061641405"^^xsd:anyURI ;
                 cco:ont00001760 "https://www.commoncoreontologies.org/ArtifactOntology"^^xsd:anyURI .


###  https://www.commoncoreontologies.org/ont00001323
cco:ont00001323 rdf:type owl:Class ;
                 rdfs:subClassOf cco:ont00000323 ;
                 rdfs:label "Bearing Artifact Function"@en ;
                 skos:definition "An Artifact Function that is realized in processes in which the Artifact constrains relative motion to only the desired motion, and reduces friction between moving parts."@en ;
                 cco:ont00001754 "https://en.wikipedia.org/wiki/Bearing_(mechanical)" ;
                 cco:ont00001760 "https://www.commoncoreontologies.org/ArtifactOntology"^^xsd:anyURI .


###  https://www.commoncoreontologies.org/ont00001326
cco:ont00001326 rdf:type owl:Class ;
                 rdfs:subClassOf cco:ont00000254 ;
                 rdfs:label "Land Transportation Artifact"@en ;
                 skos:definition "A Transportation Artifact that is fixed in place and designed to bear a Function, the realization of which is sometimes part of a process moving Vehicles and Agents from one location to another via land."@en ;
                 cco:ont00001760 "https://www.commoncoreontologies.org/ArtifactOntology"^^xsd:anyURI .


###  https://www.commoncoreontologies.org/ont00001329
cco:ont00001329 rdf:type owl:Class ;
                 rdfs:subClassOf cco:ont00001301 ;
                 rdfs:label "Education Artifact Function"@en ;
                 skos:definition "A Service Artifact Function that is realized in processes of transmiting accumulated knowledge skills and values from one generation to another."@en ;
                 cco:ont00001754 "https://en.wikipedia.org/w/index.php?title=Education&oldid=1064011752"^^xsd:anyURI ;
                 cco:ont00001760 "https://www.commoncoreontologies.org/ArtifactOntology"^^xsd:anyURI .


###  https://www.commoncoreontologies.org/ont00001341
cco:ont00001341 rdf:type owl:Class .


###  https://www.commoncoreontologies.org/ont00001342
cco:ont00001342 rdf:type owl:Class ;
                 rdfs:subClassOf cco:ont00000427 ;
                 rdfs:label "Infantry Fighting Vehicle"@en ;
                 skos:definition "An Armored Fighting Vehicle that is designed to carry infantry into battle and to provide fire support for them."@en ;
                 skos:scopeNote "Infantry Fighting Vehicles (IFVs) are differentiated from Armored Personnel Carriers (APCs) because they are designed to give direct fire support to the dismounted infantry and so usually have significantly enhanced armament. IFVs also often have improved armour and firing ports (allowing the infantry to fire personal weapons while mounted)."@en ;
                 cco:ont00001753 "IFV" ;
                 cco:ont00001754 "https://en.wikipedia.org/w/index.php?title=Infantry_fighting_vehicle&oldid=1062470745"^^xsd:anyURI ;
                 cco:ont00001760 "https://www.commoncoreontologies.org/ArtifactOntology"^^xsd:anyURI .


###  https://www.commoncoreontologies.org/ont00001343
cco:ont00001343 rdf:type owl:Class ;
                 rdfs:subClassOf cco:ont00000995 ;
                 rdfs:label "Circuit Breaker"@en ;
                 skos:definition "A Material Artifact that is designed to protect an electrical circuit from damage caused by excess current from an overload or short circuit."@en ;
                 cco:ont00001754 "https://en.wikipedia.org/w/index.php?title=Circuit_breaker&oldid=1060854893"^^xsd:anyURI ;
                 cco:ont00001760 "https://www.commoncoreontologies.org/ArtifactOntology"^^xsd:anyURI .


###  https://www.commoncoreontologies.org/ont00001346
cco:ont00001346 rdf:type owl:Class ;
                 rdfs:subClassOf cco:ont00000995 ;
                 rdfs:label "Legal Instrument"@en ;
                 skos:definition "A Material Artifact that is designed as a formally executed written document that can be formally attributed to its author, records and formally expresses a legally enforceable act, process, or contractual duty, obligation, or right, and therefore evidences that act, process, or agreement."@en ;
                 cco:ont00001754 "https://en.wikipedia.org/w/index.php?title=Legal_instrument&oldid=1054387344"^^xsd:anyURI ;
                 cco:ont00001760 "https://www.commoncoreontologies.org/ArtifactOntology"^^xsd:anyURI .


###  https://www.commoncoreontologies.org/ont00001350
cco:ont00001350 rdf:type owl:Class ;
                 rdfs:subClassOf cco:ont00000323 ;
                 rdfs:label "Thermal Control Artifact Function"@en ;
                 skos:definition "An Artifact Function that is realized by an Artifact increasing, decreasing, or maintaining the temperature of itself, a part of itself, or another object."@en ;
                 cco:ont00001760 "https://www.commoncoreontologies.org/ArtifactOntology"^^xsd:anyURI .


###  https://www.commoncoreontologies.org/ont00001353
cco:ont00001353 rdf:type owl:Class ;
                 rdfs:subClassOf cco:ont00000448 ;
                 rdfs:label "Speed Artifact Function"@en ;
                 skos:definition "A Motion Artifact Function that is realized in some process in which its bearer has some speed."@en ;
                 cco:ont00001760 "https://www.commoncoreontologies.org/ArtifactOntology"^^xsd:anyURI .


###  https://www.commoncoreontologies.org/ont00001355
cco:ont00001355 rdf:type owl:Class ;
                 rdfs:subClassOf cco:ont00000928 ;
                 rdfs:label "Freight Train Car"@en ;
                 skos:altLabel "Freight Car"@en ;
                 skos:definition "A Train Car that is designed to transport cargo."@en ;
                 cco:ont00001754 "https://en.wikipedia.org/w/index.php?title=Goods_wagon&oldid=1062686785"^^xsd:anyURI ;
                 cco:ont00001760 "https://www.commoncoreontologies.org/ArtifactOntology"^^xsd:anyURI .


###  https://www.commoncoreontologies.org/ont00001361
cco:ont00001361 rdf:type owl:Class ;
                 rdfs:subClassOf cco:ont00000323 ;
                 rdfs:label "Healing Artifact Function"@en ;
                 skos:definition "An Artifact Function that is realized in a process in which health is restored to an unbalanced, diseased, or damaged organism."@en ;
                 cco:ont00001754 "https://en.wikipedia.org/w/index.php?title=Healing&oldid=1053920678"^^xsd:anyURI ;
                 cco:ont00001760 "https://www.commoncoreontologies.org/ArtifactOntology"^^xsd:anyURI .


###  https://www.commoncoreontologies.org/ont00001365
cco:ont00001365 rdf:type owl:Class ;
                 rdfs:subClassOf cco:ont00001353 ;
                 rdfs:label "Maximum Speed Artifact Function"@en ;
                 skos:definition "A Speed Artifact Function that is realized in some process in which the Artifact bearing the Artifact Function attains the highest speed at which that Artifact is designed to operate."@en ;
                 cco:ont00001760 "https://www.commoncoreontologies.org/ArtifactOntology"^^xsd:anyURI .


###  https://www.commoncoreontologies.org/ont00001366
cco:ont00001366 rdf:type owl:Class ;
                 rdfs:subClassOf cco:ont00000323 ;
                 rdfs:label "Powering Artifact Function"@en ;
                 skos:definition "An Artifact Function that is realized by processes in which some Artifact is used to supply power to some Artifact."@en ;
                 cco:ont00001760 "https://www.commoncoreontologies.org/ArtifactOntology"^^xsd:anyURI .


###  https://www.commoncoreontologies.org/ont00001368
cco:ont00001368 rdf:type owl:Class ;
                 rdfs:subClassOf cco:ont00001306 ;
                 rdfs:label "Motion Observation Artifact Function"@en ;
                 skos:definition "An Observation Artifact Function that is realized during events in which an Artifact is used to collect information about the Motion of a specified object or class of objects."@en ;
                 cco:ont00001760 "https://www.commoncoreontologies.org/ArtifactOntology"^^xsd:anyURI .


###  https://www.commoncoreontologies.org/ont00001370
cco:ont00001370 rdf:type owl:Class ;
                 rdfs:subClassOf cco:ont00000995 ;
                 rdfs:label "Machine Bearing"@en ;
                 skos:definition "A Material Artifact that is designed to constrain relative motion to only desired motion and reduces friction between moving parts."@en ;
                 cco:ont00001754 "https://en.wikipedia.org/wiki/Bearing_(mechanical)" ;
                 cco:ont00001760 "https://www.commoncoreontologies.org/ArtifactOntology"^^xsd:anyURI .


###  https://www.commoncoreontologies.org/ont00001371
cco:ont00001371 rdf:type owl:Class ;
                 rdfs:subClassOf cco:ont00000323 ;
                 rdfs:label "Electromagnetic Induction Artifact Function"@en ;
                 skos:definition "An Artifact Function that is realized by processes in which some Artifact that is used to produce electromotive force across an electrical conductor due to its dynamic interaction with a magnetic field."@en ;
                 cco:ont00001754 "https://en.wikipedia.org/w/index.php?title=Electromagnetic_induction&oldid=1061836930"^^xsd:anyURI ;
                 cco:ont00001760 "https://www.commoncoreontologies.org/ArtifactOntology"^^xsd:anyURI .


###  https://www.commoncoreontologies.org/ont00001372
cco:ont00001372 rdf:type owl:Class ;
                 rdfs:subClassOf cco:ont00000437 ;
                 rdfs:label "Fertilizer Artifact Function"@en ;
                 skos:definition "An Enhancing Artifact Function that is realized in processes of supplying soilds or plant tissues with one or more plant nutrients essential to growth."@en ;
                 cco:ont00001754 "https://en.wikipedia.org/w/index.php?title=Fertilizer&oldid=1062923261"^^xsd:anyURI ;
                 cco:ont00001760 "https://www.commoncoreontologies.org/ArtifactOntology"^^xsd:anyURI .


###  https://www.commoncoreontologies.org/ont00001373
cco:ont00001373 rdf:type owl:Class ;
                 rdfs:subClassOf cco:ont00001051 ;
                 rdfs:label "Bow"@en ;
                 skos:definition "A Projectile Launcher that is designed to launch Arrows."@en ;
                 cco:ont00001754 "https://en.wikipedia.org/w/index.php?title=Bow_and_arrow&oldid=1062193194"^^xsd:anyURI ;
                 cco:ont00001760 "https://www.commoncoreontologies.org/ArtifactOntology"^^xsd:anyURI .


###  https://www.commoncoreontologies.org/ont00001378
cco:ont00001378 rdf:type owl:Class ;
                 rdfs:subClassOf cco:ont00001301 ;
                 rdfs:label "Hospitality Artifact Function"@en ;
                 skos:definition "A Service Artifact Function that is realized in processes of accommodation food and beverage meeting and events gaming entertainment and recreation tourism services and visitor information."@en ;
                 cco:ont00001754 "https://en.wikipedia.org/w/index.php?title=Hospitality&oldid=1049599161"^^xsd:anyURI ;
                 cco:ont00001760 "https://www.commoncoreontologies.org/ArtifactOntology"^^xsd:anyURI .


###  https://www.commoncoreontologies.org/ont00001381
cco:ont00001381 rdf:type owl:Class ;
                 rdfs:subClassOf cco:ont00000995 ;
                 rdfs:label "Medical Artifact"@en ;
                 skos:definition "A Material Artifact that is designed for diagnosing, treating, or preventing disease, disability, or death."@en ;
                 cco:ont00001760 "https://www.commoncoreontologies.org/ArtifactOntology"^^xsd:anyURI .


###  https://www.commoncoreontologies.org/ont00001382
cco:ont00001382 rdf:type owl:Class ;
                 rdfs:subClassOf cco:ont00000475 ;
                 rdfs:label "Electronic Cash"@en ;
                 skos:definition "A Portion of Cash that consists of Bytes."@en ;
                 cco:ont00001760 "https://www.commoncoreontologies.org/ArtifactOntology"^^xsd:anyURI .


###  https://www.commoncoreontologies.org/ont00001999
cco:ont00001999 rdf:type owl:Class ;
                 rdfs:subClassOf cco:ont00000323 ;
                 rdfs:comment """Although its basic function remains the same, a Filter can be used in 2 different ways:
(1) to allow only the desired entities to pass through (e.g. removing dirt from engine oil); or
(2) to allow everything except the desired entities to pass through (e.g. panning for gold)."""@en ;
                 rdfs:label "Filter Function"@en ;
                 skos:definition "An Artifact Function that is realized in a process where entities of a specific type or which have specified properties enter it or pass through it."@en ;
                 cco:ont00001760 "https://www.commoncoreontologies.org/ArtifactOntology"^^xsd:anyURI .


###  Generated by the OWL API (version 4.5.29) https://github.com/owlcs/owlapi
