@prefix : <https://www.commoncoreontologies.org/ExtendedRelationOntology#> .
@prefix cco: <http://www.ontologyrepository.com/CommonCoreOntologies/> .
@prefix obo: <http://purl.obolibrary.org/obo/> .
@prefix owl: <http://www.w3.org/2002/07/owl#> .
@prefix rdf: <http://www.w3.org/1999/02/22-rdf-syntax-ns#> .
@prefix xml: <http://www.w3.org/XML/1998/namespace> .
@prefix xsd: <http://www.w3.org/2001/XMLSchema#> .
@prefix cco: <https://www.commoncoreontologies.org/> .
@prefix rdfs: <http://www.w3.org/2000/01/rdf-schema#> .
@prefix skos: <http://www.w3.org/2004/02/skos/core#> .
@prefix dcterms: <http://purl.org/dc/terms/> .
@base <https://www.commoncoreontologies.org/ExtendedRelationOntology> .

<https://www.commoncoreontologies.org/ExtendedRelationOntology> rdf:type owl:Ontology ;
                                                                                       owl:versionIRI <https://www.commoncoreontologies.org/2024-11-06/ExtendedRelationOntology> ;
                                                                                       owl:imports <http://purl.obolibrary.org/obo/bfo/2020/bfo-core.ttl> ;
                                                                                       dcterms:license "BSD 3-Clause: https://github.com/CommonCoreOntology/CommonCoreOntologies/blob/master/LICENSE"@en ;
                                                                                       dcterms:rights "CUBRC Inc., see full license."@en ;
                                                                                       rdfs:comment "This ontology is designed to represent many of the relations (i.e. object properties) that hold between entities at the level of the mid-level Common Core Ontologies."@en ;
                                                                                       rdfs:label "Extended Relation Ontology"@en ;
                                                                                       owl:versionInfo "Version 2.0"@en .

#################################################################
#    Annotation properties
#################################################################

###  http://purl.org/dc/terms/created
dcterms:created rdf:type owl:AnnotationProperty .


###  http://purl.org/dc/terms/creator
dcterms:creator rdf:type owl:AnnotationProperty .


###  http://purl.org/dc/terms/rights
dcterms:rights rdf:type owl:AnnotationProperty .


###  http://www.w3.org/2004/02/skos/core#editorialNote
skos:editorialNote rdf:type owl:AnnotationProperty .


###  https://www.commoncoreontologies.org/ont00001735
cco:ont00001735 rdf:type owl:AnnotationProperty ;
                 rdfs:label "query text"@en ;
                 skos:definition "The text of a query that is associated with a class"@en ;
                 cco:ont00001760 "https://www.commoncoreontologies.org/ExtendedRelationOntology"^^xsd:anyURI .


###  https://www.commoncoreontologies.org/ont00001737
cco:ont00001737 rdf:type owl:AnnotationProperty ;
                 rdfs:label "doctrinal definition"@en ;
                 skos:definition "A Definition that is taken directly from a Doctrinal Source."@en ;
                 skos:scopeNote "There is only one definition for any given term in an ontology; however, a Doctrinal Definition may be provided in addition to the asserted Definition if the preservation of this information is important. When both a Definition and a Doctrinal Definition are provided for a term, the Definition takes precedence."@en ;
                 cco:ont00001760 "https://www.commoncoreontologies.org/ExtendedRelationOntology"^^xsd:anyURI ;
                 rdfs:subPropertyOf skos:definition .


###  https://www.commoncoreontologies.org/ont00001739
cco:ont00001739 rdf:type owl:AnnotationProperty ;
                 rdfs:label "ordinal measurement annotation"@en ;
                 skos:definition "An ordinal measurement value of an instance of a quality, realizable or process profile"@en ;
                 cco:ont00001760 "https://www.commoncoreontologies.org/ExtendedRelationOntology"^^xsd:anyURI ;
                 rdfs:subPropertyOf cco:ont00001746 .


###  https://www.commoncoreontologies.org/ont00001741
cco:ont00001741 rdf:type owl:AnnotationProperty ;
                 rdfs:label "nominal measurement annotation"@en ;
                 skos:definition "A nominal measurement value of an instance of a quality, realizable or process profile"@en ;
                 cco:ont00001760 "https://www.commoncoreontologies.org/ExtendedRelationOntology"^^xsd:anyURI ;
                 rdfs:subPropertyOf cco:ont00001746 .


###  https://www.commoncoreontologies.org/ont00001742
cco:ont00001742 rdf:type owl:AnnotationProperty ;
                 rdfs:label "term creator"@en ;
                 skos:definition "The name of the Term Editor who added the term to the ontology."@en ;
                 cco:ont00001760 "https://www.commoncoreontologies.org/ExtendedRelationOntology"^^xsd:anyURI ;
                 rdfs:subPropertyOf cco:ont00001762 .


###  https://www.commoncoreontologies.org/ont00001743
cco:ont00001743 rdf:type owl:AnnotationProperty ;
                 rdfs:label "content license"@en ;
                 skos:definition "The name and description of the license under which the ideas, concepts and other informational content expressed in the .owl file are released."@en ;
                 cco:ont00001760 "https://www.commoncoreontologies.org/ExtendedRelationOntology"^^xsd:anyURI .


###  https://www.commoncoreontologies.org/ont00001744
cco:ont00001744 rdf:type owl:AnnotationProperty ;
                 rdfs:label "copyright"@en ;
                 skos:definition "An assertion of copyright"@en ;
                 cco:ont00001760 "https://www.commoncoreontologies.org/ExtendedRelationOntology"^^xsd:anyURI .


###  https://www.commoncoreontologies.org/ont00001745
cco:ont00001745 rdf:type owl:AnnotationProperty ;
                 rdfs:label "doctrinal source"@en ;
                 skos:definition "A Definition Source that consists of a formalized doctrine in which the term is authoritatively defined."@en ;
                 cco:ont00001760 "https://www.commoncoreontologies.org/ExtendedRelationOntology"^^xsd:anyURI ;
                 rdfs:subPropertyOf cco:ont00001754 .


###  https://www.commoncoreontologies.org/ont00001746
cco:ont00001746 rdf:type owl:AnnotationProperty ;
                 rdfs:label "measurement annotation"@en ;
                 skos:definition "A measurement value of an instance of a quality, realizable or process profile"@en ;
                 cco:ont00001760 "https://www.commoncoreontologies.org/ExtendedRelationOntology"^^xsd:anyURI .


###  https://www.commoncoreontologies.org/ont00001747
cco:ont00001747 rdf:type owl:AnnotationProperty ;
                 rdfs:label "ratio measurement annotation"@en ;
                 skos:definition "A ratio measurement value of an instance of a quality, realizable or process profile"@en ;
                 cco:ont00001760 "https://www.commoncoreontologies.org/ExtendedRelationOntology"^^xsd:anyURI ;
                 rdfs:subPropertyOf cco:ont00001746 .


###  https://www.commoncoreontologies.org/ont00001748
cco:ont00001748 rdf:type owl:AnnotationProperty ;
                 rdfs:label "doctrinal label"@en ;
                 skos:definition "An Alternative Label that consists of the preferred term or phrase used by a Doctrinal Source to denote the entity."@en ;
                 skos:scopeNote "When the cco:doctrinal_label is identical to the rdfs:label, the cco:doctrinal_label annotation is superfluous. As a subclass of 'alternative label', 'doctrinal label' is intended to be used to provide additional information about the entity when its preferred doctrinal designator is ambiguous or otherwise inappropriate for use as the rdfs:label."@en ;
                 cco:ont00001760 "https://www.commoncoreontologies.org/ExtendedRelationOntology"^^xsd:anyURI ;
                 rdfs:subPropertyOf skos:altLabel .


###  https://www.commoncoreontologies.org/ont00001749
cco:ont00001749 rdf:type owl:AnnotationProperty ;
                 rdfs:label "doctrinal acronym"@en ;
                 skos:definition "An Acronym that is used by a Doctrinal Source to denote the entity."@en ;
                 cco:ont00001760 "https://www.commoncoreontologies.org/ExtendedRelationOntology"^^xsd:anyURI ;
                 rdfs:subPropertyOf cco:ont00001753 .


###  https://www.commoncoreontologies.org/ont00001752
cco:ont00001752 rdf:type owl:AnnotationProperty ;
                 rdfs:label "has token unit"@en ;
                 skos:definition "A relation between an information content entity and a widely used measurement unit of the token used to express it."@en ;
                 cco:ont00001760 "https://www.commoncoreontologies.org/ExtendedRelationOntology"^^xsd:anyURI .


###  https://www.commoncoreontologies.org/ont00001753
cco:ont00001753 rdf:type owl:AnnotationProperty ;
                 rdfs:label "acronym"@en ;
                 skos:definition "An Alternative Label that consists of a shortened or abbreviated form of the rdfs:label and is used to denote the entity."@en ;
                 cco:ont00001760 "https://www.commoncoreontologies.org/ExtendedRelationOntology"^^xsd:anyURI ;
                 rdfs:subPropertyOf skos:altLabel .


###  https://www.commoncoreontologies.org/ont00001754
cco:ont00001754 rdf:type owl:AnnotationProperty ;
                 rdfs:label "definition source"@en ;
                 skos:definition "A citation of where all or some of the information used to create the term's Definition was acquired from."@en ;
                 cco:ont00001760 "https://www.commoncoreontologies.org/ExtendedRelationOntology"^^xsd:anyURI .


###  https://www.commoncoreontologies.org/ont00001756
cco:ont00001756 rdf:type owl:AnnotationProperty ;
                 rdfs:label "interval measurement annotation"@en ;
                 skos:definition "A interval measurement value of an instance of a quality, realizable or process profile "@en ;
                 cco:ont00001760 "https://www.commoncoreontologies.org/ExtendedRelationOntology"^^xsd:anyURI ;
                 rdfs:subPropertyOf cco:ont00001746 .


###  https://www.commoncoreontologies.org/ont00001757
cco:ont00001757 rdf:type owl:AnnotationProperty ;
                 rdfs:label "designator annotation"@en ;
                 skos:definition "A name or other identifier that is used to designate an individual."@en ;
                 cco:ont00001760 "https://www.commoncoreontologies.org/ExtendedRelationOntology"^^xsd:anyURI .


###  https://www.commoncoreontologies.org/ont00001758
cco:ont00001758 rdf:type owl:AnnotationProperty ;
                 rdfs:label "http query string"@en ;
                 skos:definition "The text of an HTTP request that can be sent to a SPARQL Protocol service."@en ;
                 cco:ont00001760 "https://www.commoncoreontologies.org/ExtendedRelationOntology"^^xsd:anyURI .


###  https://www.commoncoreontologies.org/ont00001759
cco:ont00001759 rdf:type owl:AnnotationProperty ;
                 rdfs:label "code license"@en ;
                 skos:definition "The name and description of the license under which the .owl file is released."@en ;
                 cco:ont00001760 "https://www.commoncoreontologies.org/ExtendedRelationOntology"^^xsd:anyURI .


###  https://www.commoncoreontologies.org/ont00001760
cco:ont00001760 rdf:type owl:AnnotationProperty ;
                 rdfs:label "is curated in ontology"@en ;
                 skos:definition "An annotation property that links a class, property, or named individual to the URI of the ontology where it is located."@en ;
                 cco:ont00001760 "https://www.commoncoreontologies.org/ExtendedRelationOntology"^^xsd:anyURI .


###  https://www.commoncoreontologies.org/ont00001761
cco:ont00001761 rdf:type owl:AnnotationProperty ;
                 rdfs:label "is tokenized by"@en ;
                 skos:definition "A relation between an information content entity and a widely used token used to express it."@en ;
                 cco:ont00001760 "https://www.commoncoreontologies.org/ExtendedRelationOntology"^^xsd:anyURI .


###  https://www.commoncoreontologies.org/ont00001762
cco:ont00001762 rdf:type owl:AnnotationProperty ;
                 rdfs:label "term editor"@en ;
                 skos:definition "The name of a person who contributed to the development or enhancement of the term."@en ;
                 cco:ont00001760 "https://www.commoncoreontologies.org/ExtendedRelationOntology"^^xsd:anyURI .


#################################################################
#    Object Properties
#################################################################

###  http://purl.obolibrary.org/obo/BFO_0000199
obo:BFO_0000199 owl:inverseOf cco:ont00001874 .


###  https://www.commoncoreontologies.org/ont00001775
cco:ont00001775 rdf:type owl:ObjectProperty ;
                 owl:inverseOf cco:ont00001928 ;
                 rdfs:domain obo:BFO_0000004 ;
                 rdfs:range obo:BFO_0000004 ;
                 rdfs:label "is successor of"@en ;
                 skos:definition "A continuant c2 is a successor of some continuant c1 iff there is some process p1 and c1 is an input to p1 and c2 is an output of p1. Inverse of is predecessor. "@en ;
                 cco:ont00001760 "https://www.commoncoreontologies.org/ExtendedRelationOntology"^^xsd:anyURI .


###  https://www.commoncoreontologies.org/ont00001777
cco:ont00001777 rdf:type owl:ObjectProperty ;
                 rdfs:subPropertyOf obo:BFO_0000117 ;
                 owl:inverseOf cco:ont00001857 ;
                 rdfs:domain obo:BFO_0000015 ;
                 rdfs:range obo:BFO_0000015 ;
                 rdfs:label "has process part"@en ;
                 skos:definition "x has_process_part y iff x and y are instances of Process, such that y occurs during the temporal interval of x, and y either provides an input to x or receives an output of x, or both."@en ;
                 cco:ont00001760 "https://www.commoncoreontologies.org/ExtendedRelationOntology"^^xsd:anyURI .


###  https://www.commoncoreontologies.org/ont00001778
cco:ont00001778 rdf:type owl:ObjectProperty ;
                 rdfs:subPropertyOf obo:BFO_0000057 ;
                 owl:inverseOf cco:ont00001936 ;
                 rdfs:label "has object"@en ;
                 skos:definition "If p is a process and c is a continuant, then p has object c if and only if p is performed by an agent and c is part of the projected state that agent intends to achieve by performing p."@en ;
                 cco:ont00001760 "https://www.commoncoreontologies.org/ExtendedRelationOntology"^^xsd:anyURI .


###  https://www.commoncoreontologies.org/ont00001782
cco:ont00001782 rdf:type owl:ObjectProperty ;
                 rdfs:subPropertyOf cco:ont00001832 ;
                 rdfs:domain obo:BFO_0000027 ;
                 rdfs:range [ owl:intersectionOf ( obo:BFO_0000004
                                                   [ rdf:type owl:Class ;
                                                     owl:complementOf obo:BFO_0000006
                                                   ]
                                                 ) ;
                              rdf:type owl:Class
                            ] ;
                 rdfs:label "has all members located in"@en ;
                 skos:definition "x has all members located in y iff x is an instance of Object Aggregate and y is an instance of independent continuant but not a spatial region, and every member of x is located in y."@en ;
                 cco:ont00001760 "https://www.commoncoreontologies.org/ExtendedRelationOntology"^^xsd:anyURI .


###  https://www.commoncoreontologies.org/ont00001799
cco:ont00001799 rdf:type owl:ObjectProperty ;
                 rdfs:subPropertyOf cco:ont00001809 ;
                 rdfs:domain obo:BFO_0000023 ;
                 rdfs:range obo:BFO_0000027 ;
                 rdfs:label "role of aggregate"@en ;
                 skos:definition "x role_of_aggregate y iff y is an instance of Object Aggregate and x is an instance of Role, and x inheres_in_aggregate y."@en ;
                 cco:ont00001760 "https://www.commoncoreontologies.org/ExtendedRelationOntology"^^xsd:anyURI .


###  https://www.commoncoreontologies.org/ont00001803
cco:ont00001803 rdf:type owl:ObjectProperty ;
                 owl:inverseOf cco:ont00001819 ;
                 rdfs:domain obo:BFO_0000003 ;
                 rdfs:range obo:BFO_0000003 ;
                 rdfs:label "is cause of"@en ;
                 skos:definition "x is_cause_of y iff x and y are instances of Occurrent, and y is a consequence of x."@en ;
                 cco:ont00001760 "https://www.commoncoreontologies.org/ExtendedRelationOntology"^^xsd:anyURI .


###  https://www.commoncoreontologies.org/ont00001805
cco:ont00001805 rdf:type owl:ObjectProperty ;
                 owl:inverseOf cco:ont00001888 ;
                 rdfs:domain obo:BFO_0000015 ;
                 rdfs:range obo:BFO_0000015 ;
                 dcterms:created "2022-12-30T21:32:27-05:00"^^xsd:dateTime ;
                 dcterms:creator "https://cubrc.org"^^xsd:anyURI ;
                 rdfs:label "is disrupted by"@en ;
                 skos:definition "Inverse of disrupts." ;
                 skos:prefLabel "is disrupted by"@en ;
                 cco:ont00001760 "https://www.commoncoreontologies.org/ExtendedRelationOntology"^^xsd:anyURI .


###  https://www.commoncoreontologies.org/ont00001809
cco:ont00001809 rdf:type owl:ObjectProperty ;
                 owl:inverseOf cco:ont00001836 ;
                 rdfs:domain [ rdf:type owl:Class ;
                               owl:unionOf ( obo:BFO_0000020
                                             obo:BFO_0000031
                                           )
                             ] ;
                 rdfs:range obo:BFO_0000027 ;
                 rdfs:label "inheres in aggregate"@en ;
                 skos:definition "x inheres_in_aggregate y iff x is an instance of Specifically Dependent Continuant and y is an instance of Object Aggregate and z is an instance of Object, such that z bearer_of x, and all other members of y are bearers of a unique instance of the same type as x."@en ;
                 cco:ont00001760 "https://www.commoncoreontologies.org/ExtendedRelationOntology"^^xsd:anyURI .


###  https://www.commoncoreontologies.org/ont00001816
cco:ont00001816 rdf:type owl:ObjectProperty ;
                 rdfs:subPropertyOf obo:BFO_0000056 ;
                 owl:inverseOf cco:ont00001986 ;
                 rdfs:domain obo:BFO_0000002 ;
                 rdfs:range obo:BFO_0000015 ;
                 rdfs:label "is output of"@en ;
                 skos:definition "x is_output_of y iff x is an instance of Continuant and y is an instance of Process, such that the presence of x at the end of y is a necessary condition for the completion of y."@en ;
                 cco:ont00001760 "https://www.commoncoreontologies.org/ExtendedRelationOntology"^^xsd:anyURI .


###  https://www.commoncoreontologies.org/ont00001819
cco:ont00001819 rdf:type owl:ObjectProperty ;
                 rdfs:domain obo:BFO_0000003 ;
                 rdfs:range obo:BFO_0000003 ;
                 rdfs:label "caused by"@en ;
                 skos:definition "x caused_by y iff x and y are instances of Occurrent, and x is a consequence of y."@en ;
                 cco:ont00001760 "https://www.commoncoreontologies.org/ExtendedRelationOntology"^^xsd:anyURI .


###  https://www.commoncoreontologies.org/ont00001829
cco:ont00001829 rdf:type owl:ObjectProperty ;
                 rdfs:subPropertyOf cco:ont00001809 ;
                 owl:inverseOf cco:ont00001956 ;
                 rdfs:domain obo:BFO_0000016 ;
                 rdfs:range obo:BFO_0000027 ;
                 rdfs:label "disposition of aggregate"@en ;
                 skos:definition "x disposition_of_aggregate y iff y is an instance of Object Aggregate and x is an instance of Disposition, and x inheres_in_aggregate y."@en ;
                 cco:ont00001760 "https://www.commoncoreontologies.org/ExtendedRelationOntology"^^xsd:anyURI .


###  https://www.commoncoreontologies.org/ont00001830
cco:ont00001830 rdf:type owl:ObjectProperty ;
                 rdfs:subPropertyOf obo:BFO_0000057 ;
                 owl:inverseOf cco:ont00001895 ;
                 rdfs:domain obo:BFO_0000015 ;
                 rdfs:range obo:BFO_0000040 ;
                 rdfs:label "has accomplice"@en ;
                 skos:definition "A Processual Entity p1 has_accomplice some agent a1 iff a1 assists in the commission of p1, is located at the location of p1, but is not agent_in p1."@en ;
                 cco:ont00001754 "https://en.wikipedia.org/w/index.php?title=Accomplice&oldid=1002047204"^^xsd:anyURI ;
                 cco:ont00001760 "https://www.commoncoreontologies.org/ExtendedRelationOntology"^^xsd:anyURI .


###  https://www.commoncoreontologies.org/ont00001832
cco:ont00001832 rdf:type owl:ObjectProperty ;
                 rdfs:subPropertyOf owl:topObjectProperty ;
                 rdfs:domain obo:BFO_0000027 ;
                 rdfs:range [ owl:intersectionOf ( obo:BFO_0000004
                                                   [ rdf:type owl:Class ;
                                                     owl:complementOf obo:BFO_0000006
                                                   ]
                                                 ) ;
                              rdf:type owl:Class
                            ] ;
                 rdfs:label "has some member located in"@en ;
                 skos:definition "x has some member located in y iff x is an instance of Object Aggregate and y is an instance of independent continuant but not a spatial region, and at least one member of x is located in y."@en ;
                 cco:ont00001760 "https://www.commoncoreontologies.org/ExtendedRelationOntology"^^xsd:anyURI .


###  https://www.commoncoreontologies.org/ont00001834
cco:ont00001834 rdf:type owl:ObjectProperty ;
                 rdfs:subPropertyOf obo:BFO_0000057 ;
                 owl:inverseOf cco:ont00001886 ;
                 rdfs:domain obo:BFO_0000015 ;
                 rdfs:range obo:BFO_0000002 ;
                 rdfs:label "affects"@en ;
                 skos:definition "x affects y iff x is an instance of Process and y is an instance of Continuant, and x influences y in some manner, most often by producing a change in y."@en ;
                 cco:ont00001760 "https://www.commoncoreontologies.org/ExtendedRelationOntology"^^xsd:anyURI .


###  https://www.commoncoreontologies.org/ont00001836
cco:ont00001836 rdf:type owl:ObjectProperty ;
                 rdfs:domain obo:BFO_0000027 ;
                 rdfs:range [ rdf:type owl:Class ;
                              owl:unionOf ( obo:BFO_0000020
                                            obo:BFO_0000031
                                          )
                            ] ;
                 rdfs:label "aggregate bearer of"@en ;
                 skos:definition "x aggregate_bearer_of y iff x is an instance of Object Aggregate and y is an instance of Specifically Dependent Continuant and z is an instance of Object, such that z bearer of y, and all other members of x are bearers of a unique instance of the same type as y."@en ;
                 cco:ont00001760 "https://www.commoncoreontologies.org/ExtendedRelationOntology"^^xsd:anyURI .


###  https://www.commoncoreontologies.org/ont00001841
cco:ont00001841 rdf:type owl:ObjectProperty ;
                 rdfs:subPropertyOf obo:BFO_0000056 ;
                 owl:inverseOf cco:ont00001921 ;
                 rdfs:domain obo:BFO_0000002 ;
                 rdfs:range obo:BFO_0000015 ;
                 rdfs:label "is input of"@en ;
                 skos:definition "x is_input_of y iff x is an instance of Continuant and y is an instance of Process, such that the presence of x at the beginning of y is a necessary condition for the start of y."@en ;
                 cco:ont00001760 "https://www.commoncoreontologies.org/ExtendedRelationOntology"^^xsd:anyURI .


###  https://www.commoncoreontologies.org/ont00001845
cco:ont00001845 rdf:type owl:ObjectProperty ;
                 rdfs:subPropertyOf obo:BFO_0000183 ;
                 owl:inverseOf cco:ont00001918 ;
                 rdfs:domain obo:BFO_0000029 ;
                 rdfs:range obo:BFO_0000015 ;
                 rdfs:label "is site of"@en ;
                 skos:definition "x is_site_of y iff x is an instance of Site and y is an instance of Process, such that y occurs in x."@en ;
                 cco:ont00001760 "https://www.commoncoreontologies.org/ExtendedRelationOntology"^^xsd:anyURI .


###  https://www.commoncoreontologies.org/ont00001852
cco:ont00001852 rdf:type owl:ObjectProperty ;
                 rdfs:subPropertyOf obo:BFO_0000056 ;
                 owl:inverseOf cco:ont00001949 ;
                 rdfs:domain obo:BFO_0000040 ;
                 rdfs:range obo:BFO_0000015 ;
                 rdfs:label "accessory in"@en ;
                 skos:definition "y is_accessory_in x iff x is an instance of Process and y is an instance of Agent, such that y assists another agent in the commission of x, and y was not located at the location of x when x occurred, and y was not an agent_in x."@en ;
                 cco:ont00001754 "http://en.wikipedia.org/wiki/Accessory_(legal_term)" ;
                 cco:ont00001760 "https://www.commoncoreontologies.org/ExtendedRelationOntology"^^xsd:anyURI .


###  https://www.commoncoreontologies.org/ont00001857
cco:ont00001857 rdf:type owl:ObjectProperty ;
                 rdfs:subPropertyOf obo:BFO_0000132 ;
                 rdfs:domain obo:BFO_0000015 ;
                 rdfs:range obo:BFO_0000015 ;
                 rdfs:label "is part of process"@en ;
                 skos:definition "x is_part_of_process y iff x and y are instances of Process, such that x occurs during the temporal interval of y, and x either provides an input to y or receives an output of y."@en ;
                 cco:ont00001760 "https://www.commoncoreontologies.org/ExtendedRelationOntology"^^xsd:anyURI .


###  https://www.commoncoreontologies.org/ont00001861
cco:ont00001861 rdf:type owl:ObjectProperty ;
                 owl:inverseOf cco:ont00001991 ;
                 rdfs:domain obo:BFO_0000030 ;
                 rdfs:range obo:BFO_0000030 ;
                 rdfs:label "is material of"@en ;
                 skos:definition "An object m is material of an object o when m is the material of which o consists and that material does not undergo a change of kind during the creation of o"@en ;
                 cco:ont00001760 "https://www.commoncoreontologies.org/ExtendedRelationOntology"^^xsd:anyURI .


###  https://www.commoncoreontologies.org/ont00001874
cco:ont00001874 rdf:type owl:ObjectProperty ;
                 rdfs:domain obo:BFO_0000008 ;
                 rdfs:range [ rdf:type owl:Class ;
                              owl:unionOf ( obo:BFO_0000015
                                            obo:BFO_0000035
                                          )
                            ] ;
                 rdfs:label "is temporal region of"@en ;
                 skos:definition "t is temporal region of p iff p occupies temporal region t."@en ;
                 skos:editorialNote "Leaving this is in ERO for now since BFO2020 has no inverse of occupies-temporal-region yet."@en ;
                 cco:ont00001760 "https://www.commoncoreontologies.org/ExtendedRelationOntology"^^xsd:anyURI .


###  https://www.commoncoreontologies.org/ont00001886
cco:ont00001886 rdf:type owl:ObjectProperty ;
                 rdfs:subPropertyOf obo:BFO_0000056 ;
                 rdfs:domain obo:BFO_0000002 ;
                 rdfs:range obo:BFO_0000015 ;
                 rdfs:label "is affected by"@en ;
                 skos:definition "x is_affected_by y iff x is an instance of Continuant and y is an instance of Process, and y influences x in some manner, most often by producing a change in x."@en ;
                 cco:ont00001760 "https://www.commoncoreontologies.org/ExtendedRelationOntology"^^xsd:anyURI .


###  https://www.commoncoreontologies.org/ont00001888
cco:ont00001888 rdf:type owl:ObjectProperty ;
                 rdfs:domain obo:BFO_0000015 ;
                 rdfs:range obo:BFO_0000015 ;
                 dcterms:created "2022-12-30T21:32:27-05:00"^^xsd:dateTime ;
                 dcterms:creator "https://cubrc.org"^^xsd:anyURI ;
                 rdfs:label "disrupts"@en ;
                 skos:definition "A relation where one process disrupts another process from occurring as it would have."@en ;
                 skos:editorialNote "To lower the grade of a process is to lower the quality of a process according to some standard, for example when realizing a capability or a function."@en ;
                 skos:prefLabel "disrupts"@en ;
                 skos:scopeNote "A process can disrupt another process from occurring as it would have by 1) preventing a disposition or role from being realized by that process, 2) lowering the grade of the process, or 3) stopping the process from continuing to occur."@en ;
                 cco:ont00001760 "https://www.commoncoreontologies.org/ExtendedRelationOntology"^^xsd:anyURI .


###  https://www.commoncoreontologies.org/ont00001895
cco:ont00001895 rdf:type owl:ObjectProperty ;
                 rdfs:subPropertyOf obo:BFO_0000056 ;
                 rdfs:domain obo:BFO_0000040 ;
                 rdfs:range obo:BFO_0000015 ;
                 rdfs:label "accomplice in"@en ;
                 skos:definition "An agent a1 is accomplice_in some Processual Entity p1 iff a1 assists in the commission of p1, is located at the location of p1, but is not agent_in p1."@en ;
                 cco:ont00001754 "https://en.wikipedia.org/w/index.php?title=Accomplice&oldid=1002047204"^^xsd:anyURI ;
                 cco:ont00001760 "https://www.commoncoreontologies.org/ExtendedRelationOntology"^^xsd:anyURI .


###  https://www.commoncoreontologies.org/ont00001901
cco:ont00001901 rdf:type owl:ObjectProperty ;
                 rdfs:subPropertyOf cco:ont00001836 ;
                 rdfs:domain obo:BFO_0000027 ;
                 rdfs:range obo:BFO_0000023 ;
                 rdfs:label "aggregate has role"@en ;
                 skos:definition "x aggregate_has_role y iff x is an instance of Object Aggregate and y is an instance of Role, such that x aggregate_bearer_of y."@en ;
                 cco:ont00001760 "https://www.commoncoreontologies.org/ExtendedRelationOntology"^^xsd:anyURI .


###  https://www.commoncoreontologies.org/ont00001907
cco:ont00001907 rdf:type owl:ObjectProperty ;
                 rdfs:subPropertyOf cco:ont00001836 ;
                 rdfs:domain obo:BFO_0000027 ;
                 rdfs:range obo:BFO_0000019 ;
                 rdfs:label "aggregate has quality"@en ;
                 skos:definition "x aggregate_has_quality y iff x is an instance of Object Aggregate and y is an instance of Quality, such that x aggregate_bearer_of y."@en ;
                 cco:ont00001760 "https://www.commoncoreontologies.org/ExtendedRelationOntology"^^xsd:anyURI .


###  https://www.commoncoreontologies.org/ont00001918
cco:ont00001918 rdf:type owl:ObjectProperty ;
                 rdfs:subPropertyOf obo:BFO_0000066 ;
                 rdfs:domain obo:BFO_0000015 ;
                 rdfs:range obo:BFO_0000029 ;
                 rdfs:label "occurs at"@en ;
                 skos:definition "x occurs_at y iff x is an instance of Process and y is an instance of Site, such that x occurs in y."@en ;
                 cco:ont00001760 "https://www.commoncoreontologies.org/ExtendedRelationOntology"^^xsd:anyURI .


###  https://www.commoncoreontologies.org/ont00001921
cco:ont00001921 rdf:type owl:ObjectProperty ;
                 rdfs:subPropertyOf obo:BFO_0000057 ;
                 rdfs:domain obo:BFO_0000015 ;
                 rdfs:range obo:BFO_0000002 ;
                 rdfs:label "has input"@en ;
                 skos:definition "y has_input x iff x is an instance of Continuant and y is an instance of Process, such that the presence of x at the beginning of y is a necessary condition for the start of y."@en ;
                 cco:ont00001760 "https://www.commoncoreontologies.org/ExtendedRelationOntology"^^xsd:anyURI .


###  https://www.commoncoreontologies.org/ont00001928
cco:ont00001928 rdf:type owl:ObjectProperty ;
                 rdfs:domain obo:BFO_0000004 ;
                 rdfs:range obo:BFO_0000004 ;
                 rdfs:label "is predecessor of"@en ;
                 skos:definition "A continuant c1 is a predecessor of some continuant c2 iff there is some process p1 and c1 is an input to p1 and c2 is an output of p1."@en ;
                 skos:scopeNote "More informally, c1 is a predecessor of c2 iff c1 has been followed or replaced by c2."@en ;
                 cco:ont00001760 "https://www.commoncoreontologies.org/ExtendedRelationOntology"^^xsd:anyURI .


###  https://www.commoncoreontologies.org/ont00001933
cco:ont00001933 rdf:type owl:ObjectProperty ;
                 rdfs:subPropertyOf cco:ont00001803 ;
                 owl:inverseOf cco:ont00001962 ;
                 rdfs:label "process starts"@en ;
                 skos:definition "x process_starts y iff x and y are instances of processes, and x is_cause_of y, and i is an instance of a temporal instant, and r is an instant of a temporal interval, and y has starting instance i, and x occurs on r, and r interval contains i."@en ;
                 skos:scopeNote "A process x starts another process y when x causes y while x is still occurring."@en ;
                 cco:ont00001760 "https://www.commoncoreontologies.org/ExtendedRelationOntology"^^xsd:anyURI .


###  https://www.commoncoreontologies.org/ont00001936
cco:ont00001936 rdf:type owl:ObjectProperty ;
                 rdfs:subPropertyOf obo:BFO_0000056 ;
                 rdfs:label "is object of"@en ;
                 skos:definition "If p is a process and c is a continuant, then c is object of p if and only if the c is part of the projected state that the agent intends to achieve by performing p."@en ;
                 cco:ont00001760 "https://www.commoncoreontologies.org/ExtendedRelationOntology"^^xsd:anyURI .


###  https://www.commoncoreontologies.org/ont00001947
cco:ont00001947 rdf:type owl:ObjectProperty ;
                 rdfs:subPropertyOf cco:ont00001809 ;
                 rdfs:domain obo:BFO_0000019 ;
                 rdfs:range obo:BFO_0000027 ;
                 rdfs:label "quality of aggregate"@en ;
                 skos:definition "x quality_of_aggregate y iff y is an instance of Object Aggregate and x is an instance of Quality, and x inheres_in_aggregate y."@en ;
                 cco:ont00001760 "https://www.commoncoreontologies.org/ExtendedRelationOntology"^^xsd:anyURI .


###  https://www.commoncoreontologies.org/ont00001949
cco:ont00001949 rdf:type owl:ObjectProperty ;
                 rdfs:subPropertyOf obo:BFO_0000057 ;
                 rdfs:domain obo:BFO_0000015 ;
                 rdfs:range obo:BFO_0000040 ;
                 rdfs:label "has accessory"@en ;
                 skos:definition "x has_accessory y iff x is an instance of Process and y is an instance of Agent, such that y assists another agent in the commission of x, and y was not located at the location of x when x occurred, and y was not an agent_in x."@en ;
                 cco:ont00001754 "http://en.wikipedia.org/wiki/Accessory_(legal_term)" ;
                 cco:ont00001760 "https://www.commoncoreontologies.org/ExtendedRelationOntology"^^xsd:anyURI .


###  https://www.commoncoreontologies.org/ont00001956
cco:ont00001956 rdf:type owl:ObjectProperty ;
                 rdfs:subPropertyOf cco:ont00001836 ;
                 rdfs:domain obo:BFO_0000027 ;
                 rdfs:range obo:BFO_0000016 ;
                 rdfs:label "aggregate has disposition"@en ;
                 skos:definition "x aggregate_has_disposition y iff x is an instance of Object Aggregate and y is an instance of Disposition, such that x aggregate_bearer_of y."@en ;
                 cco:ont00001760 "https://www.commoncoreontologies.org/ExtendedRelationOntology"^^xsd:anyURI .


###  https://www.commoncoreontologies.org/ont00001959
cco:ont00001959 rdf:type owl:ObjectProperty ;
                 owl:inverseOf cco:ont00001970 ;
                 rdfs:domain obo:BFO_0000015 ;
                 rdfs:range obo:BFO_0000015 ;
                 rdfs:label "inhibits"@en ;
                 skos:definition "x inhibits y iff x and y are non-identical Processes, d is a Decrease of Realizable Entity, and x is_cause_of d, and r is a Realizable Entity, and d has_participant r, and r realized_in y."@en ;
                 cco:ont00001760 "https://www.commoncoreontologies.org/ExtendedRelationOntology"^^xsd:anyURI .


###  https://www.commoncoreontologies.org/ont00001962
cco:ont00001962 rdf:type owl:ObjectProperty ;
                 rdfs:subPropertyOf cco:ont00001819 ;
                 rdfs:label "process started by"@en ;
                 skos:definition "x process_started_by y iff x and y are instances of processes, and x is caused_by y, and i is an instance of a temporal instant, and r is an instant of a temporal interval, and x has starting instance i, and y occurs on r, and r interval contains i."@en ;
                 skos:scopeNote "A process x is started by another process y when y causes x while y is still occurring."@en ;
                 cco:ont00001760 "https://www.commoncoreontologies.org/ExtendedRelationOntology"^^xsd:anyURI .


###  https://www.commoncoreontologies.org/ont00001970
cco:ont00001970 rdf:type owl:ObjectProperty ;
                 rdfs:domain obo:BFO_0000015 ;
                 rdfs:range obo:BFO_0000015 ;
                 rdfs:label "inhibited by"@en ;
                 skos:definition "y inhibited_by x iff x and y are non-identical Processes, d is a Decrease of Realizable Entity, and x is_cause_of d, and r is a Realizable Entity, and d has_participant r, and r realized_in y."@en ;
                 cco:ont00001760 "https://www.commoncoreontologies.org/ExtendedRelationOntology"^^xsd:anyURI .


###  https://www.commoncoreontologies.org/ont00001986
cco:ont00001986 rdf:type owl:ObjectProperty ;
                 rdfs:subPropertyOf obo:BFO_0000057 ;
                 rdfs:domain obo:BFO_0000015 ;
                 rdfs:range obo:BFO_0000002 ;
                 rdfs:label "has output"@en ;
                 skos:definition "y has_output x iff x is an instance of Continuant and y is an instance of Process, such that the presence of x at the end of y is a necessary condition for the completion of y."@en ;
                 cco:ont00001754 "https://en.wikipedia.org/w/index.php?title=IPO_model&oldid=1024398398"^^xsd:anyURI ;
                 cco:ont00001760 "https://www.commoncoreontologies.org/ExtendedRelationOntology"^^xsd:anyURI .


###  https://www.commoncoreontologies.org/ont00001991
cco:ont00001991 rdf:type owl:ObjectProperty ;
                 rdfs:subPropertyOf owl:topObjectProperty ;
                 rdfs:domain obo:BFO_0000030 ;
                 rdfs:range obo:BFO_0000030 ;
                 rdfs:label "is made of"@en ;
                 skos:definition "An object o is made of an object m when m is the material that o consists of and that material does not undergo a change of kind during the creation of o"@en ;
                 cco:ont00001760 "https://www.commoncoreontologies.org/ExtendedRelationOntology"^^xsd:anyURI .


###  Generated by the OWL API (version 4.5.29) https://github.com/owlcs/owlapi
