@prefix : <http://www.ontologyrepository.com/CommonCoreOntologies/Mid/FacilityOntology#> .
@prefix cco: <http://www.ontologyrepository.com/CommonCoreOntologies/> .
@prefix obo: <http://purl.obolibrary.org/obo/> .
@prefix owl: <http://www.w3.org/2002/07/owl#> .
@prefix rdf: <http://www.w3.org/1999/02/22-rdf-syntax-ns#> .
@prefix xml: <http://www.w3.org/XML/1998/namespace> .
@prefix xsd: <http://www.w3.org/2001/XMLSchema#> .
@prefix rdfs: <http://www.w3.org/2000/01/rdf-schema#> .
@prefix dcterms: <http://purl.org/dc/terms/> .
@base <http://www.ontologyrepository.com/CommonCoreOntologies/Mid/FacilityOntology> .

<http://www.ontologyrepository.com/CommonCoreOntologies/Mid/FacilityOntology> rdf:type owl:Ontology ;
                                                                               owl:versionIRI <http://www.ontologyrepository.com/CommonCoreOntologies/Mid/2024-09-26/FacilityOntology> ;
                                                                               owl:imports <http://www.ontologyrepository.com/CommonCoreOntologies/Mid/ArtifactOntology> ;
                                                                               dcterms:license "BSD 3-Clause: https://github.com/CommonCoreOntology/CommonCoreOntologies/blob/master/LICENSE"@en ;
                                                                               dcterms:rights "CUBRC Inc., see full license."@en ;
                                                                               rdfs:comment "This ontology is designed to represent buildings and campuses that  are designed to serve some specific purpose and which are common to multiple domains."@en ;
                                                                               rdfs:label "Facility Ontology"@en ;
                                                                               owl:versionInfo "Version 1.6"@en .

#################################################################
#    Annotation properties
#################################################################

###  http://purl.org/dc/terms/rights
dcterms:rights rdf:type owl:AnnotationProperty .


#################################################################
#    Classes
#################################################################

###  http://www.ontologyrepository.com/CommonCoreOntologies/AgriculturalFacility
cco:AgriculturalFacility rdf:type owl:Class ;
                         rdfs:subClassOf cco:Facility ;
                         cco:definition_source "https://en.wikipedia.org/w/index.php?title=Agriculture&oldid=1063222666"^^xsd:anyURI ;
                         cco:is_curated_in_ontology "http://www.ontologyrepository.com/CommonCoreOntologies/Mid/FacilityOntology"^^xsd:anyURI ;
                         rdfs:label "Agricultural Facility"@en ;
                         <http://www.w3.org/2004/02/skos/core#definition> "A Facility that is designed as a building or campus for agricultural processes with the aim of cultivating animals, plants, or fungi for food, fiber, biofuel, medicinal plants, or other products to sustain and enhance human life."@en .


###  http://www.ontologyrepository.com/CommonCoreOntologies/AircraftManufacturingFacility
cco:AircraftManufacturingFacility rdf:type owl:Class ;
                                  rdfs:subClassOf cco:Factory ;
                                  cco:definition_source "https://en.wikipedia.org/w/index.php?title=Aerospace_manufacturer&oldid=1059223410"^^xsd:anyURI ;
                                  cco:is_curated_in_ontology "http://www.ontologyrepository.com/CommonCoreOntologies/Mid/FacilityOntology"^^xsd:anyURI ;
                                  rdfs:label "Aircraft Manufacturing Facility"@en ;
                                  <http://www.w3.org/2004/02/skos/core#definition> "A Factory that is designed to manufacture Aircraft."@en .


###  http://www.ontologyrepository.com/CommonCoreOntologies/Airport
cco:Airport rdf:type owl:Class ;
            rdfs:subClassOf cco:TransportationFacility ;
            cco:definition_source "https://en.wikipedia.org/w/index.php?title=Airport&oldid=1063243963"^^xsd:anyURI ;
            cco:is_curated_in_ontology "http://www.ontologyrepository.com/CommonCoreOntologies/Mid/FacilityOntology"^^xsd:anyURI ;
            rdfs:label "Airport"@en ;
            <http://www.w3.org/2004/02/skos/core#definition> "A Transportation Facility that is designed for launching, receiving, and housing Aircraft."@en .


###  http://www.ontologyrepository.com/CommonCoreOntologies/AmmunitionDepot
cco:AmmunitionDepot rdf:type owl:Class ;
                    rdfs:subClassOf cco:StorageFacility ;
                    cco:definition_source "https://en.wikipedia.org/w/index.php?title=Ammunition_dump&oldid=1044466765"^^xsd:anyURI ;
                    cco:is_curated_in_ontology "http://www.ontologyrepository.com/CommonCoreOntologies/Mid/FacilityOntology"^^xsd:anyURI ;
                    rdfs:label "Ammunition Depot"@en ;
                    <http://www.w3.org/2004/02/skos/core#definition> "A Storage Facility that is designed to store Portions of Ammunition."@en .


###  http://www.ontologyrepository.com/CommonCoreOntologies/ApartmentBuilding
cco:ApartmentBuilding rdf:type owl:Class ;
                      rdfs:subClassOf cco:ResidentialFacility ;
                      cco:definition_source "https://en.wikipedia.org/w/index.php?title=Apartment&oldid=1064019048"^^xsd:anyURI ;
                      cco:is_curated_in_ontology "http://www.ontologyrepository.com/CommonCoreOntologies/Mid/FacilityOntology"^^xsd:anyURI ;
                      rdfs:label "Apartment Building"@en ;
                      <http://www.w3.org/2004/02/skos/core#definition> "A Residential Facility that is designed to contain multiple permanent residences comprised of a suite of rooms."@en .


###  http://www.ontologyrepository.com/CommonCoreOntologies/BaseOfOperations
cco:BaseOfOperations rdf:type owl:Class ;
                     rdfs:subClassOf cco:MilitaryBase ;
                     cco:acronym "MOB" ;
                     cco:definition_source "http://www.jcs.mil/Portals/36/Documents/Doctrine/pubs/dictionary.pdf?ver=2018-08-27-122235-653" ;
                     cco:is_curated_in_ontology "http://www.ontologyrepository.com/CommonCoreOntologies/Mid/FacilityOntology"^^xsd:anyURI ;
                     rdfs:label "Base of Operations"@en ;
                     <http://www.w3.org/2004/02/skos/core#altLabel> "Main Operating Base"@en ;
                     <http://www.w3.org/2004/02/skos/core#definition> "A Military Base with permanently stationed operating forces, robust Infrastructure, and strengthened force protection measures such that it is designed to launch and support large-scale operations, support smaller or less-permanent bases, and organize supply facilities."@en .


###  http://www.ontologyrepository.com/CommonCoreOntologies/Biological_Depot
cco:Biological_Depot rdf:type owl:Class ;
                     rdfs:subClassOf cco:StorageFacility ;
                     cco:is_curated_in_ontology "http://www.ontologyrepository.com/CommonCoreOntologies/Mid/FacilityOntology"^^xsd:anyURI ;
                     rdfs:label "Biological Depot"@en ;
                     <http://www.w3.org/2004/02/skos/core#definition> "A Storage Facility that is designed to store biological agents."@en .


###  http://www.ontologyrepository.com/CommonCoreOntologies/ChemicalDepot
cco:ChemicalDepot rdf:type owl:Class ;
                  rdfs:subClassOf cco:StorageFacility ;
                  cco:is_curated_in_ontology "http://www.ontologyrepository.com/CommonCoreOntologies/Mid/FacilityOntology"^^xsd:anyURI ;
                  rdfs:label "Chemical Depot"@en ;
                  <http://www.w3.org/2004/02/skos/core#definition> "A Storage Facility that is designed to store chemicals."@en .


###  http://www.ontologyrepository.com/CommonCoreOntologies/ChemicalManufacturingFacility
cco:ChemicalManufacturingFacility rdf:type owl:Class ;
                                  rdfs:subClassOf cco:Factory ;
                                  cco:definition_source "https://en.wikipedia.org/w/index.php?title=Chemical_industry&oldid=1061177027"^^xsd:anyURI ;
                                  cco:is_curated_in_ontology "http://www.ontologyrepository.com/CommonCoreOntologies/Mid/FacilityOntology"^^xsd:anyURI ;
                                  rdfs:label "Chemical Manufacturing Facility"@en ;
                                  <http://www.w3.org/2004/02/skos/core#definition> "A Factory that is designed to manufacture or process chemicals."@en .


###  http://www.ontologyrepository.com/CommonCoreOntologies/Church
cco:Church rdf:type owl:Class ;
           rdfs:subClassOf cco:ReligiousFacility ;
           cco:definition_source "https://en.wikipedia.org/wiki/Church_(building)" ;
           cco:is_curated_in_ontology "http://www.ontologyrepository.com/CommonCoreOntologies/Mid/FacilityOntology"^^xsd:anyURI ;
           rdfs:label "Church"@en ;
           <http://www.w3.org/2004/02/skos/core#definition> "A Religious Facility that is designed for Christian worship and prayer."@en .


###  http://www.ontologyrepository.com/CommonCoreOntologies/CombatOutpost
cco:CombatOutpost rdf:type owl:Class ;
                  rdfs:subClassOf cco:MilitaryFacility ;
                  cco:definition_source "https://en.wikipedia.org/wiki/Outpost_(military)" ;
                  cco:is_curated_in_ontology "http://www.ontologyrepository.com/CommonCoreOntologies/Mid/FacilityOntology"^^xsd:anyURI ;
                  rdfs:label "Combat Outpost"@en ;
                  <http://www.w3.org/2004/02/skos/core#definition> "A Military Facility that is designed to support the conduction of combat operations of limited scope or size."@en .


###  http://www.ontologyrepository.com/CommonCoreOntologies/CommandPostFacility
cco:CommandPostFacility rdf:type owl:Class ;
                        rdfs:subClassOf cco:MilitaryFacility ;
                        cco:definition_source "http://www.dictionary.com/browse/command-post" ;
                        cco:is_curated_in_ontology "http://www.ontologyrepository.com/CommonCoreOntologies/Mid/FacilityOntology"^^xsd:anyURI ;
                        rdfs:label "Command Post Facility"@en ;
                        <http://www.w3.org/2004/02/skos/core#definition> "A Military Facility that is designed to support the command and control of Military Operations or Forces."@en .


###  http://www.ontologyrepository.com/CommonCoreOntologies/CommunicationsFacility
cco:CommunicationsFacility rdf:type owl:Class ;
                           rdfs:subClassOf cco:Facility ;
                           cco:is_curated_in_ontology "http://www.ontologyrepository.com/CommonCoreOntologies/Mid/FacilityOntology"^^xsd:anyURI ;
                           rdfs:label "Communications Facility"@en ;
                           <http://www.w3.org/2004/02/skos/core#definition> "A Facility that is designed to support processes of receiving or transmitting information."@en .


###  http://www.ontologyrepository.com/CommonCoreOntologies/DecontaminationFacility
cco:DecontaminationFacility rdf:type owl:Class ;
                            rdfs:subClassOf cco:WashingFacility ;
                            cco:definition_source "https://en.wikipedia.org/w/index.php?title=Decontamination&oldid=1049850150"^^xsd:anyURI ;
                            cco:is_curated_in_ontology "http://www.ontologyrepository.com/CommonCoreOntologies/Mid/FacilityOntology"^^xsd:anyURI ;
                            rdfs:label "Decontamination Facility"@en ;
                            <http://www.w3.org/2004/02/skos/core#definition> "A Washing Facility that is designed to wash personnel or equipment after (potential) contamination by radioactive, biological, or chemical material."@en .


###  http://www.ontologyrepository.com/CommonCoreOntologies/DistributionPort
cco:DistributionPort rdf:type owl:Class ;
                     rdfs:subClassOf cco:Port ;
                     cco:definition_source "https://en.wikipedia.org/w/index.php?title=Port&oldid=1064091505"^^xsd:anyURI ;
                     cco:is_curated_in_ontology "http://www.ontologyrepository.com/CommonCoreOntologies/Mid/FacilityOntology"^^xsd:anyURI ;
                     rdfs:label "Distribution Port"@en ;
                     <http://www.w3.org/2004/02/skos/core#definition> "A Port that is designed with the cargo handling equipment necessary for the loading and unloading of Watercraft"@en .


###  http://www.ontologyrepository.com/CommonCoreOntologies/EducationalFacility
cco:EducationalFacility rdf:type owl:Class ;
                        rdfs:subClassOf cco:Facility ;
                        cco:definition_source "https://en.wikipedia.org/w/index.php?title=Education&oldid=1064011752"^^xsd:anyURI ;
                        cco:is_curated_in_ontology "http://www.ontologyrepository.com/CommonCoreOntologies/Mid/FacilityOntology"^^xsd:anyURI ;
                        rdfs:label "Educational Facility"@en ;
                        <http://www.w3.org/2004/02/skos/core#definition> "A Facility that is designed for facilitating learning, or the acquisition of knowledge, skills, values, beliefs, and habits."@en .


###  http://www.ontologyrepository.com/CommonCoreOntologies/ElectricPowerStation
cco:ElectricPowerStation rdf:type owl:Class ;
                         rdfs:subClassOf cco:Facility ;
                         cco:definition_source "https://en.wikipedia.org/w/index.php?title=Power_station&oldid=1052973815"^^xsd:anyURI ;
                         cco:is_curated_in_ontology "http://www.ontologyrepository.com/CommonCoreOntologies/Mid/FacilityOntology"^^xsd:anyURI ;
                         rdfs:label "Electric Power Station"@en ;
                         <http://www.w3.org/2004/02/skos/core#altLabel> "Power Plant"@en ;
                         <http://www.w3.org/2004/02/skos/core#definition> "A Facility that is designed to generate electrical power."@en .


###  http://www.ontologyrepository.com/CommonCoreOntologies/EntertainmentFacility
cco:EntertainmentFacility rdf:type owl:Class ;
                          rdfs:subClassOf cco:Facility ;
                          cco:definition_source "https://en.wikipedia.org/w/index.php?title=Entertainment&oldid=1061851778"^^xsd:anyURI ;
                          cco:is_curated_in_ontology "http://www.ontologyrepository.com/CommonCoreOntologies/Mid/FacilityOntology"^^xsd:anyURI ;
                          rdfs:label "Entertainment Facility"@en ;
                          <http://www.w3.org/2004/02/skos/core#definition> "A Facility that is designed to host activities that are intended to hold the interest of, or give pleasure or delight to, an audience."@en .


###  http://www.ontologyrepository.com/CommonCoreOntologies/Factory
cco:Factory rdf:type owl:Class ;
            rdfs:subClassOf cco:Facility ;
            cco:definition_source "https://en.wikipedia.org/w/index.php?title=Factory&oldid=1064125324"^^xsd:anyURI ;
            cco:is_curated_in_ontology "http://www.ontologyrepository.com/CommonCoreOntologies/Mid/FacilityOntology"^^xsd:anyURI ;
            rdfs:label "Factory"@en ;
            <http://www.w3.org/2004/02/skos/core#definition> "A Facility that is designed for manufacturing or refining material products."@en .


###  http://www.ontologyrepository.com/CommonCoreOntologies/Farm
cco:Farm rdf:type owl:Class ;
         rdfs:subClassOf cco:AgriculturalFacility ;
         cco:definition_source "https://en.wikipedia.org/w/index.php?title=Farm&oldid=1058311769"^^xsd:anyURI ;
         cco:is_curated_in_ontology "http://www.ontologyrepository.com/CommonCoreOntologies/Mid/FacilityOntology"^^xsd:anyURI ;
         rdfs:label "Farm"@en ;
         <http://www.w3.org/2004/02/skos/core#definition> "An Agricultural Facility that is designed to produce food and other crops."@en .


###  http://www.ontologyrepository.com/CommonCoreOntologies/FinancialFacility
cco:FinancialFacility rdf:type owl:Class ;
                      rdfs:subClassOf cco:Facility ;
                      cco:definition_source "https://en.wikipedia.org/w/index.php?title=Finance&oldid=1062402926"^^xsd:anyURI ;
                      cco:is_curated_in_ontology "http://www.ontologyrepository.com/CommonCoreOntologies/Mid/FacilityOntology"^^xsd:anyURI ;
                      rdfs:label "Financial Facility"@en ;
                      <http://www.w3.org/2004/02/skos/core#definition> "A Facility that is designed to support the management of money."@en .


###  http://www.ontologyrepository.com/CommonCoreOntologies/FireStation
cco:FireStation rdf:type owl:Class ;
                rdfs:subClassOf cco:PublicSafetyFacility ;
                cco:definition_source "https://en.wikipedia.org/w/index.php?title=Fire_station&oldid=1060666629"^^xsd:anyURI ;
                cco:is_curated_in_ontology "http://www.ontologyrepository.com/CommonCoreOntologies/Mid/FacilityOntology"^^xsd:anyURI ;
                rdfs:label "Fire Station"@en ;
                <http://www.w3.org/2004/02/skos/core#altLabel> "Fire Hall"@en ,
                                                               "Fire House"@en ;
                <http://www.w3.org/2004/02/skos/core#definition> "A Public Safety Facility that is designed for the storage of firefighting apparatus."@en .


###  http://www.ontologyrepository.com/CommonCoreOntologies/Fort
cco:Fort rdf:type owl:Class ;
         rdfs:subClassOf cco:MilitaryFacility ;
         cco:definition_source "https://en.wikipedia.org/w/index.php?title=Fortification&oldid=1060156408"^^xsd:anyURI ;
         cco:is_curated_in_ontology "http://www.ontologyrepository.com/CommonCoreOntologies/Mid/FacilityOntology"^^xsd:anyURI ;
         rdfs:label "Fort"@en ;
         <http://www.w3.org/2004/02/skos/core#definition> "A Military Facility that is designed to support the defense of or solidification of rule over some Geospatial Region and its inhabitants."@en .


###  http://www.ontologyrepository.com/CommonCoreOntologies/ForwardOperationsBase
cco:ForwardOperationsBase rdf:type owl:Class ;
                          rdfs:subClassOf cco:MilitaryBase ;
                          cco:acronym "FOB" ;
                          cco:definition_source "https://en.wikipedia.org/w/index.php?title=Forward_operating_base&oldid=1059263624"^^xsd:anyURI ;
                          cco:is_curated_in_ontology "http://www.ontologyrepository.com/CommonCoreOntologies/Mid/FacilityOntology"^^xsd:anyURI ;
                          rdfs:label "Forward Operations Base"@en ;
                          <http://www.w3.org/2004/02/skos/core#altLabel> "Forward Operating Base"@en ;
                          <http://www.w3.org/2004/02/skos/core#definition> "A Military Base that is located relatively close to an offensive Area of Operations, is supported by the Base of Operations, and is designed to support local strategic objectives and tactical operations."@en .


###  http://www.ontologyrepository.com/CommonCoreOntologies/FossilFuelPowerPlant
cco:FossilFuelPowerPlant rdf:type owl:Class ;
                         rdfs:subClassOf cco:ElectricPowerStation ;
                         cco:definition_source "https://en.wikipedia.org/w/index.php?title=Fossil_fuel&oldid=1062298144"^^xsd:anyURI ;
                         cco:is_curated_in_ontology "http://www.ontologyrepository.com/CommonCoreOntologies/Mid/FacilityOntology"^^xsd:anyURI ;
                         rdfs:label "Fossil Fuel Power Plant"@en ;
                         <http://www.w3.org/2004/02/skos/core#definition> "An Electric Power Station that is designed to convert fossil fuels (e.g. coal, natural gas, or petroleum) into electrical energy."@en .


###  http://www.ontologyrepository.com/CommonCoreOntologies/GasProcessingFacility
cco:GasProcessingFacility rdf:type owl:Class ;
                          rdfs:subClassOf cco:Refinery ;
                          cco:definition_source "https://en.wikipedia.org/w/index.php?title=Natural-gas_processing&oldid=1056700541"^^xsd:anyURI ;
                          cco:is_curated_in_ontology "http://www.ontologyrepository.com/CommonCoreOntologies/Mid/FacilityOntology"^^xsd:anyURI ;
                          rdfs:label "Gas Processing Facility"@en ;
                          <http://www.w3.org/2004/02/skos/core#definition> "A Refinery that is designed for refining natural gas into products of value."@en .


###  http://www.ontologyrepository.com/CommonCoreOntologies/GovernmentBuilding
cco:GovernmentBuilding rdf:type owl:Class ;
                       rdfs:subClassOf cco:Facility ;
                       cco:definition_source "https://en.wikipedia.org/wiki/Administration_(government)" ;
                       cco:is_curated_in_ontology "http://www.ontologyrepository.com/CommonCoreOntologies/Mid/FacilityOntology"^^xsd:anyURI ;
                       rdfs:label "Government Building"@en ;
                       <http://www.w3.org/2004/02/skos/core#definition> "A Facility that is designed for the administration of a community."@en .


###  http://www.ontologyrepository.com/CommonCoreOntologies/GroceryStore
cco:GroceryStore rdf:type owl:Class ;
                 rdfs:subClassOf cco:RetailFacility ;
                 cco:definition_source "https://en.wikipedia.org/w/index.php?title=Grocery_store&oldid=1060022873"^^xsd:anyURI ;
                 cco:is_curated_in_ontology "http://www.ontologyrepository.com/CommonCoreOntologies/Mid/FacilityOntology"^^xsd:anyURI ;
                 rdfs:label "Grocery Store"@en ;
                 <http://www.w3.org/2004/02/skos/core#definition> "A Commercial Facility that is designed to sell food."@en .


###  http://www.ontologyrepository.com/CommonCoreOntologies/HealthcareFacility
cco:HealthcareFacility rdf:type owl:Class ;
                       rdfs:subClassOf cco:Facility ;
                       cco:definition_source "https://en.wikipedia.org/w/index.php?title=Medicine&oldid=1062226814"^^xsd:anyURI ;
                       cco:is_curated_in_ontology "http://www.ontologyrepository.com/CommonCoreOntologies/Mid/FacilityOntology"^^xsd:anyURI ;
                       rdfs:label "Healthcare Facility"@en ;
                       <http://www.w3.org/2004/02/skos/core#definition> "A Facility that is designed for the diagnosis, treatment, and prevention of disease."@en .


###  http://www.ontologyrepository.com/CommonCoreOntologies/Heliport
cco:Heliport rdf:type owl:Class ;
             rdfs:subClassOf cco:Airport ;
             cco:definition_source "https://en.wikipedia.org/w/index.php?title=Heliport&oldid=1049937701"^^xsd:anyURI ;
             cco:is_curated_in_ontology "http://www.ontologyrepository.com/CommonCoreOntologies/Mid/FacilityOntology"^^xsd:anyURI ;
             rdfs:label "Heliport"@en ;
             <http://www.w3.org/2004/02/skos/core#definition> "An Airport that is designed for launching, receiving, and housing Rotorcraft."@en .


###  http://www.ontologyrepository.com/CommonCoreOntologies/Hospital
cco:Hospital rdf:type owl:Class ;
             rdfs:subClassOf cco:HealthcareFacility ;
             cco:definition_source "https://en.wikipedia.org/w/index.php?title=Hospital&oldid=1063047817"^^xsd:anyURI ;
             cco:is_curated_in_ontology "http://www.ontologyrepository.com/CommonCoreOntologies/Mid/FacilityOntology"^^xsd:anyURI ;
             rdfs:label "Hospital"@en ;
             <http://www.w3.org/2004/02/skos/core#definition> "A Healthcare Facility that is designed to provide patient treatment with specialized staff and equipment."@en .


###  http://www.ontologyrepository.com/CommonCoreOntologies/Hostel
cco:Hostel rdf:type owl:Class ;
           rdfs:subClassOf cco:ResidentialFacility ;
           cco:definition_source "https://en.wikipedia.org/w/index.php?title=Hostel&oldid=1057812930"^^xsd:anyURI ;
           cco:is_curated_in_ontology "http://www.ontologyrepository.com/CommonCoreOntologies/Mid/FacilityOntology"^^xsd:anyURI ;
           rdfs:label "Hostel"@en ;
           <http://www.w3.org/2004/02/skos/core#definition> "A Residential Facility that is designed to temporarily lodge guests in a sociable environment for relatively low costs."@en .


###  http://www.ontologyrepository.com/CommonCoreOntologies/Hotel
cco:Hotel rdf:type owl:Class ;
          rdfs:subClassOf cco:ResidentialFacility ;
          cco:definition_source "https://en.wikipedia.org/w/index.php?title=Hotel&oldid=1063583593"^^xsd:anyURI ;
          cco:is_curated_in_ontology "http://www.ontologyrepository.com/CommonCoreOntologies/Mid/FacilityOntology"^^xsd:anyURI ;
          rdfs:label "Hotel"@en ;
          <http://www.w3.org/2004/02/skos/core#definition> "A Residential Facility that is designed to provide lodging that is paid for on a short-term basis."@en .


###  http://www.ontologyrepository.com/CommonCoreOntologies/House
cco:House rdf:type owl:Class ;
          rdfs:subClassOf cco:ResidentialFacility ;
          cco:definition_source "https://en.wikipedia.org/w/index.php?title=House&oldid=1062818553"^^xsd:anyURI ;
          cco:is_curated_in_ontology "http://www.ontologyrepository.com/CommonCoreOntologies/Mid/FacilityOntology"^^xsd:anyURI ;
          rdfs:label "House"@en ;
          <http://www.w3.org/2004/02/skos/core#definition> "A Residential Facility that is designed to provide a self-standing, permanent residence for an individual, family, household, multiple families, or similar-sized group."@en .


###  http://www.ontologyrepository.com/CommonCoreOntologies/HydroelectricPowerPlant
cco:HydroelectricPowerPlant rdf:type owl:Class ;
                            rdfs:subClassOf cco:ElectricPowerStation ;
                            cco:definition_source "https://en.wikipedia.org/w/index.php?title=Hydroelectricity&oldid=1062438236"^^xsd:anyURI ;
                            cco:is_curated_in_ontology "http://www.ontologyrepository.com/CommonCoreOntologies/Mid/FacilityOntology"^^xsd:anyURI ;
                            rdfs:label "Hydroelectric Power Plant"@en ;
                            <http://www.w3.org/2004/02/skos/core#definition> "An Electric Power Station that is designed to convert hydropower into electrical power."@en .


###  http://www.ontologyrepository.com/CommonCoreOntologies/Landfill
cco:Landfill rdf:type owl:Class ;
             rdfs:subClassOf cco:WasteManagementFacility ;
             cco:definition_source "https://en.wikipedia.org/w/index.php?title=Landfill&oldid=1058364420"^^xsd:anyURI ;
             cco:is_curated_in_ontology "http://www.ontologyrepository.com/CommonCoreOntologies/Mid/FacilityOntology"^^xsd:anyURI ;
             rdfs:label "Landfill"@en ;
             <http://www.w3.org/2004/02/skos/core#definition> "A Waste Management Facility that is designed for disposing of waste by burial."@en .


###  http://www.ontologyrepository.com/CommonCoreOntologies/MailingFacility
cco:MailingFacility rdf:type owl:Class ;
                    rdfs:subClassOf cco:Facility ;
                    cco:definition_source "https://en.wikipedia.org/w/index.php?title=Mail&oldid=1057401839"^^xsd:anyURI ;
                    cco:is_curated_in_ontology "http://www.ontologyrepository.com/CommonCoreOntologies/Mid/FacilityOntology"^^xsd:anyURI ;
                    rdfs:label "Mailing Facility"@en ;
                    <http://www.w3.org/2004/02/skos/core#definition> "A Facility that is designed for the systematic physical transportation of documents and packages."@en .


###  http://www.ontologyrepository.com/CommonCoreOntologies/MaintenanceFacility
cco:MaintenanceFacility rdf:type owl:Class ;
                        rdfs:subClassOf cco:Facility ;
                        cco:definition_source "http://www.dictionary.com/browse/maintain" ;
                        cco:is_curated_in_ontology "http://www.ontologyrepository.com/CommonCoreOntologies/Mid/FacilityOntology"^^xsd:anyURI ;
                        rdfs:label "Maintenance Facility"@en ;
                        <http://www.w3.org/2004/02/skos/core#definition> "A Facility that is designed to be used to perform actions to maintain or improve the state of some property or equipment."@en .


###  http://www.ontologyrepository.com/CommonCoreOntologies/MedicalDepot
cco:MedicalDepot rdf:type owl:Class ;
                 rdfs:subClassOf cco:StorageFacility ;
                 cco:is_curated_in_ontology "http://www.ontologyrepository.com/CommonCoreOntologies/Mid/FacilityOntology"^^xsd:anyURI ;
                 rdfs:label "Medical Depot"@en ;
                 <http://www.w3.org/2004/02/skos/core#definition> "A Storage Facility that is designed to store medical supplies."@en .


###  http://www.ontologyrepository.com/CommonCoreOntologies/MilitaryBase
cco:MilitaryBase rdf:type owl:Class ;
                 rdfs:subClassOf cco:MilitaryFacility ;
                 cco:definition_source "https://en.wikipedia.org/w/index.php?title=Military_base&oldid=1047077734"^^xsd:anyURI ;
                 cco:is_curated_in_ontology "http://www.ontologyrepository.com/CommonCoreOntologies/Mid/FacilityOntology"^^xsd:anyURI ;
                 rdfs:label "Military Base"@en ;
                 <http://www.w3.org/2004/02/skos/core#definition> "A Military Facility that is designed to shelter military equipment and personnel and to facilitate training and operations."@en .


###  http://www.ontologyrepository.com/CommonCoreOntologies/MilitaryFacility
cco:MilitaryFacility rdf:type owl:Class ;
                     rdfs:subClassOf cco:Facility ;
                     cco:definition_source "https://en.wikipedia.org/w/index.php?title=Military&oldid=1063431234"^^xsd:anyURI ;
                     cco:is_curated_in_ontology "http://www.ontologyrepository.com/CommonCoreOntologies/Mid/FacilityOntology"^^xsd:anyURI ;
                     rdfs:label "Military Facility"@en ;
                     <http://www.w3.org/2004/02/skos/core#definition> "A Facility that is designed to support a Military Force."@en .


###  http://www.ontologyrepository.com/CommonCoreOntologies/MilitaryHeadquartersFacility
cco:MilitaryHeadquartersFacility rdf:type owl:Class ;
                                 rdfs:subClassOf cco:MilitaryFacility ;
                                 cco:definition_source "https://en.wikipedia.org/w/index.php?title=Headquarters&oldid=1046429636"^^xsd:anyURI ;
                                 cco:is_curated_in_ontology "http://www.ontologyrepository.com/CommonCoreOntologies/Mid/FacilityOntology"^^xsd:anyURI ;
                                 rdfs:label "Military Headquarters Facility"@en ;
                                 <http://www.w3.org/2004/02/skos/core#definition> "A Military Facility that is designed for military administration and coordination."@en .


###  http://www.ontologyrepository.com/CommonCoreOntologies/Mine
cco:Mine rdf:type owl:Class ;
         rdfs:subClassOf cco:Facility ;
         cco:definition_source "https://en.wikipedia.org/w/index.php?title=Mining&oldid=1062844924"^^xsd:anyURI ;
         cco:is_curated_in_ontology "http://www.ontologyrepository.com/CommonCoreOntologies/Mid/FacilityOntology"^^xsd:anyURI ;
         rdfs:label "Mine"@en ;
         <http://www.w3.org/2004/02/skos/core#definition> "A Facility that is designed to support the extraction of minerals or other geological materials from an orebody, lode, vein, seam, reef, or placer deposit within the earth."@en .


###  http://www.ontologyrepository.com/CommonCoreOntologies/MissileLaunchSite
cco:MissileLaunchSite rdf:type owl:Class ;
                      rdfs:subClassOf cco:MilitaryFacility ;
                      cco:definition_source "https://en.wikipedia.org/w/index.php?title=Missile_launch_facility&oldid=1062709375"^^xsd:anyURI ;
                      cco:is_curated_in_ontology "http://www.ontologyrepository.com/CommonCoreOntologies/Mid/FacilityOntology"^^xsd:anyURI ;
                      rdfs:label "Missile Launch Site"@en ;
                      <http://www.w3.org/2004/02/skos/core#definition> "A Military Facility that is designed for storing and launching missiles."@en .


###  http://www.ontologyrepository.com/CommonCoreOntologies/Mosque
cco:Mosque rdf:type owl:Class ;
           rdfs:subClassOf cco:ReligiousFacility ;
           cco:definition_source "https://en.wikipedia.org/w/index.php?title=Mosque&oldid=1062609892"^^xsd:anyURI ;
           cco:is_curated_in_ontology "http://www.ontologyrepository.com/CommonCoreOntologies/Mid/FacilityOntology"^^xsd:anyURI ;
           rdfs:label "Mosque"@en ;
           <http://www.w3.org/2004/02/skos/core#definition> "A Religious Facility that is designed for Islamic worship and prayer."@en .


###  http://www.ontologyrepository.com/CommonCoreOntologies/Motel
cco:Motel rdf:type owl:Class ;
          rdfs:subClassOf cco:Hotel ;
          cco:definition_source "https://en.wikipedia.org/w/index.php?title=Motel&oldid=1063898961"^^xsd:anyURI ;
          cco:is_curated_in_ontology "http://www.ontologyrepository.com/CommonCoreOntologies/Mid/FacilityOntology"^^xsd:anyURI ;
          rdfs:label "Motel"@en ;
          <http://www.w3.org/2004/02/skos/core#definition> "A Hotel that is designed to accommodate motor vehicles along with their occupants."@en .


###  http://www.ontologyrepository.com/CommonCoreOntologies/MotorVehicleManufacturingFacility
cco:MotorVehicleManufacturingFacility rdf:type owl:Class ;
                                      rdfs:subClassOf cco:Factory ;
                                      cco:definition_source "https://en.wikipedia.org/w/index.php?title=Automotive_industry&oldid=1061661751"^^xsd:anyURI ;
                                      cco:is_curated_in_ontology "http://www.ontologyrepository.com/CommonCoreOntologies/Mid/FacilityOntology"^^xsd:anyURI ;
                                      rdfs:label "Motor Vehicle Manufacturing Facility"@en ;
                                      <http://www.w3.org/2004/02/skos/core#definition> "A Factory that is designed to manufacture automobiles."@en .


###  http://www.ontologyrepository.com/CommonCoreOntologies/NuclearPowerPlant
cco:NuclearPowerPlant rdf:type owl:Class ;
                      rdfs:subClassOf cco:ThermalPowerPlant ;
                      cco:definition_source "https://en.wikipedia.org/w/index.php?title=Nuclear_power_plant&oldid=1062752651"^^xsd:anyURI ;
                      cco:is_curated_in_ontology "http://www.ontologyrepository.com/CommonCoreOntologies/Mid/FacilityOntology"^^xsd:anyURI ;
                      rdfs:label "Nuclear Power Plant"@en ;
                      <http://www.w3.org/2004/02/skos/core#definition> "A Thermal Power Plant that is designed to produce heat by means of a nuclear reactor, which is then converted to electrical energy."@en .


###  http://www.ontologyrepository.com/CommonCoreOntologies/NuclearStorageDepot
cco:NuclearStorageDepot rdf:type owl:Class ;
                        rdfs:subClassOf cco:StorageFacility ;
                        cco:is_curated_in_ontology "http://www.ontologyrepository.com/CommonCoreOntologies/Mid/FacilityOntology"^^xsd:anyURI ;
                        rdfs:label "Nuclear Storage Depot"@en ;
                        <http://www.w3.org/2004/02/skos/core#definition> "A Storage Facility that is designed to store nuclear material."@en .


###  http://www.ontologyrepository.com/CommonCoreOntologies/OfficeBuilding
cco:OfficeBuilding rdf:type owl:Class ;
                   rdfs:subClassOf cco:RetailFacility ;
                   cco:definition_source "https://en.wikipedia.org/w/index.php?title=Office&oldid=1063508719"^^xsd:anyURI ;
                   cco:is_curated_in_ontology "http://www.ontologyrepository.com/CommonCoreOntologies/Mid/FacilityOntology"^^xsd:anyURI ;
                   rdfs:label "Office Building"@en ;
                   <http://www.w3.org/2004/02/skos/core#definition> "A Commercial Facility that is designed as an environment for conducting commercial, professional, or bureaucratic work."@en .


###  http://www.ontologyrepository.com/CommonCoreOntologies/OpenPitMine
cco:OpenPitMine rdf:type owl:Class ;
                rdfs:subClassOf cco:Mine ;
                cco:definition_source "https://en.wikipedia.org/w/index.php?title=Open-pit_mining&oldid=1059271938"^^xsd:anyURI ;
                cco:is_curated_in_ontology "http://www.ontologyrepository.com/CommonCoreOntologies/Mid/FacilityOntology"^^xsd:anyURI ;
                rdfs:label "Open Pit Mine"@en ;
                <http://www.w3.org/2004/02/skos/core#definition> "A Mine that is designed to support the extraction of materials from the ground directly without using tunnels."@en .


###  http://www.ontologyrepository.com/CommonCoreOntologies/PetrochemicalRefinery
cco:PetrochemicalRefinery rdf:type owl:Class ;
                          rdfs:subClassOf cco:Refinery ;
                          cco:definition_source "https://en.wikipedia.org/w/index.php?title=Petrochemical&oldid=1060574535"^^xsd:anyURI ;
                          cco:is_curated_in_ontology "http://www.ontologyrepository.com/CommonCoreOntologies/Mid/FacilityOntology"^^xsd:anyURI ;
                          rdfs:label "Petrochemical Refinery"@en ;
                          <http://www.w3.org/2004/02/skos/core#definition> "A Refinery that is designed for refining crude oil, intermediate petroleum products, or synthetic petroleum into products of value."@en .


###  http://www.ontologyrepository.com/CommonCoreOntologies/PetroleumDepot
cco:PetroleumDepot rdf:type owl:Class ;
                   rdfs:subClassOf cco:StorageFacility ;
                   cco:is_curated_in_ontology "http://www.ontologyrepository.com/CommonCoreOntologies/Mid/FacilityOntology"^^xsd:anyURI ;
                   rdfs:label "Petroleum Depot"@en ;
                   <http://www.w3.org/2004/02/skos/core#definition> "A Storage Facility that is designed to store petroleum, oil, or lubricants."@en .


###  http://www.ontologyrepository.com/CommonCoreOntologies/PetroleumManufacturingFacility
cco:PetroleumManufacturingFacility rdf:type owl:Class ;
                                   rdfs:subClassOf cco:Factory ;
                                   cco:definition_source "https://en.wikipedia.org/w/index.php?title=Petroleum&oldid=1062956217"^^xsd:anyURI ;
                                   cco:is_curated_in_ontology "http://www.ontologyrepository.com/CommonCoreOntologies/Mid/FacilityOntology"^^xsd:anyURI ;
                                   rdfs:label "Petroleum Manufacturing Facility"@en ;
                                   <http://www.w3.org/2004/02/skos/core#definition> "A Factory that is designed to manufacture petroleum-based products."@en .


###  http://www.ontologyrepository.com/CommonCoreOntologies/Pier
cco:Pier rdf:type owl:Class ;
         rdfs:subClassOf cco:TransportationFacility ;
         cco:definition_source "https://en.wikipedia.org/w/index.php?title=Pier&oldid=1057802753"^^xsd:anyURI ;
         cco:is_curated_in_ontology "http://www.ontologyrepository.com/CommonCoreOntologies/Mid/FacilityOntology"^^xsd:anyURI ;
         rdfs:label "Pier"@en ;
         <http://www.w3.org/2004/02/skos/core#definition> "A Transportation Facility that is designed to partially enclose a harbor and form a landing place for Watercraft."@en .


###  http://www.ontologyrepository.com/CommonCoreOntologies/Pipeline
cco:Pipeline rdf:type owl:Class ;
             rdfs:subClassOf cco:ProductTransportFacility ;
             cco:definition_source "https://en.wikipedia.org/w/index.php?title=Pipeline&oldid=1024308788"^^xsd:anyURI ;
             cco:is_curated_in_ontology "http://www.ontologyrepository.com/CommonCoreOntologies/Mid/FacilityOntology"^^xsd:anyURI ;
             rdfs:label "Pipeline"@en ;
             <http://www.w3.org/2004/02/skos/core#definition> "A Product Transport Facility that is designed to transport goods or materials through a pipe."@en .


###  http://www.ontologyrepository.com/CommonCoreOntologies/PoliceStation
cco:PoliceStation rdf:type owl:Class ;
                  rdfs:subClassOf cco:PublicSafetyFacility ;
                  cco:definition_source "https://en.wikipedia.org/w/index.php?title=Police_station&oldid=1056208781"^^xsd:anyURI ;
                  cco:is_curated_in_ontology "http://www.ontologyrepository.com/CommonCoreOntologies/Mid/FacilityOntology"^^xsd:anyURI ;
                  rdfs:label "Police Station"@en ;
                  <http://www.w3.org/2004/02/skos/core#definition> "A Public Safety Facility that is designed for the professional and clerical processes of a local police force."@en .


###  http://www.ontologyrepository.com/CommonCoreOntologies/Port
cco:Port rdf:type owl:Class ;
         rdfs:subClassOf cco:TransportationFacility ;
         cco:definition_source "https://en.wikipedia.org/w/index.php?title=Port&oldid=1064091505"^^xsd:anyURI ;
         cco:is_curated_in_ontology "http://www.ontologyrepository.com/CommonCoreOntologies/Mid/FacilityOntology"^^xsd:anyURI ;
         rdfs:label "Port"@en ;
         <http://www.w3.org/2004/02/skos/core#definition> "A Transportation Facility that is designed to contain harbors for docking Watercraft and for transfering people or cargo to and from land."@en .


###  http://www.ontologyrepository.com/CommonCoreOntologies/PostOffice
cco:PostOffice rdf:type owl:Class ;
               rdfs:subClassOf cco:MailingFacility ;
               cco:definition_source "https://en.wikipedia.org/w/index.php?title=Post_office&oldid=1063684373"^^xsd:anyURI ;
               cco:is_curated_in_ontology "http://www.ontologyrepository.com/CommonCoreOntologies/Mid/FacilityOntology"^^xsd:anyURI ;
               rdfs:label "Post Office"@en ;
               <http://www.w3.org/2004/02/skos/core#definition> "A Mailing Facility that is designed for serving customers of the national postal system."@en .


###  http://www.ontologyrepository.com/CommonCoreOntologies/PowerTransmissionLine
cco:PowerTransmissionLine rdf:type owl:Class ;
                          rdfs:subClassOf cco:ProductTransportFacility ;
                          cco:definition_source "https://en.wikipedia.org/w/index.php?title=Electric_power_transmission&oldid=1062551058"^^xsd:anyURI ;
                          cco:is_curated_in_ontology "http://www.ontologyrepository.com/CommonCoreOntologies/Mid/FacilityOntology"^^xsd:anyURI ;
                          rdfs:label "Power Transmission Line"@en ;
                          <http://www.w3.org/2004/02/skos/core#definition> "A Product Transport Facility that is designed to transmit electricity over distance via a system of above ground wires including their supports."@en .


###  http://www.ontologyrepository.com/CommonCoreOntologies/ProductTransportFacility
cco:ProductTransportFacility rdf:type owl:Class ;
                             rdfs:subClassOf cco:Facility ;
                             cco:is_curated_in_ontology "http://www.ontologyrepository.com/CommonCoreOntologies/Mid/FacilityOntology"^^xsd:anyURI ;
                             rdfs:label "Product Transport Facility"@en ;
                             <http://www.w3.org/2004/02/skos/core#definition> "A Facility that is designed to transport some product."@en .


###  http://www.ontologyrepository.com/CommonCoreOntologies/PublicSafetyFacility
cco:PublicSafetyFacility rdf:type owl:Class ;
                         rdfs:subClassOf cco:Facility ;
                         cco:definition_source "https://en.wikipedia.org/w/index.php?title=Public_security&oldid=1058257389"^^xsd:anyURI ;
                         cco:is_curated_in_ontology "http://www.ontologyrepository.com/CommonCoreOntologies/Mid/FacilityOntology"^^xsd:anyURI ;
                         rdfs:label "Public Safety Facility"@en ;
                         <http://www.w3.org/2004/02/skos/core#definition> "A Facility that is designed for the prevention of and protection from events that could endanger, injure, or damage the general public."@en .


###  http://www.ontologyrepository.com/CommonCoreOntologies/PumpingStation
cco:PumpingStation rdf:type owl:Class ;
                   rdfs:subClassOf cco:ProductTransportFacility ;
                   cco:definition_source "https://en.wikipedia.org/w/index.php?title=Pumping_station&oldid=1045678418"^^xsd:anyURI ;
                   cco:is_curated_in_ontology "http://www.ontologyrepository.com/CommonCoreOntologies/Mid/FacilityOntology"^^xsd:anyURI ;
                   rdfs:label "Pumping Station"@en ;
                   <http://www.w3.org/2004/02/skos/core#definition> "A Product Transport Facility that is designed to pump fluids from one place to another."@en .


###  http://www.ontologyrepository.com/CommonCoreOntologies/RadioRelayStation
cco:RadioRelayStation rdf:type owl:Class ;
                      rdfs:subClassOf cco:CommunicationsFacility ;
                      cco:is_curated_in_ontology "http://www.ontologyrepository.com/CommonCoreOntologies/Mid/FacilityOntology"^^xsd:anyURI ;
                      rdfs:label "Radio Relay Station"@en ;
                      <http://www.w3.org/2004/02/skos/core#definition> "A Communications Facility that is designed to support the receiving and re-transmitting of radio signals."@en .


###  http://www.ontologyrepository.com/CommonCoreOntologies/RailFacility
cco:RailFacility rdf:type owl:Class ;
                 rdfs:subClassOf cco:TransportationFacility ;
                 cco:definition_source "https://en.wikipedia.org/w/index.php?title=Train_station&oldid=1063922802"^^xsd:anyURI ;
                 cco:is_curated_in_ontology "http://www.ontologyrepository.com/CommonCoreOntologies/Mid/FacilityOntology"^^xsd:anyURI ;
                 rdfs:label "Rail Facility"@en ;
                 <http://www.w3.org/2004/02/skos/core#definition> "A Transportation Facility that is designed for transferring people or cargo to and from Trains."@en .


###  http://www.ontologyrepository.com/CommonCoreOntologies/Refinery
cco:Refinery rdf:type owl:Class ;
             rdfs:subClassOf cco:Factory ;
             cco:definition_source "https://en.wikipedia.org/w/index.php?title=Refinery&oldid=1027092124"^^xsd:anyURI ;
             cco:is_curated_in_ontology "http://www.ontologyrepository.com/CommonCoreOntologies/Mid/FacilityOntology"^^xsd:anyURI ;
             rdfs:label "Refinery"@en ;
             <http://www.w3.org/2004/02/skos/core#definition> "A Factory that is designed for refining raw materials into products of value."@en .


###  http://www.ontologyrepository.com/CommonCoreOntologies/ReligiousFacility
cco:ReligiousFacility rdf:type owl:Class ;
                      rdfs:subClassOf cco:Facility ;
                      cco:definition_source "https://en.wikipedia.org/w/index.php?title=Religion&oldid=1063431202"^^xsd:anyURI ;
                      cco:is_curated_in_ontology "http://www.ontologyrepository.com/CommonCoreOntologies/Mid/FacilityOntology"^^xsd:anyURI ;
                      rdfs:label "Religious Facility"@en ;
                      <http://www.w3.org/2004/02/skos/core#definition> "A Facility that is designed for worship and prayer."@en .


###  http://www.ontologyrepository.com/CommonCoreOntologies/Reservoir
cco:Reservoir rdf:type owl:Class ;
              rdfs:subClassOf cco:StorageFacility ;
              cco:definition_source "https://en.wikipedia.org/w/index.php?title=Reservoir&oldid=1055068000"^^xsd:anyURI ;
              cco:is_curated_in_ontology "http://www.ontologyrepository.com/CommonCoreOntologies/Mid/FacilityOntology"^^xsd:anyURI ;
              rdfs:label "Reservoir"@en ;
              <http://www.w3.org/2004/02/skos/core#definition> "A Storage Facility that is designed to store water in a man-made open enclosure or area."@en .


###  http://www.ontologyrepository.com/CommonCoreOntologies/ResidentialFacility
cco:ResidentialFacility rdf:type owl:Class ;
                        rdfs:subClassOf cco:Facility ;
                        cco:definition_source "https://en.wikipedia.org/w/index.php?title=Residence&oldid=1019728937"^^xsd:anyURI ;
                        cco:is_curated_in_ontology "http://www.ontologyrepository.com/CommonCoreOntologies/Mid/FacilityOntology"^^xsd:anyURI ;
                        rdfs:label "Residential Facility"@en ;
                        <http://www.w3.org/2004/02/skos/core#definition> "A Facility that is designed to house one or more Persons."@en .


###  http://www.ontologyrepository.com/CommonCoreOntologies/RetailFacility
cco:RetailFacility rdf:type owl:Class ;
                   rdfs:subClassOf cco:Facility ;
                   cco:definition_source "https://en.wikipedia.org/w/index.php?title=Commerce&oldid=1063120985"^^xsd:anyURI ;
                   cco:is_curated_in_ontology "http://www.ontologyrepository.com/CommonCoreOntologies/Mid/FacilityOntology"^^xsd:anyURI ;
                   rdfs:label "Commercial Facility"@en ;
                   <http://www.w3.org/2004/02/skos/core#definition> "A Facility that is designed for buying and selling goods and services, especially on a large scale."@en .


###  http://www.ontologyrepository.com/CommonCoreOntologies/School
cco:School rdf:type owl:Class ;
           rdfs:subClassOf cco:EducationalFacility ;
           cco:definition_source "https://en.wikipedia.org/w/index.php?title=School&oldid=1063515394"^^xsd:anyURI ;
           cco:is_curated_in_ontology "http://www.ontologyrepository.com/CommonCoreOntologies/Mid/FacilityOntology"^^xsd:anyURI ;
           rdfs:label "School"@en ;
           <http://www.w3.org/2004/02/skos/core#definition> "An Education Facility that is designed to provide learning space and environments for teaching of students under the direction of teachers."@en .


###  http://www.ontologyrepository.com/CommonCoreOntologies/SeatOfLocalGovernment
cco:SeatOfLocalGovernment rdf:type owl:Class ;
                          rdfs:subClassOf cco:GovernmentBuilding ;
                          cco:definition_source "https://en.wikipedia.org/w/index.php?title=Seat_of_government&oldid=1063047501"^^xsd:anyURI ;
                          cco:is_curated_in_ontology "http://www.ontologyrepository.com/CommonCoreOntologies/Mid/FacilityOntology"^^xsd:anyURI ;
                          rdfs:label "Seat of Local Government"@en ;
                          <http://www.w3.org/2004/02/skos/core#altLabel> "City Hall"@en ,
                                                                         "Town Hall"@en ;
                          <http://www.w3.org/2004/02/skos/core#definition> "A Government Building that is designed for the administration of a local community."@en .


###  http://www.ontologyrepository.com/CommonCoreOntologies/SeatOfNationalGovernment
cco:SeatOfNationalGovernment rdf:type owl:Class ;
                             rdfs:subClassOf cco:GovernmentBuilding ;
                             cco:definition_source "https://en.wikipedia.org/w/index.php?title=Seat_of_government&oldid=1063047501"^^xsd:anyURI ;
                             cco:example_of_usage "Parliament of Canada" ,
                                                  "United States Capitol" ;
                             cco:is_curated_in_ontology "http://www.ontologyrepository.com/CommonCoreOntologies/Mid/FacilityOntology"^^xsd:anyURI ;
                             rdfs:label "Seat of National Government"@en ;
                             <http://www.w3.org/2004/02/skos/core#definition> "A Government Building that is designed for the administration of a sovereign nation."@en .


###  http://www.ontologyrepository.com/CommonCoreOntologies/SewageTreatmentFacility
cco:SewageTreatmentFacility rdf:type owl:Class ;
                            rdfs:subClassOf cco:WasteManagementFacility ;
                            cco:definition_source "https://en.wikipedia.org/w/index.php?title=Sewage_treatment&oldid=1062966352"^^xsd:anyURI ;
                            cco:is_curated_in_ontology "http://www.ontologyrepository.com/CommonCoreOntologies/Mid/FacilityOntology"^^xsd:anyURI ;
                            rdfs:label "Sewage Treatment Facility"@en ;
                            <http://www.w3.org/2004/02/skos/core#definition> "A Waste Management Facility that is designed for removing contaminants from wastewater, especially sewage."@en .


###  http://www.ontologyrepository.com/CommonCoreOntologies/Shop
cco:Shop rdf:type owl:Class ;
         rdfs:subClassOf cco:RetailFacility ;
         cco:definition_source "https://en.wikipedia.org/w/index.php?title=Retail&oldid=1061431295"^^xsd:anyURI ;
         cco:is_curated_in_ontology "http://www.ontologyrepository.com/CommonCoreOntologies/Mid/FacilityOntology"^^xsd:anyURI ;
         rdfs:label "Shop"@en ;
         <http://www.w3.org/2004/02/skos/core#definition> "A Commercial Facility designed to sell small lots of goods to consumers."@en .


###  http://www.ontologyrepository.com/CommonCoreOntologies/Stage
cco:Stage rdf:type owl:Class ;
          rdfs:subClassOf cco:EntertainmentFacility ;
          cco:definition_source "https://en.wikipedia.org/wiki/Stage_(theatre)" ;
          cco:is_curated_in_ontology "http://www.ontologyrepository.com/CommonCoreOntologies/Mid/FacilityOntology"^^xsd:anyURI ;
          rdfs:label "Stage"@en ;
          <http://www.w3.org/2004/02/skos/core#definition> "An Entertainment Facility that is designed to provide a space upon which entertaining performances or productions can occur."@en .


###  http://www.ontologyrepository.com/CommonCoreOntologies/StorageFacility
cco:StorageFacility rdf:type owl:Class ;
                    rdfs:subClassOf cco:Facility ;
                    cco:definition_source "https://en.wikipedia.org/w/index.php?title=Storage&oldid=1048222564"^^xsd:anyURI ;
                    cco:is_curated_in_ontology "http://www.ontologyrepository.com/CommonCoreOntologies/Mid/FacilityOntology"^^xsd:anyURI ;
                    rdfs:label "Storage Facility"@en ;
                    <http://www.w3.org/2004/02/skos/core#definition> "A Facility that is designed to store materials or goods."@en .


###  http://www.ontologyrepository.com/CommonCoreOntologies/Synagogue
cco:Synagogue rdf:type owl:Class ;
              rdfs:subClassOf cco:ReligiousFacility ;
              cco:definition_source "https://en.wikipedia.org/w/index.php?title=Synagogue&oldid=1063773298"^^xsd:anyURI ;
              cco:is_curated_in_ontology "http://www.ontologyrepository.com/CommonCoreOntologies/Mid/FacilityOntology"^^xsd:anyURI ;
              rdfs:label "Synagogue"@en ;
              <http://www.w3.org/2004/02/skos/core#definition> "A Religious Facility that is designed for Judaic worship and prayer."@en .


###  http://www.ontologyrepository.com/CommonCoreOntologies/TerroristTrainingCamp
cco:TerroristTrainingCamp rdf:type owl:Class ;
                          rdfs:subClassOf cco:TrainingCamp ;
                          cco:definition_source "https://en.wikipedia.org/w/index.php?title=Terrorist_training_camp&oldid=1037856600"^^xsd:anyURI ;
                          cco:is_curated_in_ontology "http://www.ontologyrepository.com/CommonCoreOntologies/Mid/FacilityOntology"^^xsd:anyURI ;
                          rdfs:label "Terrorist Training Camp"@en ;
                          <http://www.w3.org/2004/02/skos/core#definition> "A Training Camp designed to teach students methods of terrorism."@en .


###  http://www.ontologyrepository.com/CommonCoreOntologies/ThermalPowerPlant
cco:ThermalPowerPlant rdf:type owl:Class ;
                      rdfs:subClassOf cco:ElectricPowerStation ;
                      cco:definition_source "https://en.wikipedia.org/w/index.php?title=Thermal_power_station&oldid=1062208548"^^xsd:anyURI ;
                      cco:is_curated_in_ontology "http://www.ontologyrepository.com/CommonCoreOntologies/Mid/FacilityOntology"^^xsd:anyURI ;
                      rdfs:label "Thermal Power Plant"@en ;
                      <http://www.w3.org/2004/02/skos/core#definition> "An Electric Power Station that is designed to convert heat energy into electrical energy."@en .


###  http://www.ontologyrepository.com/CommonCoreOntologies/TrainingCamp
cco:TrainingCamp rdf:type owl:Class ;
                 rdfs:subClassOf cco:Facility ;
                 cco:definition_source "https://en.wikipedia.org/w/index.php?title=Training_camp&oldid=1059977631"^^xsd:anyURI ;
                 cco:is_curated_in_ontology "http://www.ontologyrepository.com/CommonCoreOntologies/Mid/FacilityOntology"^^xsd:anyURI ;
                 rdfs:label "Training Camp"@en ;
                 <http://www.w3.org/2004/02/skos/core#definition> "A Facility that is designed for rigorous and focused training in order to learn or improve skills, usually involving physical actions."@en .


###  http://www.ontologyrepository.com/CommonCoreOntologies/TransportationFacility
cco:TransportationFacility rdf:type owl:Class ;
                           rdfs:subClassOf cco:Facility ;
                           cco:definition_source "https://en.wikipedia.org/w/index.php?title=Transport&oldid=1063526665"^^xsd:anyURI ;
                           cco:is_curated_in_ontology "http://www.ontologyrepository.com/CommonCoreOntologies/Mid/FacilityOntology"^^xsd:anyURI ;
                           rdfs:label "Transportation Facility"@en ;
                           <http://www.w3.org/2004/02/skos/core#definition> "A Facility that is designed for commencing or concluding the transportation of transportation artifacts, or for housing transportation artifacts."@en .


###  http://www.ontologyrepository.com/CommonCoreOntologies/UndergroundMine
cco:UndergroundMine rdf:type owl:Class ;
                    rdfs:subClassOf cco:Mine ;
                    cco:definition_source "https://en.wikipedia.org/wiki/Underground_mining_(hard_rock)" ;
                    cco:is_curated_in_ontology "http://www.ontologyrepository.com/CommonCoreOntologies/Mid/FacilityOntology"^^xsd:anyURI ;
                    rdfs:label "Underground Mine"@en ;
                    <http://www.w3.org/2004/02/skos/core#definition> "A Mine that is designed to support the extraction of materials from the ground using underground tunnels and shafts."@en .


###  http://www.ontologyrepository.com/CommonCoreOntologies/UnderwaterMine
cco:UnderwaterMine rdf:type owl:Class ;
                   rdfs:subClassOf cco:Mine ;
                   cco:definition_source "https://en.wikipedia.org/w/index.php?title=Naval_mine&oldid=1062538523"^^xsd:anyURI ;
                   cco:is_curated_in_ontology "http://www.ontologyrepository.com/CommonCoreOntologies/Mid/FacilityOntology"^^xsd:anyURI ;
                   rdfs:label "Underwater Mine"@en ;
                   <http://www.w3.org/2004/02/skos/core#definition> "A Mine that is designed to support the extraction of materials from the ocean floor."@en .


###  http://www.ontologyrepository.com/CommonCoreOntologies/Warehouse
cco:Warehouse rdf:type owl:Class ;
              rdfs:subClassOf cco:StorageFacility ;
              cco:definition_source "https://en.wikipedia.org/w/index.php?title=Warehouse&oldid=1063721454"^^xsd:anyURI ;
              cco:is_curated_in_ontology "http://www.ontologyrepository.com/CommonCoreOntologies/Mid/FacilityOntology"^^xsd:anyURI ;
              rdfs:label "Warehouse"@en ;
              <http://www.w3.org/2004/02/skos/core#definition> "A Storage Facility that is designed to store commercial goods."@en .


###  http://www.ontologyrepository.com/CommonCoreOntologies/WashingFacility
cco:WashingFacility rdf:type owl:Class ;
                    rdfs:subClassOf cco:Facility ;
                    cco:definition_source "https://en.wikipedia.org/w/index.php?title=Washing&oldid=1035998791"^^xsd:anyURI ;
                    cco:is_curated_in_ontology "http://www.ontologyrepository.com/CommonCoreOntologies/Mid/FacilityOntology"^^xsd:anyURI ;
                    rdfs:label "Washing Facility"@en ;
                    <http://www.w3.org/2004/02/skos/core#definition> "A Facility that is designed to wash personnel or equipment."@en .


###  http://www.ontologyrepository.com/CommonCoreOntologies/WasteManagementFacility
cco:WasteManagementFacility rdf:type owl:Class ;
                            rdfs:subClassOf cco:Facility ;
                            cco:definition_source "https://en.wikipedia.org/w/index.php?title=Waste_management&oldid=1062844209"^^xsd:anyURI ;
                            cco:is_curated_in_ontology "http://www.ontologyrepository.com/CommonCoreOntologies/Mid/FacilityOntology"^^xsd:anyURI ;
                            rdfs:label "Waste Management Facility"@en ;
                            <http://www.w3.org/2004/02/skos/core#definition> "A Facility that is designed for managing waste for some portion of the waste's existence."@en .


###  http://www.ontologyrepository.com/CommonCoreOntologies/WaterTower
cco:WaterTower rdf:type owl:Class ;
               rdfs:subClassOf cco:StorageFacility ;
               cco:definition_source "https://en.wikipedia.org/w/index.php?title=Water_tower&oldid=1059754959"^^xsd:anyURI ;
               cco:is_curated_in_ontology "http://www.ontologyrepository.com/CommonCoreOntologies/Mid/FacilityOntology"^^xsd:anyURI ;
               rdfs:label "Water Tower"@en ;
               <http://www.w3.org/2004/02/skos/core#definition> "A Facility that is the bearer of functions realized in processes of storing water in an elevated container."@en .


###  http://www.ontologyrepository.com/CommonCoreOntologies/WaterTreatmentFacility
cco:WaterTreatmentFacility rdf:type owl:Class ;
                           rdfs:subClassOf cco:Facility ;
                           cco:definition_source "https://en.wikipedia.org/w/index.php?title=Water_treatment&oldid=1061706931"^^xsd:anyURI ;
                           cco:is_curated_in_ontology "http://www.ontologyrepository.com/CommonCoreOntologies/Mid/FacilityOntology"^^xsd:anyURI ;
                           rdfs:label "Water Treatment Facility"@en ;
                           <http://www.w3.org/2004/02/skos/core#definition> "A Facility that is designed for making water more acceptable for a specific end-use."@en .


###  http://www.ontologyrepository.com/CommonCoreOntologies/WeaponManufacturingFacility
cco:WeaponManufacturingFacility rdf:type owl:Class ;
                                rdfs:subClassOf cco:Factory ;
                                cco:definition_source "https://en.wikipedia.org/w/index.php?title=Arms_industry&oldid=1063811497"^^xsd:anyURI ;
                                cco:is_curated_in_ontology "http://www.ontologyrepository.com/CommonCoreOntologies/Mid/FacilityOntology"^^xsd:anyURI ;
                                rdfs:label "Weapon Manufacturing Facility"@en ;
                                <http://www.w3.org/2004/02/skos/core#definition> "A Factory that is designed to produce or assemble weapons."@en .


###  http://www.ontologyrepository.com/CommonCoreOntologies/WindFarm
cco:WindFarm rdf:type owl:Class ;
             rdfs:subClassOf cco:ElectricPowerStation ;
             cco:definition_source "https://en.wikipedia.org/w/index.php?title=Wind_farm&oldid=1062817899"^^xsd:anyURI ;
             cco:is_curated_in_ontology "http://www.ontologyrepository.com/CommonCoreOntologies/Mid/FacilityOntology"^^xsd:anyURI ;
             rdfs:label "Wind Farm"@en ;
             <http://www.w3.org/2004/02/skos/core#definition> "An Electric Power Station that is designed to convert the wind's kinetic energy into electrical power by means of wind turbines."@en .


###  Generated by the OWL API (version 4.5.29) https://github.com/owlcs/owlapi
