@prefix : <https://www.commoncoreontologies.org/QualityOntology/> .
@prefix cco: <https://www.commoncoreontologies.org/> .
@prefix obo: <http://purl.obolibrary.org/obo/> .
@prefix owl: <http://www.w3.org/2002/07/owl#> .
@prefix rdf: <http://www.w3.org/1999/02/22-rdf-syntax-ns#> .
@prefix xml: <http://www.w3.org/XML/1998/namespace> .
@prefix xsd: <http://www.w3.org/2001/XMLSchema#> .
@prefix cco: <https://www.commoncoreontologies.org/> .
@prefix rdfs: <http://www.w3.org/2000/01/rdf-schema#> .
@prefix skos: <http://www.w3.org/2004/02/skos/core#> .
@prefix dcterms: <http://purl.org/dc/terms/> .
@base <https://www.commoncoreontologies.org/QualityOntology> .

<https://www.commoncoreontologies.org/QualityOntology> rdf:type owl:Ontology ;
                                                                              owl:versionIRI <https://www.commoncoreontologies.org/2024-11-06/QualityOntology> ;
                                                                              owl:imports <https://www.commoncoreontologies.org/InformationEntityOntology> ;
                                                                              dcterms:license "BSD 3-Clause: https://github.com/CommonCoreOntology/CommonCoreOntologies/blob/master/LICENSE"@en ;
                                                                              dcterms:rights "CUBRC Inc., see full license."@en ;
                                                                              rdfs:comment "This ontology is designed to represent a range of attributes of entities especially qualities, realizable entities, and process profiles."@en ;
                                                                              rdfs:label "Quality Ontology"@en ;
                                                                              owl:versionInfo "Version 2.0"@en .

#################################################################
#    Annotation properties
#################################################################

###  http://purl.org/dc/terms/bibliographicCitation
dcterms:bibliographicCitation rdf:type owl:AnnotationProperty .


###  http://purl.org/dc/terms/rights
dcterms:rights rdf:type owl:AnnotationProperty .


###  https://www.commoncoreontologies.org/ont00001754
cco:ont00001754 rdf:type owl:AnnotationProperty .


###  https://www.commoncoreontologies.org/ont00001760
cco:ont00001760 rdf:type owl:AnnotationProperty .


#################################################################
#    Classes
#################################################################

###  https://www.commoncoreontologies.org/ont00000009
cco:ont00000009 rdf:type owl:Class ;
                rdfs:subClassOf obo:BFO_0000019 ;
                rdfs:label "Mass Density"@en ;
                skos:altLabel "Density"@en ;
                skos:definition "A Quality that inheres in a bearer in virtue of that bearer's mass per unit volume."@en ;
                cco:ont00001760 "https://www.commoncoreontologies.org/QualityOntology"^^xsd:anyURI .


###  https://www.commoncoreontologies.org/ont00000042
cco:ont00000042 rdf:type owl:Class ;
                rdfs:subClassOf cco:ont00001059 ;
                rdfs:label "Semicircular"@en ;
                skos:definition "A Shape quality inhering in a bearer in virtue of the bearer having the shape of half a circle."@en ;
                cco:ont00001760 "https://www.commoncoreontologies.org/QualityOntology"^^xsd:anyURI .


###  https://www.commoncoreontologies.org/ont00000082
cco:ont00000082 rdf:type owl:Class ;
                rdfs:subClassOf cco:ont00000378 ;
                rdfs:label "Green"@en ;
                skos:definition "A Color that is between Yellow and Cyan with a wavelength in the visible spectrum, typically between 520 to 560 nanometers."@en ;
                cco:ont00001760 "https://www.commoncoreontologies.org/QualityOntology"^^xsd:anyURI .


###  https://www.commoncoreontologies.org/ont00000105
cco:ont00000105 rdf:type owl:Class ;
                rdfs:subClassOf cco:ont00001369 ;
                rdfs:label "Square"@en ;
                skos:definition "A Rectangular shape which has four equal length sides and four 90 degree angles."@en ;
                cco:ont00001760 "https://www.commoncoreontologies.org/QualityOntology"^^xsd:anyURI .


###  https://www.commoncoreontologies.org/ont00000112
cco:ont00000112 rdf:type owl:Class ;
                rdfs:subClassOf cco:ont00001384 ;
                rdfs:label "Translucent"@en ;
                skos:definition "An Opacity that inheres in a bearer in virtue of that bearer's capacity to transmit some but not all electromagnetic radiation of a given frequency through the bearer such that the bearer reflects, scatters, or absorbs some but not all electromagnetic radiation of that frequency."@en ;
                cco:ont00001760 "https://www.commoncoreontologies.org/QualityOntology"^^xsd:anyURI .


###  https://www.commoncoreontologies.org/ont00000119
cco:ont00000119 rdf:type owl:Class ;
                rdfs:subClassOf obo:BFO_0000145 ;
                rdfs:label "Spatial Orientation"@en ;
                skos:altLabel "Attitude"@en ;
                skos:definition "A Relational Quality that is the angle of Rotation of an Object relative to one or more Plane of Reference or Axis of Rotation."@en ;
                cco:ont00001754 "https://en.wikipedia.org/wiki/Orientation_(geometry)" ;
                cco:ont00001760 "https://www.commoncoreontologies.org/QualityOntology"^^xsd:anyURI .


###  https://www.commoncoreontologies.org/ont00000185
cco:ont00000185 rdf:type owl:Class ;
                rdfs:subClassOf cco:ont00001059 ;
                rdfs:label "Blunt"@en ;
                skos:definition "A Shape Quality inhering in a bearer in virtue of the bearer not having a sharp edge or point."@en ;
                cco:ont00001760 "https://www.commoncoreontologies.org/QualityOntology"^^xsd:anyURI .


###  https://www.commoncoreontologies.org/ont00000196
cco:ont00000196 rdf:type owl:Class ;
                rdfs:subClassOf cco:ont00000378 ;
                rdfs:label "Purple"@en ;
                skos:definition "A Color that is aproximately midway between Red and Blue."@en ;
                cco:ont00001760 "https://www.commoncoreontologies.org/QualityOntology"^^xsd:anyURI .


###  https://www.commoncoreontologies.org/ont00000257
cco:ont00000257 rdf:type owl:Class ;
                rdfs:subClassOf cco:ont00000620 ;
                rdfs:label "Radiopaque"@en ;
                skos:altLabel "Radiodense"@en ;
                skos:definition "A Radiopacity that inheres in a bearer in virtue of its capacity to prevent most X-rays from passing through it."@en ;
                cco:ont00001760 "https://www.commoncoreontologies.org/QualityOntology"^^xsd:anyURI .


###  https://www.commoncoreontologies.org/ont00000281
cco:ont00000281 rdf:type owl:Class ;
                rdfs:subClassOf cco:ont00001137 ;
                rdfs:label "Albedo"@en ;
                skos:definition "A Radiation Reflectivity that inheres in a bearer in virtue of the capacity of its surface to reflect incident electromagnetic radiation of a particular wavelength."@en ;
                skos:scopeNote "Albedo is a reflection coefficient and is measured as the ratio of radiation reflected from the surface to the incident radiation. Albedo is dimensionless, can be expressed as a percentage, and is measured on a scale from 0 for no reflection to 1 for perfect reflection of a surface. Albedo depends on the wavelength of the radiation; when no wavelength is specified, it typically refers to some appropriate average across the spectrum of visible light."@en ;
                cco:ont00001754 "https://en.wikipedia.org/w/index.php?title=Albedo&oldid=1063352646"^^xsd:anyURI ;
                cco:ont00001760 "https://www.commoncoreontologies.org/QualityOntology"^^xsd:anyURI .


###  https://www.commoncoreontologies.org/ont00000283
cco:ont00000283 rdf:type owl:Class ;
                rdfs:subClassOf cco:ont00001360 ;
                rdfs:label "Cylindrical"@en ;
                skos:altLabel "Columnar"@en ;
                skos:definition "A Three Dimensional Shape inhering in a bearer in virtue of the bearer having an elongated shape with round bases."@en ;
                cco:ont00001760 "https://www.commoncoreontologies.org/QualityOntology"^^xsd:anyURI .


###  https://www.commoncoreontologies.org/ont00000284
cco:ont00000284 rdf:type owl:Class ;
                rdfs:subClassOf obo:BFO_0000017 ;
                rdfs:label "Strength"@en ;
                skos:definition "A Realizable Entity that is realized when its bearer exerts or resists some power, influence, or force."@en ;
                skos:scopeNote "Strength is intended to be understood broadly here. Physical strength is only one type of Strength. Other subtypes of Strength may include military strength, psychological strength, emotional strength, political strength, technological strength, and so on."@en ;
                cco:ont00001760 "https://www.commoncoreontologies.org/QualityOntology"^^xsd:anyURI .


###  https://www.commoncoreontologies.org/ont00000295
cco:ont00000295 rdf:type owl:Class ;
                rdfs:subClassOf obo:BFO_0000019 ;
                rdfs:label "Wetness"@en ;
                skos:definition "A Quality that inheres in a bearer in virtue of the degree to which the bearer is covered by a liquid, typically on a continuum of dry to wet."@en ;
                cco:ont00001760 "https://www.commoncoreontologies.org/QualityOntology"^^xsd:anyURI .


###  https://www.commoncoreontologies.org/ont00000324
cco:ont00000324 rdf:type owl:Class ;
                rdfs:subClassOf cco:ont00001367 ;
                rdfs:label "Width"@en ;
                skos:definition "A One Dimensional Extent that inheres in a bearer in virtue of the bearer's extension in a horizontal direction."@en ;
                cco:ont00001754 "International Organization for Standardization. 2019. Quantities and units -- Part 3: Space and time (ISO 80000-3:2019). International Organization for Standardization. Available at: https://www.iso.org/standard/64974.html."@en ;
                cco:ont00001760 "https://www.commoncoreontologies.org/QualityOntology"^^xsd:anyURI .


###  https://www.commoncoreontologies.org/ont00000327
cco:ont00000327 rdf:type owl:Class ;
                rdfs:subClassOf obo:BFO_0000019 ;
                rdfs:label "Texture"@en ;
                skos:definition "A Quality that inheres in a bearer in virtue of the size, shape, and distribution of features on its surface, typically on a continuum from smooth to rough."@en ;
                cco:ont00001760 "https://www.commoncoreontologies.org/QualityOntology"^^xsd:anyURI .


###  https://www.commoncoreontologies.org/ont00000378
cco:ont00000378 rdf:type owl:Class ;
                rdfs:subClassOf cco:ont00000784 ;
                rdfs:label "Color"@en ;
                skos:definition "An Optical Property that inheres in a bearer in virtue of that bearer's Color Hue, Color Saturation and Color Brightness."@en ;
                cco:ont00001760 "https://www.commoncoreontologies.org/QualityOntology"^^xsd:anyURI .


###  https://www.commoncoreontologies.org/ont00000385
cco:ont00000385 rdf:type owl:Class ;
                rdfs:subClassOf cco:ont00001059 ;
                rdfs:label "Wide"@en ;
                skos:altLabel "Broad"@en ,
                              "Fat"@en ;
                skos:definition "A Shape Quality inhering in a bearer in virtue of the bearer having a width or depth which is significantly larger in proportion to its length or height."@en ;
                cco:ont00001760 "https://www.commoncoreontologies.org/QualityOntology"^^xsd:anyURI .


###  https://www.commoncoreontologies.org/ont00000424
cco:ont00000424 rdf:type owl:Class ;
                rdfs:subClassOf cco:ont00001059 ;
                rdfs:label "Sharp"@en ;
                skos:definition "A Shape Quality inhering in a bearer in virtue of the bearer having a fine point or thin edge."@en ;
                cco:ont00001760 "https://www.commoncoreontologies.org/QualityOntology"^^xsd:anyURI .


###  https://www.commoncoreontologies.org/ont00000439
cco:ont00000439 rdf:type owl:Class ;
                rdfs:subClassOf cco:ont00000378 ;
                rdfs:label "Black"@en ;
                skos:definition "A Color that lacks any hues as parts."@en ;
                cco:ont00001760 "https://www.commoncoreontologies.org/QualityOntology"^^xsd:anyURI .


###  https://www.commoncoreontologies.org/ont00000441
cco:ont00000441 rdf:type owl:Class ;
                rdfs:subClassOf obo:BFO_0000019 ;
                rdfs:label "Temperature"@en ;
                skos:definition "A Quality that inheres in a bearer in virtue of its thermal energy."@en ;
                cco:ont00001760 "https://www.commoncoreontologies.org/QualityOntology"^^xsd:anyURI .


###  https://www.commoncoreontologies.org/ont00000442
cco:ont00000442 rdf:type owl:Class ;
                rdfs:subClassOf obo:BFO_0000019 ;
                rdfs:label "Radioactive"@en ;
                skos:definition "A Quality that inheres in a bearer in virtue of that bearer exhibiting or being caused by radioactivity."@en ;
                cco:ont00001760 "https://www.commoncoreontologies.org/QualityOntology"^^xsd:anyURI .


###  https://www.commoncoreontologies.org/ont00000446
cco:ont00000446 rdf:type owl:Class ;
                rdfs:subClassOf cco:ont00001293 ;
                rdfs:label "Circumference"@en ;
                skos:definition "A Perimeter that inheres in a circle or ellipse."@en ;
                cco:ont00001760 "https://www.commoncoreontologies.org/QualityOntology"^^xsd:anyURI .


###  https://www.commoncoreontologies.org/ont00000447
cco:ont00000447 rdf:type owl:Class ;
                rdfs:subClassOf cco:ont00001059 ;
                rdfs:label "Triangular"@en ;
                skos:definition "A Shape Quality inhering in a bearer in virtue of it having exactly three angles and exactly three sides."@en ;
                cco:ont00001760 "https://www.commoncoreontologies.org/QualityOntology"^^xsd:anyURI .


###  https://www.commoncoreontologies.org/ont00000450
cco:ont00000450 rdf:type owl:Class ;
                rdfs:subClassOf cco:ont00000378 ;
                rdfs:label "Silver Color"@en ;
                skos:definition "A Color that resembles Grey with the added feature of having a metallic shine."@en ;
                cco:ont00001760 "https://www.commoncoreontologies.org/QualityOntology"^^xsd:anyURI .


###  https://www.commoncoreontologies.org/ont00000459
cco:ont00000459 rdf:type owl:Class ;
                rdfs:subClassOf cco:ont00001126 ;
                rdfs:label "Fluorescence"@en ;
                skos:definition "A Luminescent Property that inheres in a bearer in virtue of that bearer's capacity to emit visible light while absorbing shorter wavelength radiation, but not after."@en ;
                cco:ont00001754 "https://en.wikipedia.org/w/index.php?title=Fluorescence&oldid=1061358510"^^xsd:anyURI ;
                cco:ont00001760 "https://www.commoncoreontologies.org/QualityOntology"^^xsd:anyURI .


###  https://www.commoncoreontologies.org/ont00000464
cco:ont00000464 rdf:type owl:Class ;
                rdfs:subClassOf cco:ont00001059 ;
                rdfs:label "Oblong"@en ;
                skos:definition "A Shape Quality inhering in a bearer in virtue of the bearer having an long thin shape with approximately parallel sides."@en ;
                cco:ont00001760 "https://www.commoncoreontologies.org/QualityOntology"^^xsd:anyURI .


###  https://www.commoncoreontologies.org/ont00000474
cco:ont00000474 rdf:type owl:Class ;
                rdfs:subClassOf cco:ont00001059 ;
                rdfs:label "Curved"@en ;
                skos:definition "A Shape Quality inhering in a bearer in virtue of the bearer having borders which are smoothly rounded."@en ;
                cco:ont00001760 "https://www.commoncoreontologies.org/QualityOntology"^^xsd:anyURI .


###  https://www.commoncoreontologies.org/ont00000478
cco:ont00000478 rdf:type owl:Class ;
                rdfs:subClassOf cco:ont00001360 ;
                rdfs:label "Cuboidal"@en ;
                skos:definition "A Three Dimensional Shape that inheres in a bearer in virtue of it having six Rectangular faces."@en ;
                cco:ont00001760 "https://www.commoncoreontologies.org/QualityOntology"^^xsd:anyURI .


###  https://www.commoncoreontologies.org/ont00000484
cco:ont00000484 rdf:type owl:Class ;
                rdfs:subClassOf cco:ont00001059 ;
                rdfs:label "Concave Shape"@en ;
                skos:definition "A Shape Quality that inheres in a bearer in virtue of the bearer having one or more cavities, such that at least one line connecting a pair of points on the surface of the bearer will lie outside."@en ;
                cco:ont00001760 "https://www.commoncoreontologies.org/QualityOntology"^^xsd:anyURI .


###  https://www.commoncoreontologies.org/ont00000494
cco:ont00000494 rdf:type owl:Class ;
                rdfs:subClassOf cco:ont00001059 ;
                rdfs:label "Serrated"@en ;
                skos:definition "A Shape Quality inhering in a bearer in virtue of the bearer having multiple sharp points along a edge."@en ;
                cco:ont00001760 "https://www.commoncoreontologies.org/QualityOntology"^^xsd:anyURI .


###  https://www.commoncoreontologies.org/ont00000512
cco:ont00000512 rdf:type owl:Class ;
                rdfs:subClassOf cco:ont00000628 ;
                rdfs:label "Radiation Emissivity"@en ;
                skos:definition "An Electromagnetic Radiation Property that inheres in a bearer in virtue of the capacity of that bearer to emit electromagnetic radiation of a given frequency."@en ;
                cco:ont00001760 "https://www.commoncoreontologies.org/QualityOntology"^^xsd:anyURI .


###  https://www.commoncoreontologies.org/ont00000525
cco:ont00000525 rdf:type owl:Class ;
                rdfs:subClassOf cco:ont00001384 ;
                rdfs:label "Transparent"@en ;
                skos:definition "An Opacity that inheres in a bearer in virtue of that bearer's capacity to transmit all or nearly all electromagnetic radiation of a given frequency through the bearer such that the bearer reflects, scatters, or absorbs little or no electromagnetic radiation of that frequency."@en ;
                cco:ont00001760 "https://www.commoncoreontologies.org/QualityOntology"^^xsd:anyURI .


###  https://www.commoncoreontologies.org/ont00000528
cco:ont00000528 rdf:type owl:Class ;
                rdfs:subClassOf cco:ont00000378 ;
                rdfs:label "White"@en ;
                skos:definition "A Color of maximum brightness, the color of objects that reflect nearly all wavelengths of the visible light spectrum, thus considered achromatic."@en ;
                cco:ont00001760 "https://www.commoncoreontologies.org/QualityOntology"^^xsd:anyURI .


###  https://www.commoncoreontologies.org/ont00000541
cco:ont00000541 rdf:type owl:Class ;
                rdfs:subClassOf cco:ont00001367 ;
                rdfs:label "Diameter"@en ;
                skos:definition "A One Dimensional Extent that inheres in a circle in virtue of the extent of a straight line that passes through the center of the circle and starts and ends on the circle's boundary."@en ;
                cco:ont00001754 "International Organization for Standardization. 2019. Quantities and units -- Part 3: Space and time (ISO 80000-3:2019). International Organization for Standardization. Available at: https://www.iso.org/standard/64974.html."@en ;
                cco:ont00001760 "https://www.commoncoreontologies.org/QualityOntology"^^xsd:anyURI .


###  https://www.commoncoreontologies.org/ont00000548
cco:ont00000548 rdf:type owl:Class ;
                rdfs:subClassOf cco:ont00000997 ;
                dcterms:bibliographicCitation "Vulnerability | Definition of Vulnerability by Oxford Dictionary on Lexico.Com Also Meaning of Vulnerability. https://web.archive.org/web/20210118111731/https://www.lexico.com/en/definition/vulnerability. Accessed 19 Dec. 2022. " ;
                dcterms:creator "https://cubrc.org"^^xsd:anyURI ;
                rdfs:label "Vulnerability"@en ;
                skos:definition "A Disrupting Disposition the realization of which would disrupt a process that the bearer of the Disrupting Disposition has an interest in."@en ;
                skos:editorialNote "This is defined class. A Vulnerability is indexed by the interest_in object property. A disposition can be a Vulnerability according to one index and not a Vulnerability according to another index." ;
                skos:prefLabel "Vulnerability"@en ;
                cco:ont00001760 "https://www.commoncoreontologies.org/QualityOntology"^^xsd:anyURI .


###  https://www.commoncoreontologies.org/ont00000560
cco:ont00000560 rdf:type owl:Class ;
                rdfs:subClassOf cco:ont00001360 ;
                rdfs:label "Cone Shape"@en ;
                skos:definition "A Three Dimensional Shape that inheres in a bearer in virtue of it having a Round base that tapers smoothly to an apex."@en ;
                cco:ont00001754 "https://en.wikipedia.org/w/index.php?title=Cone&oldid=1058362269"^^xsd:anyURI ;
                cco:ont00001760 "https://www.commoncoreontologies.org/QualityOntology"^^xsd:anyURI .


###  https://www.commoncoreontologies.org/ont00000565
cco:ont00000565 rdf:type owl:Class ;
                rdfs:subClassOf cco:ont00000478 ;
                rdfs:label "Cube Shape"@en ;
                skos:definition "A Cuboidal shape inhering in a bearer in virtue of it having six Square faces."@en ;
                cco:ont00001760 "https://www.commoncoreontologies.org/QualityOntology"^^xsd:anyURI .


###  https://www.commoncoreontologies.org/ont00000578
cco:ont00000578 rdf:type owl:Class ;
                rdfs:subClassOf cco:ont00001059 ;
                rdfs:label "Sloped"@en ;
                skos:definition "A Shape Quality inhering in a bearer in virtue of the bearer having a horizontal border which is not level."@en ;
                cco:ont00001760 "https://www.commoncoreontologies.org/QualityOntology"^^xsd:anyURI .


###  https://www.commoncoreontologies.org/ont00000579
cco:ont00000579 rdf:type owl:Class ;
                rdfs:subClassOf cco:ont00001059 ;
                rdfs:label "Thin"@en ;
                skos:altLabel "Narrow"@en ,
                              "Slender"@en ;
                skos:definition "A Shape Quality inhering in a bearer in virtue of the bearer having a width or depth which is significantly smaller in proportion to its length or height."@en ;
                cco:ont00001760 "https://www.commoncoreontologies.org/QualityOntology"^^xsd:anyURI .


###  https://www.commoncoreontologies.org/ont00000590
cco:ont00000590 rdf:type owl:Class ;
                rdfs:subClassOf cco:ont00001059 ;
                rdfs:label "Convex Shape"@en ;
                skos:definition "A Shape Quality that inheres in a bearer in virtue of the bearer not having a cavity, such that no line connecting a pair of points on the surface of the bearer will lie outside."@en ;
                cco:ont00001760 "https://www.commoncoreontologies.org/QualityOntology"^^xsd:anyURI .


###  https://www.commoncoreontologies.org/ont00000607
cco:ont00000607 rdf:type owl:Class ;
                rdfs:subClassOf cco:ont00000892 ;
                rdfs:label "Thickness"@en ;
                skos:definition "A Depth that inheres in a bearer in virtue of it extending inward through an object."@en ;
                cco:ont00001754 "International Organization for Standardization. 2019. Quantities and units -- Part 3: Space and time (ISO 80000-3:2019). International Organization for Standardization. Available at: https://www.iso.org/standard/64974.html."@en ;
                cco:ont00001760 "https://www.commoncoreontologies.org/QualityOntology"^^xsd:anyURI .


###  https://www.commoncoreontologies.org/ont00000614
cco:ont00000614 rdf:type owl:Class ;
                rdfs:subClassOf obo:BFO_0000019 ;
                rdfs:comment "'Matter' here can also refer to the inertial energy of an object."@en ,
                             "Typical unit of measure is the kilogram or pound."@en ;
                rdfs:label "Mass"@en ;
                skos:definition "A Quality that inheres in a bearer in virtue of the amount of matter in that bearer."@en ;
                cco:ont00001760 "https://www.commoncoreontologies.org/QualityOntology"^^xsd:anyURI .


###  https://www.commoncoreontologies.org/ont00000620
cco:ont00000620 rdf:type owl:Class ;
                rdfs:subClassOf cco:ont00001384 ;
                rdfs:label "Radiopacity"@en ;
                skos:altLabel "Radiodensity"@en ;
                skos:definition "An Opacity that inheres in a bearer in virtue of its capacity to allow or prevent X-rays to pass through it."@en ;
                cco:ont00001754 "https://en.wikipedia.org/w/index.php?title=Radiodensity&oldid=1048274724"^^xsd:anyURI ;
                cco:ont00001760 "https://www.commoncoreontologies.org/QualityOntology"^^xsd:anyURI .


###  https://www.commoncoreontologies.org/ont00000628
cco:ont00000628 rdf:type owl:Class ;
                rdfs:subClassOf obo:BFO_0000016 ;
                rdfs:label "Electromagnetic Radiation Property"@en ;
                skos:definition "A Disposition that inheres in an bearer in virtue of how that bearer interacts with electromagnetic radiation."@en ;
                cco:ont00001760 "https://www.commoncoreontologies.org/QualityOntology"^^xsd:anyURI .


###  https://www.commoncoreontologies.org/ont00000632
cco:ont00000632 rdf:type owl:Class ;
                rdfs:subClassOf obo:BFO_0000016 ;
                rdfs:label "Magnetism"@en ;
                skos:definition "A Disposition that is realized when its bearer exerts a magnetic force on another entity."@en ;
                cco:ont00001760 "https://www.commoncoreontologies.org/QualityOntology"^^xsd:anyURI .


###  https://www.commoncoreontologies.org/ont00000633
cco:ont00000633 rdf:type owl:Class ;
                rdfs:subClassOf obo:BFO_0000019 ;
                rdfs:comment "When an object is \"weighed\", in the typical case, it is done so by taking into account the local force of gravity to determine the object's mass, whose standard of measure is the kilogram. The actual unit of measure of weight is the newton."@en ;
                rdfs:label "Weight"@en ;
                skos:definition "A Quality that inheres in some material entity with a mass in virtue of its location in some gravitational field."@en ;
                cco:ont00001760 "https://www.commoncoreontologies.org/QualityOntology"^^xsd:anyURI .


###  https://www.commoncoreontologies.org/ont00000648
cco:ont00000648 rdf:type owl:Class ;
                rdfs:subClassOf cco:ont00000784 ;
                rdfs:label "Color Brightness"@en ;
                skos:altLabel "Color Intensity"@en ;
                skos:definition "An Optical Property that inheres in a bearer in virtue of its capacity to reflect or radiate light."@en ;
                cco:ont00001760 "https://www.commoncoreontologies.org/QualityOntology"^^xsd:anyURI .


###  https://www.commoncoreontologies.org/ont00000695
cco:ont00000695 rdf:type owl:Class ;
                rdfs:subClassOf cco:ont00000620 ;
                rdfs:label "Radiolucent"@en ;
                skos:altLabel "Hypodense"@en ,
                              "Transradiance"@en ;
                skos:definition "A Radiopacity that inheres in a bearer in virtue of its capacity to permit most X-rays to pass through it."@en ;
                cco:ont00001760 "https://www.commoncoreontologies.org/QualityOntology"^^xsd:anyURI .


###  https://www.commoncoreontologies.org/ont00000733
cco:ont00000733 rdf:type owl:Class ;
                rdfs:subClassOf cco:ont00001360 ;
                rdfs:label "Spherical"@en ;
                skos:definition "A Three Dimensional Shape inhering in a bearer in virtue of all of its cross sections being round."@en ;
                cco:ont00001760 "https://www.commoncoreontologies.org/QualityOntology"^^xsd:anyURI .


###  https://www.commoncoreontologies.org/ont00000738
cco:ont00000738 rdf:type owl:Class ;
                rdfs:subClassOf cco:ont00001367 ;
                rdfs:label "Length"@en ;
                skos:definition "A One Dimensional Extent that inheres in a bearer in virtue of the bearer's greatest extent in one direction."@en ;
                cco:ont00001754 "International Organization for Standardization. 2019. Quantities and units -- Part 3: Space and time (ISO 80000-3:2019). International Organization for Standardization. Available at: https://www.iso.org/standard/64974.html."@en ;
                cco:ont00001760 "https://www.commoncoreontologies.org/QualityOntology"^^xsd:anyURI .


###  https://www.commoncoreontologies.org/ont00000759
cco:ont00000759 rdf:type owl:Class ;
                rdfs:subClassOf cco:ont00000784 ;
                rdfs:label "Color Saturation"@en ;
                skos:definition "An Optical Property that inheres in a bearer in virtue of its capacity to reflect high intensity light distributed across fewer wavelengths, typically considered on a continuum of purity."@en ;
                cco:ont00001760 "https://www.commoncoreontologies.org/QualityOntology"^^xsd:anyURI .


###  https://www.commoncoreontologies.org/ont00000766
cco:ont00000766 rdf:type owl:Class ;
                rdfs:subClassOf obo:BFO_0000019 ;
                rdfs:label "Hardness"@en ;
                skos:definition "A Quality that inheres in a bearer in virtue of the degree to which it can be turned, bowed, or twisted without breaking."@en ;
                cco:ont00001760 "https://www.commoncoreontologies.org/QualityOntology"^^xsd:anyURI .


###  https://www.commoncoreontologies.org/ont00000768
cco:ont00000768 rdf:type owl:Class ;
                rdfs:subClassOf obo:BFO_0000019 ;
                rdfs:label "Amount"@en ;
                skos:definition "A Quality that inheres in a bearer in virtue of the total, aggregate or sum of a number of discrete items or material the entity contains as parts."@en ;
                cco:ont00001754 "http://en.wiktionary.org/wiki/amount" ;
                cco:ont00001760 "https://www.commoncoreontologies.org/QualityOntology"^^xsd:anyURI .


###  https://www.commoncoreontologies.org/ont00000784
cco:ont00000784 rdf:type owl:Class ;
                rdfs:subClassOf cco:ont00000628 ;
                rdfs:label "Optical Property"@en ;
                skos:definition "An Electromagnetic Radiation Property that is realized when its bearer interacts with electromagnetic waves within the visible light spectrum."@en ;
                cco:ont00001760 "https://www.commoncoreontologies.org/QualityOntology"^^xsd:anyURI .


###  https://www.commoncoreontologies.org/ont00000787
cco:ont00000787 rdf:type owl:Class ;
                rdfs:subClassOf cco:ont00000967 ;
                rdfs:label "Altitude"@en ;
                skos:definition "A Height that inheres in a Site that externally connects an Independent Continuant to either the surface of the Earth or the Earth's mean Sea Level."@en ;
                cco:ont00001754 "International Organization for Standardization. 2019. Quantities and units -- Part 3: Space and time (ISO 80000-3:2019). International Organization for Standardization. Available at: https://www.iso.org/standard/64974.html."@en ;
                cco:ont00001760 "https://www.commoncoreontologies.org/QualityOntology"^^xsd:anyURI .


###  https://www.commoncoreontologies.org/ont00000797
cco:ont00000797 rdf:type owl:Class ;
                rdfs:subClassOf cco:ont00000378 ;
                rdfs:label "Hazel"@en ;
                skos:definition "A Color that is a combination of Brown and Green, typically associated with eye color."@en ;
                cco:ont00001760 "https://www.commoncoreontologies.org/QualityOntology"^^xsd:anyURI .


###  https://www.commoncoreontologies.org/ont00000803
cco:ont00000803 rdf:type owl:Class ;
                rdfs:subClassOf cco:ont00001059 ;
                rdfs:label "Round"@en ;
                skos:altLabel "Circular"@en ;
                skos:definition "A Shape Quality that inheres in a bearer in virtue of every point along its circumference being equidistant from the center."@en ;
                cco:ont00001754 "http://www.merriam-webster.com/dictionary/round" ;
                cco:ont00001760 "https://www.commoncoreontologies.org/QualityOntology"^^xsd:anyURI .


###  https://www.commoncoreontologies.org/ont00000805
cco:ont00000805 rdf:type owl:Class ;
                rdfs:subClassOf cco:ont00001059 ;
                rdfs:label "Coiled"@en ;
                skos:definition "A Shape Quality inhering in a bearer in virtue of the bearer being wound in concentric rings or spirals."@en ;
                cco:ont00001760 "https://www.commoncoreontologies.org/QualityOntology"^^xsd:anyURI .


###  https://www.commoncoreontologies.org/ont00000815
cco:ont00000815 rdf:type owl:Class ;
                rdfs:subClassOf cco:ont00001059 ;
                rdfs:label "Folded"@en ;
                skos:definition "A Shape Quality inhering in a bearer in virtue of one part of the bearer being layered over another connected part."@en ;
                cco:ont00001760 "https://www.commoncoreontologies.org/QualityOntology"^^xsd:anyURI .


###  https://www.commoncoreontologies.org/ont00000818
cco:ont00000818 rdf:type owl:Class ;
                rdfs:subClassOf cco:ont00000378 ;
                rdfs:label "Orange"@en ;
                skos:definition "A Color that is between Red and Yellow with a wavelength in the visible spectrum typically between 590 to 635 nanometers."@en ;
                cco:ont00001760 "https://www.commoncoreontologies.org/QualityOntology"^^xsd:anyURI .


###  https://www.commoncoreontologies.org/ont00000826
cco:ont00000826 rdf:type owl:Class ;
                rdfs:subClassOf cco:ont00001137 ;
                rdfs:label "Refractivity"@en ;
                skos:definition "A Radiation Reflectivity that inheres in a bearer in virtue of the capacity of that bearer to change the direction of a propagating wave when passing through it."@en ;
                cco:ont00001754 "https://en.wikipedia.org/w/index.php?title=Refractive_index&oldid=1062519140"^^xsd:anyURI ;
                cco:ont00001760 "https://www.commoncoreontologies.org/QualityOntology"^^xsd:anyURI .


###  https://www.commoncoreontologies.org/ont00000835
cco:ont00000835 rdf:type owl:Class ;
                rdfs:subClassOf cco:ont00001059 ;
                rdfs:label "Body Shape"@en ;
                skos:definition "A Shape Quality inhering in a Person's body by virtue of the body's general outline or figure."@en ;
                cco:ont00001760 "https://www.commoncoreontologies.org/QualityOntology"^^xsd:anyURI .


###  https://www.commoncoreontologies.org/ont00000861
cco:ont00000861 rdf:type owl:Class ;
                rdfs:subClassOf cco:ont00001059 ;
                rdfs:label "Split"@en ;
                skos:definition "A Shape Quality inhering in a bearer in virtue of the bearer having a linear opening, or having been divided into parts."@en ;
                cco:ont00001760 "https://www.commoncoreontologies.org/QualityOntology"^^xsd:anyURI .


###  https://www.commoncoreontologies.org/ont00000872
cco:ont00000872 rdf:type owl:Class ;
                rdfs:subClassOf cco:ont00000378 ;
                rdfs:label "Brown"@en ;
                skos:definition "A Color that consists of dark orange and red, and of very low intensity."@en ;
                cco:ont00001760 "https://www.commoncoreontologies.org/QualityOntology"^^xsd:anyURI .


###  https://www.commoncoreontologies.org/ont00000885
cco:ont00000885 rdf:type owl:Class ;
                rdfs:subClassOf cco:ont00001059 ;
                rdfs:label "Wavy"@en ;
                skos:altLabel "Undulate"@en ;
                skos:definition "A Shape Quality inhering in a bearer in virtue of it having a sinuous or rippled border."@en ;
                cco:ont00001760 "https://www.commoncoreontologies.org/QualityOntology"^^xsd:anyURI .


###  https://www.commoncoreontologies.org/ont00000892
cco:ont00000892 rdf:type owl:Class ;
                rdfs:subClassOf cco:ont00001367 ;
                rdfs:label "Depth"@en ;
                skos:definition "A One Dimensional Extent that inheres in a bearer in virtue of the bearer's extension in a downward, backward, or inward direction."@en ;
                cco:ont00001754 "International Organization for Standardization. 2019. Quantities and units -- Part 3: Space and time (ISO 80000-3:2019). International Organization for Standardization. Available at: https://www.iso.org/standard/64974.html."@en ;
                cco:ont00001760 "https://www.commoncoreontologies.org/QualityOntology"^^xsd:anyURI .


###  https://www.commoncoreontologies.org/ont00000912
cco:ont00000912 rdf:type owl:Class ;
                rdfs:subClassOf cco:ont00001360 ;
                rdfs:label "Pyramidal"@en ;
                skos:definition "A Three Dimensional Shape that inheres in a bearer in virtue of it having a polygonal base with vertices that all connect to the same apex to form triangular faces."@en ;
                cco:ont00001754 "https://en.wikipedia.org/wiki/Pyramid_(geometry)" ;
                cco:ont00001760 "https://www.commoncoreontologies.org/QualityOntology"^^xsd:anyURI .


###  https://www.commoncoreontologies.org/ont00000913
cco:ont00000913 rdf:type owl:Class ;
                rdfs:subClassOf cco:ont00000378 ;
                rdfs:label "Maroon"@en ;
                skos:definition "A Color consisting of purple and brown hue."@en ;
                cco:ont00001760 "https://www.commoncoreontologies.org/QualityOntology"^^xsd:anyURI .


###  https://www.commoncoreontologies.org/ont00000941
cco:ont00000941 rdf:type owl:Class ;
                rdfs:subClassOf cco:ont00001126 ;
                rdfs:label "Phosphorescence"@en ;
                skos:definition "A Luminescent Property that inheres in a bearer in virtue of that bearer's capacity to emit visible light after absorbing shorter wavelength radiation, and to continue emitting after the absorbing process has ceased."@en ;
                cco:ont00001754 "https://en.wikipedia.org/w/index.php?title=Phosphorescence&oldid=1060815719"^^xsd:anyURI ;
                cco:ont00001760 "https://www.commoncoreontologies.org/QualityOntology"^^xsd:anyURI .


###  https://www.commoncoreontologies.org/ont00000967
cco:ont00000967 rdf:type owl:Class ;
                rdfs:subClassOf cco:ont00001367 ;
                rdfs:label "Height"@en ;
                skos:definition "A One Dimensional Extent that inheres in a bearer in virtue of the bearer's extension in a vertical direction."@en ;
                cco:ont00001754 "International Organization for Standardization. 2019. Quantities and units -- Part 3: Space and time (ISO 80000-3:2019). International Organization for Standardization. Available at: https://www.iso.org/standard/64974.html."@en ;
                cco:ont00001760 "https://www.commoncoreontologies.org/QualityOntology"^^xsd:anyURI .


###  https://www.commoncoreontologies.org/ont00000975
cco:ont00000975 rdf:type owl:Class ;
                rdfs:subClassOf cco:ont00000378 ;
                rdfs:label "Cyan"@en ;
                skos:definition "A Color that is between Green and Blue with a wavelength in the visible spectrum typically between 490 and 520 nanometers."@en ;
                cco:ont00001760 "https://www.commoncoreontologies.org/QualityOntology"^^xsd:anyURI .


###  https://www.commoncoreontologies.org/ont00000979
cco:ont00000979 rdf:type owl:Class ;
                rdfs:subClassOf obo:BFO_0000019 ;
                rdfs:label "Closure"@en ;
                skos:definition "A Quality that inheres in a bearer in virtue of the degree to which that bearer affords passage or sightline through it via an opening, aperture, orifice, or vent."@en ;
                cco:ont00001760 "https://www.commoncoreontologies.org/QualityOntology"^^xsd:anyURI .


###  https://www.commoncoreontologies.org/ont00000991
cco:ont00000991 rdf:type owl:Class ;
                rdfs:subClassOf cco:ont00001059 ;
                rdfs:label "Bent"@en ;
                skos:altLabel "Angular"@en ,
                              "Kinked"@en ;
                skos:definition "A Shape Quality inhering in a bearer in virtue of the bearer having one or more angles along its border."@en ;
                cco:ont00001760 "https://www.commoncoreontologies.org/QualityOntology"^^xsd:anyURI .


###  https://www.commoncoreontologies.org/ont00000997
cco:ont00000997 rdf:type owl:Class ;
                rdfs:subClassOf obo:BFO_0000016 ;
                dcterms:created "2022-12-30T21:32:27-05:00"^^xsd:dateTime ;
                dcterms:creator "https://cubrc.org"^^xsd:anyURI ;
                rdfs:label "Disrupting Disposition"@en ;
                skos:definition "A disposition the realization of which would disrupt a process some entity has an interest in."@en ;
                skos:editorialNote "This is a defined class. A Disrupting Disposition is indexed by the interest_in object property. A disposition can be a Disrupting Disposition according to one index and not a Disrupting Disposition according to another index." ;
                skos:prefLabel "Threat"@en ;
                cco:ont00001760 "https://www.commoncoreontologies.org/QualityOntology"^^xsd:anyURI .


###  https://www.commoncoreontologies.org/ont00001001
cco:ont00001001 rdf:type owl:Class ;
                rdfs:subClassOf cco:ont00001059 ;
                rdfs:label "Drooping"@en ;
                skos:definition "A Shape Quality inhering in a bearer in virtue of the bearer having a border that hangs downwards."@en ;
                cco:ont00001760 "https://www.commoncoreontologies.org/QualityOntology"^^xsd:anyURI .


###  https://www.commoncoreontologies.org/ont00001026
cco:ont00001026 rdf:type owl:Class ;
                rdfs:subClassOf cco:ont00000119 ;
                rdfs:label "Pointing Orientation"@en ;
                skos:altLabel "Facing Orientation"@en ;
                skos:definition "A Spatial Orientation of a Material Entity in which one or more of its designated components are oriented toward a specified direction."@en ;
                cco:ont00001760 "https://www.commoncoreontologies.org/QualityOntology"^^xsd:anyURI .


###  https://www.commoncoreontologies.org/ont00001055
cco:ont00001055 rdf:type owl:Class ;
                rdfs:subClassOf cco:ont00001059 ;
                rdfs:label "Branched"@en ;
                skos:definition "A Shape Quality inhering in a bearer in virtue of the bearer having subdivisions or offshoots."@en ;
                cco:ont00001760 "https://www.commoncoreontologies.org/QualityOntology"^^xsd:anyURI .


###  https://www.commoncoreontologies.org/ont00001059
cco:ont00001059 rdf:type owl:Class ;
                rdfs:subClassOf obo:BFO_0000019 ;
                rdfs:label "Shape Quality"@en ;
                skos:definition "A Quality that inheres in a bearer in virtue of the ratios between dimensions of external features of that bearer."@en ;
                cco:ont00001760 "https://www.commoncoreontologies.org/QualityOntology"^^xsd:anyURI .


###  https://www.commoncoreontologies.org/ont00001063
cco:ont00001063 rdf:type owl:Class ;
                rdfs:subClassOf cco:ont00001059 ;
                rdfs:label "Straight"@en ;
                skos:altLabel "Linear"@en ;
                skos:definition "A Shape Quality inhering in a bearer in virtue of the bearer not having curves, bends, or angles along its borders."@en ;
                cco:ont00001760 "https://www.commoncoreontologies.org/QualityOntology"^^xsd:anyURI .


###  https://www.commoncoreontologies.org/ont00001065
cco:ont00001065 rdf:type owl:Class ;
                rdfs:subClassOf cco:ont00001202 ;
                rdfs:label "Two Dimensional Extent"@en ;
                skos:altLabel "Area"@en ;
                skos:definition "A Size Quality that inheres in a bearer in virtue of the bearer's extension in two dimensions."@en ;
                cco:ont00001754 "International Organization for Standardization. 2019. Quantities and units -- Part 3: Space and time (ISO 80000-3:2019). International Organization for Standardization. Available at: https://www.iso.org/standard/64974.html."@en ;
                cco:ont00001760 "https://www.commoncoreontologies.org/QualityOntology"^^xsd:anyURI .


###  https://www.commoncoreontologies.org/ont00001079
cco:ont00001079 rdf:type owl:Class ;
                rdfs:subClassOf cco:ont00000378 ;
                rdfs:label "Blond"@en ;
                skos:definition "A Color that ranges from nearly white to a light greyish yellow"@en ;
                cco:ont00001760 "https://www.commoncoreontologies.org/QualityOntology"^^xsd:anyURI .


###  https://www.commoncoreontologies.org/ont00001113
cco:ont00001113 rdf:type owl:Class ;
                rdfs:subClassOf cco:ont00000378 ;
                rdfs:label "Magenta"@en ;
                skos:definition "A Color consisting of red and blue hues."@en ;
                cco:ont00001760 "https://www.commoncoreontologies.org/QualityOntology"^^xsd:anyURI .


###  https://www.commoncoreontologies.org/ont00001118
cco:ont00001118 rdf:type owl:Class ;
                rdfs:subClassOf obo:BFO_0000016 ;
                rdfs:label "Surface Tension"@en ;
                skos:definition "A Disposition that inheres in a liquid and is realized when the cohesive forces of the molecules in the bearer at the surface are greater than the adhesive forces of the molecules in the surrounding air."@en ;
                cco:ont00001754 "https://en.wikipedia.org/w/index.php?title=Surface_tension&oldid=1062753527"^^xsd:anyURI ;
                cco:ont00001760 "https://www.commoncoreontologies.org/QualityOntology"^^xsd:anyURI .


###  https://www.commoncoreontologies.org/ont00001126
cco:ont00001126 rdf:type owl:Class ;
                rdfs:subClassOf cco:ont00000784 ;
                rdfs:comment "There are a variety of photometric measurements, such as luminous flux/power or luminous intensity, whose units are lumen and candela respectively, which attempt to describe properties associated with the perception of light. These are weighted measurements, typically by the luminosity function, as thus exist on the side of information content. It is a point of further development to add the needed intrinsic properties of radiation that such measurements are about."@en ;
                rdfs:label "Luminescent Property"@en ;
                skos:definition "An Optical Property that inheres in a bearer in virtue of that bearer's capacity to emit visible light, but which isn't the result of the bearer being heated."@en ;
                cco:ont00001754 "https://en.wikipedia.org/w/index.php?title=Luminescence&oldid=1050169944"^^xsd:anyURI ;
                cco:ont00001760 "https://www.commoncoreontologies.org/QualityOntology"^^xsd:anyURI .


###  https://www.commoncoreontologies.org/ont00001137
cco:ont00001137 rdf:type owl:Class ;
                rdfs:subClassOf cco:ont00000628 ;
                rdfs:label "Radiation Reflectivity"@en ;
                skos:definition "An Electromagnetic Radiation Property that inheres in a bearer in virtue of the capacity of that bearer to scatter or reflect electromagnetic radiation of a given frequency."@en ;
                cco:ont00001760 "https://www.commoncoreontologies.org/QualityOntology"^^xsd:anyURI .


###  https://www.commoncoreontologies.org/ont00001142
cco:ont00001142 rdf:type owl:Class ;
                rdfs:subClassOf cco:ont00000378 ;
                rdfs:label "Violet"@en ;
                skos:definition "A Color that is lower than Blue with a wavelength in the visible spectrum typically between 400 and 450 nanometers."@en ;
                cco:ont00001760 "https://www.commoncoreontologies.org/QualityOntology"^^xsd:anyURI .


###  https://www.commoncoreontologies.org/ont00001177
cco:ont00001177 rdf:type owl:Class ;
                rdfs:subClassOf cco:ont00000119 ;
                rdfs:label "Roll Orientation"@en ;
                skos:altLabel "Roll"@en ;
                skos:definition "A Spatial Orientation of an Object relative to its Roll Axis."@en ;
                cco:ont00001760 "https://www.commoncoreontologies.org/QualityOntology"^^xsd:anyURI .


###  https://www.commoncoreontologies.org/ont00001182
cco:ont00001182 rdf:type owl:Class ;
                rdfs:subClassOf obo:BFO_0000145 ;
                rdfs:label "Phase Angle"@en ;
                skos:altLabel "Orbital Phase Angle"@en ;
                skos:definition "A Relational Quality that is the angle between the light incident onto an observed Object and the light reflected from the Object."@en ;
                cco:ont00001754 "https://en.wikipedia.org/wiki/Phase_angle_(astronomy)" ;
                cco:ont00001760 "https://www.commoncoreontologies.org/QualityOntology"^^xsd:anyURI .


###  https://www.commoncoreontologies.org/ont00001186
cco:ont00001186 rdf:type owl:Class ;
                rdfs:subClassOf cco:ont00000784 ;
                rdfs:label "Color Hue"@en ;
                skos:definition "An Optical Property that inheres in a bearer in virtue of its capacity to reflect a dominant wavelength of the visible light spectrum, which is typically divided up into 6 to 8 ranges."@en ;
                cco:ont00001760 "https://www.commoncoreontologies.org/QualityOntology"^^xsd:anyURI .


###  https://www.commoncoreontologies.org/ont00001189
cco:ont00001189 rdf:type owl:Class ;
                rdfs:subClassOf cco:ont00000378 ;
                rdfs:label "Blue"@en ;
                skos:definition "A Color that is between Cyan and Violet with a wavelength in the visible spectrum typically between 450 to 490 nanometers."@en ;
                cco:ont00001760 "https://www.commoncoreontologies.org/QualityOntology"^^xsd:anyURI .


###  https://www.commoncoreontologies.org/ont00001193
cco:ont00001193 rdf:type owl:Class ;
                rdfs:subClassOf obo:BFO_0000017 ;
                rdfs:label "Fatigability"@en ;
                skos:definition "A Realizable Entity that is realized when its bearer loses strength and tires quickly."@en ;
                cco:ont00001760 "https://www.commoncoreontologies.org/QualityOntology"^^xsd:anyURI .


###  https://www.commoncoreontologies.org/ont00001199
cco:ont00001199 rdf:type owl:Class ;
                rdfs:subClassOf cco:ont00001059 ;
                rdfs:label "Protruding"@en ;
                skos:definition "A Shape Quality inhering in a part of an object in virtue of the part extending out above or beyond the surface of the object."@en ;
                cco:ont00001760 "https://www.commoncoreontologies.org/QualityOntology"^^xsd:anyURI .


###  https://www.commoncoreontologies.org/ont00001202
cco:ont00001202 rdf:type owl:Class ;
                rdfs:subClassOf obo:BFO_0000019 ;
                rdfs:label "Size Quality"@en ;
                skos:definition "A Quality that inheres in a bearer in virtue of the bearer's extension in one or more dimensions."@en ;
                cco:ont00001760 "https://www.commoncoreontologies.org/QualityOntology"^^xsd:anyURI .


###  https://www.commoncoreontologies.org/ont00001220
cco:ont00001220 rdf:type owl:Class ;
                rdfs:subClassOf cco:ont00001384 ;
                rdfs:label "Opaque"@en ;
                skos:definition "An Opacity that inheres in a bearer in virtue of that bearer's incapacity to transmit electromagnetic radiation of a given frequency through the bearer such that the bearer reflects, scatters, or absorbs all electromagnetic radiation of that frequency."@en ;
                cco:ont00001760 "https://www.commoncoreontologies.org/QualityOntology"^^xsd:anyURI .


###  https://www.commoncoreontologies.org/ont00001225
cco:ont00001225 rdf:type owl:Class ;
                rdfs:subClassOf cco:ont00000378 ;
                rdfs:label "Yellow"@en ;
                skos:definition "A Color that is between Orange and Green with a wavelength in the visible spectrum typically between 560 to 590 nanometers."@en ;
                cco:ont00001760 "https://www.commoncoreontologies.org/QualityOntology"^^xsd:anyURI .


###  https://www.commoncoreontologies.org/ont00001277
cco:ont00001277 rdf:type owl:Class ;
                rdfs:subClassOf cco:ont00000378 ;
                rdfs:label "Red"@en ;
                skos:definition "A Color that is above Orange with a wavelength in the visible spectrum typically between 635 to 700 nanometers."@en ;
                cco:ont00001760 "https://www.commoncoreontologies.org/QualityOntology"^^xsd:anyURI .


###  https://www.commoncoreontologies.org/ont00001280
cco:ont00001280 rdf:type owl:Class ;
                rdfs:subClassOf cco:ont00001059 ;
                rdfs:label "Flat"@en ;
                skos:definition "A Shape Quality inhering in a bearer in virtue of the bearer having a horizontal border without a significant deviation."@en ;
                cco:ont00001760 "https://www.commoncoreontologies.org/QualityOntology"^^xsd:anyURI .


###  https://www.commoncoreontologies.org/ont00001291
cco:ont00001291 rdf:type owl:Class ;
                rdfs:subClassOf cco:ont00000628 ;
                rdfs:label "Radiation Absorptivity"@en ;
                skos:definition "An Electromagnetic Radiation Property that inheres in a bearer in virtue of the capacity of that bearer to absorb electromagnetic radiation of a given frequency."@en ;
                cco:ont00001760 "https://www.commoncoreontologies.org/QualityOntology"^^xsd:anyURI .


###  https://www.commoncoreontologies.org/ont00001293
cco:ont00001293 rdf:type owl:Class ;
                rdfs:subClassOf cco:ont00001367 ;
                rdfs:label "Perimeter"@en ;
                skos:definition "A One Dimensional Extent that inheres in a bearer in virtue of the extent of a boundary which encloses the bearer."@en ;
                cco:ont00001760 "https://www.commoncoreontologies.org/QualityOntology"^^xsd:anyURI .


###  https://www.commoncoreontologies.org/ont00001294
cco:ont00001294 rdf:type owl:Class ;
                rdfs:subClassOf cco:ont00001202 ;
                rdfs:label "Three Dimensional Extent"@en ;
                skos:altLabel "Volume"@en ;
                skos:definition "A Size Quality that inheres in a bearer in virtue of the bearer's extension in three dimensions."@en ;
                cco:ont00001754 "International Organization for Standardization. 2019. Quantities and units -- Part 3: Space and time (ISO 80000-3:2019). International Organization for Standardization. Available at: https://www.iso.org/standard/64974.html."@en ;
                cco:ont00001760 "https://www.commoncoreontologies.org/QualityOntology"^^xsd:anyURI .


###  https://www.commoncoreontologies.org/ont00001296
cco:ont00001296 rdf:type owl:Class ;
                rdfs:subClassOf cco:ont00000119 ;
                rdfs:label "Pitch Orientation"@en ;
                skos:altLabel "Pitch"@en ;
                skos:definition "A Spatial Orientation of an Object relative to its Pitch Axis."@en ;
                cco:ont00001760 "https://www.commoncoreontologies.org/QualityOntology"^^xsd:anyURI .


###  https://www.commoncoreontologies.org/ont00001318
cco:ont00001318 rdf:type owl:Class ;
                rdfs:subClassOf cco:ont00000119 ;
                rdfs:label "Yaw Orientation"@en ;
                skos:altLabel "Yaw"@en ;
                skos:definition "A Spatial Orientation of an Object relative to its Yaw Axis."@en ;
                cco:ont00001760 "https://www.commoncoreontologies.org/QualityOntology"^^xsd:anyURI .


###  https://www.commoncoreontologies.org/ont00001333
cco:ont00001333 rdf:type owl:Class ;
                rdfs:subClassOf cco:ont00000378 ;
                rdfs:label "Rosy"@en ;
                skos:definition "A Color consisting of red hue and yellow hue and high brightness."@en ;
                cco:ont00001760 "https://www.commoncoreontologies.org/QualityOntology"^^xsd:anyURI .


###  https://www.commoncoreontologies.org/ont00001349
cco:ont00001349 rdf:type owl:Class ;
                rdfs:subClassOf cco:ont00000378 ;
                rdfs:label "Grey"@en ;
                skos:definition "A Color between white and black colors."@en ;
                cco:ont00001760 "https://www.commoncoreontologies.org/QualityOntology"^^xsd:anyURI .


###  https://www.commoncoreontologies.org/ont00001354
cco:ont00001354 rdf:type owl:Class ;
                rdfs:subClassOf cco:ont00000378 ;
                rdfs:label "Vermilion"@en ;
                skos:definition "A Color consisting of red and orange hue with a slight amount of gray."@en ;
                cco:ont00001760 "https://www.commoncoreontologies.org/QualityOntology"^^xsd:anyURI .


###  https://www.commoncoreontologies.org/ont00001360
cco:ont00001360 rdf:type owl:Class ;
                rdfs:subClassOf cco:ont00001059 ;
                rdfs:label "Three Dimensional Shape"@en ;
                skos:definition "A Shape Quality that inheres only in a three dimensional entity."@en ;
                cco:ont00001760 "https://www.commoncoreontologies.org/QualityOntology"^^xsd:anyURI .


###  https://www.commoncoreontologies.org/ont00001367
cco:ont00001367 rdf:type owl:Class ;
                rdfs:subClassOf cco:ont00001202 ;
                rdfs:comment "Subclasses of one dimensional extent are included for usability. It is doubtful any of them can be objectively distinguished (on the side of the bearing entity) without some reference to external properties such as orientation and perspective."@en ;
                rdfs:label "One Dimensional Extent"@en ;
                skos:definition "A Size Quality that inheres in a bearer in virtue of the bearer's extension in one dimension."@en ;
                cco:ont00001754 "International Organization for Standardization. 2019. Quantities and units -- Part 3: Space and time (ISO 80000-3:2019). International Organization for Standardization. Available at: https://www.iso.org/standard/64974.html."@en ;
                cco:ont00001760 "https://www.commoncoreontologies.org/QualityOntology"^^xsd:anyURI .


###  https://www.commoncoreontologies.org/ont00001369
cco:ont00001369 rdf:type owl:Class ;
                rdfs:subClassOf cco:ont00001059 ;
                rdfs:label "Rectangular"@en ;
                skos:definition "A Shape Quality inhering in a bearer in virtue of having four sides and four 90 degree angles."@en ;
                cco:ont00001760 "https://www.commoncoreontologies.org/QualityOntology"^^xsd:anyURI .


###  https://www.commoncoreontologies.org/ont00001377
cco:ont00001377 rdf:type owl:Class ;
                rdfs:subClassOf cco:ont00000378 ;
                rdfs:label "Gold Color"@en ;
                skos:definition "A Color that resembles a yellow-orange Hue with the added feature of having a metallic shine."@en ;
                cco:ont00001760 "https://www.commoncoreontologies.org/QualityOntology"^^xsd:anyURI .


###  https://www.commoncoreontologies.org/ont00001384
cco:ont00001384 rdf:type owl:Class ;
                rdfs:subClassOf cco:ont00000628 ;
                rdfs:comment "Note that it is important to specify the frequency of electromagnetic radiation when representing a bearer's Opacity since a bearer may be Opaque with respect to electromagnetic radiation of one frequency, but be transparent with respect to electromagnetic radiation of another frequency. Unless otherwise stated, statements about a bearer's Opacity are assumed to be about electromagnetic radiation with a frequency in the visible spectrum."@en ;
                rdfs:label "Opacity"@en ;
                skos:definition "An Electromagnetic Radiation Property that inheres in a bearer in virtue of that bearer's capacity to transmit electromagnetic radiation of a given frequency through the bearer instead of reflecting, scattering, or absorbing electromangentic radiation of that frequency."@en ;
                cco:ont00001754 "https://en.wikipedia.org/wiki/Opacity_(optics)" ;
                cco:ont00001760 "https://www.commoncoreontologies.org/QualityOntology"^^xsd:anyURI .


###  Generated by the OWL API (version 4.5.25.2023-02-15T19:15:49Z) https://github.com/owlcs/owlapi
