@prefix : <http://www.ontologyrepository.com/CommonCoreOntologies/Mid/TimeOntology#> .
@prefix cco: <http://www.ontologyrepository.com/CommonCoreOntologies/> .
@prefix obo: <http://purl.obolibrary.org/obo/> .
@prefix owl: <http://www.w3.org/2002/07/owl#> .
@prefix rdf: <http://www.w3.org/1999/02/22-rdf-syntax-ns#> .
@prefix xml: <http://www.w3.org/XML/1998/namespace> .
@prefix xsd: <http://www.w3.org/2001/XMLSchema#> .
@prefix rdfs: <http://www.w3.org/2000/01/rdf-schema#> .
@prefix dcterms: <http://purl.org/dc/terms/> .
@base <http://www.ontologyrepository.com/CommonCoreOntologies/Mid/TimeOntology> .

<http://www.ontologyrepository.com/CommonCoreOntologies/Mid/TimeOntology> rdf:type owl:Ontology ;
                                                                           owl:versionIRI <http://www.ontologyrepository.com/CommonCoreOntologies/Mid/2024-09-26/TimeOntology> ;
                                                                           owl:imports <http://www.ontologyrepository.com/CommonCoreOntologies/Mid/ExtendedRelationOntology> ;
                                                                           dcterms:license "BSD 3-Clause: https://github.com/CommonCoreOntology/CommonCoreOntologies/blob/master/LICENSE"@en ;
                                                                           dcterms:rights "CUBRC Inc., see full license."@en ;
                                                                           rdfs:comment "This ontology is designed to represent temporal regions and the relations that hold between them."@en ;
                                                                           rdfs:label "Time Ontology"@en ;
                                                                           owl:versionInfo "Version 1.6"@en .

#################################################################
#    Annotation properties
#################################################################

###  http://purl.org/dc/terms/rights
dcterms:rights rdf:type owl:AnnotationProperty .


#################################################################
#    Object Properties
#################################################################

###  http://www.ontologyrepository.com/CommonCoreOntologies/has_inside_instant
cco:has_inside_instant rdf:type owl:ObjectProperty ;
                       owl:inverseOf cco:is_inside_instant_of ;
                       rdfs:domain obo:BFO_0000038 ;
                       rdfs:range obo:BFO_0000148 ;
                       cco:is_curated_in_ontology "http://www.ontologyrepository.com/CommonCoreOntologies/Mid/TimeOntology"^^xsd:anyURI ;
                       rdfs:label "has inside instant"@en ;
                       <http://www.w3.org/2004/02/skos/core#definition> "For Temporal Interval t1 and Temporal Instant t2, t1 has inside instant t2 if and only if there exists Temporal Instants t3 and t4 that are part of t1 and non-identical with t2, such that t3 is before t2 and t4 is after t2."@en .


###  http://www.ontologyrepository.com/CommonCoreOntologies/has_inside_interval
cco:has_inside_interval rdf:type owl:ObjectProperty ;
                        rdfs:subPropertyOf cco:interval_contains ;
                        owl:inverseOf cco:interval_during ;
                        rdfs:domain obo:BFO_0000038 ;
                        rdfs:range obo:BFO_0000038 ;
                        cco:is_curated_in_ontology "http://www.ontologyrepository.com/CommonCoreOntologies/Mid/TimeOntology"^^xsd:anyURI ;
                        rdfs:label "has inside interval"@en ;
                        <http://www.w3.org/2004/02/skos/core#definition> "A Temporal Interval INT2 has inside interval some Temporal Interval INT1 iff there exist Temporal Instants inst1, inst2, inst3, and inst4 such that inst1 is the starting instant of INT1, inst2 is the ending instant of INT1, inst3 is the starting instant of INT2, inst4 is the ending instant of INT2, inst3 is before inst1, and inst2 is before inst4."@en .


###  http://www.ontologyrepository.com/CommonCoreOntologies/instant_is_after
cco:instant_is_after rdf:type owl:ObjectProperty ;
                     owl:inverseOf cco:instant_is_before ;
                     rdf:type owl:TransitiveProperty ;
                     rdfs:domain obo:BFO_0000148 ;
                     rdfs:range obo:BFO_0000148 ;
                     cco:elucidation "'instant is after' is a primitive relationship. Informally, a temporal instant t2 is after some temporal instant t1 if and only if t1 precedes t2."@en ;
                     cco:is_curated_in_ontology "http://www.ontologyrepository.com/CommonCoreOntologies/Mid/TimeOntology"^^xsd:anyURI ;
                     rdfs:label "instant is after"@en ;
                     <http://www.w3.org/2004/02/skos/core#definition> "A temporal instant t2 (a instance of a zero-dimensional temporal region) is after another temporal instant t1 iff there exists some instance of a temporal interval ti1 such that t1 is the starting instant of ti1 and t2 is the ending instant of ti1."@en .


###  http://www.ontologyrepository.com/CommonCoreOntologies/instant_is_before
cco:instant_is_before rdf:type owl:ObjectProperty ,
                               owl:TransitiveProperty ;
                      rdfs:domain obo:BFO_0000148 ;
                      rdfs:range obo:BFO_0000148 ;
                      cco:elucidation "'instant is before' is a primitive relationship. Informally, a temporal instant t1 is before some temporal instant t2 if and only if t1 precedes t2."@en ;
                      cco:is_curated_in_ontology "http://www.ontologyrepository.com/CommonCoreOntologies/Mid/TimeOntology"^^xsd:anyURI ;
                      rdfs:label "instant is before"@en ;
                      <http://www.w3.org/2004/02/skos/core#definition> "A temporal instant t1 (a instance of a zero-dimensional temporal region) is before another temporal instant t2 iff there exists some instance of a temporal interval ti1 such that t1 is the starting instant of ti1 and t2 is the ending instant of ti1."@en .


###  http://www.ontologyrepository.com/CommonCoreOntologies/interval_contained_by
cco:interval_contained_by rdf:type owl:ObjectProperty ;
                          owl:inverseOf cco:interval_contains ;
                          rdfs:domain obo:BFO_0000038 ;
                          rdfs:range obo:BFO_0000038 ;
                          owl:propertyDisjointWith cco:interval_disjoint ;
                          cco:is_curated_in_ontology "http://www.ontologyrepository.com/CommonCoreOntologies/Mid/TimeOntology"^^xsd:anyURI ;
                          rdfs:label "interval contained by"@en ;
                          <http://www.w3.org/2004/02/skos/core#definition> "A Temporal Interval INT1 is contained by some Temporal Interval INT2 iff there exist Temporal Instants inst1, inst2, inst3, and inst4 such that inst1 is the starting instant of INT1, inst2 is the ending instant of INT1, inst3 is the starting instant of INT2, inst4 is the ending instant of INT2, inst3 is before or identical to inst1, inst2 is before or identical to inst4, and it is not the case that both inst3 is identical to inst1 and inst2 is identical to inst4."@en .


###  http://www.ontologyrepository.com/CommonCoreOntologies/interval_contains
cco:interval_contains rdf:type owl:ObjectProperty ;
                      rdfs:domain obo:BFO_0000038 ;
                      rdfs:range obo:BFO_0000038 ;
                      owl:propertyDisjointWith cco:interval_disjoint ;
                      cco:is_curated_in_ontology "http://www.ontologyrepository.com/CommonCoreOntologies/Mid/TimeOntology"^^xsd:anyURI ;
                      rdfs:label "interval contains"@en ;
                      <http://www.w3.org/2004/02/skos/core#definition> "A Temporal Interval INT2 contains some Temporal Interval INT1 iff there exist Temporal Instants inst1, inst2, inst3, and inst4 such that inst1 is the starting instant of INT1, inst2 is the ending instant of INT1, inst3 is the starting instant of INT2, inst4 is the ending instant of INT2, inst3 is before or identical to inst1, and inst2 is before or identical to inst4, but it is not the case that both inst3 is identical to inst1 and inst2 is identical to inst4."@en .


###  http://www.ontologyrepository.com/CommonCoreOntologies/interval_disjoint
cco:interval_disjoint rdf:type owl:ObjectProperty ;
                      rdfs:domain obo:BFO_0000038 ;
                      rdfs:range obo:BFO_0000038 ;
                      owl:propertyDisjointWith cco:interval_equals ,
                                               cco:interval_overlapped_by ,
                                               cco:interval_overlaps ;
                      cco:is_curated_in_ontology "http://www.ontologyrepository.com/CommonCoreOntologies/Mid/TimeOntology"^^xsd:anyURI ;
                      rdfs:label "interval disjoint"@en ;
                      <http://www.w3.org/2004/02/skos/core#definition> "A Temporal Interval INT1 is disjoint with a Temporal Interval INT2 iff INT1 is before or meets INT2 OR INT2 is before or meets INT1. In other words, INT1 and INT2 are disjoint iff INT1 and INT2 do not overlap, contain, or equal one another."@en .


###  http://www.ontologyrepository.com/CommonCoreOntologies/interval_during
cco:interval_during rdf:type owl:ObjectProperty ;
                    rdfs:subPropertyOf cco:interval_contained_by ;
                    rdfs:domain obo:BFO_0000038 ;
                    rdfs:range obo:BFO_0000038 ;
                    cco:is_curated_in_ontology "http://www.ontologyrepository.com/CommonCoreOntologies/Mid/TimeOntology"^^xsd:anyURI ;
                    rdfs:label "interval during"@en ;
                    <http://www.w3.org/2004/02/skos/core#definition> "A Temporal Interval INT1 is during some Temporal Interval INT2 iff there exist Temporal Instants inst1, inst2, inst3, and inst4 such that inst1 is the starting instant of INT1, inst2 is the ending instant of INT1, inst3 is the starting instant of INT2, inst4 is the ending instant of INT2, inst3 is before inst1, and inst2 is before inst4."@en .


###  http://www.ontologyrepository.com/CommonCoreOntologies/interval_equals
cco:interval_equals rdf:type owl:ObjectProperty ,
                             owl:SymmetricProperty ;
                    rdfs:domain obo:BFO_0000038 ;
                    rdfs:range obo:BFO_0000038 ;
                    cco:is_curated_in_ontology "http://www.ontologyrepository.com/CommonCoreOntologies/Mid/TimeOntology"^^xsd:anyURI ;
                    rdfs:label "interval equals"@en ;
                    <http://www.w3.org/2004/02/skos/core#definition> "A Temporal Interval INT1 is equal to some Temporal Interval INT2 iff there exists Temporal Instants inst1 and inst2 such that inst1 is the starting instant of both INT1 and INT2 and inst2 is the ending instant of both INT1 and INT2."@en .


###  http://www.ontologyrepository.com/CommonCoreOntologies/interval_finished_by
cco:interval_finished_by rdf:type owl:ObjectProperty ;
                         rdfs:subPropertyOf cco:interval_contains ;
                         owl:inverseOf cco:interval_finishes ;
                         rdfs:domain obo:BFO_0000038 ;
                         rdfs:range obo:BFO_0000038 ;
                         cco:is_curated_in_ontology "http://www.ontologyrepository.com/CommonCoreOntologies/Mid/TimeOntology"^^xsd:anyURI ;
                         rdfs:label "interval finished by"@en ;
                         <http://www.w3.org/2004/02/skos/core#definition> "A Temporal Interval INT2 is finished by some Temporal Interval INT1 iff there exists Temporal Instants inst1, inst2, and inst3 such that inst 1 is the starting instant of INT1, inst2 is the ending instant of both INT1 and INT2, inst3 is the starting instant of INT2, and inst3 is before inst1."@en .


###  http://www.ontologyrepository.com/CommonCoreOntologies/interval_finishes
cco:interval_finishes rdf:type owl:ObjectProperty ;
                      rdfs:subPropertyOf cco:interval_contained_by ;
                      rdfs:domain obo:BFO_0000038 ;
                      rdfs:range obo:BFO_0000038 ;
                      cco:is_curated_in_ontology "http://www.ontologyrepository.com/CommonCoreOntologies/Mid/TimeOntology"^^xsd:anyURI ;
                      rdfs:label "interval finishes"@en ;
                      <http://www.w3.org/2004/02/skos/core#definition> "A Temporal Interval INT1 finishes some Temporal Interval INT2 iff there exists Temporal Instants inst1, inst2, and inst3 such that inst 1 is the starting instant of INT1, inst2 is the ending instant of both INT1 and INT2, inst3 is the starting instant of INT2, and inst3 is before inst1."@en .


###  http://www.ontologyrepository.com/CommonCoreOntologies/interval_is_after
cco:interval_is_after rdf:type owl:ObjectProperty ;
                      rdfs:subPropertyOf cco:interval_disjoint ;
                      owl:inverseOf cco:interval_is_before ;
                      rdfs:domain obo:BFO_0000038 ;
                      rdfs:range obo:BFO_0000038 ;
                      cco:is_curated_in_ontology "http://www.ontologyrepository.com/CommonCoreOntologies/Mid/TimeOntology"^^xsd:anyURI ;
                      rdfs:label "interval is after"@en ;
                      <http://www.w3.org/2004/02/skos/core#definition> "A TemporalInterval INT2 is after some TemporalInterval INT1 iff there exists TemporalInstants inst2, inst1 such that inst2 is the starting instant of INT2 and inst1 is the ending instant of INT1 and inst2 is after inst1."@en .


###  http://www.ontologyrepository.com/CommonCoreOntologies/interval_is_before
cco:interval_is_before rdf:type owl:ObjectProperty ;
                       rdfs:subPropertyOf cco:interval_disjoint ;
                       rdfs:domain obo:BFO_0000038 ;
                       rdfs:range obo:BFO_0000038 ;
                       cco:is_curated_in_ontology "http://www.ontologyrepository.com/CommonCoreOntologies/Mid/TimeOntology"^^xsd:anyURI ;
                       rdfs:label "interval is before"@en ;
                       <http://www.w3.org/2004/02/skos/core#definition> "A TemporalInterval INT1 is before some TemporalInterval INT2 iff there exists TemporalInstants inst1, inst2 such that inst1 is the ending instant of INT1 and inst2 is the starting instant of INT2 and inst1 is before inst2."@en .


###  http://www.ontologyrepository.com/CommonCoreOntologies/interval_meets
cco:interval_meets rdf:type owl:ObjectProperty ;
                   rdfs:subPropertyOf cco:interval_disjoint ;
                   owl:inverseOf cco:interval_met_by ;
                   rdf:type owl:IrreflexiveProperty ;
                   rdfs:domain obo:BFO_0000038 ;
                   rdfs:range obo:BFO_0000038 ;
                   cco:is_curated_in_ontology "http://www.ontologyrepository.com/CommonCoreOntologies/Mid/TimeOntology"^^xsd:anyURI ;
                   rdfs:label "interval meets"@en ;
                   <http://www.w3.org/2004/02/skos/core#definition> "A Temporal Interval INT1 meets some Temporal Interval INT2 iff there exists some Temporal Instant inst1 such that inst1 is the ending instant of INT1 and inst1 is the starting instant of INT2."@en .


###  http://www.ontologyrepository.com/CommonCoreOntologies/interval_met_by
cco:interval_met_by rdf:type owl:ObjectProperty ;
                    rdfs:subPropertyOf cco:interval_disjoint ;
                    rdf:type owl:IrreflexiveProperty ;
                    rdfs:domain obo:BFO_0000038 ;
                    rdfs:range obo:BFO_0000038 ;
                    cco:is_curated_in_ontology "http://www.ontologyrepository.com/CommonCoreOntologies/Mid/TimeOntology"^^xsd:anyURI ;
                    rdfs:label "interval met by"@en ;
                    <http://www.w3.org/2004/02/skos/core#definition> "A Temporal Interval INT2 is met by some Temporal Interval INT1 iff there exists some Temporal Instant inst1 such that inst1 is the starting instant of INT2 and inst1 is the ending instant of INT1."@en .


###  http://www.ontologyrepository.com/CommonCoreOntologies/interval_overlapped_by
cco:interval_overlapped_by rdf:type owl:ObjectProperty ;
                           owl:inverseOf cco:interval_overlaps ;
                           rdfs:domain obo:BFO_0000038 ;
                           rdfs:range obo:BFO_0000038 ;
                           cco:is_curated_in_ontology "http://www.ontologyrepository.com/CommonCoreOntologies/Mid/TimeOntology"^^xsd:anyURI ;
                           rdfs:label "interval overlapped by"@en ;
                           <http://www.w3.org/2004/02/skos/core#definition> "A Temporal Interval INT2 is overlapped by some Temporal Interval INT1 iff there exist Temporal Instants inst1, inst2, inst3, inst4 such that inst1 is the starting instant of INT1, inst2 is the ending instant of INT1, inst3 is the starting instant of INT2, inst4 is the ending instant of INT2, inst1 is before inst3, inst3 is before inst2, and inst2 is before inst4."@en .


###  http://www.ontologyrepository.com/CommonCoreOntologies/interval_overlaps
cco:interval_overlaps rdf:type owl:ObjectProperty ;
                      rdfs:domain obo:BFO_0000038 ;
                      rdfs:range obo:BFO_0000038 ;
                      cco:is_curated_in_ontology "http://www.ontologyrepository.com/CommonCoreOntologies/Mid/TimeOntology"^^xsd:anyURI ;
                      rdfs:label "interval overlaps"@en ;
                      <http://www.w3.org/2004/02/skos/core#definition> "A Temporal Interval INT1 overlaps some Temporal Interval INT2 iff there exist Temporal Instants inst1, inst2, inst3, inst4 such that inst1 is the starting instant of INT1, inst2 is the ending instant of INT1, inst3 is the starting instant of INT2, inst4 is the ending instant of INT2, inst1 is before inst3, inst3 is before inst2, and inst2 is before inst4."@en .


###  http://www.ontologyrepository.com/CommonCoreOntologies/interval_started_by
cco:interval_started_by rdf:type owl:ObjectProperty ;
                        rdfs:subPropertyOf cco:interval_contains ;
                        owl:inverseOf cco:interval_starts ;
                        rdfs:domain obo:BFO_0000038 ;
                        rdfs:range obo:BFO_0000038 ;
                        cco:is_curated_in_ontology "http://www.ontologyrepository.com/CommonCoreOntologies/Mid/TimeOntology"^^xsd:anyURI ;
                        rdfs:label "interval started by"@en ;
                        <http://www.w3.org/2004/02/skos/core#definition> "A Temporal Interval INT2 is started by some Temporal Interval INT1 iff there exist Temporal Instants inst1, inst2, and inst3 such that inst1 is the starting instant of both INT1 and INT2, inst2 is the ending instant of INT1, inst3 is the ending instant of INT2 and inst2 is before inst3."@en .


###  http://www.ontologyrepository.com/CommonCoreOntologies/interval_starts
cco:interval_starts rdf:type owl:ObjectProperty ;
                    rdfs:subPropertyOf cco:interval_contained_by ;
                    rdfs:domain obo:BFO_0000038 ;
                    rdfs:range obo:BFO_0000038 ;
                    cco:is_curated_in_ontology "http://www.ontologyrepository.com/CommonCoreOntologies/Mid/TimeOntology"^^xsd:anyURI ;
                    rdfs:label "interval starts"@en ;
                    <http://www.w3.org/2004/02/skos/core#definition> "A Temporal Interval INT1 starts some Temporal Interval INT2 iff there exist Temporal Instants inst1, inst2, and inst3 such that inst1 is the starting instant of both INT1 and INT2, inst2 is the ending instant of INT1, inst3 is the ending instant of INT2 and inst2 is before inst3."@en .


###  http://www.ontologyrepository.com/CommonCoreOntologies/is_inside_instant_of
cco:is_inside_instant_of rdf:type owl:ObjectProperty ;
                         rdfs:domain obo:BFO_0000148 ;
                         rdfs:range obo:BFO_0000038 ;
                         cco:is_curated_in_ontology "http://www.ontologyrepository.com/CommonCoreOntologies/Mid/TimeOntology"^^xsd:anyURI ;
                         rdfs:label "is inside instant of"@en ;
                         <http://www.w3.org/2004/02/skos/core#definition> "For Temporal Instant t1 and Temporal Interval t2, t1 is inside instant of t2 if and only if there are Temporal Instants t3 and t4 non-identical to t1 and part of t2 such that t3 is before t1 and t4 is after t1."@en .


#################################################################
#    Classes
#################################################################

###  http://www.ontologyrepository.com/CommonCoreOntologies/Afternoon
cco:Afternoon rdf:type owl:Class ;
              rdfs:subClassOf obo:BFO_0000202 ;
              cco:is_curated_in_ontology "http://www.ontologyrepository.com/CommonCoreOntologies/Mid/TimeOntology"^^xsd:anyURI ;
              rdfs:label "Afternoon"@en ;
              <http://www.w3.org/2004/02/skos/core#definition> "A Temporal Interval that consists of the temporal regions between when the sun is at its apex (approximately 12:00pm) and when it sets (approximately 6:00pm)."@en .


###  http://www.ontologyrepository.com/CommonCoreOntologies/AxialRotationPeriod
cco:AxialRotationPeriod rdf:type owl:Class ;
                        rdfs:subClassOf obo:BFO_0000202 ;
                        cco:is_curated_in_ontology "http://www.ontologyrepository.com/CommonCoreOntologies/Mid/TimeOntology"^^xsd:anyURI ;
                        rdfs:label "Axial Rotation Period"@en ;
                        <http://www.w3.org/2004/02/skos/core#definition> "A Temporal Interval that is equal to the length of time required for a spinning Object to complete one rotation around its Axis of Rotation."@en .


###  http://www.ontologyrepository.com/CommonCoreOntologies/CalendarDay
cco:CalendarDay rdf:type owl:Class ;
                rdfs:subClassOf cco:Day ;
                cco:is_curated_in_ontology "http://www.ontologyrepository.com/CommonCoreOntologies/Mid/TimeOntology"^^xsd:anyURI ;
                rdfs:label "Calendar Day"@en ;
                <http://www.w3.org/2004/02/skos/core#definition> "A Day that begins and ends concurrently with the Seconds specified by a Calendar System to be the first and last Seconds of the Day."@en .


###  http://www.ontologyrepository.com/CommonCoreOntologies/CalendarMonth
cco:CalendarMonth rdf:type owl:Class ;
                  rdfs:subClassOf cco:Month ;
                  cco:example_of_usage "January; February; March; April; May; June; July; August; September; October; November; December" ;
                  cco:is_curated_in_ontology "http://www.ontologyrepository.com/CommonCoreOntologies/Mid/TimeOntology"^^xsd:anyURI ;
                  rdfs:label "Calendar Month"@en ;
                  <http://www.w3.org/2004/02/skos/core#definition> "A Month that begins and ends concurrently with the Days specified by a Calendar System to be the first and last Days of the Month."@en .


###  http://www.ontologyrepository.com/CommonCoreOntologies/CalendarWeek
cco:CalendarWeek rdf:type owl:Class ;
                 rdfs:subClassOf cco:Week ;
                 cco:definition_source "http://wordnetweb.princeton.edu/perl/webwn?s=calendar+week" ;
                 cco:is_curated_in_ontology "http://www.ontologyrepository.com/CommonCoreOntologies/Mid/TimeOntology"^^xsd:anyURI ;
                 rdfs:label "Calendar Week"@en ;
                 <http://www.w3.org/2004/02/skos/core#definition> "A Week that begins and ends concurrently with the Days specified by a Calendar System to be the first and last Days of the Week."@en .


###  http://www.ontologyrepository.com/CommonCoreOntologies/CalendarYear
cco:CalendarYear rdf:type owl:Class ;
                 rdfs:subClassOf cco:Year ;
                 cco:is_curated_in_ontology "http://www.ontologyrepository.com/CommonCoreOntologies/Mid/TimeOntology"^^xsd:anyURI ;
                 rdfs:label "Calendar Year"@en ;
                 <http://www.w3.org/2004/02/skos/core#definition> "A Year that begins and ends concurrently with the Days specified by a Calendar System to be the first and last Days of the Year."@en .


###  http://www.ontologyrepository.com/CommonCoreOntologies/Day
cco:Day rdf:type owl:Class ;
        rdfs:subClassOf obo:BFO_0000202 ,
                        [ rdf:type owl:Restriction ;
                          owl:onProperty cco:interval_during ;
                          owl:someValuesFrom cco:Week
                        ] ;
        cco:definition_source "http://wordnetweb.princeton.edu/perl/webwn?s=day" ;
        cco:elucidation "Unless otherwise specified, a Day is assumed to be relative to the rotational motion of the Earth and is approximately equal to a twenty-four hour temporal region for which the start and end times are specified by the Temporal Reference System used."@en ;
        cco:is_curated_in_ontology "http://www.ontologyrepository.com/CommonCoreOntologies/Mid/TimeOntology"^^xsd:anyURI ;
        rdfs:label "Day"@en ;
        <http://www.w3.org/2004/02/skos/core#definition> "A Temporal Interval that is equal to the approximate length of time required for an Astronomical Body to complete one rotation around its Rotational Axis as specified relative to a particular Temporal Reference System."@en .


###  http://www.ontologyrepository.com/CommonCoreOntologies/Decade
cco:Decade rdf:type owl:Class ;
           rdfs:subClassOf obo:BFO_0000202 ;
           cco:definition_source "http://wordnetweb.princeton.edu/perl/webwn?s=decade" ;
           cco:is_curated_in_ontology "http://www.ontologyrepository.com/CommonCoreOntologies/Mid/TimeOntology"^^xsd:anyURI ;
           rdfs:label "Decade"@en ;
           <http://www.w3.org/2004/02/skos/core#definition> "A Temporal Interval that is equal to a period of ten consecutive Years."@en .


###  http://www.ontologyrepository.com/CommonCoreOntologies/Evening
cco:Evening rdf:type owl:Class ;
            rdfs:subClassOf obo:BFO_0000202 ;
            cco:is_curated_in_ontology "http://www.ontologyrepository.com/CommonCoreOntologies/Mid/TimeOntology"^^xsd:anyURI ;
            rdfs:label "Evening"@en ;
            <http://www.w3.org/2004/02/skos/core#definition> "A Temporal Interval that consists of the temporal regions between when the sun sets (approximately 6:00pm) and when people typically retire to sleep (approximately 9:00pm)."@en .


###  http://www.ontologyrepository.com/CommonCoreOntologies/GregorianDay
cco:GregorianDay rdf:type owl:Class ;
                 rdfs:subClassOf cco:CalendarDay ;
                 cco:is_curated_in_ontology "http://www.ontologyrepository.com/CommonCoreOntologies/Mid/TimeOntology"^^xsd:anyURI ;
                 rdfs:comment "A Gregorian Day is twenty-four Hours in duration."@en ;
                 rdfs:label "Gregorian Day"@en ;
                 <http://www.w3.org/2004/02/skos/core#definition> "A Calendar Day in the Gregorian Calendar."@en .


###  http://www.ontologyrepository.com/CommonCoreOntologies/GregorianYear
cco:GregorianYear rdf:type owl:Class ;
                  rdfs:subClassOf cco:CalendarYear ;
                  cco:is_curated_in_ontology "http://www.ontologyrepository.com/CommonCoreOntologies/Mid/TimeOntology"^^xsd:anyURI ;
                  rdfs:comment "A Gregorian Year begins concurrently with January 1, ends concurrently with December 31, and has an average duration of exactly 365.2425 Gregorian Days. The Gregorian Year is based upon the vernal equinox year. Unless otherwise stated, instances of Calendar Year are assumed to be instances of Gregorian Year since the Gregorian Calendar is the most widely used civil Calendar System."@en ;
                  rdfs:label "Gregorian Year"@en ;
                  <http://www.w3.org/2004/02/skos/core#definition> "A Calendar Year in the Gregorian Calendar."@en .


###  http://www.ontologyrepository.com/CommonCoreOntologies/Hour
cco:Hour rdf:type owl:Class ;
         rdfs:subClassOf obo:BFO_0000202 ,
                         [ rdf:type owl:Restriction ;
                           owl:onProperty cco:interval_during ;
                           owl:someValuesFrom cco:Day
                         ] ;
         cco:definition_source "http://wordnetweb.princeton.edu/perl/webwn?s=hour" ;
         cco:is_curated_in_ontology "http://www.ontologyrepository.com/CommonCoreOntologies/Mid/TimeOntology"^^xsd:anyURI ;
         rdfs:label "Hour"@en ;
         <http://www.w3.org/2004/02/skos/core#definition> "A Temporal Interval that is equal to sixty consecutive Minutes."@en .


###  http://www.ontologyrepository.com/CommonCoreOntologies/JulianDate
cco:JulianDate rdf:type owl:Class ;
               rdfs:subClassOf cco:TimeOfDay ,
                               [ rdf:type owl:Restriction ;
                                 owl:onProperty obo:BFO_0000132 ;
                                 owl:someValuesFrom cco:JulianDay
                               ] ;
               cco:acronym "JD" ;
               cco:definition_source "https://www.defit.org/julian-date/" ;
               cco:is_curated_in_ontology "http://www.ontologyrepository.com/CommonCoreOntologies/Mid/TimeOntology"^^xsd:anyURI ;
               rdfs:label "Julian Date"@en ;
               <http://www.w3.org/2004/02/skos/core#definition> "A Time of Day as specified according to the Julian Calendar using the Julian Date epoch."@en .


###  http://www.ontologyrepository.com/CommonCoreOntologies/JulianDay
cco:JulianDay rdf:type owl:Class ;
              rdfs:subClassOf cco:CalendarDay ;
              cco:definition_source "https://www.defit.org/julian-date/" ;
              cco:is_curated_in_ontology "http://www.ontologyrepository.com/CommonCoreOntologies/Mid/TimeOntology"^^xsd:anyURI ;
              rdfs:comment "A Julian Day begins at noon Universal Time and is twenty-four Hours in duration."@en ;
              rdfs:label "Julian Day"@en ;
              <http://www.w3.org/2004/02/skos/core#definition> "A Calendar Day in the Julian Calendar."@en .


###  http://www.ontologyrepository.com/CommonCoreOntologies/JulianYear
cco:JulianYear rdf:type owl:Class ;
               rdfs:subClassOf cco:CalendarYear ;
               cco:is_curated_in_ontology "http://www.ontologyrepository.com/CommonCoreOntologies/Mid/TimeOntology"^^xsd:anyURI ;
               rdfs:comment "A Julian Year begins concurrently with January 1, ends concurrently with December 31, and has an average duration of exactly 365.25 Julian Days. Julian Years are typically indicated by prefixing a capital 'J' in front of the Year number, e.g. J2000.0 or J2018."@en ;
               rdfs:label "Julian Year"@en ;
               <http://www.w3.org/2004/02/skos/core#definition> "A Calendar Year in the Julian Calendar."@en .


###  http://www.ontologyrepository.com/CommonCoreOntologies/Minute
cco:Minute rdf:type owl:Class ;
           rdfs:subClassOf obo:BFO_0000202 ,
                           [ rdf:type owl:Restriction ;
                             owl:onProperty cco:interval_during ;
                             owl:someValuesFrom cco:Hour
                           ] ;
           cco:definition_source "http://wordnetweb.princeton.edu/perl/webwn?s=minute" ;
           cco:is_curated_in_ontology "http://www.ontologyrepository.com/CommonCoreOntologies/Mid/TimeOntology"^^xsd:anyURI ;
           rdfs:label "Minute"@en ;
           <http://www.w3.org/2004/02/skos/core#definition> "A Temporal Interval that is equal to sixty consecutive Seconds."@en .


###  http://www.ontologyrepository.com/CommonCoreOntologies/ModifiedJulianDate
cco:ModifiedJulianDate rdf:type owl:Class ;
                       rdfs:subClassOf cco:TimeOfDay ;
                       cco:acronym "MJD" ;
                       cco:definition_source "http://aa.usno.navy.mil/data/docs/JulianDate.php" ;
                       cco:is_curated_in_ontology "http://www.ontologyrepository.com/CommonCoreOntologies/Mid/TimeOntology"^^xsd:anyURI ;
                       rdfs:comment """A Day begins at midnight GMT within the Modified Julian Date reference system. The Modified Julian Date (MJD) is related to the Julian Date (JD) by the formula:
MJD = JD - 2400000.5"""@en ;
                       rdfs:label "Modified Julian Date"@en ;
                       <http://www.w3.org/2004/02/skos/core#definition> "A Time of Day as specified according to the Julian Calendar using the Modified Julian Date epoch."@en .


###  http://www.ontologyrepository.com/CommonCoreOntologies/Month
cco:Month rdf:type owl:Class ;
          rdfs:subClassOf obo:BFO_0000202 ,
                          [ rdf:type owl:Restriction ;
                            owl:onProperty cco:interval_during ;
                            owl:someValuesFrom cco:Year
                          ] ;
          cco:definition_source "http://wordnetweb.princeton.edu/perl/webwn?s=month" ;
          cco:elucidation "Unless otherwise specified, it is assumed that a Month is specified relative to the Rotational Motion of the Moon around the Earth. Earth Months are approximately equal to four consecutive Weeks or 30 consecutive Days."@en ;
          cco:is_curated_in_ontology "http://www.ontologyrepository.com/CommonCoreOntologies/Mid/TimeOntology"^^xsd:anyURI ;
          rdfs:label "Month"@en ;
          <http://www.w3.org/2004/02/skos/core#definition> "A Temporal Interval that is based on the approximate length of time required for a Natural Satellite to complete one cycle of its rotational motion around its Primary Body."@en .


###  http://www.ontologyrepository.com/CommonCoreOntologies/Morning
cco:Morning rdf:type owl:Class ;
            rdfs:subClassOf obo:BFO_0000202 ;
            cco:is_curated_in_ontology "http://www.ontologyrepository.com/CommonCoreOntologies/Mid/TimeOntology"^^xsd:anyURI ;
            rdfs:label "Morning"@en ;
            <http://www.w3.org/2004/02/skos/core#definition> "A Temporal Interval that consists of the temporal regions between when the sun dawns (approximately 6:00am) and reaches its apex (approximately 12:00pm)."@en .


###  http://www.ontologyrepository.com/CommonCoreOntologies/MultiDayTemporalInterval
cco:MultiDayTemporalInterval rdf:type owl:Class ;
                             rdfs:subClassOf obo:BFO_0000038 ,
                                             [ rdf:type owl:Restriction ;
                                               owl:onProperty cco:interval_contains ;
                                               owl:someValuesFrom cco:Day
                                             ] ;
                             cco:is_curated_in_ontology "http://www.ontologyrepository.com/CommonCoreOntologies/Mid/TimeOntology"^^xsd:anyURI ;
                             rdfs:comment "This is a defined class."@en ;
                             rdfs:label "Multi-Day Temporal Interval"@en ;
                             <http://www.w3.org/2004/02/skos/core#definition> "A one-dimensional temporal region that is measured in Days and spans at least one Day."@en .


###  http://www.ontologyrepository.com/CommonCoreOntologies/MultiHourTemporalInterval
cco:MultiHourTemporalInterval rdf:type owl:Class ;
                              rdfs:subClassOf obo:BFO_0000038 ,
                                              [ rdf:type owl:Restriction ;
                                                owl:onProperty cco:interval_contains ;
                                                owl:someValuesFrom cco:Hour
                                              ] ;
                              cco:is_curated_in_ontology "http://www.ontologyrepository.com/CommonCoreOntologies/Mid/TimeOntology"^^xsd:anyURI ;
                              rdfs:comment "This is a defined class."@en ;
                              rdfs:label "Multi-Hour Temporal Interval"@en ;
                              <http://www.w3.org/2004/02/skos/core#definition> "A one-dimensional temporal region that is measured in Hours and spans at least one Hour."@en .


###  http://www.ontologyrepository.com/CommonCoreOntologies/MultiMinuteTemporalInterval
cco:MultiMinuteTemporalInterval rdf:type owl:Class ;
                                rdfs:subClassOf obo:BFO_0000038 ,
                                                [ rdf:type owl:Restriction ;
                                                  owl:onProperty cco:interval_contains ;
                                                  owl:someValuesFrom cco:Minute
                                                ] ;
                                cco:is_curated_in_ontology "http://www.ontologyrepository.com/CommonCoreOntologies/Mid/TimeOntology"^^xsd:anyURI ;
                                rdfs:comment "This is a defined class."@en ;
                                rdfs:label "Multi-Minute Temporal Interval"@en ;
                                <http://www.w3.org/2004/02/skos/core#definition> "A one-dimensional temporal region that is measured in Minutes and spans at least one Minute."@en .


###  http://www.ontologyrepository.com/CommonCoreOntologies/MultiMonthTemporalInterval
cco:MultiMonthTemporalInterval rdf:type owl:Class ;
                               rdfs:subClassOf obo:BFO_0000038 ,
                                               [ rdf:type owl:Restriction ;
                                                 owl:onProperty cco:interval_contains ;
                                                 owl:someValuesFrom cco:Month
                                               ] ;
                               cco:is_curated_in_ontology "http://www.ontologyrepository.com/CommonCoreOntologies/Mid/TimeOntology"^^xsd:anyURI ;
                               rdfs:comment "This is a defined class."@en ;
                               rdfs:label "Multi-Month Temporal Interval"@en ;
                               <http://www.w3.org/2004/02/skos/core#definition> "A one-dimensional temporal region that is measured in Months and spans at least one Month."@en .


###  http://www.ontologyrepository.com/CommonCoreOntologies/MultiSecondTemporalInterval
cco:MultiSecondTemporalInterval rdf:type owl:Class ;
                                rdfs:subClassOf obo:BFO_0000038 ,
                                                [ rdf:type owl:Restriction ;
                                                  owl:onProperty cco:interval_contains ;
                                                  owl:someValuesFrom cco:Second
                                                ] ;
                                cco:is_curated_in_ontology "http://www.ontologyrepository.com/CommonCoreOntologies/Mid/TimeOntology"^^xsd:anyURI ;
                                rdfs:comment "This is a defined class."@en ;
                                rdfs:label "Multi-Second Temporal Interval"@en ;
                                <http://www.w3.org/2004/02/skos/core#definition> "A one-dimensional temporal region that is measured in Seconds and spans at least one Second."@en .


###  http://www.ontologyrepository.com/CommonCoreOntologies/MultiWeekTemporalInterval
cco:MultiWeekTemporalInterval rdf:type owl:Class ;
                              rdfs:subClassOf obo:BFO_0000038 ,
                                              [ rdf:type owl:Restriction ;
                                                owl:onProperty cco:interval_contains ;
                                                owl:someValuesFrom cco:Week
                                              ] ;
                              cco:is_curated_in_ontology "http://www.ontologyrepository.com/CommonCoreOntologies/Mid/TimeOntology"^^xsd:anyURI ;
                              rdfs:comment "This is a defined class."@en ;
                              rdfs:label "Multi-Week Temporal Interval"@en ;
                              <http://www.w3.org/2004/02/skos/core#definition> "A one-dimensional temporal region that is measured in Weeks and spans at least one Week."@en .


###  http://www.ontologyrepository.com/CommonCoreOntologies/MultiYearTemporalInterval
cco:MultiYearTemporalInterval rdf:type owl:Class ;
                              rdfs:subClassOf obo:BFO_0000038 ,
                                              [ rdf:type owl:Restriction ;
                                                owl:onProperty cco:interval_contains ;
                                                owl:someValuesFrom cco:Year
                                              ] ;
                              cco:is_curated_in_ontology "http://www.ontologyrepository.com/CommonCoreOntologies/Mid/TimeOntology"^^xsd:anyURI ;
                              rdfs:comment "This is a defined class."@en ;
                              rdfs:label "Multi-Year Temporal Interval"@en ;
                              <http://www.w3.org/2004/02/skos/core#definition> "A one-dimensional temporal region that is measured in Years and spans at least one Year."@en .


###  http://www.ontologyrepository.com/CommonCoreOntologies/Night
cco:Night rdf:type owl:Class ;
          rdfs:subClassOf obo:BFO_0000202 ;
          cco:is_curated_in_ontology "http://www.ontologyrepository.com/CommonCoreOntologies/Mid/TimeOntology"^^xsd:anyURI ;
          rdfs:label "Night"@en ;
          <http://www.w3.org/2004/02/skos/core#definition> "A Temporal Interval that consists of the temporal regions between when people typically retire to sleep (approximately 9:00pm) and when the sun dawns (approximately 6:00am)."@en .


###  http://www.ontologyrepository.com/CommonCoreOntologies/ReferenceTime
cco:ReferenceTime rdf:type owl:Class ;
                  rdfs:subClassOf obo:BFO_0000203 ;
                  cco:definition_source "https://en.wikipedia.org/wiki/Epoch_(reference_date)" ;
                  cco:is_curated_in_ontology "http://www.ontologyrepository.com/CommonCoreOntologies/Mid/TimeOntology"^^xsd:anyURI ;
                  rdfs:label "Reference Time"@en ;
                  <http://www.w3.org/2004/02/skos/core#altLabel> "Epoch"@en ,
                                                                 "Epoch Time"@en ,
                                                                 "Reference Date"@en ;
                  <http://www.w3.org/2004/02/skos/core#definition> "A Temporal Instant specified as the origin for which other Temporal Regions are measured or identified."@en .


###  http://www.ontologyrepository.com/CommonCoreOntologies/Second
cco:Second rdf:type owl:Class ;
           rdfs:subClassOf obo:BFO_0000202 ,
                           [ rdf:type owl:Restriction ;
                             owl:onProperty cco:interval_during ;
                             owl:someValuesFrom cco:Minute
                           ] ;
           cco:definition_source "https://physics.nist.gov/cuu/Units/second.html" ;
           cco:is_curated_in_ontology "http://www.ontologyrepository.com/CommonCoreOntologies/Mid/TimeOntology"^^xsd:anyURI ;
           rdfs:comment "The Second is used as the basic SI unit of time."@en ;
           rdfs:label "Second"@en ;
           <http://www.w3.org/2004/02/skos/core#definition> "A Temporal Interval that is equal to the duration of 9,192,631,770 periods of the radiation corresponding to the transition between the two hyperfine levels of the ground state of the cesium 133 atom."@en .


###  http://www.ontologyrepository.com/CommonCoreOntologies/TimeOfDay
cco:TimeOfDay rdf:type owl:Class ;
              rdfs:subClassOf obo:BFO_0000203 ,
                              [ rdf:type owl:Restriction ;
                                owl:onProperty obo:BFO_0000132 ;
                                owl:someValuesFrom cco:Day
                              ] ;
              cco:is_curated_in_ontology "http://www.ontologyrepository.com/CommonCoreOntologies/Mid/TimeOntology"^^xsd:anyURI ;
              rdfs:label "Time of Day"@en ;
              <http://www.w3.org/2004/02/skos/core#definition> "A Temporal Instant that is part of a Day."@en .


###  http://www.ontologyrepository.com/CommonCoreOntologies/UnixTemporalInstant
cco:UnixTemporalInstant rdf:type owl:Class ;
                        rdfs:subClassOf obo:BFO_0000203 ;
                        cco:is_curated_in_ontology "http://www.ontologyrepository.com/CommonCoreOntologies/Mid/TimeOntology"^^xsd:anyURI ;
                        rdfs:label "Unix Temporal Instant"@en ;
                        <http://www.w3.org/2004/02/skos/core#definition> "A Temporal Instant as specified by the number of Seconds that have elapsed since the specified Epoch Time as described by an implementation of Unix Time."@en .


###  http://www.ontologyrepository.com/CommonCoreOntologies/Week
cco:Week rdf:type owl:Class ;
         rdfs:subClassOf obo:BFO_0000202 ,
                         [ rdf:type owl:Restriction ;
                           owl:onProperty cco:interval_during ;
                           owl:someValuesFrom cco:Month
                         ] ;
         cco:definition_source "http://wordnetweb.princeton.edu/perl/webwn?s=week" ;
         cco:is_curated_in_ontology "http://www.ontologyrepository.com/CommonCoreOntologies/Mid/TimeOntology"^^xsd:anyURI ;
         rdfs:label "Week"@en ;
         <http://www.w3.org/2004/02/skos/core#definition> "A Temporal Interval that is equal to seven consecutive Days."@en .


###  http://www.ontologyrepository.com/CommonCoreOntologies/Year
cco:Year rdf:type owl:Class ;
         rdfs:subClassOf obo:BFO_0000202 ,
                         [ rdf:type owl:Restriction ;
                           owl:onProperty cco:interval_during ;
                           owl:someValuesFrom cco:Decade
                         ] ;
         cco:definition_source "http://wordnetweb.princeton.edu/perl/webwn?s=year" ;
         cco:elucidation "Unless otherwise specified, a Year is assumed to be relative to the Orbiting of the Earth around the Sun and is approximately equal to 12 Months or 365 Days."@en ;
         cco:is_curated_in_ontology "http://www.ontologyrepository.com/CommonCoreOntologies/Mid/TimeOntology"^^xsd:anyURI ;
         rdfs:label "Year"@en ;
         <http://www.w3.org/2004/02/skos/core#definition> "A Temporal Interval that is equal to the approximate length of time required for an Astronomical Body to complete one Orbital Revolution around its Primary Body as specified relative to a particular Temporal Reference System."@en .


###  Generated by the OWL API (version 4.5.29) https://github.com/owlcs/owlapi
