@prefix : <https://www.commoncoreontologies.org/mro/> .
@prefix cco: <https://www.commoncoreontologies.org/> .
@prefix mro: <https://www.commoncoreontologies.org/mro/> .
@prefix obo: <http://purl.obolibrary.org/obo/> .
@prefix owl: <http://www.w3.org/2002/07/owl#> .
@prefix rdf: <http://www.w3.org/1999/02/22-rdf-syntax-ns#> .
@prefix xml: <http://www.w3.org/XML/1998/namespace> .
@prefix xsd: <http://www.w3.org/2001/XMLSchema#> .
@prefix rdfs: <http://www.w3.org/2000/01/rdf-schema#> .
@base <https://www.commoncoreontologies.org/mro/> .

<https://www.commoncoreontologies.org/ModalRelationOntology> rdf:type owl:Ontology ;
                                                              owl:versionIRI <https://www.commoncoreontologies.org/2024-11-06/ModalRelationOntology> ;
                                                              <http://purl.org/dc/terms/license> "BSD 3-Clause: https://github.com/CommonCoreOntology/CommonCoreOntologies/blob/master/LICENSE"@en ;
                                                              <http://purl.org/dc/terms/rights> "CUBRC Inc., see full license."@en ;
                                                              rdfs:comment "The modal counterparts to the object and data properties contained in CCO and BFO2020-core." ;
                                                              rdfs:label "Modal Relation Ontology" ;
                                                              owl:versionInfo "v2.0" .

#################################################################
#    Annotation properties
#################################################################

###  http://purl.org/dc/elements/1.1/identifier
<http://purl.org/dc/elements/1.1/identifier> rdf:type owl:AnnotationProperty .


###  http://purl.org/dc/terms/created
<http://purl.org/dc/terms/created> rdf:type owl:AnnotationProperty .


###  http://purl.org/dc/terms/creator
<http://purl.org/dc/terms/creator> rdf:type owl:AnnotationProperty .


###  http://purl.org/dc/terms/license
<http://purl.org/dc/terms/license> rdf:type owl:AnnotationProperty .


###  http://purl.org/dc/terms/rights
<http://purl.org/dc/terms/rights> rdf:type owl:AnnotationProperty .


###  http://www.w3.org/2004/02/skos/core#altLabel
<http://www.w3.org/2004/02/skos/core#altLabel> rdf:type owl:AnnotationProperty .


###  http://www.w3.org/2004/02/skos/core#definition
<http://www.w3.org/2004/02/skos/core#definition> rdf:type owl:AnnotationProperty .


###  http://www.w3.org/2004/02/skos/core#editorialNote
<http://www.w3.org/2004/02/skos/core#editorialNote> rdf:type owl:AnnotationProperty .


###  http://www.w3.org/2004/02/skos/core#example
<http://www.w3.org/2004/02/skos/core#example> rdf:type owl:AnnotationProperty .


###  http://www.w3.org/2004/02/skos/core#prefLabel
<http://www.w3.org/2004/02/skos/core#prefLabel> rdf:type owl:AnnotationProperty .


###  http://www.w3.org/2004/02/skos/core#scopeNote
<http://www.w3.org/2004/02/skos/core#scopeNote> rdf:type owl:AnnotationProperty .


###  https://www.commoncoreontologies.org/ont00001754
cco:ont00001754 rdf:type owl:AnnotationProperty .


###  https://www.commoncoreontologies.org/ont00001760
cco:ont00001760 rdf:type owl:AnnotationProperty .


#################################################################
#    Object Properties
#################################################################

###  https://www.commoncoreontologies.org/mro/BFO_0000054
mro:BFO_0000054 rdf:type owl:ObjectProperty ;
                rdfs:subPropertyOf mro:mro00000001 ;
                owl:inverseOf mro:BFO_0000055 ;
                rdfs:domain obo:BFO_0000017 ;
                rdfs:range obo:BFO_0000015 ;
                <http://purl.org/dc/elements/1.1/identifier> "206-BFO" ;
                rdfs:label "has realization"@en ;
                <http://www.w3.org/2004/02/skos/core#altLabel> "realized in"@en ;
                <http://www.w3.org/2004/02/skos/core#definition> "b has realization c =Def c realizes b"@en ;
                <http://www.w3.org/2004/02/skos/core#example> "As for realizes"@en .


###  https://www.commoncoreontologies.org/mro/BFO_0000055
mro:BFO_0000055 rdf:type owl:ObjectProperty ;
                rdfs:subPropertyOf mro:mro00000001 ;
                rdfs:domain obo:BFO_0000015 ;
                rdfs:range obo:BFO_0000017 ;
                <http://purl.org/dc/elements/1.1/identifier> "059-BFO" ;
                rdfs:label "realizes"@en ;
                <http://www.w3.org/2004/02/skos/core#definition> "(Elucidation) realizes is a relation between a process b and realizable entity c such that c inheres in some d & for all t, if b has participant d then c exists & the type instantiated by b is correlated with the type instantiated by c"@en ;
                <http://www.w3.org/2004/02/skos/core#example> "A balding process realizes a disposition to go bald; a studying process realizes a student role; a process of pumping blood realizes the pumping function of a heart"@en .


###  https://www.commoncoreontologies.org/mro/BFO_0000056
mro:BFO_0000056 rdf:type owl:ObjectProperty ;
                rdfs:subPropertyOf mro:mro00000001 ;
                owl:inverseOf mro:BFO_0000057 ;
                rdfs:domain [ rdf:type owl:Class ;
                              owl:unionOf ( obo:BFO_0000020
                                            obo:BFO_0000031
                                            [ owl:intersectionOf ( obo:BFO_0000004
                                                                   [ rdf:type owl:Class ;
                                                                     owl:complementOf obo:BFO_0000006
                                                                   ]
                                                                 ) ;
                                              rdf:type owl:Class
                                            ]
                                          )
                            ] ;
                rdfs:range obo:BFO_0000015 ;
                <http://purl.org/dc/elements/1.1/identifier> "250-BFO" ;
                rdfs:label "participates in"@en ;
                <http://www.w3.org/2004/02/skos/core#definition> "(Elucidation) participates in holds between some b that is either a specifically dependent continuant or generically dependent continuant or independent continuant that is not a spatial region & some process p such that b participates in p some way"@en ;
                <http://www.w3.org/2004/02/skos/core#scopeNote> "Users that require more sophisticated representations of time are encouraged to import a temporal extension of BFO-Core provided by the BFO development team. See documentation for guidance: <https://github.com/BFO-ontology/BFO-2020/tree/master/src/owl/profiles/temporal%20extensions>"@en .


###  https://www.commoncoreontologies.org/mro/BFO_0000057
mro:BFO_0000057 rdf:type owl:ObjectProperty ;
                rdfs:subPropertyOf mro:mro00000001 ;
                rdfs:domain obo:BFO_0000015 ;
                rdfs:range [ rdf:type owl:Class ;
                             owl:unionOf ( obo:BFO_0000020
                                           obo:BFO_0000031
                                           [ owl:intersectionOf ( obo:BFO_0000004
                                                                  [ rdf:type owl:Class ;
                                                                    owl:complementOf obo:BFO_0000006
                                                                  ]
                                                                ) ;
                                             rdf:type owl:Class
                                           ]
                                         )
                           ] ;
                <http://purl.org/dc/elements/1.1/identifier> "248-BFO" ;
                rdfs:label "has participant"@en ;
                <http://www.w3.org/2004/02/skos/core#definition> "p has participant c =Def c participates in p"@en ;
                <http://www.w3.org/2004/02/skos/core#scopeNote> "Users that require more sophisticated representations of time are encouraged to import a temporal extension of BFO-Core provided by the BFO development team. See documentation for guidance: <https://github.com/BFO-ontology/BFO-2020/tree/master/src/owl/profiles/temporal%20extensions>"@en .


###  https://www.commoncoreontologies.org/mro/BFO_0000058
mro:BFO_0000058 rdf:type owl:ObjectProperty ;
                rdfs:subPropertyOf mro:mro00000001 ;
                owl:inverseOf mro:BFO_0000059 ;
                rdfs:domain obo:BFO_0000031 ;
                rdfs:range [ rdf:type owl:Class ;
                             owl:unionOf ( obo:BFO_0000015
                                           obo:BFO_0000020
                                         )
                           ] ;
                <http://purl.org/dc/elements/1.1/identifier> "258-BFO" ;
                rdfs:label "is concretized by"@en ;
                <http://www.w3.org/2004/02/skos/core#definition> "c is concretized by b =Def b concretizes c"@en ;
                <http://www.w3.org/2004/02/skos/core#scopeNote> "Users that require more sophisticated representations of time are encouraged to import a temporal extension of BFO-Core provided by the BFO development team. See documentation for guidance: <https://github.com/BFO-ontology/BFO-2020/tree/master/src/owl/profiles/temporal%20extensions>"@en .


###  https://www.commoncoreontologies.org/mro/BFO_0000059
mro:BFO_0000059 rdf:type owl:ObjectProperty ;
                rdfs:subPropertyOf mro:mro00000001 ;
                rdfs:domain [ rdf:type owl:Class ;
                              owl:unionOf ( obo:BFO_0000015
                                            obo:BFO_0000020
                                          )
                            ] ;
                rdfs:range obo:BFO_0000031 ;
                <http://purl.org/dc/elements/1.1/identifier> "256-BFO" ;
                rdfs:label "concretizes"@en ;
                <http://www.w3.org/2004/02/skos/core#definition> "b concretizes c =Def b is a process or a specifically dependent continuant & c is a generically dependent continuant & there is some time t such that c is the pattern or content which b shares at t with actual or potential copies"@en ;
                <http://www.w3.org/2004/02/skos/core#scopeNote> "Users that require more sophisticated representations of time are encouraged to import a temporal extension of BFO-Core provided by the BFO development team. See documentation for guidance: <https://github.com/BFO-ontology/BFO-2020/tree/master/src/owl/profiles/temporal%20extensions>"@en .


###  https://www.commoncoreontologies.org/mro/BFO_0000062
mro:BFO_0000062 rdf:type owl:ObjectProperty ;
                rdfs:subPropertyOf mro:mro00000001 ;
                owl:inverseOf mro:BFO_0000063 ;
                rdf:type owl:TransitiveProperty ;
                rdfs:domain obo:BFO_0000003 ;
                rdfs:range obo:BFO_0000003 ;
                <http://purl.org/dc/elements/1.1/identifier> "213-BFO" ;
                rdfs:label "preceded by"@en ;
                <http://www.w3.org/2004/02/skos/core#definition> "b preceded by c =Def b precedes c"@en ;
                <http://www.w3.org/2004/02/skos/core#example> "The temporal region occupied by the second half of the match is preceded by the temporal region occupied by the first half of the match"@en .


###  https://www.commoncoreontologies.org/mro/BFO_0000063
mro:BFO_0000063 rdf:type owl:ObjectProperty ;
                rdfs:subPropertyOf mro:mro00000001 ;
                rdf:type owl:TransitiveProperty ;
                rdfs:domain obo:BFO_0000003 ;
                rdfs:range obo:BFO_0000003 ;
                <http://purl.org/dc/elements/1.1/identifier> "270-BFO" ;
                rdfs:label "precedes"@en ;
                <http://www.w3.org/2004/02/skos/core#definition> "(Elucidation) precedes is a relation between occurrents o, o' such that if t is the temporal extent of o & t' is the temporal extent of o' then either the last instant of o is before the first instant of o' or the last instant of o is the first instant of o' & neither o nor o' are temporal instants"@en ;
                <http://www.w3.org/2004/02/skos/core#example> "The temporal region occupied by Mary's birth precedes the temporal region occupied by Mary's death."@en ;
                <http://www.w3.org/2004/02/skos/core#scopeNote> "Each temporal region is its own temporal extent. The temporal extent of a spatiotemporal region is the temporal region it temporally projects onto. The temporal extent of a process or process boundary that occupies temporal region t is t." ,
                                                                "Precedes defines a strict partial order on occurrents." .


###  https://www.commoncoreontologies.org/mro/BFO_0000066
mro:BFO_0000066 rdf:type owl:ObjectProperty ;
                rdfs:subPropertyOf mro:mro00000001 ;
                owl:inverseOf mro:BFO_0000183 ;
                rdfs:domain [ rdf:type owl:Class ;
                              owl:unionOf ( obo:BFO_0000015
                                            obo:BFO_0000035
                                          )
                            ] ;
                rdfs:range [ rdf:type owl:Class ;
                             owl:unionOf ( obo:BFO_0000029
                                           obo:BFO_0000040
                                         )
                           ] ;
                <http://purl.org/dc/elements/1.1/identifier> "143-BFO" ;
                rdfs:label "occurs in"@en ;
                <http://www.w3.org/2004/02/skos/core#definition> "b occurs in c =Def b is a process or a process boundary & c is a material entity or site & there exists a spatiotemporal region r & b occupies spatiotemporal region r & for all time t, if b exists at t then c exists at t & there exist spatial regions s and s' where b spatially projects onto s at t & c occupies spatial region s' at t & s is a continuant part of s' at t"@en ;
                <http://www.w3.org/2004/02/skos/core#example> "A process of digestion occurs in the interior of an organism; a process of loading artillery rounds into a tank cannon occurs in the interior of the tank"@en .


###  https://www.commoncoreontologies.org/mro/BFO_0000084
mro:BFO_0000084 rdf:type owl:ObjectProperty ;
                rdfs:subPropertyOf mro:mro00000001 ;
                owl:inverseOf mro:BFO_0000101 ;
                rdfs:domain obo:BFO_0000031 ;
                rdfs:range [ owl:intersectionOf ( obo:BFO_0000004
                                                  [ rdf:type owl:Class ;
                                                    owl:complementOf obo:BFO_0000006
                                                  ]
                                                ) ;
                             rdf:type owl:Class
                           ] ;
                <http://purl.org/dc/elements/1.1/identifier> "252-BFO" ;
                rdfs:label "generically depends on"@en ;
                <http://www.w3.org/2004/02/skos/core#altLabel> "g-depends on"@en ;
                <http://www.w3.org/2004/02/skos/core#definition> "b generically depends on c =Def b is a generically dependent continuant & c is an independent continuant that is not a spatial region & at some time t there inheres in c a specifically dependent continuant which concretizes b at t"@en ;
                <http://www.w3.org/2004/02/skos/core#scopeNote> "Users that require more sophisticated representations of time are encouraged to import a temporal extension of BFO-Core provided by the BFO development team. See documentation for guidance: <https://github.com/BFO-ontology/BFO-2020/tree/master/src/owl/profiles/temporal%20extensions>"@en .


###  https://www.commoncoreontologies.org/mro/BFO_0000101
mro:BFO_0000101 rdf:type owl:ObjectProperty ;
                rdfs:subPropertyOf mro:mro00000001 ;
                rdfs:domain [ owl:intersectionOf ( obo:BFO_0000004
                                                   [ rdf:type owl:Class ;
                                                     owl:complementOf obo:BFO_0000006
                                                   ]
                                                 ) ;
                              rdf:type owl:Class
                            ] ;
                rdfs:range obo:BFO_0000031 ;
                <http://purl.org/dc/elements/1.1/identifier> "254-BFO" ;
                rdfs:label "is carrier of"@en ;
                <http://www.w3.org/2004/02/skos/core#definition> "b is carrier of c =Def there is some time t such that c generically depends on b at t"@en ;
                <http://www.w3.org/2004/02/skos/core#scopeNote> "Users that require more sophisticated representations of time are encouraged to import a temporal extension of BFO-Core provided by the BFO development team. See documentation for guidance: <https://github.com/BFO-ontology/BFO-2020/tree/master/src/owl/profiles/temporal%20extensions>"@en .


###  https://www.commoncoreontologies.org/mro/BFO_0000108
mro:BFO_0000108 rdf:type owl:ObjectProperty ;
                rdfs:subPropertyOf mro:mro00000001 ;
                rdfs:domain obo:BFO_0000001 ;
                rdfs:range obo:BFO_0000008 ;
                <http://purl.org/dc/elements/1.1/identifier> "118-BFO" ;
                rdfs:label "exists at"@en ;
                <http://www.w3.org/2004/02/skos/core#definition> "(Elucidation) exists at is a relation between a particular and some temporal region at which the particular exists"@en ;
                <http://www.w3.org/2004/02/skos/core#example> "First World War exists at 1914-1916; Mexico exists at January 1, 2000"@en .


###  https://www.commoncoreontologies.org/mro/BFO_0000115
mro:BFO_0000115 rdf:type owl:ObjectProperty ;
                rdfs:subPropertyOf mro:BFO_0000178 ;
                owl:inverseOf mro:BFO_0000129 ;
                rdfs:domain obo:BFO_0000040 ;
                rdfs:range obo:BFO_0000040 ;
                <http://purl.org/dc/elements/1.1/identifier> "230-BFO" ;
                rdfs:label "has member part"@en ;
                <http://www.w3.org/2004/02/skos/core#definition> "b has member part c =Def c member part of b"@en ;
                <http://www.w3.org/2004/02/skos/core#scopeNote> "Users that require more sophisticated representations of time are encouraged to import a temporal extension of BFO-Core provided by the BFO development team. See documentation for guidance: <https://github.com/BFO-ontology/BFO-2020/tree/master/src/owl/profiles/temporal%20extensions>"@en .


###  https://www.commoncoreontologies.org/mro/BFO_0000117
mro:BFO_0000117 rdf:type owl:ObjectProperty ;
                rdfs:subPropertyOf mro:mro00000001 ;
                owl:inverseOf mro:BFO_0000132 ;
                rdf:type owl:TransitiveProperty ;
                rdfs:domain obo:BFO_0000003 ;
                rdfs:range obo:BFO_0000003 ;
                <http://purl.org/dc/elements/1.1/identifier> "202-BFO" ;
                rdfs:label "has occurrent part"@en ;
                <http://www.w3.org/2004/02/skos/core#definition> "b has occurrent part c =Def c occurrent part of b"@en ;
                <http://www.w3.org/2004/02/skos/core#example> "Mary's life has occurrent part Mary's 5th birthday"@en .


###  https://www.commoncoreontologies.org/mro/BFO_0000121
mro:BFO_0000121 rdf:type owl:ObjectProperty ;
                rdfs:subPropertyOf mro:BFO_0000117 ;
                owl:inverseOf mro:BFO_0000139 ;
                rdf:type owl:TransitiveProperty ;
                rdfs:domain obo:BFO_0000003 ;
                rdfs:range obo:BFO_0000003 ;
                <http://purl.org/dc/elements/1.1/identifier> "211-BFO" ;
                rdfs:label "has temporal part"@en ;
                <http://www.w3.org/2004/02/skos/core#definition> "b has temporal part c =Def c temporal part of b"@en ;
                <http://www.w3.org/2004/02/skos/core#example> "Your life has temporal part the first year of your life"@en .


###  https://www.commoncoreontologies.org/mro/BFO_0000124
mro:BFO_0000124 rdf:type owl:ObjectProperty ;
                rdfs:subPropertyOf mro:mro00000001 ;
                owl:inverseOf mro:BFO_0000171 ;
                rdfs:domain [ owl:intersectionOf ( obo:BFO_0000004
                                                   [ rdf:type owl:Class ;
                                                     owl:complementOf obo:BFO_0000006
                                                   ]
                                                 ) ;
                              rdf:type owl:Class
                            ] ;
                rdfs:range [ owl:intersectionOf ( obo:BFO_0000004
                                                  [ rdf:type owl:Class ;
                                                    owl:complementOf obo:BFO_0000006
                                                  ]
                                                ) ;
                             rdf:type owl:Class
                           ] ;
                <http://purl.org/dc/elements/1.1/identifier> "236-BFO" ;
                rdfs:label "location of"@en ;
                <http://www.w3.org/2004/02/skos/core#definition> "b location of c =Def c located in b"@en ;
                <http://www.w3.org/2004/02/skos/core#scopeNote> "Users that require more sophisticated representations of time are encouraged to import a temporal extension of BFO-Core provided by the BFO development team. See documentation for guidance: <https://github.com/BFO-ontology/BFO-2020/tree/master/src/owl/profiles/temporal%20extensions>"@en .


###  https://www.commoncoreontologies.org/mro/BFO_0000127
mro:BFO_0000127 rdf:type owl:ObjectProperty ;
                rdfs:subPropertyOf mro:mro00000001 ;
                owl:inverseOf mro:BFO_0000218 ;
                rdfs:domain obo:BFO_0000040 ;
                rdfs:range obo:BFO_0000016 ;
                <http://purl.org/dc/elements/1.1/identifier> "244-BFO" ;
                rdfs:label "material basis of"@en ;
                <http://www.w3.org/2004/02/skos/core#definition> "b material basis of c =Def c has material basis b"@en ;
                <http://www.w3.org/2004/02/skos/core#scopeNote> "Users that require more sophisticated representations of time are encouraged to import a temporal extension of BFO-Core provided by the BFO development team. See documentation for guidance: <https://github.com/BFO-ontology/BFO-2020/tree/master/src/owl/profiles/temporal%20extensions>"@en .


###  https://www.commoncoreontologies.org/mro/BFO_0000129
mro:BFO_0000129 rdf:type owl:ObjectProperty ;
                rdfs:subPropertyOf mro:BFO_0000176 ;
                rdfs:domain obo:BFO_0000040 ;
                rdfs:range obo:BFO_0000040 ;
                <http://purl.org/dc/elements/1.1/identifier> "228-BFO" ;
                rdfs:label "member part of"@en ;
                <http://www.w3.org/2004/02/skos/core#definition> "b member part of c =Def b is an object & c is a material entity & there is some time t such that b continuant part of c at t & there is a mutually exhaustive and pairwise disjoint partition of c into objects x1, ..., xn (for some n ≠ 1) with b = xi (for some 1 <= i <= n)"@en ;
                <http://www.w3.org/2004/02/skos/core#scopeNote> "Users that require more sophisticated representations of time are encouraged to import a temporal extension of BFO-Core provided by the BFO development team. See documentation for guidance: <https://github.com/BFO-ontology/BFO-2020/tree/master/src/owl/profiles/temporal%20extensions>"@en .


###  https://www.commoncoreontologies.org/mro/BFO_0000132
mro:BFO_0000132 rdf:type owl:ObjectProperty ;
                rdfs:subPropertyOf mro:mro00000001 ;
                rdf:type owl:TransitiveProperty ;
                rdfs:domain obo:BFO_0000003 ;
                rdfs:range obo:BFO_0000003 ;
                <http://purl.org/dc/elements/1.1/identifier> "003-BFO" ;
                rdfs:label "occurrent part of"@en ;
                <http://www.w3.org/2004/02/skos/core#definition> "(Elucidation) occurrent part of is a relation between occurrents b and c when b is part of c"@en ;
                <http://www.w3.org/2004/02/skos/core#example> "Mary's 5th birthday is an occurrent part of Mary's life; the first set of the tennis match is an occurrent part of the tennis match"@en .


###  https://www.commoncoreontologies.org/mro/BFO_0000139
mro:BFO_0000139 rdf:type owl:ObjectProperty ;
                rdfs:subPropertyOf mro:BFO_0000132 ;
                rdf:type owl:TransitiveProperty ;
                rdfs:domain obo:BFO_0000003 ;
                rdfs:range obo:BFO_0000003 ;
                <http://purl.org/dc/elements/1.1/identifier> "078-BFO" ;
                rdfs:label "temporal part of"@en ;
                <http://www.w3.org/2004/02/skos/core#definition> "b temporal part of c =Def b occurrent part of c & (b and c are temporal regions) or (b and c are spatiotemporal regions & b temporally projects onto an occurrent part of the temporal region that c temporally projects onto) or (b and c are processes or process boundaries & b occupies a temporal region that is an occurrent part of the temporal region that c occupies)"@en ;
                <http://www.w3.org/2004/02/skos/core#example> "Your heart beating from 4pm to 5pm today is a temporal part of the process of your heart beating; the 4th year of your life is a temporal part of your life, as is the process boundary which separates the 3rd and 4th years of your life; the first quarter of a game of football is a temporal part of the whole game"@en .


###  https://www.commoncoreontologies.org/mro/BFO_0000153
mro:BFO_0000153 rdf:type owl:ObjectProperty ;
                rdfs:subPropertyOf mro:mro00000001 ;
                rdf:type owl:FunctionalProperty ;
                rdfs:domain obo:BFO_0000011 ;
                rdfs:range obo:BFO_0000008 ;
                <http://purl.org/dc/elements/1.1/identifier> "080-BFO" ;
                rdfs:label "temporally projects onto"@en ;
                <http://www.w3.org/2004/02/skos/core#definition> "(Elucidation) temporally projects onto is a relation between a spatiotemporal region s and some temporal region which is the temporal extent of s"@en ;
                <http://www.w3.org/2004/02/skos/core#example> "The world line of a particle temporally projects onto the temporal region extending from the beginning to the end of the existence of the particle"@en .


###  https://www.commoncoreontologies.org/mro/BFO_0000171
mro:BFO_0000171 rdf:type owl:ObjectProperty ;
                rdfs:subPropertyOf mro:mro00000001 ;
                rdfs:domain [ owl:intersectionOf ( obo:BFO_0000004
                                                   [ rdf:type owl:Class ;
                                                     owl:complementOf obo:BFO_0000006
                                                   ]
                                                 ) ;
                              rdf:type owl:Class
                            ] ;
                rdfs:range [ owl:intersectionOf ( obo:BFO_0000004
                                                  [ rdf:type owl:Class ;
                                                    owl:complementOf obo:BFO_0000006
                                                  ]
                                                ) ;
                             rdf:type owl:Class
                           ] ;
                <http://purl.org/dc/elements/1.1/identifier> "234-BFO" ;
                rdfs:label "located in"@en ;
                <http://www.w3.org/2004/02/skos/core#definition> "b located in c =Def b is an independent continuant & c is an independent & neither is a spatial region & there is some time t such that the spatial region which b occupies at t is continuant part of the spatial region which c occupies at t"@en ;
                <http://www.w3.org/2004/02/skos/core#scopeNote> "Users that require more sophisticated representations of time are encouraged to import a temporal extension of BFO-Core provided by the BFO development team. See documentation for guidance: <https://github.com/BFO-ontology/BFO-2020/tree/master/src/owl/profiles/temporal%20extensions>"@en .


###  https://www.commoncoreontologies.org/mro/BFO_0000176
mro:BFO_0000176 rdf:type owl:ObjectProperty ;
                rdfs:subPropertyOf mro:mro00000001 ;
                owl:inverseOf mro:BFO_0000178 ;
                rdfs:domain obo:BFO_0000002 ;
                rdfs:range obo:BFO_0000002 ;
                <http://purl.org/dc/elements/1.1/identifier> "221-BFO" ;
                rdfs:label "continuant part of"@en ;
                <http://www.w3.org/2004/02/skos/core#definition> "b continuant part of c =Def b and c are continuants & there is some time t such that b and c exist at t & b continuant part of c at t"@en ;
                <http://www.w3.org/2004/02/skos/core#example> "Milk teeth continuant part of human; surgically removed tumour continuant part of organism"@en ;
                <http://www.w3.org/2004/02/skos/core#scopeNote> "Users that require more sophisticated representations of time are encouraged to import a temporal extension of BFO-Core provided by the BFO development team. See documentation for guidance: <https://github.com/BFO-ontology/BFO-2020/tree/master/src/owl/profiles/temporal%20extensions>"@en .


###  https://www.commoncoreontologies.org/mro/BFO_0000178
mro:BFO_0000178 rdf:type owl:ObjectProperty ;
                rdfs:subPropertyOf mro:mro00000001 ;
                rdfs:domain obo:BFO_0000002 ;
                rdfs:range obo:BFO_0000002 ;
                <http://purl.org/dc/elements/1.1/identifier> "271-BFO" ;
                rdfs:label "has continuant part"@en ;
                <http://www.w3.org/2004/02/skos/core#definition> "b has continuant part c =Def c continuant part of b"@en ;
                <http://www.w3.org/2004/02/skos/core#scopeNote> "Users that require more sophisticated representations of time are encouraged to import a temporal extension of BFO-Core provided by the BFO development team. See documentation for guidance: <https://github.com/BFO-ontology/BFO-2020/tree/master/src/owl/profiles/temporal%20extensions>"@en .


###  https://www.commoncoreontologies.org/mro/BFO_0000183
mro:BFO_0000183 rdf:type owl:ObjectProperty ;
                rdfs:subPropertyOf mro:mro00000001 ;
                rdfs:domain [ rdf:type owl:Class ;
                              owl:unionOf ( obo:BFO_0000029
                                            obo:BFO_0000040
                                          )
                            ] ;
                rdfs:range [ rdf:type owl:Class ;
                             owl:unionOf ( obo:BFO_0000015
                                           obo:BFO_0000035
                                         )
                           ] ;
                <http://purl.org/dc/elements/1.1/identifier> "267-BFO" ;
                rdfs:label "environs"@en ;
                <http://www.w3.org/2004/02/skos/core#altLabel> "contains process"@en ;
                <http://www.w3.org/2004/02/skos/core#definition> "b environs c =Def c occurs in b"@en ;
                <http://www.w3.org/2004/02/skos/core#example> "Mouth environs process of mastication; city environs traffic"@en .


###  https://www.commoncoreontologies.org/mro/BFO_0000184
mro:BFO_0000184 rdf:type owl:ObjectProperty ;
                rdfs:subPropertyOf mro:mro00000001 ;
                owl:inverseOf mro:BFO_0000185 ;
                rdf:type owl:FunctionalProperty ,
                         owl:InverseFunctionalProperty ;
                rdfs:domain obo:BFO_0000182 ;
                rdfs:range obo:BFO_0000040 ;
                <http://purl.org/dc/elements/1.1/identifier> "144-BFO" ;
                rdfs:label "history of"@en ;
                <http://www.w3.org/2004/02/skos/core#definition> "(Elucidation) history of is a relation between history b and material entity c such that b is the unique history of c"@en ;
                <http://www.w3.org/2004/02/skos/core#example> "This life is the history of this organism"@en .


###  https://www.commoncoreontologies.org/mro/BFO_0000185
mro:BFO_0000185 rdf:type owl:ObjectProperty ;
                rdfs:subPropertyOf mro:mro00000001 ;
                rdfs:domain obo:BFO_0000040 ;
                rdfs:range obo:BFO_0000182 ;
                <http://purl.org/dc/elements/1.1/identifier> "145-BFO" ;
                rdfs:label "has history"@en ;
                <http://www.w3.org/2004/02/skos/core#definition> "b has history c =Def c history of b"@en ;
                <http://www.w3.org/2004/02/skos/core#example> "This organism has history this life"@en .


###  https://www.commoncoreontologies.org/mro/BFO_0000194
mro:BFO_0000194 rdf:type owl:ObjectProperty ;
                rdfs:subPropertyOf mro:mro00000001 ;
                owl:inverseOf mro:BFO_0000195 ;
                rdfs:domain [ rdf:type owl:Class ;
                              owl:unionOf ( obo:BFO_0000020
                                            [ owl:intersectionOf ( obo:BFO_0000004
                                                                   [ rdf:type owl:Class ;
                                                                     owl:complementOf obo:BFO_0000006
                                                                   ]
                                                                 ) ;
                                              rdf:type owl:Class
                                            ]
                                          )
                            ] ;
                rdfs:range obo:BFO_0000020 ;
                <http://purl.org/dc/elements/1.1/identifier> "260-BFO" ;
                rdfs:label "specifically depended on by"@en ;
                <http://www.w3.org/2004/02/skos/core#altLabel> "s-depended on by"@en ;
                <http://www.w3.org/2004/02/skos/core#definition> "b specifically depended on by c =Def c specifically depends on b"@en ;
                <http://www.w3.org/2004/02/skos/core#example> "Coloured object specifically depended on by colour"@en .


###  https://www.commoncoreontologies.org/mro/BFO_0000195
mro:BFO_0000195 rdf:type owl:ObjectProperty ;
                rdfs:subPropertyOf mro:mro00000001 ;
                rdfs:domain obo:BFO_0000020 ;
                rdfs:range [ rdf:type owl:Class ;
                             owl:unionOf ( obo:BFO_0000020
                                           [ owl:intersectionOf ( obo:BFO_0000004
                                                                  [ rdf:type owl:Class ;
                                                                    owl:complementOf obo:BFO_0000006
                                                                  ]
                                                                ) ;
                                             rdf:type owl:Class
                                           ]
                                         )
                           ] ;
                <http://purl.org/dc/elements/1.1/identifier> "012-BFO" ;
                rdfs:label "specifically depends on"@en ;
                <http://www.w3.org/2004/02/skos/core#altLabel> "s-depends on"@en ;
                <http://www.w3.org/2004/02/skos/core#definition> "(Elucidation) specifically depends on is a relation between a specifically dependent continuant b and specifically dependent continuant or independent continuant that is not a spatial region c such that b and c share no parts in common & b is of a nature such that at all times t it cannot exist unless c exists & b is not a boundary of c"@en ;
                <http://www.w3.org/2004/02/skos/core#example> "A shape specifically depends on the shaped object; hue, saturation and brightness of a colour sample specifically depends on each other"@en ;
                <http://www.w3.org/2004/02/skos/core#scopeNote> "The analogue of specifically depends on for occurrents is has participant."@en .


###  https://www.commoncoreontologies.org/mro/BFO_0000196
mro:BFO_0000196 rdf:type owl:ObjectProperty ;
                rdfs:subPropertyOf mro:BFO_0000194 ;
                owl:inverseOf mro:BFO_0000197 ;
                rdfs:domain [ owl:intersectionOf ( obo:BFO_0000004
                                                   [ rdf:type owl:Class ;
                                                     owl:complementOf obo:BFO_0000006
                                                   ]
                                                 ) ;
                              rdf:type owl:Class
                            ] ;
                rdfs:range obo:BFO_0000020 ;
                <http://purl.org/dc/elements/1.1/identifier> "053-BFO" ;
                rdfs:label "bearer of"@en ;
                <http://www.w3.org/2004/02/skos/core#definition> "b bearer of c =Def c inheres in b"@en ;
                <http://www.w3.org/2004/02/skos/core#example> "A patch of ink is the bearer of a colour quality; an organism is the bearer of a temperature quality"@en .


###  https://www.commoncoreontologies.org/mro/BFO_0000197
mro:BFO_0000197 rdf:type owl:ObjectProperty ;
                rdfs:subPropertyOf mro:BFO_0000195 ;
                rdfs:domain obo:BFO_0000020 ;
                rdfs:range [ owl:intersectionOf ( obo:BFO_0000004
                                                  [ rdf:type owl:Class ;
                                                    owl:complementOf obo:BFO_0000006
                                                  ]
                                                ) ;
                             rdf:type owl:Class
                           ] ;
                <http://purl.org/dc/elements/1.1/identifier> "051-BFO" ;
                rdfs:label "inheres in"@en ;
                <http://www.w3.org/2004/02/skos/core#definition> "b inheres in c =Def b is a specifically dependent continuant & c is an independent continuant that is not a spatial region & b specifically depends on c"@en ;
                <http://www.w3.org/2004/02/skos/core#example> "A shape inheres in a shaped object; a mass inheres in a material entity"@en .


###  https://www.commoncoreontologies.org/mro/BFO_0000199
mro:BFO_0000199 rdf:type owl:ObjectProperty ;
                rdfs:subPropertyOf mro:mro00000001 ;
                owl:inverseOf mro:ont00001874 ;
                rdf:type owl:FunctionalProperty ;
                rdfs:domain [ rdf:type owl:Class ;
                              owl:unionOf ( obo:BFO_0000015
                                            obo:BFO_0000035
                                          )
                            ] ;
                rdfs:range obo:BFO_0000008 ;
                <http://purl.org/dc/elements/1.1/identifier> "132-BFO" ;
                rdfs:label "occupies temporal region"@en ;
                <http://www.w3.org/2004/02/skos/core#definition> "p occupies temporal region t =Def p is a process or process boundary & the spatiotemporal region occupied by p temporally projects onto t"@en ;
                <http://www.w3.org/2004/02/skos/core#example> "The Second World War occupies the temporal region September 1, 1939 - September 2, 1945"@en .


###  https://www.commoncoreontologies.org/mro/BFO_0000200
mro:BFO_0000200 rdf:type owl:ObjectProperty ;
                rdfs:subPropertyOf mro:mro00000001 ;
                rdf:type owl:FunctionalProperty ;
                rdfs:domain [ rdf:type owl:Class ;
                              owl:unionOf ( obo:BFO_0000015
                                            obo:BFO_0000035
                                          )
                            ] ;
                rdfs:range obo:BFO_0000011 ;
                <http://purl.org/dc/elements/1.1/identifier> "082-BFO" ;
                rdfs:label "occupies spatiotemporal region"@en ;
                <http://www.w3.org/2004/02/skos/core#definition> "(Elucidation) occupies spatiotemporal region is a relation between a process or process boundary p and the spatiotemporal region s which is its spatiotemporal extent"@en ;
                <http://www.w3.org/2004/02/skos/core#example> "A particle emitted by a nuclear reactor occupies the spatiotemporal region which is its trajectory"@en .


###  https://www.commoncoreontologies.org/mro/BFO_0000210
mro:BFO_0000210 rdf:type owl:ObjectProperty ;
                rdfs:subPropertyOf mro:mro00000001 ;
                rdfs:domain [ owl:intersectionOf ( obo:BFO_0000004
                                                   [ rdf:type owl:Class ;
                                                     owl:complementOf obo:BFO_0000006
                                                   ]
                                                 ) ;
                              rdf:type owl:Class
                            ] ;
                rdfs:range obo:BFO_0000006 ;
                <http://purl.org/dc/elements/1.1/identifier> "232-BFO" ;
                rdfs:label "occupies spatial region"@en ;
                <http://www.w3.org/2004/02/skos/core#definition> "b occupies spatial region r =Def b is an independent continuant that is not a spatial region & r is a spatial region & there is some time t such that every continuant part of b occupies some continuant part of r at t and no continuant part of b occupies any spatial region that is not a continuant part of r at t"@en ;
                <http://www.w3.org/2004/02/skos/core#scopeNote> "Users that require more sophisticated representations of time are encouraged to import a temporal extension of BFO-Core provided by the BFO development team. See documentation for guidance: <https://github.com/BFO-ontology/BFO-2020/tree/master/src/owl/profiles/temporal%20extensions>"@en .


###  https://www.commoncoreontologies.org/mro/BFO_0000216
mro:BFO_0000216 rdf:type owl:ObjectProperty ;
                rdfs:subPropertyOf mro:mro00000001 ;
                rdfs:domain obo:BFO_0000011 ;
                rdfs:range obo:BFO_0000006 ;
                <http://purl.org/dc/elements/1.1/identifier> "246-BFO" ;
                rdfs:label "spatially projects onto"@en ;
                <http://www.w3.org/2004/02/skos/core#definition> "(Elucidation) spatially projects onto is a relation between some spatiotemporal region b and spatial region c such that at some time t, c is the spatial extent of b at t"@en ;
                <http://www.w3.org/2004/02/skos/core#scopeNote> "Users that require more sophisticated representations of time are encouraged to import a temporal extension of BFO-Core provided by the BFO development team. See documentation for guidance: <https://github.com/BFO-ontology/BFO-2020/tree/master/src/owl/profiles/temporal%20extensions>"@en .


###  https://www.commoncoreontologies.org/mro/BFO_0000218
mro:BFO_0000218 rdf:type owl:ObjectProperty ;
                rdfs:subPropertyOf mro:mro00000001 ;
                rdfs:domain obo:BFO_0000016 ;
                rdfs:range obo:BFO_0000040 ;
                <http://purl.org/dc/elements/1.1/identifier> "242-BFO" ;
                rdfs:label "has material basis"@en ;
                <http://www.w3.org/2004/02/skos/core#definition> "b has material basis c =Def b is a disposition & c is a material entity & there is some d bearer of b & there is some time t such that c is a continuant part of d at t & d has disposition b because c is a continuant part of d at t"@en ;
                <http://www.w3.org/2004/02/skos/core#scopeNote> "Users that require more sophisticated representations of time are encouraged to import a temporal extension of BFO-Core provided by the BFO development team. See documentation for guidance: <https://github.com/BFO-ontology/BFO-2020/tree/master/src/owl/profiles/temporal%20extensions>"@en .


###  https://www.commoncoreontologies.org/mro/BFO_0000221
mro:BFO_0000221 rdf:type owl:ObjectProperty ;
                rdfs:subPropertyOf mro:mro00000001 ;
                owl:inverseOf mro:BFO_0000222 ;
                rdfs:domain obo:BFO_0000203 ;
                rdfs:range obo:BFO_0000008 ;
                <http://purl.org/dc/elements/1.1/identifier> "268-BFO" ;
                rdfs:label "first instant of"@en ;
                <http://www.w3.org/2004/02/skos/core#definition> "t first instant of t' =Def t is a temporal instant & t' is a temporal region t' & t precedes all temporal parts of t' other than t"@en ;
                <http://www.w3.org/2004/02/skos/core#example> "An hour starting at midnight yesterday has first instant midnight yesterday"@en .


###  https://www.commoncoreontologies.org/mro/BFO_0000222
mro:BFO_0000222 rdf:type owl:ObjectProperty ;
                rdfs:subPropertyOf mro:mro00000001 ;
                rdf:type owl:FunctionalProperty ;
                rdfs:domain obo:BFO_0000008 ;
                rdfs:range obo:BFO_0000203 ;
                <http://purl.org/dc/elements/1.1/identifier> "261-BFO" ;
                rdfs:label "has first instant"@en ;
                <http://www.w3.org/2004/02/skos/core#definition> "t has first instant t' =Def t' first instant of t"@en ;
                <http://www.w3.org/2004/02/skos/core#example> "The first hour of a year has first instant midnight on December 31"@en .


###  https://www.commoncoreontologies.org/mro/BFO_0000223
mro:BFO_0000223 rdf:type owl:ObjectProperty ;
                rdfs:subPropertyOf mro:mro00000001 ;
                owl:inverseOf mro:BFO_0000224 ;
                rdfs:domain obo:BFO_0000203 ;
                rdfs:range obo:BFO_0000008 ;
                <http://purl.org/dc/elements/1.1/identifier> "269-BFO" ;
                rdfs:label "last instant of"@en ;
                <http://www.w3.org/2004/02/skos/core#definition> "t last instant of t' =Def t is a temporal instant & t' is a temporal region & all temporal parts of t' other than t precede t"@en ;
                <http://www.w3.org/2004/02/skos/core#example> "Last midnight is the last instant of yesterday"@en .


###  https://www.commoncoreontologies.org/mro/BFO_0000224
mro:BFO_0000224 rdf:type owl:ObjectProperty ;
                rdfs:subPropertyOf mro:mro00000001 ;
                rdf:type owl:FunctionalProperty ;
                rdfs:domain obo:BFO_0000008 ;
                rdfs:range obo:BFO_0000203 ;
                <http://purl.org/dc/elements/1.1/identifier> "215-BFO" ;
                rdfs:label "has last instant"@en ;
                <http://www.w3.org/2004/02/skos/core#definition> "t has last instant t' =Def t' last instant of t"@en ;
                <http://www.w3.org/2004/02/skos/core#example> "The last hour of a year has last instant midnight December 31"@en .


###  https://www.commoncoreontologies.org/mro/mro00000001
mro:mro00000001 rdf:type owl:ObjectProperty ;
                rdfs:label "Modal Object Property"@en .


###  https://www.commoncoreontologies.org/mro/ont00001774
mro:ont00001774 rdf:type owl:ObjectProperty ;
                rdfs:subPropertyOf mro:ont00001902 ;
                owl:inverseOf mro:ont00001883 ;
                rdfs:label "has brother"@en ;
                cco:ont00001760 <https://www.commoncoreontologies.org/ModalRelationOntology> .


###  https://www.commoncoreontologies.org/mro/ont00001775
mro:ont00001775 rdf:type owl:ObjectProperty ;
                rdfs:subPropertyOf mro:mro00000001 ;
                owl:inverseOf mro:ont00001928 ;
                rdfs:domain obo:BFO_0000004 ;
                rdfs:range obo:BFO_0000004 ;
                rdfs:label "is successor of"@en ;
                <http://www.w3.org/2004/02/skos/core#definition> "A continuant c2 is a successor of some continuant c1 iff there is some process p1 and c1 is an input to p1 and c2 is an output of p1. Inverse of is predecessor. "@en ;
                cco:ont00001760 <https://www.commoncoreontologies.org/ModalRelationOntology> .


###  https://www.commoncoreontologies.org/mro/ont00001776
mro:ont00001776 rdf:type owl:ObjectProperty ;
                rdfs:subPropertyOf mro:ont00001945 ;
                owl:inverseOf mro:ont00001876 ;
                rdfs:label "has grandfather"@en ;
                cco:ont00001760 <https://www.commoncoreontologies.org/ModalRelationOntology> .


###  https://www.commoncoreontologies.org/mro/ont00001777
mro:ont00001777 rdf:type owl:ObjectProperty ;
                rdfs:subPropertyOf mro:BFO_0000117 ;
                owl:inverseOf mro:ont00001857 ;
                rdfs:domain obo:BFO_0000015 ;
                rdfs:range obo:BFO_0000015 ;
                rdfs:label "has process part"@en ;
                <http://www.w3.org/2004/02/skos/core#definition> "x has_process_part y iff x and y are instances of Process, such that y occurs during the temporal interval of x, and y either provides an input to x or receives an output of x, or both."@en ;
                cco:ont00001760 <https://www.commoncoreontologies.org/ModalRelationOntology> .


###  https://www.commoncoreontologies.org/mro/ont00001778
mro:ont00001778 rdf:type owl:ObjectProperty ;
                rdfs:subPropertyOf mro:BFO_0000057 ;
                owl:inverseOf mro:ont00001936 ;
                rdfs:label "has object"@en ;
                <http://www.w3.org/2004/02/skos/core#definition> "If p is a process and c is a continuant, then p has object c if and only if p is performed by an agent and c is part of the projected state that agent intends to achieve by performing p."@en ;
                cco:ont00001760 <https://www.commoncoreontologies.org/ModalRelationOntology> .


###  https://www.commoncoreontologies.org/mro/ont00001779
mro:ont00001779 rdf:type owl:ObjectProperty ;
                rdfs:subPropertyOf mro:mro00000001 ;
                owl:inverseOf mro:ont00001848 ;
                rdfs:domain obo:BFO_0000038 ;
                rdfs:range obo:BFO_0000148 ;
                rdfs:label "has inside instant"@en ;
                <http://www.w3.org/2004/02/skos/core#definition> "For Temporal Interval t1 and Temporal Instant t2, t1 has inside instant t2 if and only if there exists Temporal Instants t3 and t4 that are part of t1 and non-identical with t2, such that t3 is before t2 and t4 is after t2."@en ;
                cco:ont00001754 "J. F. Allen and J. A. G. M. Koomen. Planning using a temporal world model. In Proceedings of the 8th International Joint Conference on Artificial Intelligence (IJCAI-1983)  pages 741–747. Available at: https://www.ijcai.org/Proceedings/83-2/Papers/036.pdf"@en ;
                cco:ont00001760 <https://www.commoncoreontologies.org/ModalRelationOntology> .


###  https://www.commoncoreontologies.org/mro/ont00001780
mro:ont00001780 rdf:type owl:ObjectProperty ;
                rdfs:subPropertyOf mro:ont00001842 ;
                owl:inverseOf mro:ont00001786 ;
                rdfs:label "has mother"@en ;
                cco:ont00001760 <https://www.commoncoreontologies.org/ModalRelationOntology> .


###  https://www.commoncoreontologies.org/mro/ont00001781
mro:ont00001781 rdf:type owl:ObjectProperty ;
                rdfs:subPropertyOf mro:ont00001996 ;
                owl:inverseOf mro:ont00001979 ;
                rdfs:label "has step sister"@en ;
                cco:ont00001760 <https://www.commoncoreontologies.org/ModalRelationOntology> .


###  https://www.commoncoreontologies.org/mro/ont00001782
mro:ont00001782 rdf:type owl:ObjectProperty ;
                rdfs:subPropertyOf mro:ont00001832 ;
                rdfs:domain obo:BFO_0000027 ;
                rdfs:range [ owl:intersectionOf ( obo:BFO_0000004
                                                  [ rdf:type owl:Class ;
                                                    owl:complementOf obo:BFO_0000006
                                                  ]
                                                ) ;
                             rdf:type owl:Class
                           ] ;
                rdfs:label "has all members located in"@en ;
                <http://www.w3.org/2004/02/skos/core#definition> "x has all members located in y iff x is an instance of Object Aggregate and y is an instance of independent continuant but not a spatial region, and every member of x is located in y."@en ;
                cco:ont00001760 <https://www.commoncoreontologies.org/ModalRelationOntology> .


###  https://www.commoncoreontologies.org/mro/ont00001783
mro:ont00001783 rdf:type owl:ObjectProperty ;
                rdfs:subPropertyOf mro:ont00001945 ;
                owl:inverseOf mro:ont00001820 ;
                rdfs:label "is granddaughter of"@en ;
                cco:ont00001760 <https://www.commoncoreontologies.org/ModalRelationOntology> .


###  https://www.commoncoreontologies.org/mro/ont00001784
mro:ont00001784 rdf:type owl:ObjectProperty ;
                rdfs:subPropertyOf mro:ont00001818 ;
                owl:inverseOf mro:ont00001881 ;
                rdfs:label "has son in law"@en ;
                cco:ont00001760 <https://www.commoncoreontologies.org/ModalRelationOntology> .


###  https://www.commoncoreontologies.org/mro/ont00001785
mro:ont00001785 rdf:type owl:ObjectProperty ;
                rdfs:subPropertyOf mro:ont00001865 ;
                owl:inverseOf mro:ont00001988 ;
                rdfs:label "has uncle"@en ;
                cco:ont00001760 <https://www.commoncoreontologies.org/ModalRelationOntology> .


###  https://www.commoncoreontologies.org/mro/ont00001786
mro:ont00001786 rdf:type owl:ObjectProperty ;
                rdfs:subPropertyOf mro:ont00001995 ;
                rdfs:label "is mother of"@en ;
                cco:ont00001760 <https://www.commoncoreontologies.org/ModalRelationOntology> .


###  https://www.commoncoreontologies.org/mro/ont00001787
mro:ont00001787 rdf:type owl:ObjectProperty ;
                rdfs:subPropertyOf mro:BFO_0000056 ;
                owl:inverseOf mro:ont00001833 ;
                rdfs:label "agent in"@en ;
                <http://www.w3.org/2004/02/skos/core#definition> "x agent_in y iff y is an instance of Process and x is an instance of Agent, such that x is causally active in y."@en ;
                cco:ont00001760 <https://www.commoncoreontologies.org/ModalRelationOntology> .


###  https://www.commoncoreontologies.org/mro/ont00001788
mro:ont00001788 rdf:type owl:ObjectProperty ;
                rdfs:subPropertyOf mro:ont00001789 ;
                owl:inverseOf mro:ont00001994 ;
                rdfs:label "has paternal aunt"@en ;
                cco:ont00001760 <https://www.commoncoreontologies.org/ModalRelationOntology> .


###  https://www.commoncoreontologies.org/mro/ont00001789
mro:ont00001789 rdf:type owl:ObjectProperty ;
                rdfs:subPropertyOf mro:ont00001865 ;
                owl:inverseOf mro:ont00001955 ;
                rdfs:label "has aunt"@en ;
                cco:ont00001760 <https://www.commoncoreontologies.org/ModalRelationOntology> .


###  https://www.commoncoreontologies.org/mro/ont00001790
mro:ont00001790 rdf:type owl:ObjectProperty ;
                rdfs:subPropertyOf mro:ont00001785 ;
                owl:inverseOf mro:ont00001929 ;
                rdfs:label "has maternal uncle"@en ;
                cco:ont00001760 <https://www.commoncoreontologies.org/ModalRelationOntology> .


###  https://www.commoncoreontologies.org/mro/ont00001791
mro:ont00001791 rdf:type owl:ObjectProperty ;
                rdfs:subPropertyOf mro:ont00001810 ;
                rdfs:domain obo:BFO_0000141 ;
                rdfs:range obo:BFO_0000141 ;
                rdfs:label "coincides with"@en ;
                <http://www.w3.org/2004/02/skos/core#definition> "An immaterial entity im1 coincides with some immaterial entity im2 iff im1 is a spatial part of im2 and im2 is a spatial part of im1."@en ;
                <http://www.w3.org/2004/02/skos/core#scopeNote> "Given a stronger temporal interpretation, this property may be transitive and symmetric. For more info please refer to https://github.com/BFO-ontology/BFO-2020/tree/master/src/owl/temporal%20extensions."@en ;
                cco:ont00001760 <https://www.commoncoreontologies.org/ModalRelationOntology> .


###  https://www.commoncoreontologies.org/mro/ont00001792
mro:ont00001792 rdf:type owl:ObjectProperty ;
                rdfs:subPropertyOf mro:ont00001902 ;
                owl:inverseOf mro:ont00001851 ;
                rdfs:label "has sister"@en ;
                cco:ont00001760 <https://www.commoncoreontologies.org/ModalRelationOntology> .


###  https://www.commoncoreontologies.org/mro/ont00001793
mro:ont00001793 rdf:type owl:ObjectProperty ;
                rdfs:subPropertyOf mro:ont00001975 ;
                owl:inverseOf mro:ont00001948 ;
                rdfs:label "has half sister"@en ;
                cco:ont00001760 <https://www.commoncoreontologies.org/ModalRelationOntology> .


###  https://www.commoncoreontologies.org/mro/ont00001794
mro:ont00001794 rdf:type owl:ObjectProperty ;
                rdfs:subPropertyOf mro:ont00001977 ;
                owl:inverseOf mro:ont00001815 ;
                rdfs:domain cco:ont00001180 ;
                rdfs:range cco:ont00001180 ;
                rdfs:label "has subsidiary"@en ;
                <http://www.w3.org/2004/02/skos/core#definition> "An Organization o1 has_subsidiary Organization o2 iff o1 controls o2 by having the capacity to determine the outcome of decisions about o2's financial and operating policies."@en ;
                cco:ont00001754 "http://www.austlii.edu.au/legis/cth/consol_act/ca2001172/s50aa.html" ;
                cco:ont00001760 <https://www.commoncoreontologies.org/ModalRelationOntology> .


###  https://www.commoncoreontologies.org/mro/ont00001795
mro:ont00001795 rdf:type owl:ObjectProperty ;
                rdfs:subPropertyOf mro:ont00001924 ;
                owl:inverseOf mro:ont00001869 ;
                rdfs:domain obo:BFO_0000038 ;
                rdfs:range obo:BFO_0000038 ;
                rdfs:label "has inside interval"@en ;
                <http://www.w3.org/2004/02/skos/core#definition> "A Temporal Interval INT2 has inside interval some Temporal Interval INT1 iff there exist Temporal Instants inst1, inst2, inst3, and inst4 such that inst1 is the starting instant of INT1, inst2 is the ending instant of INT1, inst3 is the starting instant of INT2, inst4 is the ending instant of INT2, inst3 is before inst1, and inst2 is before inst4."@en ;
                cco:ont00001754 "J. F. Allen and J. A. G. M. Koomen. Planning using a temporal world model. In Proceedings of the 8th International Joint Conference on Artificial Intelligence (IJCAI-1983)  pages 741–747. Available at: https://www.ijcai.org/Proceedings/83-2/Papers/036.pdf"@en ;
                cco:ont00001760 <https://www.commoncoreontologies.org/ModalRelationOntology> .


###  https://www.commoncoreontologies.org/mro/ont00001796
mro:ont00001796 rdf:type owl:ObjectProperty ;
                rdfs:subPropertyOf mro:ont00001944 ;
                owl:inverseOf mro:ont00001909 ;
                rdfs:domain obo:BFO_0000141 ;
                rdfs:range obo:BFO_0000141 ;
                rdfs:label "tangential part of"@en ;
                <http://www.w3.org/2004/02/skos/core#definition> "An immaterial entity im1 is a tangential part of some immaterial entity im2 iff im1 is a spatial part of im2 and there exists some immaterial entity im3 such that im3 externally connects with im1 and im3 externally connects with im2."@en ;
                <http://www.w3.org/2004/02/skos/core#scopeNote> "Given a stronger temporal interpretation, this property may be transitive. For more info please refer to https://github.com/BFO-ontology/BFO-2020/tree/master/src/owl/temporal%20extensions."@en ;
                cco:ont00001754 "Randell, D. A., Cui, Z. and Cohn, A. G.: 1992, \"A spatial logic based on regions and connection,\" Proc. 3rd Int. Conf. on Knowledge Representation and Reasoning, Morgan Kaufmann, San Mateo, pp. 165-176. Available at: https://www.dpi.inpe.br/gilberto/references/cohn_rcc.pdf"@en ;
                cco:ont00001760 <https://www.commoncoreontologies.org/ModalRelationOntology> .


###  https://www.commoncoreontologies.org/mro/ont00001797
mro:ont00001797 rdf:type owl:ObjectProperty ;
                rdfs:subPropertyOf mro:ont00001810 ;
                rdfs:domain obo:BFO_0000141 ;
                rdfs:range obo:BFO_0000141 ;
                rdfs:label "partially overlaps with"@en ;
                <http://www.w3.org/2004/02/skos/core#definition> "An immaterial entity im1 partially overlaps with some immaterial entity im2 iff im1 overlaps with im2 and im1 is not a spatial part of im2 and im2 is not a spatial part of im1."@en ;
                <http://www.w3.org/2004/02/skos/core#scopeNote> "Given a stronger temporal interpretation, this property may be symmetric. For more info please refer to https://github.com/BFO-ontology/BFO-2020/tree/master/src/owl/temporal%20extensions."@en ;
                cco:ont00001754 "Randell, D. A., Cui, Z. and Cohn, A. G.: 1992, \"A spatial logic based on regions and connection,\" Proc. 3rd Int. Conf. on Knowledge Representation and Reasoning, Morgan Kaufmann, San Mateo, pp. 165-176. Available at: https://www.dpi.inpe.br/gilberto/references/cohn_rcc.pdf"@en ;
                cco:ont00001760 <https://www.commoncoreontologies.org/ModalRelationOntology> .


###  https://www.commoncoreontologies.org/mro/ont00001798
mro:ont00001798 rdf:type owl:ObjectProperty ;
                rdfs:subPropertyOf mro:ont00001939 ;
                owl:inverseOf mro:ont00001943 ;
                rdfs:domain cco:ont00001262 ;
                rdfs:range cco:ont00001262 ;
                rdfs:label "is supervised by"@en ;
                <http://www.w3.org/2004/02/skos/core#definition> "A person p1 is supervised by a person p2 by virtue of p1 being directed, managed, or overseen by p2."@en ;
                cco:ont00001754 "http://en.wiktionary.org/wiki/supervise)" ;
                cco:ont00001760 <https://www.commoncoreontologies.org/ModalRelationOntology> .


###  https://www.commoncoreontologies.org/mro/ont00001799
mro:ont00001799 rdf:type owl:ObjectProperty ;
                rdfs:subPropertyOf mro:ont00001809 ;
                rdfs:domain obo:BFO_0000023 ;
                rdfs:range obo:BFO_0000027 ;
                rdfs:label "role of aggregate"@en ;
                <http://www.w3.org/2004/02/skos/core#definition> "x role_of_aggregate y iff y is an instance of Object Aggregate and x is an instance of Role, and x inheres_in_aggregate y."@en ;
                cco:ont00001760 <https://www.commoncoreontologies.org/ModalRelationOntology> .


###  https://www.commoncoreontologies.org/mro/ont00001800
mro:ont00001800 rdf:type owl:ObjectProperty ;
                rdfs:subPropertyOf mro:ont00001942 ;
                owl:inverseOf mro:ont00001817 ;
                rdfs:domain cco:ont00001324 ;
                rdfs:range obo:BFO_0000015 ;
                rdfs:label "prohibits"@en ;
                <http://www.w3.org/2004/02/skos/core#definition> "x prohibits y at t iff: x is an instance of Process Regulation at time t, and y is an instance of Process at time t, and x prescribes that some y must not occur."@en ;
                <http://www.w3.org/2004/02/skos/core#scopeNote> "Given a stronger temporal interpretation, this property may be asymmetric and irreflexive. For more info please refer to https://github.com/BFO-ontology/BFO-2020/tree/master/src/owl/temporal%20extensions."@en ;
                cco:ont00001760 <https://www.commoncoreontologies.org/ModalRelationOntology> .


###  https://www.commoncoreontologies.org/mro/ont00001801
mro:ont00001801 rdf:type owl:ObjectProperty ;
                rdfs:subPropertyOf mro:mro00000001 ;
                owl:inverseOf mro:ont00001808 ;
                rdfs:range cco:ont00000958 ;
                rdfs:label "is subject of"@en ;
                <http://www.w3.org/2004/02/skos/core#definition> "A primitive relationship between an instance of an Entity and an instance of an Information Content Entity."@en ;
                cco:ont00001760 <https://www.commoncoreontologies.org/ModalRelationOntology> .


###  https://www.commoncoreontologies.org/mro/ont00001802
mro:ont00001802 rdf:type owl:ObjectProperty ;
                rdfs:subPropertyOf mro:ont00001804 ;
                owl:inverseOf mro:ont00001957 ;
                rdfs:label "has husband"@en ;
                cco:ont00001760 <https://www.commoncoreontologies.org/ModalRelationOntology> .


###  https://www.commoncoreontologies.org/mro/ont00001803
mro:ont00001803 rdf:type owl:ObjectProperty ;
                rdfs:subPropertyOf mro:mro00000001 ;
                owl:inverseOf mro:ont00001819 ;
                rdfs:domain obo:BFO_0000003 ;
                rdfs:range obo:BFO_0000003 ;
                rdfs:label "is cause of"@en ;
                <http://www.w3.org/2004/02/skos/core#definition> "x is_cause_of y iff x and y are instances of Occurrent, and y is a consequence of x."@en ;
                cco:ont00001760 <https://www.commoncoreontologies.org/ModalRelationOntology> .


###  https://www.commoncoreontologies.org/mro/ont00001804
mro:ont00001804 rdf:type owl:ObjectProperty ;
                rdfs:subPropertyOf mro:ont00001865 ;
                owl:inverseOf mro:ont00001804 ;
                rdfs:label "is spouse of"@en ;
                <http://www.w3.org/2004/02/skos/core#scopeNote> "Given a stronger temporal interpretation, this property may be symmetric. For more info please refer to https://github.com/BFO-ontology/BFO-2020/tree/master/src/owl/temporal%20extensions."@en ;
                cco:ont00001760 <https://www.commoncoreontologies.org/ModalRelationOntology> .


###  https://www.commoncoreontologies.org/mro/ont00001805
mro:ont00001805 rdf:type owl:ObjectProperty ;
                rdfs:subPropertyOf mro:mro00000001 ;
                owl:inverseOf mro:ont00001888 ;
                rdfs:domain obo:BFO_0000015 ;
                rdfs:range obo:BFO_0000015 ;
                <http://purl.org/dc/terms/created> "2022-12-30T21:32:27-05:00"^^xsd:dateTime ;
                <http://purl.org/dc/terms/creator> "https://cubrc.org"^^xsd:anyURI ;
                rdfs:label "is disrupted by"@en ;
                <http://www.w3.org/2004/02/skos/core#definition> "Inverse of disrupts." ;
                <http://www.w3.org/2004/02/skos/core#prefLabel> "is disrupted by"@en ;
                cco:ont00001760 <https://www.commoncoreontologies.org/ModalRelationOntology> .


###  https://www.commoncoreontologies.org/mro/ont00001806
mro:ont00001806 rdf:type owl:ObjectProperty ;
                rdfs:subPropertyOf mro:ont00001865 ;
                owl:inverseOf mro:ont00001806 ;
                rdf:type owl:SymmetricProperty ;
                rdfs:label "is first cousin of"@en ;
                cco:ont00001760 <https://www.commoncoreontologies.org/ModalRelationOntology> .


###  https://www.commoncoreontologies.org/mro/ont00001807
mro:ont00001807 rdf:type owl:ObjectProperty ;
                rdfs:subPropertyOf mro:ont00001920 ;
                owl:inverseOf mro:ont00001974 ;
                rdfs:domain obo:BFO_0000015 ;
                rdfs:range cco:ont00001324 ;
                rdfs:label "is required by"@en ;
                <http://www.w3.org/2004/02/skos/core#definition> "y is_required_by x at t iff: x is an instance of Process Regulation at time t, and y is an instance of Process at time t, and x prescribes that y must occur."@en ;
                <http://www.w3.org/2004/02/skos/core#scopeNote> "Given a stronger temporal interpretation, this property may be asymmetric and irreflexive. For more info please refer to https://github.com/BFO-ontology/BFO-2020/tree/master/src/owl/temporal%20extensions."@en ;
                cco:ont00001760 <https://www.commoncoreontologies.org/ModalRelationOntology> .


###  https://www.commoncoreontologies.org/mro/ont00001808
mro:ont00001808 rdf:type owl:ObjectProperty ;
                rdfs:subPropertyOf mro:mro00000001 ;
                rdfs:domain cco:ont00000958 ;
                rdfs:range obo:BFO_0000001 ;
                rdfs:label "is about"@en ;
                <http://www.w3.org/2004/02/skos/core#definition> "A primitive relationship between an Information Content Entity and some Entity."@en ;
                cco:ont00001754 "http://purl.obolibrary.org/obo/IAO_0000136" ;
                cco:ont00001760 <https://www.commoncoreontologies.org/ModalRelationOntology> .


###  https://www.commoncoreontologies.org/mro/ont00001809
mro:ont00001809 rdf:type owl:ObjectProperty ;
                rdfs:subPropertyOf mro:mro00000001 ;
                owl:inverseOf mro:ont00001836 ;
                rdfs:domain [ rdf:type owl:Class ;
                              owl:unionOf ( obo:BFO_0000020
                                            obo:BFO_0000031
                                          )
                            ] ;
                rdfs:range obo:BFO_0000027 ;
                rdfs:label "inheres in aggregate"@en ;
                <http://www.w3.org/2004/02/skos/core#definition> "x inheres_in_aggregate y iff x is an instance of Specifically Dependent Continuant and y is an instance of Object Aggregate and z is an instance of Object, such that z bearer_of x, and all other members of y are bearers of a unique instance of the same type as x."@en ;
                cco:ont00001760 <https://www.commoncoreontologies.org/ModalRelationOntology> .


###  https://www.commoncoreontologies.org/mro/ont00001810
mro:ont00001810 rdf:type owl:ObjectProperty ;
                rdfs:subPropertyOf mro:mro00000001 ;
                rdfs:domain obo:BFO_0000141 ;
                rdfs:range obo:BFO_0000141 ;
                rdfs:label "connected with"@en ;
                <http://www.w3.org/2004/02/skos/core#definition> "An immaterial entity im1 is connected with some immaterial entity im2 iff there exists some immaterial entity im3 that is common to both im1 and im2."@en ;
                <http://www.w3.org/2004/02/skos/core#scopeNote> "Given a stronger temporal interpretation, this property may be symmetric. For more info please refer to https://github.com/BFO-ontology/BFO-2020/tree/master/src/owl/temporal%20extensions."@en ;
                cco:ont00001760 <https://www.commoncoreontologies.org/ModalRelationOntology> .


###  https://www.commoncoreontologies.org/mro/ont00001811
mro:ont00001811 rdf:type owl:ObjectProperty ;
                rdfs:subPropertyOf mro:ont00001966 ;
                owl:inverseOf mro:ont00001963 ;
                rdfs:domain cco:ont00001010 ;
                rdfs:label "is a ordinal measurement of"@en ;
                <http://www.w3.org/2004/02/skos/core#definition> "x is_a_ordinal_measurement_of y iff x is an instance of Information Content Entity and y is an instance of Entity, such that x describes some attribute of y relative to a scale ordered by rank."@en ;
                cco:ont00001760 <https://www.commoncoreontologies.org/ModalRelationOntology> .


###  https://www.commoncoreontologies.org/mro/ont00001812
mro:ont00001812 rdf:type owl:ObjectProperty ;
                rdfs:subPropertyOf mro:ont00001945 ;
                owl:inverseOf mro:ont00001981 ;
                rdfs:label "is grandson of"@en ;
                cco:ont00001760 <https://www.commoncoreontologies.org/ModalRelationOntology> .


###  https://www.commoncoreontologies.org/mro/ont00001813
mro:ont00001813 rdf:type owl:ObjectProperty ;
                rdfs:subPropertyOf mro:mro00000001 ;
                owl:inverseOf mro:ont00001925 ;
                rdfs:label "uses"@en ;
                <http://www.w3.org/2004/02/skos/core#definition> "x uses y iff x is an instance of an Agent and y is an instance of a Material Entity, such that both x and y participate in some instance of a Process wherein x attempts to accomplish a goal by manipulating, deploying, or leveraging some attribute of y."@en ;
                cco:ont00001760 <https://www.commoncoreontologies.org/ModalRelationOntology> .


###  https://www.commoncoreontologies.org/mro/ont00001814
mro:ont00001814 rdf:type owl:ObjectProperty ;
                rdfs:subPropertyOf mro:ont00001971 ;
                owl:inverseOf mro:ont00001821 ;
                rdfs:domain obo:BFO_0000038 ;
                rdfs:range obo:BFO_0000038 ;
                rdfs:label "interval finishes"@en ;
                <http://www.w3.org/2004/02/skos/core#definition> "A Temporal Interval INT1 finishes some Temporal Interval INT2 iff there exists Temporal Instants inst1, inst2, and inst3 such that inst 1 is the starting instant of INT1, inst2 is the ending instant of both INT1 and INT2, inst3 is the starting instant of INT2, and inst3 is before inst1."@en ;
                cco:ont00001754 "J. F. Allen and J. A. G. M. Koomen. Planning using a temporal world model. In Proceedings of the 8th International Joint Conference on Artificial Intelligence (IJCAI-1983)  pages 741–747. Available at: https://www.ijcai.org/Proceedings/83-2/Papers/036.pdf"@en ;
                cco:ont00001760 <https://www.commoncoreontologies.org/ModalRelationOntology> .


###  https://www.commoncoreontologies.org/mro/ont00001815
mro:ont00001815 rdf:type owl:ObjectProperty ;
                rdfs:subPropertyOf mro:ont00001939 ;
                rdfs:domain cco:ont00001180 ;
                rdfs:range cco:ont00001180 ;
                rdfs:label "is subsidiary of"@en ;
                <http://www.w3.org/2004/02/skos/core#definition> "An Organization o2 is_subsidiary_of Organization o1 iff o1 controls o2 by having the capacity to determine the outcome of decisions about o2's financial and operating policies. "@en ;
                cco:ont00001754 "http://www.austlii.edu.au/legis/cth/consol_act/ca2001172/s50aa.html)" ;
                cco:ont00001760 <https://www.commoncoreontologies.org/ModalRelationOntology> .


###  https://www.commoncoreontologies.org/mro/ont00001816
mro:ont00001816 rdf:type owl:ObjectProperty ;
                rdfs:subPropertyOf mro:BFO_0000056 ;
                owl:inverseOf mro:ont00001986 ;
                rdfs:domain obo:BFO_0000002 ;
                rdfs:range obo:BFO_0000015 ;
                rdfs:label "is output of"@en ;
                <http://www.w3.org/2004/02/skos/core#definition> "x is_output_of y iff x is an instance of Continuant and y is an instance of Process, such that the presence of x at the end of y is a necessary condition for the completion of y."@en ;
                cco:ont00001760 <https://www.commoncoreontologies.org/ModalRelationOntology> .


###  https://www.commoncoreontologies.org/mro/ont00001817
mro:ont00001817 rdf:type owl:ObjectProperty ;
                rdfs:subPropertyOf mro:ont00001920 ;
                rdfs:domain obo:BFO_0000015 ;
                rdfs:range cco:ont00001324 ;
                rdfs:label "is prohibited by"@en ;
                <http://www.w3.org/2004/02/skos/core#definition> "y is_prohibited_by y at t iff: x is an instance of Process Regulation at time t, and y is an instance of Process at time t, and x prescribes that y must not occur."@en ;
                <http://www.w3.org/2004/02/skos/core#scopeNote> "Given a stronger temporal interpretation, this property may be asymmetric and irreflexive. For more info please refer to https://github.com/BFO-ontology/BFO-2020/tree/master/src/owl/temporal%20extensions."@en ;
                cco:ont00001760 <https://www.commoncoreontologies.org/ModalRelationOntology> .


###  https://www.commoncoreontologies.org/mro/ont00001818
mro:ont00001818 rdf:type owl:ObjectProperty ;
                rdfs:subPropertyOf mro:ont00001865 ;
                owl:inverseOf mro:ont00001818 ;
                rdfs:label "is in-law of"@en ;
                <http://www.w3.org/2004/02/skos/core#scopeNote> "Given a stronger temporal interpretation, this property may be symmetric. For more info please refer to https://github.com/BFO-ontology/BFO-2020/tree/master/src/owl/temporal%20extensions."@en ;
                cco:ont00001760 <https://www.commoncoreontologies.org/ModalRelationOntology> .


###  https://www.commoncoreontologies.org/mro/ont00001819
mro:ont00001819 rdf:type owl:ObjectProperty ;
                rdfs:subPropertyOf mro:mro00000001 ;
                rdfs:domain obo:BFO_0000003 ;
                rdfs:range obo:BFO_0000003 ;
                rdfs:label "caused by"@en ;
                <http://www.w3.org/2004/02/skos/core#definition> "x caused_by y iff x and y are instances of Occurrent, and x is a consequence of y."@en ;
                cco:ont00001760 <https://www.commoncoreontologies.org/ModalRelationOntology> .


###  https://www.commoncoreontologies.org/mro/ont00001820
mro:ont00001820 rdf:type owl:ObjectProperty ;
                rdfs:subPropertyOf mro:ont00001850 ;
                rdfs:label "has granddaughter"@en ;
                cco:ont00001760 <https://www.commoncoreontologies.org/ModalRelationOntology> .


###  https://www.commoncoreontologies.org/mro/ont00001821
mro:ont00001821 rdf:type owl:ObjectProperty ;
                rdfs:subPropertyOf mro:ont00001924 ;
                rdfs:domain obo:BFO_0000038 ;
                rdfs:range obo:BFO_0000038 ;
                rdfs:label "interval finished by"@en ;
                <http://www.w3.org/2004/02/skos/core#definition> "A Temporal Interval INT2 is finished by some Temporal Interval INT1 iff there exists Temporal Instants inst1, inst2, and inst3 such that inst 1 is the starting instant of INT1, inst2 is the ending instant of both INT1 and INT2, inst3 is the starting instant of INT2, and inst3 is before inst1."@en ;
                cco:ont00001754 "J. F. Allen and J. A. G. M. Koomen. Planning using a temporal world model. In Proceedings of the 8th International Joint Conference on Artificial Intelligence (IJCAI-1983)  pages 741–747. Available at: https://www.ijcai.org/Proceedings/83-2/Papers/036.pdf"@en ;
                cco:ont00001760 <https://www.commoncoreontologies.org/ModalRelationOntology> .


###  https://www.commoncoreontologies.org/mro/ont00001822
mro:ont00001822 rdf:type owl:ObjectProperty ;
                rdfs:subPropertyOf mro:mro00000001 ;
                rdf:type owl:SymmetricProperty ;
                rdfs:domain obo:BFO_0000038 ;
                rdfs:range obo:BFO_0000038 ;
                owl:propertyDisjointWith mro:ont00001862 ;
                rdfs:label "interval equals"@en ;
                <http://www.w3.org/2004/02/skos/core#definition> "A Temporal Interval INT1 is equal to some Temporal Interval INT2 iff there exists Temporal Instants inst1 and inst2 such that inst1 is the starting instant of both INT1 and INT2 and inst2 is the ending instant of both INT1 and INT2."@en ;
                cco:ont00001754 "J. F. Allen and J. A. G. M. Koomen. Planning using a temporal world model. In Proceedings of the 8th International Joint Conference on Artificial Intelligence (IJCAI-1983)  pages 741–747. Available at: https://www.ijcai.org/Proceedings/83-2/Papers/036.pdf"@en ;
                cco:ont00001760 <https://www.commoncoreontologies.org/ModalRelationOntology> .


###  https://www.commoncoreontologies.org/mro/ont00001823
mro:ont00001823 rdf:type owl:ObjectProperty ;
                rdfs:subPropertyOf mro:ont00001785 ;
                owl:inverseOf mro:ont00001926 ;
                rdfs:label "has paternal uncle"@en ;
                cco:ont00001760 <https://www.commoncoreontologies.org/ModalRelationOntology> .


###  https://www.commoncoreontologies.org/mro/ont00001824
mro:ont00001824 rdf:type owl:ObjectProperty ;
                rdfs:subPropertyOf mro:mro00000001 ;
                rdfs:domain cco:ont00000253 ;
                rdfs:range cco:ont00000253 ;
                rdfs:label "is excerpted from"@en ;
                <http://www.w3.org/2004/02/skos/core#definition> "An Information Bearing Entity b1 is excerpted from another Information Bearing Entity B2 iff b1 is part of some Information Bearing Entity B1 that is carrier of some Information Content Entity C1, B2 is carrier of some Information Content Entity C2, C1 is not identical with C2, b1 is carrier of some Information Content Entity c1, b2 is an Information Bearing Entity that is part of B2 and b2 is carrier of c1 (i.e. the same Information Content Entity as borne by b1)."@en ;
                cco:ont00001760 <https://www.commoncoreontologies.org/ModalRelationOntology> .


###  https://www.commoncoreontologies.org/mro/ont00001825
mro:ont00001825 rdf:type owl:ObjectProperty ;
                rdfs:subPropertyOf mro:mro00000001 ;
                owl:inverseOf mro:ont00001870 ;
                rdfs:domain obo:BFO_0000038 ;
                rdfs:range obo:BFO_0000038 ;
                owl:propertyDisjointWith mro:ont00001862 ;
                rdfs:label "interval overlaps"@en ;
                <http://www.w3.org/2004/02/skos/core#definition> "A Temporal Interval INT1 overlaps some Temporal Interval INT2 iff there exist Temporal Instants inst1, inst2, inst3, inst4 such that inst1 is the starting instant of INT1, inst2 is the ending instant of INT1, inst3 is the starting instant of INT2, inst4 is the ending instant of INT2, inst1 is before inst3, inst3 is before inst2, and inst2 is before inst4."@en ;
                cco:ont00001754 "J. F. Allen and J. A. G. M. Koomen. Planning using a temporal world model. In Proceedings of the 8th International Joint Conference on Artificial Intelligence (IJCAI-1983)  pages 741–747. Available at: https://www.ijcai.org/Proceedings/83-2/Papers/036.pdf"@en ;
                cco:ont00001760 <https://www.commoncoreontologies.org/ModalRelationOntology> .


###  https://www.commoncoreontologies.org/mro/ont00001826
mro:ont00001826 rdf:type owl:ObjectProperty ;
                rdfs:subPropertyOf mro:ont00001818 ;
                owl:inverseOf mro:ont00001828 ;
                rdfs:label "is sister-in-law of"@en ;
                cco:ont00001760 <https://www.commoncoreontologies.org/ModalRelationOntology> .


###  https://www.commoncoreontologies.org/mro/ont00001827
mro:ont00001827 rdf:type owl:ObjectProperty ;
                rdfs:subPropertyOf mro:ont00001944 ;
                owl:inverseOf mro:ont00001989 ;
                rdfs:domain obo:BFO_0000141 ;
                rdfs:range obo:BFO_0000141 ;
                rdfs:label "nontangential part of"@en ;
                <http://www.w3.org/2004/02/skos/core#definition> "An immaterial entity im1 is a nontangential part of some immaterial entity im2 iff im1 is a spatial part of im2 and there does not exist an immaterial entity im3 such that im3 externally connects with im1 and im3 externally connects with im2."@en ;
                <http://www.w3.org/2004/02/skos/core#scopeNote> "Given a stronger temporal interpretation, this property may be transitive. For more info please refer to https://github.com/BFO-ontology/BFO-2020/tree/master/src/owl/temporal%20extensions."@en ;
                cco:ont00001754 "Randell, D. A., Cui, Z. and Cohn, A. G.: 1992, \"A spatial logic based on regions and connection,\" Proc. 3rd Int. Conf. on Knowledge Representation and Reasoning, Morgan Kaufmann, San Mateo, pp. 165-176. Available at: https://www.dpi.inpe.br/gilberto/references/cohn_rcc.pdf"@en ;
                cco:ont00001760 <https://www.commoncoreontologies.org/ModalRelationOntology> .


###  https://www.commoncoreontologies.org/mro/ont00001828
mro:ont00001828 rdf:type owl:ObjectProperty ;
                rdfs:subPropertyOf mro:ont00001818 ;
                rdfs:label "has sister in law"@en ;
                cco:ont00001760 <https://www.commoncoreontologies.org/ModalRelationOntology> .


###  https://www.commoncoreontologies.org/mro/ont00001829
mro:ont00001829 rdf:type owl:ObjectProperty ;
                rdfs:subPropertyOf mro:ont00001809 ;
                owl:inverseOf mro:ont00001956 ;
                rdfs:domain obo:BFO_0000016 ;
                rdfs:range obo:BFO_0000027 ;
                rdfs:label "disposition of aggregate"@en ;
                <http://www.w3.org/2004/02/skos/core#definition> "x disposition_of_aggregate y iff y is an instance of Object Aggregate and x is an instance of Disposition, and x inheres_in_aggregate y."@en ;
                cco:ont00001760 <https://www.commoncoreontologies.org/ModalRelationOntology> .


###  https://www.commoncoreontologies.org/mro/ont00001830
mro:ont00001830 rdf:type owl:ObjectProperty ;
                rdfs:subPropertyOf mro:BFO_0000057 ;
                owl:inverseOf mro:ont00001895 ;
                rdfs:domain obo:BFO_0000015 ;
                rdfs:range obo:BFO_0000040 ;
                rdfs:label "has accomplice"@en ;
                <http://www.w3.org/2004/02/skos/core#definition> "A Processual Entity p1 has_accomplice some agent a1 iff a1 assists in the commission of p1, is located at the location of p1, but is not agent_in p1."@en ;
                cco:ont00001754 "https://en.wikipedia.org/w/index.php?title=Accomplice&oldid=1002047204"^^xsd:anyURI ;
                cco:ont00001760 <https://www.commoncoreontologies.org/ModalRelationOntology> .


###  https://www.commoncoreontologies.org/mro/ont00001831
mro:ont00001831 rdf:type owl:ObjectProperty ;
                rdfs:subPropertyOf mro:mro00000001 ;
                owl:inverseOf mro:ont00001951 ;
                rdfs:domain obo:BFO_0000023 ;
                rdfs:range obo:BFO_0000023 ;
                rdfs:label "is subordinate role to"@en ;
                <http://www.w3.org/2004/02/skos/core#definition> "For all x,y,t: y is subordinate role to x at t iff: x is an instance of Role at time t, and y is an instance of Role at time t, and there is some z such that x is realized by z and z is an instance of Process which creates, modifies, transfers, or eliminates some u such that u is a Process Regulation at time t, and u is addressed to the bearer of y."@en ;
                cco:ont00001760 <https://www.commoncoreontologies.org/ModalRelationOntology> .


###  https://www.commoncoreontologies.org/mro/ont00001832
mro:ont00001832 rdf:type owl:ObjectProperty ;
                rdfs:subPropertyOf mro:mro00000001 ;
                rdfs:domain obo:BFO_0000027 ;
                rdfs:range [ owl:intersectionOf ( obo:BFO_0000004
                                                  [ rdf:type owl:Class ;
                                                    owl:complementOf obo:BFO_0000006
                                                  ]
                                                ) ;
                             rdf:type owl:Class
                           ] ;
                rdfs:label "has some member located in"@en ;
                <http://www.w3.org/2004/02/skos/core#definition> "x has some member located in y iff x is an instance of Object Aggregate and y is an instance of independent continuant but not a spatial region, and at least one member of x is located in y."@en ;
                cco:ont00001760 <https://www.commoncoreontologies.org/ModalRelationOntology> .


###  https://www.commoncoreontologies.org/mro/ont00001833
mro:ont00001833 rdf:type owl:ObjectProperty ;
                rdfs:subPropertyOf mro:BFO_0000057 ;
                rdfs:label "has agent"@en ;
                <http://www.w3.org/2004/02/skos/core#definition> "x has_agent y iff x is an instance of Process and y is an instance of Agent, such that y is causally active in x."@en ;
                cco:ont00001760 <https://www.commoncoreontologies.org/ModalRelationOntology> .


###  https://www.commoncoreontologies.org/mro/ont00001834
mro:ont00001834 rdf:type owl:ObjectProperty ;
                rdfs:subPropertyOf mro:BFO_0000057 ;
                owl:inverseOf mro:ont00001886 ;
                rdfs:domain obo:BFO_0000015 ;
                rdfs:range obo:BFO_0000002 ;
                rdfs:label "affects"@en ;
                <http://www.w3.org/2004/02/skos/core#definition> "x affects y iff x is an instance of Process and y is an instance of Continuant, and x influences y in some manner, most often by producing a change in y."@en ;
                cco:ont00001760 <https://www.commoncoreontologies.org/ModalRelationOntology> .


###  https://www.commoncoreontologies.org/mro/ont00001835
mro:ont00001835 rdf:type owl:ObjectProperty ;
                rdfs:subPropertyOf mro:ont00001842 ;
                owl:inverseOf mro:ont00001839 ;
                rdfs:label "is son of"@en ;
                cco:ont00001760 <https://www.commoncoreontologies.org/ModalRelationOntology> .


###  https://www.commoncoreontologies.org/mro/ont00001836
mro:ont00001836 rdf:type owl:ObjectProperty ;
                rdfs:subPropertyOf mro:mro00000001 ;
                rdfs:domain obo:BFO_0000027 ;
                rdfs:range [ rdf:type owl:Class ;
                             owl:unionOf ( obo:BFO_0000020
                                           obo:BFO_0000031
                                         )
                           ] ;
                rdfs:label "aggregate bearer of"@en ;
                <http://www.w3.org/2004/02/skos/core#definition> "x aggregate_bearer_of y iff x is an instance of Object Aggregate and y is an instance of Specifically Dependent Continuant and z is an instance of Object, such that z bearer of y, and all other members of x are bearers of a unique instance of the same type as y."@en ;
                cco:ont00001760 <https://www.commoncoreontologies.org/ModalRelationOntology> .


###  https://www.commoncoreontologies.org/mro/ont00001837
mro:ont00001837 rdf:type owl:ObjectProperty ;
                rdfs:subPropertyOf mro:BFO_0000084 ;
                owl:inverseOf mro:ont00001908 ;
                rdfs:domain cco:ont00000829 ;
                rdfs:range cco:ont00000253 ;
                rdfs:label "time zone identifier used by"@en ;
                <http://www.w3.org/2004/02/skos/core#definition> "x time_zone_identifier_used_by y iff y is an instance of Information Bearing Entity and x is an instance of Time Zone Identifier, such that x designates the spatial region associated with the time zone mentioned in y."@en ;
                cco:ont00001760 <https://www.commoncoreontologies.org/ModalRelationOntology> .


###  https://www.commoncoreontologies.org/mro/ont00001838
mro:ont00001838 rdf:type owl:ObjectProperty ;
                rdfs:subPropertyOf mro:mro00000001 ;
                rdfs:domain obo:BFO_0000141 ;
                rdfs:range obo:BFO_0000141 ;
                rdfs:label "disconnected with"@en ;
                <http://www.w3.org/2004/02/skos/core#definition> "An immaterial entity im1 is disconnected with some immaterial entity im2 iff there does not exist some immaterial entity im3 that is common to both im1 and im2."@en ;
                <http://www.w3.org/2004/02/skos/core#scopeNote> "Given a stronger temporal interpretation, this property may be symmetric. For more info please refer to https://github.com/BFO-ontology/BFO-2020/tree/master/src/owl/temporal%20extensions."@en ;
                cco:ont00001760 <https://www.commoncoreontologies.org/ModalRelationOntology> .


###  https://www.commoncoreontologies.org/mro/ont00001839
mro:ont00001839 rdf:type owl:ObjectProperty ;
                rdfs:subPropertyOf mro:ont00001995 ;
                rdfs:label "has son"@en ;
                cco:ont00001760 <https://www.commoncoreontologies.org/ModalRelationOntology> .


###  https://www.commoncoreontologies.org/mro/ont00001840
mro:ont00001840 rdf:type owl:ObjectProperty ;
                rdfs:subPropertyOf mro:ont00001945 ;
                owl:inverseOf mro:ont00001882 ;
                rdfs:label "has grandmother"@en ;
                cco:ont00001760 <https://www.commoncoreontologies.org/ModalRelationOntology> .


###  https://www.commoncoreontologies.org/mro/ont00001841
mro:ont00001841 rdf:type owl:ObjectProperty ;
                rdfs:subPropertyOf mro:BFO_0000056 ;
                owl:inverseOf mro:ont00001921 ;
                rdfs:domain obo:BFO_0000002 ;
                rdfs:range obo:BFO_0000015 ;
                rdfs:label "is input of"@en ;
                <http://www.w3.org/2004/02/skos/core#definition> "x is_input_of y iff x is an instance of Continuant and y is an instance of Process, such that the presence of x at the beginning of y is a necessary condition for the start of y."@en ;
                cco:ont00001760 <https://www.commoncoreontologies.org/ModalRelationOntology> .


###  https://www.commoncoreontologies.org/mro/ont00001842
mro:ont00001842 rdf:type owl:ObjectProperty ;
                rdfs:subPropertyOf mro:ont00001865 ;
                owl:inverseOf mro:ont00001995 ;
                rdfs:label "is child of"@en ;
                cco:ont00001760 <https://www.commoncoreontologies.org/ModalRelationOntology> .


###  https://www.commoncoreontologies.org/mro/ont00001843
mro:ont00001843 rdf:type owl:ObjectProperty ;
                rdfs:subPropertyOf mro:ont00001806 ;
                owl:inverseOf mro:ont00001894 ;
                rdfs:comment "Comment is_paternal_first_cousin_of is not a symmetric relationship as is is_first_cousin_of"@en ;
                rdfs:label "is paternal first cousin of"@en ;
                <http://www.w3.org/2004/02/skos/core#definition> "Person A is paternal first cousin of Person B iff Person B has father F and F has sibling P and P is parent of Person A."@en ;
                cco:ont00001760 <https://www.commoncoreontologies.org/ModalRelationOntology> .


###  https://www.commoncoreontologies.org/mro/ont00001844
mro:ont00001844 rdf:type owl:ObjectProperty ;
                rdfs:subPropertyOf mro:BFO_0000057 ;
                owl:inverseOf mro:ont00001993 ;
                rdfs:range cco:ont00001017 ;
                rdfs:label "has sender"@en ;
                <http://www.w3.org/2004/02/skos/core#definition> "y has_sender x iff x is an instance of Agent and y is an instance of Act Of Communication, such that x is the initiator and encoder of the InformationContentEntity intended for communication in y."@en ;
                cco:ont00001760 <https://www.commoncoreontologies.org/ModalRelationOntology> .


###  https://www.commoncoreontologies.org/mro/ont00001845
mro:ont00001845 rdf:type owl:ObjectProperty ;
                rdfs:subPropertyOf mro:BFO_0000183 ;
                owl:inverseOf mro:ont00001918 ;
                rdfs:domain obo:BFO_0000029 ;
                rdfs:range obo:BFO_0000015 ;
                rdfs:label "is site of"@en ;
                <http://www.w3.org/2004/02/skos/core#definition> "x is_site_of y iff x is an instance of Site and y is an instance of Process, such that y occurs in x."@en ;
                cco:ont00001760 <https://www.commoncoreontologies.org/ModalRelationOntology> .


###  https://www.commoncoreontologies.org/mro/ont00001846
mro:ont00001846 rdf:type owl:ObjectProperty ;
                rdfs:subPropertyOf mro:mro00000001 ;
                owl:inverseOf mro:ont00001992 ;
                rdfs:domain cco:ont00001180 ;
                rdfs:range obo:BFO_0000023 ;
                rdfs:label "is organizational context of"@en ;
                <http://www.w3.org/2004/02/skos/core#definition> "x is_organizational_context_of y iff x is an instance of an Organization and y is an instance of a Role and z is an instance of a Person, such that z's affiliation with x is a prerequisite for z bearing y, or x ascribes y to the bearer of y."@en ;
                cco:ont00001760 <https://www.commoncoreontologies.org/ModalRelationOntology> .


###  https://www.commoncoreontologies.org/mro/ont00001847
mro:ont00001847 rdf:type owl:ObjectProperty ;
                rdfs:subPropertyOf mro:ont00001862 ;
                owl:inverseOf mro:ont00001940 ;
                rdfs:domain obo:BFO_0000038 ;
                rdfs:range obo:BFO_0000038 ;
                rdfs:label "interval is after"@en ;
                <http://www.w3.org/2004/02/skos/core#definition> "A TemporalInterval INT2 is after some TemporalInterval INT1 iff there exists TemporalInstants inst2, inst1 such that inst2 is the starting instant of INT2 and inst1 is the ending instant of INT1 and inst2 is after inst1."@en ;
                cco:ont00001754 "J. F. Allen and J. A. G. M. Koomen. Planning using a temporal world model. In Proceedings of the 8th International Joint Conference on Artificial Intelligence (IJCAI-1983)  pages 741–747. Available at: https://www.ijcai.org/Proceedings/83-2/Papers/036.pdf"@en ;
                cco:ont00001760 <https://www.commoncoreontologies.org/ModalRelationOntology> .


###  https://www.commoncoreontologies.org/mro/ont00001848
mro:ont00001848 rdf:type owl:ObjectProperty ;
                rdfs:subPropertyOf mro:mro00000001 ;
                rdfs:domain obo:BFO_0000148 ;
                rdfs:range obo:BFO_0000038 ;
                rdfs:label "is inside instant of"@en ;
                <http://www.w3.org/2004/02/skos/core#definition> "For Temporal Instant t1 and Temporal Interval t2, t1 is inside instant of t2 if and only if there are Temporal Instants t3 and t4 non-identical to t1 and part of t2 such that t3 is before t1 and t4 is after t1."@en ;
                cco:ont00001754 "J. F. Allen and J. A. G. M. Koomen. Planning using a temporal world model. In Proceedings of the 8th International Joint Conference on Artificial Intelligence (IJCAI-1983)  pages 741–747. Available at: https://www.ijcai.org/Proceedings/83-2/Papers/036.pdf"@en ;
                cco:ont00001760 <https://www.commoncoreontologies.org/ModalRelationOntology> .


###  https://www.commoncoreontologies.org/mro/ont00001849
mro:ont00001849 rdf:type owl:ObjectProperty ;
                rdfs:subPropertyOf mro:ont00001818 ;
                owl:inverseOf mro:ont00001935 ;
                rdfs:label "is father in-law of"@en ;
                cco:ont00001760 <https://www.commoncoreontologies.org/ModalRelationOntology> .


###  https://www.commoncoreontologies.org/mro/ont00001850
mro:ont00001850 rdf:type owl:ObjectProperty ;
                rdfs:subPropertyOf mro:ont00001865 ;
                owl:inverseOf mro:ont00001945 ;
                rdfs:label "is grandparent of"@en ;
                cco:ont00001760 <https://www.commoncoreontologies.org/ModalRelationOntology> .


###  https://www.commoncoreontologies.org/mro/ont00001851
mro:ont00001851 rdf:type owl:ObjectProperty ;
                rdfs:subPropertyOf mro:ont00001902 ;
                rdfs:label "is sister of"@en ;
                cco:ont00001760 <https://www.commoncoreontologies.org/ModalRelationOntology> .


###  https://www.commoncoreontologies.org/mro/ont00001852
mro:ont00001852 rdf:type owl:ObjectProperty ;
                rdfs:subPropertyOf mro:BFO_0000056 ;
                owl:inverseOf mro:ont00001949 ;
                rdfs:domain obo:BFO_0000040 ;
                rdfs:range obo:BFO_0000015 ;
                rdfs:label "accessory in"@en ;
                <http://www.w3.org/2004/02/skos/core#definition> "y is_accessory_in x iff x is an instance of Process and y is an instance of Agent, such that y assists another agent in the commission of x, and y was not located at the location of x when x occurred, and y was not an agent_in x."@en ;
                cco:ont00001754 "http://en.wikipedia.org/wiki/Accessory_(legal_term)" ;
                cco:ont00001760 <https://www.commoncoreontologies.org/ModalRelationOntology> .


###  https://www.commoncoreontologies.org/mro/ont00001853
mro:ont00001853 rdf:type owl:ObjectProperty ;
                rdfs:subPropertyOf mro:ont00001818 ;
                owl:inverseOf mro:ont00001885 ;
                rdfs:label "is mother in-law of"@en ;
                cco:ont00001760 <https://www.commoncoreontologies.org/ModalRelationOntology> .


###  https://www.commoncoreontologies.org/mro/ont00001854
mro:ont00001854 rdf:type owl:ObjectProperty ;
                rdfs:subPropertyOf mro:ont00001818 ;
                owl:inverseOf mro:ont00001867 ;
                rdfs:label "has daughter in law"@en ;
                cco:ont00001760 <https://www.commoncoreontologies.org/ModalRelationOntology> .


###  https://www.commoncoreontologies.org/mro/ont00001855
mro:ont00001855 rdf:type owl:ObjectProperty ;
                rdfs:subPropertyOf mro:BFO_0000178 ,
                                   mro:ont00001810 ;
                owl:inverseOf mro:ont00001944 ;
                rdfs:domain obo:BFO_0000141 ;
                rdfs:range obo:BFO_0000141 ;
                rdfs:label "has spatial part"@en ;
                <http://www.w3.org/2004/02/skos/core#definition> "y has_spatial_part x iff x, y, z, and q are instances of Immaterial Entity, such that for any z connected with x, z is also connected with y, and q is connected with y but not connected with x."@en ;
                cco:ont00001754 "Randell, D. A., Cui, Z. and Cohn, A. G.: 1992, \"A spatial logic based on regions and connection,\" Proc. 3rd Int. Conf. on Knowledge Representation and Reasoning, Morgan Kaufmann, San Mateo, pp. 165-176. Available at: https://www.dpi.inpe.br/gilberto/references/cohn_rcc.pdf"@en ;
                cco:ont00001760 <https://www.commoncoreontologies.org/ModalRelationOntology> .


###  https://www.commoncoreontologies.org/mro/ont00001856
mro:ont00001856 rdf:type owl:ObjectProperty ;
                rdfs:subPropertyOf mro:ont00001865 ;
                owl:inverseOf mro:ont00001932 ;
                rdfs:label "has niece"@en ;
                cco:ont00001760 <https://www.commoncoreontologies.org/ModalRelationOntology> .


###  https://www.commoncoreontologies.org/mro/ont00001857
mro:ont00001857 rdf:type owl:ObjectProperty ;
                rdfs:subPropertyOf mro:BFO_0000132 ;
                rdfs:domain obo:BFO_0000015 ;
                rdfs:range obo:BFO_0000015 ;
                rdfs:label "is part of process"@en ;
                <http://www.w3.org/2004/02/skos/core#definition> "x is_part_of_process y iff x and y are instances of Process, such that x occurs during the temporal interval of y, and x either provides an input to y or receives an output of y."@en ;
                cco:ont00001760 <https://www.commoncoreontologies.org/ModalRelationOntology> .


###  https://www.commoncoreontologies.org/mro/ont00001858
mro:ont00001858 rdf:type owl:ObjectProperty ;
                rdfs:subPropertyOf mro:ont00001842 ;
                owl:inverseOf mro:ont00001987 ;
                rdfs:label "is daughter of"@en ;
                cco:ont00001760 <https://www.commoncoreontologies.org/ModalRelationOntology> .


###  https://www.commoncoreontologies.org/mro/ont00001859
mro:ont00001859 rdf:type owl:ObjectProperty ;
                rdfs:subPropertyOf mro:mro00000001 ;
                owl:inverseOf mro:ont00001864 ;
                rdfs:domain cco:ont00001180 ;
                rdfs:range cco:ont00001203 ;
                rdfs:label "is delimited by"@en ;
                <http://www.w3.org/2004/02/skos/core#definition> "An instance of Organization o1 is_delimited_by some Delimiting Domain dd1 iff dd1 is the area within which o1 can legally operate."@en ;
                cco:ont00001754 "https://en.wikipedia.org/w/index.php?title=Boundary_delimitation&oldid=1039137603"^^xsd:anyURI ;
                cco:ont00001760 <https://www.commoncoreontologies.org/ModalRelationOntology> .


###  https://www.commoncoreontologies.org/mro/ont00001860
mro:ont00001860 rdf:type owl:ObjectProperty ;
                rdfs:subPropertyOf mro:ont00001865 ;
                owl:inverseOf mro:ont00001968 ;
                rdfs:label "is ancestor of"@en ;
                cco:ont00001760 <https://www.commoncoreontologies.org/ModalRelationOntology> .


###  https://www.commoncoreontologies.org/mro/ont00001861
mro:ont00001861 rdf:type owl:ObjectProperty ;
                rdfs:subPropertyOf mro:mro00000001 ;
                owl:inverseOf mro:ont00001991 ;
                rdfs:domain obo:BFO_0000030 ;
                rdfs:range obo:BFO_0000030 ;
                rdfs:label "is material of"@en ;
                <http://www.w3.org/2004/02/skos/core#definition> "An object m is material of an object o when m is the material of which o consists and that material does not undergo a change of kind during the creation of o"@en ;
                cco:ont00001760 <https://www.commoncoreontologies.org/ModalRelationOntology> .


###  https://www.commoncoreontologies.org/mro/ont00001862
mro:ont00001862 rdf:type owl:ObjectProperty ;
                rdfs:subPropertyOf mro:mro00000001 ;
                rdfs:domain obo:BFO_0000038 ;
                rdfs:range obo:BFO_0000038 ;
                owl:propertyDisjointWith mro:ont00001870 ,
                                         mro:ont00001924 ,
                                         mro:ont00001971 ;
                rdfs:label "interval disjoint"@en ;
                <http://www.w3.org/2004/02/skos/core#definition> "A Temporal Interval INT1 is disjoint with a Temporal Interval INT2 iff INT1 is before or meets INT2 OR INT2 is before or meets INT1. In other words, INT1 and INT2 are disjoint iff INT1 and INT2 do not overlap, contain, or equal one another."@en ;
                cco:ont00001754 "J. F. Allen and J. A. G. M. Koomen. Planning using a temporal world model. In Proceedings of the 8th International Joint Conference on Artificial Intelligence (IJCAI-1983)  pages 741–747. Available at: https://www.ijcai.org/Proceedings/83-2/Papers/036.pdf"@en ;
                cco:ont00001760 <https://www.commoncoreontologies.org/ModalRelationOntology> .


###  https://www.commoncoreontologies.org/mro/ont00001863
mro:ont00001863 rdf:type owl:ObjectProperty ;
                rdfs:subPropertyOf mro:BFO_0000101 ;
                owl:inverseOf mro:ont00001961 ;
                rdfs:domain cco:ont00000253 ;
                rdfs:range cco:ont00000120 ;
                rdfs:label "uses measurement unit"@en ;
                <http://www.w3.org/2004/02/skos/core#definition> "y uses_measurement_unit x iff y is an instance of Information Bearing Entity and x is an instance of Measurement Unit, such that x describes the magnitude of measured physical quantity mentioned in y."@en ;
                cco:ont00001760 <https://www.commoncoreontologies.org/ModalRelationOntology> .


###  https://www.commoncoreontologies.org/mro/ont00001864
mro:ont00001864 rdf:type owl:ObjectProperty ;
                rdfs:subPropertyOf mro:mro00000001 ;
                rdfs:domain cco:ont00001203 ;
                rdfs:range cco:ont00001180 ;
                rdfs:label "delimits"@en ;
                <http://www.w3.org/2004/02/skos/core#definition> "An instance of Delimiting Domain dd1 delimits some Organization o1 iff dd1 is the area within which o1 can legally operate."@en ;
                cco:ont00001754 "https://en.wikipedia.org/w/index.php?title=Boundary_delimitation&oldid=1039137603"^^xsd:anyURI ;
                cco:ont00001760 <https://www.commoncoreontologies.org/ModalRelationOntology> .


###  https://www.commoncoreontologies.org/mro/ont00001865
mro:ont00001865 rdf:type owl:ObjectProperty ;
                rdfs:subPropertyOf mro:mro00000001 ;
                rdf:type owl:SymmetricProperty ;
                rdfs:domain cco:ont00001262 ;
                rdfs:range cco:ont00001262 ;
                rdfs:label "has familial relationship to"@en ;
                <http://www.w3.org/2004/02/skos/core#definition> "A relationship between persons by virtue of ancestry or legal union."@en ;
                cco:ont00001760 <https://www.commoncoreontologies.org/ModalRelationOntology> .


###  https://www.commoncoreontologies.org/mro/ont00001866
mro:ont00001866 rdf:type owl:ObjectProperty ;
                rdfs:subPropertyOf mro:mro00000001 ;
                owl:inverseOf mro:ont00001984 ;
                rdfs:domain obo:BFO_0000015 ;
                rdfs:range cco:ont00001017 ;
                <http://purl.org/dc/terms/created> "2022-12-30T21:32:27-05:00"^^xsd:dateTime ;
                <http://purl.org/dc/terms/creator> "https://cubrc.org"^^xsd:anyURI ;
                rdfs:label "is interest of"@en ;
                <http://www.w3.org/2004/02/skos/core#definition> "The inverse of has_interest_in. " ;
                <http://www.w3.org/2004/02/skos/core#prefLabel> "is interest of"@en ;
                cco:ont00001760 <https://www.commoncoreontologies.org/ModalRelationOntology> .


###  https://www.commoncoreontologies.org/mro/ont00001867
mro:ont00001867 rdf:type owl:ObjectProperty ;
                rdfs:subPropertyOf mro:ont00001818 ;
                rdfs:label "is daughter in-law of"@en ;
                cco:ont00001760 <https://www.commoncoreontologies.org/ModalRelationOntology> .


###  https://www.commoncoreontologies.org/mro/ont00001868
mro:ont00001868 rdf:type owl:ObjectProperty ;
                rdfs:subPropertyOf mro:ont00001966 ;
                owl:inverseOf mro:ont00001914 ;
                rdfs:domain cco:ont00000293 ;
                rdfs:label "is a nominal measurement of"@en ;
                <http://www.w3.org/2004/02/skos/core#definition> "x is_a_nominal_measurement_of y iff x is an instance of Information Content Entity and y is an instance of Entity, such that x classifies y relative to some set of shared, possibly arbitrary, characteristics."@en ;
                cco:ont00001760 <https://www.commoncoreontologies.org/ModalRelationOntology> .


###  https://www.commoncoreontologies.org/mro/ont00001869
mro:ont00001869 rdf:type owl:ObjectProperty ;
                rdfs:subPropertyOf mro:ont00001971 ;
                rdfs:domain obo:BFO_0000038 ;
                rdfs:range obo:BFO_0000038 ;
                rdfs:label "interval during"@en ;
                <http://www.w3.org/2004/02/skos/core#definition> "A Temporal Interval INT1 is during some Temporal Interval INT2 iff there exist Temporal Instants inst1, inst2, inst3, and inst4 such that inst1 is the starting instant of INT1, inst2 is the ending instant of INT1, inst3 is the starting instant of INT2, inst4 is the ending instant of INT2, inst3 is before inst1, and inst2 is before inst4."@en ;
                cco:ont00001754 "J. F. Allen and J. A. G. M. Koomen. Planning using a temporal world model. In Proceedings of the 8th International Joint Conference on Artificial Intelligence (IJCAI-1983)  pages 741–747. Available at: https://www.ijcai.org/Proceedings/83-2/Papers/036.pdf"@en ;
                cco:ont00001760 <https://www.commoncoreontologies.org/ModalRelationOntology> .


###  https://www.commoncoreontologies.org/mro/ont00001870
mro:ont00001870 rdf:type owl:ObjectProperty ;
                rdfs:subPropertyOf mro:mro00000001 ;
                rdfs:domain obo:BFO_0000038 ;
                rdfs:range obo:BFO_0000038 ;
                rdfs:label "interval overlapped by"@en ;
                <http://www.w3.org/2004/02/skos/core#definition> "A Temporal Interval INT2 is overlapped by some Temporal Interval INT1 iff there exist Temporal Instants inst1, inst2, inst3, inst4 such that inst1 is the starting instant of INT1, inst2 is the ending instant of INT1, inst3 is the starting instant of INT2, inst4 is the ending instant of INT2, inst1 is before inst3, inst3 is before inst2, and inst2 is before inst4."@en ;
                cco:ont00001754 "J. F. Allen and J. A. G. M. Koomen. Planning using a temporal world model. In Proceedings of the 8th International Joint Conference on Artificial Intelligence (IJCAI-1983)  pages 741–747. Available at: https://www.ijcai.org/Proceedings/83-2/Papers/036.pdf"@en ;
                cco:ont00001760 <https://www.commoncoreontologies.org/ModalRelationOntology> .


###  https://www.commoncoreontologies.org/mro/ont00001871
mro:ont00001871 rdf:type owl:ObjectProperty ;
                rdfs:subPropertyOf mro:ont00001804 ;
                owl:inverseOf mro:ont00001887 ;
                rdfs:label "has wife"@en ;
                cco:ont00001760 <https://www.commoncoreontologies.org/ModalRelationOntology> .


###  https://www.commoncoreontologies.org/mro/ont00001872
mro:ont00001872 rdf:type owl:ObjectProperty ;
                rdfs:subPropertyOf mro:ont00001996 ;
                owl:inverseOf mro:ont00001890 ;
                rdfs:label "is step-brother of"@en ;
                cco:ont00001760 <https://www.commoncoreontologies.org/ModalRelationOntology> .


###  https://www.commoncoreontologies.org/mro/ont00001873
mro:ont00001873 rdf:type owl:ObjectProperty ;
                rdfs:subPropertyOf mro:ont00001801 ;
                owl:inverseOf mro:ont00001938 ;
                rdfs:range cco:ont00001069 ;
                rdfs:comment "See notes for inverse property." ;
                rdfs:label "represented by"@en ;
                <http://www.w3.org/2004/02/skos/core#definition> "y represented_by x iff x is an instance of Information Content Entity, and y is an instance of Entity, and z is carrier of x, such that x is about y in virtue of there existing an isomorphism between characteristics of z and y."@en ;
                cco:ont00001760 <https://www.commoncoreontologies.org/ModalRelationOntology> .


###  https://www.commoncoreontologies.org/mro/ont00001874
mro:ont00001874 rdf:type owl:ObjectProperty ;
                rdfs:subPropertyOf mro:mro00000001 ;
                rdfs:domain obo:BFO_0000008 ;
                rdfs:range [ rdf:type owl:Class ;
                             owl:unionOf ( obo:BFO_0000015
                                           obo:BFO_0000035
                                         )
                           ] ;
                rdfs:label "is temporal region of"@en ;
                <http://www.w3.org/2004/02/skos/core#definition> "t is temporal region of p iff p occupies temporal region t."@en ;
                <http://www.w3.org/2004/02/skos/core#editorialNote> "Leaving this is in ERO for now since BFO2020 has no inverse of occupies-temporal-region yet."@en ;
                cco:ont00001760 <https://www.commoncoreontologies.org/ModalRelationOntology> .


###  https://www.commoncoreontologies.org/mro/ont00001875
mro:ont00001875 rdf:type owl:ObjectProperty ;
                rdfs:subPropertyOf mro:ont00001924 ;
                owl:inverseOf mro:ont00001923 ;
                rdfs:domain obo:BFO_0000038 ;
                rdfs:range obo:BFO_0000038 ;
                rdfs:label "interval started by"@en ;
                <http://www.w3.org/2004/02/skos/core#definition> "A Temporal Interval INT2 is started by some Temporal Interval INT1 iff there exist Temporal Instants inst1, inst2, and inst3 such that inst1 is the starting instant of both INT1 and INT2, inst2 is the ending instant of INT1, inst3 is the ending instant of INT2 and inst2 is before inst3."@en ;
                cco:ont00001754 "J. F. Allen and J. A. G. M. Koomen. Planning using a temporal world model. In Proceedings of the 8th International Joint Conference on Artificial Intelligence (IJCAI-1983)  pages 741–747. Available at: https://www.ijcai.org/Proceedings/83-2/Papers/036.pdf"@en ;
                cco:ont00001760 <https://www.commoncoreontologies.org/ModalRelationOntology> .


###  https://www.commoncoreontologies.org/mro/ont00001876
mro:ont00001876 rdf:type owl:ObjectProperty ;
                rdfs:subPropertyOf mro:ont00001850 ;
                rdfs:label "is grandfather of"@en ;
                cco:ont00001760 <https://www.commoncoreontologies.org/ModalRelationOntology> .


###  https://www.commoncoreontologies.org/mro/ont00001877
mro:ont00001877 rdf:type owl:ObjectProperty ;
                rdfs:subPropertyOf mro:ont00001966 ;
                owl:inverseOf mro:ont00001964 ;
                rdfs:domain cco:ont00001364 ;
                rdfs:label "is a interval measurement of"@en ;
                <http://www.w3.org/2004/02/skos/core#definition> "x is_a_interval_measurement_of y iff x is an instance of Information Content Entity and y is an instance of Entity, such that x describes some attribute of y relative to a scale which has uniform intervals but has a zero value that does not correspond to an absence of the attribute being measured."@en ;
                <http://www.w3.org/2004/02/skos/core#example> "a measurement of air temperature on the Celsius scale." ;
                cco:ont00001760 <https://www.commoncoreontologies.org/ModalRelationOntology> .


###  https://www.commoncoreontologies.org/mro/ont00001878
mro:ont00001878 rdf:type owl:ObjectProperty ;
                rdfs:subPropertyOf mro:mro00000001 ;
                owl:inverseOf mro:ont00001919 ;
                rdfs:label "is mention of"@en ;
                <http://www.w3.org/2004/02/skos/core#definition> "x is_mention_of y iff x is an instance Information Bearing Entity and y is an instance Entity, such that x is used as a reference to y."@en ;
                cco:ont00001760 <https://www.commoncoreontologies.org/ModalRelationOntology> .


###  https://www.commoncoreontologies.org/mro/ont00001879
mro:ont00001879 rdf:type owl:ObjectProperty ;
                rdfs:subPropertyOf mro:ont00001801 ;
                owl:inverseOf mro:ont00001916 ;
                rdfs:range cco:ont00000686 ;
                rdfs:label "designated by"@en ;
                <http://www.w3.org/2004/02/skos/core#definition> "x designated_by y iff y is an instance of Information Content Entity and x is an instance of Entity, such that given some context, y uniquely distinguishes x from other entities."@en ;
                cco:ont00001760 <https://www.commoncoreontologies.org/ModalRelationOntology> .


###  https://www.commoncoreontologies.org/mro/ont00001880
mro:ont00001880 rdf:type owl:ObjectProperty ;
                rdfs:subPropertyOf mro:ont00001809 ;
                owl:inverseOf mro:ont00001898 ;
                rdfs:domain cco:ont00001379 ;
                rdfs:range cco:ont00000300 ;
                rdfs:label "capability of aggregate"@en ;
                <http://www.w3.org/2004/02/skos/core#definition> "x capability_of_aggregate y iff y is an instance of Object Aggregate and x is an instance of Agent Capability, such that x inheres in aggregate y."@en ;
                cco:ont00001760 <https://www.commoncoreontologies.org/ModalRelationOntology> .


###  https://www.commoncoreontologies.org/mro/ont00001881
mro:ont00001881 rdf:type owl:ObjectProperty ;
                rdfs:subPropertyOf mro:ont00001818 ;
                rdfs:label "is son in-law of"@en ;
                cco:ont00001760 <https://www.commoncoreontologies.org/ModalRelationOntology> .


###  https://www.commoncoreontologies.org/mro/ont00001882
mro:ont00001882 rdf:type owl:ObjectProperty ;
                rdfs:subPropertyOf mro:ont00001850 ;
                rdfs:label "is grandmother of"@en ;
                cco:ont00001760 <https://www.commoncoreontologies.org/ModalRelationOntology> .


###  https://www.commoncoreontologies.org/mro/ont00001883
mro:ont00001883 rdf:type owl:ObjectProperty ;
                rdfs:subPropertyOf mro:ont00001902 ;
                rdfs:label "is brother of"@en ;
                cco:ont00001760 <https://www.commoncoreontologies.org/ModalRelationOntology> .


###  https://www.commoncoreontologies.org/mro/ont00001884
mro:ont00001884 rdf:type owl:ObjectProperty ;
                rdfs:subPropertyOf mro:ont00001801 ;
                owl:inverseOf mro:ont00001980 ;
                owl:propertyChainAxiom ( mro:ont00001917
                                         mro:BFO_0000176
                                       ) ;
                rdfs:label "condition described by"@en ;
                <http://www.w3.org/2004/02/skos/core#definition> "c condition_described_by p iff p is an instance of a Performance Specification, and p has part d, and d is an instance of a Descriptive Information Content Entity, and p prescribes an entity s, and d describes c, and c is an entity that is causally relevant to s existing as prescribed by p."@en ;
                cco:ont00001760 <https://www.commoncoreontologies.org/ModalRelationOntology> .


###  https://www.commoncoreontologies.org/mro/ont00001885
mro:ont00001885 rdf:type owl:ObjectProperty ;
                rdfs:subPropertyOf mro:ont00001818 ;
                rdfs:label "has mother in law"@en ;
                cco:ont00001760 <https://www.commoncoreontologies.org/ModalRelationOntology> .


###  https://www.commoncoreontologies.org/mro/ont00001886
mro:ont00001886 rdf:type owl:ObjectProperty ;
                rdfs:subPropertyOf mro:BFO_0000056 ;
                rdfs:domain obo:BFO_0000002 ;
                rdfs:range obo:BFO_0000015 ;
                rdfs:label "is affected by"@en ;
                <http://www.w3.org/2004/02/skos/core#definition> "x is_affected_by y iff x is an instance of Continuant and y is an instance of Process, and y influences x in some manner, most often by producing a change in x."@en ;
                cco:ont00001760 <https://www.commoncoreontologies.org/ModalRelationOntology> .


###  https://www.commoncoreontologies.org/mro/ont00001887
mro:ont00001887 rdf:type owl:ObjectProperty ;
                rdfs:subPropertyOf mro:ont00001804 ;
                rdfs:label "is wife of"@en ;
                cco:ont00001760 <https://www.commoncoreontologies.org/ModalRelationOntology> .


###  https://www.commoncoreontologies.org/mro/ont00001888
mro:ont00001888 rdf:type owl:ObjectProperty ;
                rdfs:subPropertyOf mro:mro00000001 ;
                rdfs:domain obo:BFO_0000015 ;
                rdfs:range obo:BFO_0000015 ;
                <http://purl.org/dc/terms/created> "2022-12-30T21:32:27-05:00"^^xsd:dateTime ;
                <http://purl.org/dc/terms/creator> "https://cubrc.org"^^xsd:anyURI ;
                rdfs:label "disrupts"@en ;
                <http://www.w3.org/2004/02/skos/core#definition> "A relation where one process disrupts another process from occurring as it would have."@en ;
                <http://www.w3.org/2004/02/skos/core#editorialNote> "To lower the grade of a process is to lower the quality of a process according to some standard, for example when realizing a capability or a function."@en ;
                <http://www.w3.org/2004/02/skos/core#prefLabel> "disrupts"@en ;
                <http://www.w3.org/2004/02/skos/core#scopeNote> "A process can disrupt another process from occurring as it would have by 1) preventing a disposition or role from being realized by that process, 2) lowering the grade of the process, or 3) stopping the process from continuing to occur."@en ;
                cco:ont00001760 <https://www.commoncoreontologies.org/ModalRelationOntology> .


###  https://www.commoncoreontologies.org/mro/ont00001889
mro:ont00001889 rdf:type owl:ObjectProperty ;
                rdfs:subPropertyOf mro:BFO_0000197 ;
                owl:inverseOf mro:ont00001954 ;
                rdfs:domain cco:ont00001379 ;
                rdfs:range cco:ont00001017 ;
                rdfs:label "capability of"@en ;
                <http://www.w3.org/2004/02/skos/core#definition> "x capability_of y iff y is an instance of Agent and x is an instance of Agent Capability, such that x inheres in y."@en ;
                cco:ont00001760 <https://www.commoncoreontologies.org/ModalRelationOntology> .


###  https://www.commoncoreontologies.org/mro/ont00001890
mro:ont00001890 rdf:type owl:ObjectProperty ;
                rdfs:subPropertyOf mro:ont00001996 ;
                rdfs:label "has step brother"@en ;
                cco:ont00001760 <https://www.commoncoreontologies.org/ModalRelationOntology> .


###  https://www.commoncoreontologies.org/mro/ont00001891
mro:ont00001891 rdf:type owl:ObjectProperty ;
                rdfs:subPropertyOf mro:ont00001818 ;
                owl:inverseOf mro:ont00001952 ;
                rdfs:label "has brother in law"@en ;
                cco:ont00001760 <https://www.commoncoreontologies.org/ModalRelationOntology> .


###  https://www.commoncoreontologies.org/mro/ont00001892
mro:ont00001892 rdf:type owl:ObjectProperty ;
                rdfs:subPropertyOf mro:ont00001876 ;
                owl:inverseOf mro:ont00001972 ;
                rdfs:label "is paternal grandfather of"@en ;
                cco:ont00001760 <https://www.commoncoreontologies.org/ModalRelationOntology> .


###  https://www.commoncoreontologies.org/mro/ont00001893
mro:ont00001893 rdf:type owl:ObjectProperty ;
                rdfs:subPropertyOf mro:mro00000001 ;
                owl:inverseOf mro:ont00001990 ;
                rdf:type owl:TransitiveProperty ;
                rdfs:domain obo:BFO_0000148 ;
                rdfs:range obo:BFO_0000148 ;
                rdfs:label "instant is after"@en ;
                <http://www.w3.org/2004/02/skos/core#definition> "A temporal instant t2 (a instance of a zero-dimensional temporal region) is after another temporal instant t1 iff there exists some instance of a temporal interval ti1 such that t1 is the starting instant of ti1 and t2 is the ending instant of ti1."@en ;
                <http://www.w3.org/2004/02/skos/core#scopeNote> "'instant is after' is a primitive relationship. Informally, a temporal instant t2 is after some temporal instant t1 if and only if t1 precedes t2."@en ;
                cco:ont00001754 "J. F. Allen and J. A. G. M. Koomen. Planning using a temporal world model. In Proceedings of the 8th International Joint Conference on Artificial Intelligence (IJCAI-1983)  pages 741–747. Available at: https://www.ijcai.org/Proceedings/83-2/Papers/036.pdf"@en ;
                cco:ont00001760 <https://www.commoncoreontologies.org/ModalRelationOntology> .


###  https://www.commoncoreontologies.org/mro/ont00001894
mro:ont00001894 rdf:type owl:ObjectProperty ;
                rdfs:subPropertyOf mro:ont00001806 ;
                rdfs:label "has paternal first cousin"@en ;
                cco:ont00001760 <https://www.commoncoreontologies.org/ModalRelationOntology> .


###  https://www.commoncoreontologies.org/mro/ont00001895
mro:ont00001895 rdf:type owl:ObjectProperty ;
                rdfs:subPropertyOf mro:BFO_0000056 ;
                rdfs:domain obo:BFO_0000040 ;
                rdfs:range obo:BFO_0000015 ;
                rdfs:label "accomplice in"@en ;
                <http://www.w3.org/2004/02/skos/core#definition> "An agent a1 is accomplice_in some Processual Entity p1 iff a1 assists in the commission of p1, is located at the location of p1, but is not agent_in p1."@en ;
                cco:ont00001754 "https://en.wikipedia.org/w/index.php?title=Accomplice&oldid=1002047204"^^xsd:anyURI ;
                cco:ont00001760 <https://www.commoncoreontologies.org/ModalRelationOntology> .


###  https://www.commoncoreontologies.org/mro/ont00001896
mro:ont00001896 rdf:type owl:ObjectProperty ;
                rdfs:subPropertyOf mro:ont00001862 ;
                owl:inverseOf mro:ont00001915 ;
                rdf:type owl:IrreflexiveProperty ;
                rdfs:domain obo:BFO_0000038 ;
                rdfs:range obo:BFO_0000038 ;
                rdfs:label "interval meets"@en ;
                <http://www.w3.org/2004/02/skos/core#definition> "A Temporal Interval INT1 meets some Temporal Interval INT2 iff there exists some Temporal Instant inst1 such that inst1 is the ending instant of INT1 and inst1 is the starting instant of INT2."@en ;
                cco:ont00001754 "J. F. Allen and J. A. G. M. Koomen. Planning using a temporal world model. In Proceedings of the 8th International Joint Conference on Artificial Intelligence (IJCAI-1983)  pages 741–747. Available at: https://www.ijcai.org/Proceedings/83-2/Papers/036.pdf"@en ;
                cco:ont00001760 <https://www.commoncoreontologies.org/ModalRelationOntology> .


###  https://www.commoncoreontologies.org/mro/ont00001897
mro:ont00001897 rdf:type owl:ObjectProperty ;
                rdfs:subPropertyOf mro:ont00001882 ;
                owl:inverseOf mro:ont00001960 ;
                rdfs:label "is maternal grandmother of"@en ;
                cco:ont00001760 <https://www.commoncoreontologies.org/ModalRelationOntology> .


###  https://www.commoncoreontologies.org/mro/ont00001898
mro:ont00001898 rdf:type owl:ObjectProperty ;
                rdfs:subPropertyOf mro:ont00001836 ;
                rdfs:domain cco:ont00000300 ;
                rdfs:range cco:ont00001379 ;
                rdfs:label "aggregate has capability"@en ;
                <http://www.w3.org/2004/02/skos/core#definition> "x aggregate_has_capability y iff x is an instance of Object Aggregate and y is an instance of Agent Capability, such that x is aggregate bearer of y."@en ;
                cco:ont00001760 <https://www.commoncoreontologies.org/ModalRelationOntology> .


###  https://www.commoncoreontologies.org/mro/ont00001899
mro:ont00001899 rdf:type owl:ObjectProperty ;
                rdfs:subPropertyOf mro:ont00001942 ;
                owl:inverseOf mro:ont00001976 ;
                rdfs:domain cco:ont00001175 ;
                rdfs:range cco:ont00000253 ;
                rdfs:label "language used in"@en ;
                <http://www.w3.org/2004/02/skos/core#definition> "x language_used_by y iff y is an instance of Information Bearing Entity and x is an instance of Language, such that the literal value of y is a string that is encoded according to the syntax of x."@en ;
                cco:ont00001760 <https://www.commoncoreontologies.org/ModalRelationOntology> .


###  https://www.commoncoreontologies.org/mro/ont00001900
mro:ont00001900 rdf:type owl:ObjectProperty ;
                rdfs:subPropertyOf mro:ont00001997 ;
                owl:inverseOf mro:ont00001913 ;
                rdfs:domain cco:ont00000469 ;
                rdfs:range cco:ont00000253 ;
                rdfs:label "is geospatial coordinate reference system of"@en ;
                <http://www.w3.org/2004/02/skos/core#definition> "x is_geospatial_coordinate_reference_system_of y iff y is an instance of Information Bearing Entity and x is an instance of Geospatial Coordinate Reference System, such that x describes the set of standards mentioned in y."@en ;
                cco:ont00001760 <https://www.commoncoreontologies.org/ModalRelationOntology> .


###  https://www.commoncoreontologies.org/mro/ont00001901
mro:ont00001901 rdf:type owl:ObjectProperty ;
                rdfs:subPropertyOf mro:ont00001836 ;
                rdfs:domain obo:BFO_0000027 ;
                rdfs:range obo:BFO_0000023 ;
                rdfs:label "aggregate has role"@en ;
                <http://www.w3.org/2004/02/skos/core#definition> "x aggregate_has_role y iff x is an instance of Object Aggregate and y is an instance of Role, such that x aggregate_bearer_of y."@en ;
                cco:ont00001760 <https://www.commoncoreontologies.org/ModalRelationOntology> .


###  https://www.commoncoreontologies.org/mro/ont00001902
mro:ont00001902 rdf:type owl:ObjectProperty ;
                rdfs:subPropertyOf mro:ont00001865 ;
                owl:inverseOf mro:ont00001902 ;
                rdf:type owl:SymmetricProperty ;
                rdfs:label "is sibling of"@en ;
                cco:ont00001760 <https://www.commoncoreontologies.org/ModalRelationOntology> .


###  https://www.commoncoreontologies.org/mro/ont00001903
mro:ont00001903 rdf:type owl:ObjectProperty ;
                rdfs:subPropertyOf mro:ont00001876 ;
                owl:inverseOf mro:ont00001973 ;
                rdfs:label "is maternal grandfather of"@en ;
                cco:ont00001760 <https://www.commoncoreontologies.org/ModalRelationOntology> .


###  https://www.commoncoreontologies.org/mro/ont00001904
mro:ont00001904 rdf:type owl:ObjectProperty ;
                rdfs:subPropertyOf mro:ont00001917 ;
                owl:inverseOf mro:ont00001966 ;
                rdfs:range cco:ont00001163 ;
                rdfs:label "is measured by"@en ;
                <http://www.w3.org/2004/02/skos/core#definition> "y is_measured_by x iff x is an instance of Information Content Entity and y is an instance of Entity, such that x describes some attribute of y relative to some scale or classification scheme."@en ;
                cco:ont00001760 <https://www.commoncoreontologies.org/ModalRelationOntology> .


###  https://www.commoncoreontologies.org/mro/ont00001905
mro:ont00001905 rdf:type owl:ObjectProperty ;
                rdfs:subPropertyOf mro:ont00001975 ;
                owl:inverseOf mro:ont00001927 ;
                rdfs:label "is half-brother of"@en ;
                cco:ont00001760 <https://www.commoncoreontologies.org/ModalRelationOntology> .


###  https://www.commoncoreontologies.org/mro/ont00001906
mro:ont00001906 rdf:type owl:ObjectProperty ;
                rdfs:subPropertyOf mro:ont00001806 ;
                owl:inverseOf mro:ont00001934 ;
                rdfs:comment "Comment is_maternal_first_cousin_of is not a symmetric relationship as is is_first_cousin_of"@en ;
                rdfs:label "is maternal first cousin of"@en ;
                <http://www.w3.org/2004/02/skos/core#definition> "Person A is maternal first cousin of Person B iff Person B has mother M and M has sibling P and P is parent of Person A."@en ;
                cco:ont00001760 <https://www.commoncoreontologies.org/ModalRelationOntology> .


###  https://www.commoncoreontologies.org/mro/ont00001907
mro:ont00001907 rdf:type owl:ObjectProperty ;
                rdfs:subPropertyOf mro:ont00001836 ;
                rdfs:domain obo:BFO_0000027 ;
                rdfs:range obo:BFO_0000019 ;
                rdfs:label "aggregate has quality"@en ;
                <http://www.w3.org/2004/02/skos/core#definition> "x aggregate_has_quality y iff x is an instance of Object Aggregate and y is an instance of Quality, such that x aggregate_bearer_of y."@en ;
                cco:ont00001760 <https://www.commoncoreontologies.org/ModalRelationOntology> .


###  https://www.commoncoreontologies.org/mro/ont00001908
mro:ont00001908 rdf:type owl:ObjectProperty ;
                rdfs:subPropertyOf mro:BFO_0000101 ;
                rdfs:domain cco:ont00000253 ;
                rdfs:range cco:ont00000829 ;
                rdfs:label "uses time zone identifier"@en ;
                <http://www.w3.org/2004/02/skos/core#definition> "x uses_time_zone_identifier y iff x is an instance of Information Bearing Entity and y is an instance of Time Zone Identifier, such that y designates the spatial region associated with the time zone mentioned in x."@en ;
                cco:ont00001760 <https://www.commoncoreontologies.org/ModalRelationOntology> .


###  https://www.commoncoreontologies.org/mro/ont00001909
mro:ont00001909 rdf:type owl:ObjectProperty ;
                rdfs:subPropertyOf mro:ont00001855 ;
                rdfs:domain obo:BFO_0000141 ;
                rdfs:range obo:BFO_0000141 ;
                rdfs:label "has tangential part"@en ;
                <http://www.w3.org/2004/02/skos/core#definition> "x has_tangential_part y iff x, y, and z are instances of Immaterial Entity, and x has_spatial_part y, such that z externally connects with both x and y."@en ;
                <http://www.w3.org/2004/02/skos/core#scopeNote> "Given a stronger temporal interpretation, this property may be transitive. For more info please refer to https://github.com/BFO-ontology/BFO-2020/tree/master/src/owl/temporal%20extensions."@en ;
                cco:ont00001754 "Randell, D. A., Cui, Z. and Cohn, A. G.: 1992, \"A spatial logic based on regions and connection,\" Proc. 3rd Int. Conf. on Knowledge Representation and Reasoning, Morgan Kaufmann, San Mateo, pp. 165-176. Available at: https://www.dpi.inpe.br/gilberto/references/cohn_rcc.pdf"@en ;
                cco:ont00001760 <https://www.commoncoreontologies.org/ModalRelationOntology> .


###  https://www.commoncoreontologies.org/mro/ont00001910
mro:ont00001910 rdf:type owl:ObjectProperty ;
                rdfs:subPropertyOf mro:ont00001942 ;
                owl:inverseOf mro:ont00001998 ;
                rdfs:domain cco:ont00001324 ;
                rdfs:range obo:BFO_0000015 ;
                rdfs:label "permits"@en ;
                <http://www.w3.org/2004/02/skos/core#definition> "x permits y at t iff: x is an instance of Process Regulation at time t, and y is an instance of Process at time t, and x prescribes that y may occur."@en ;
                <http://www.w3.org/2004/02/skos/core#scopeNote> "Given a stronger temporal interpretation, this property may be asymmetric and irreflexive. For more info please refer to https://github.com/BFO-ontology/BFO-2020/tree/master/src/owl/temporal%20extensions."@en ;
                cco:ont00001760 <https://www.commoncoreontologies.org/ModalRelationOntology> .


###  https://www.commoncoreontologies.org/mro/ont00001911
mro:ont00001911 rdf:type owl:ObjectProperty ;
                rdfs:subPropertyOf mro:ont00001882 ;
                owl:inverseOf mro:ont00001937 ;
                rdfs:label "is paternal grandmother of"@en ;
                cco:ont00001760 <https://www.commoncoreontologies.org/ModalRelationOntology> .


###  https://www.commoncoreontologies.org/mro/ont00001912
mro:ont00001912 rdf:type owl:ObjectProperty ;
                rdfs:subPropertyOf mro:BFO_0000101 ;
                owl:inverseOf mro:ont00001997 ;
                rdfs:domain cco:ont00000253 ;
                rdfs:range cco:ont00000398 ;
                rdfs:label "uses reference system"@en ;
                <http://www.w3.org/2004/02/skos/core#definition> "y uses_reference_system x iff y is an instance of Information Bearing Entity and x is an instance of Reference System, such that x describes the set of standards mentioned in y."@en ;
                cco:ont00001760 <https://www.commoncoreontologies.org/ModalRelationOntology> .


###  https://www.commoncoreontologies.org/mro/ont00001913
mro:ont00001913 rdf:type owl:ObjectProperty ;
                rdfs:subPropertyOf mro:ont00001912 ;
                rdfs:domain cco:ont00000253 ;
                rdfs:range cco:ont00000469 ;
                rdfs:label "uses geospatial coordinate reference system"@en ;
                <http://www.w3.org/2004/02/skos/core#definition> "y uses_geospatial_coordinate_reference_system x iff y is an instance of Information Bearing Entity and x is an instance of Geospatial Coordinate Reference System, such that x describes the set of standards mentioned in y."@en ;
                cco:ont00001760 <https://www.commoncoreontologies.org/ModalRelationOntology> .


###  https://www.commoncoreontologies.org/mro/ont00001914
mro:ont00001914 rdf:type owl:ObjectProperty ;
                rdfs:subPropertyOf mro:ont00001904 ;
                rdfs:range cco:ont00000293 ;
                rdfs:label "is measured by nominal"@en ;
                <http://www.w3.org/2004/02/skos/core#definition> "y is_measured_by_nominal x iff x is an instance of Information Content Entity and y is an instance of Entity, such that x classifies y relative to some set of shared, possibly arbitrary, characteristics."@en ;
                cco:ont00001760 <https://www.commoncoreontologies.org/ModalRelationOntology> .


###  https://www.commoncoreontologies.org/mro/ont00001915
mro:ont00001915 rdf:type owl:ObjectProperty ;
                rdfs:subPropertyOf mro:ont00001862 ;
                rdf:type owl:IrreflexiveProperty ;
                rdfs:domain obo:BFO_0000038 ;
                rdfs:range obo:BFO_0000038 ;
                rdfs:label "interval met by"@en ;
                <http://www.w3.org/2004/02/skos/core#definition> "A Temporal Interval INT2 is met by some Temporal Interval INT1 iff there exists some Temporal Instant inst1 such that inst1 is the starting instant of INT2 and inst1 is the ending instant of INT1."@en ;
                cco:ont00001754 "J. F. Allen and J. A. G. M. Koomen. Planning using a temporal world model. In Proceedings of the 8th International Joint Conference on Artificial Intelligence (IJCAI-1983)  pages 741–747. Available at: https://www.ijcai.org/Proceedings/83-2/Papers/036.pdf"@en ;
                cco:ont00001760 <https://www.commoncoreontologies.org/ModalRelationOntology> .


###  https://www.commoncoreontologies.org/mro/ont00001916
mro:ont00001916 rdf:type owl:ObjectProperty ;
                rdfs:subPropertyOf mro:ont00001808 ;
                rdfs:domain cco:ont00000686 ;
                rdfs:label "designates"@en ;
                <http://www.w3.org/2004/02/skos/core#definition> "x designates y iff x is an instance of an Information Content Entity, and y is an instance of an Entity, such that given some context, x uniquely distinguishes y from other entities."@en ;
                <http://www.w3.org/2004/02/skos/core#example> "a URL designates the location of a Web Page on the internet" ,
                                                              "a person's name designates that person" ,
                                                              "a vehicle identification number designates some vehicle" ;
                <http://www.w3.org/2004/02/skos/core#scopeNote> "Given a stronger temporal interpretation, this property may be functional. For more info please refer to https://github.com/BFO-ontology/BFO-2020/tree/master/src/owl/temporal%20extensions."@en ;
                cco:ont00001760 <https://www.commoncoreontologies.org/ModalRelationOntology> .


###  https://www.commoncoreontologies.org/mro/ont00001917
mro:ont00001917 rdf:type owl:ObjectProperty ;
                rdfs:subPropertyOf mro:ont00001801 ;
                owl:inverseOf mro:ont00001982 ;
                rdfs:range cco:ont00000853 ;
                rdfs:label "described by"@en ;
                <http://www.w3.org/2004/02/skos/core#definition> "x described_by y iff y is an instance of Information Content Entity, and x is an instance of Entity, such that y is about the characteristics by which y can be recognized or visualized."@en ;
                cco:ont00001760 <https://www.commoncoreontologies.org/ModalRelationOntology> .


###  https://www.commoncoreontologies.org/mro/ont00001918
mro:ont00001918 rdf:type owl:ObjectProperty ;
                rdfs:subPropertyOf mro:BFO_0000066 ;
                rdfs:domain obo:BFO_0000015 ;
                rdfs:range obo:BFO_0000029 ;
                rdfs:label "occurs at"@en ;
                <http://www.w3.org/2004/02/skos/core#definition> "x occurs_at y iff x is an instance of Process and y is an instance of Site, such that x occurs in y."@en ;
                cco:ont00001760 <https://www.commoncoreontologies.org/ModalRelationOntology> .


###  https://www.commoncoreontologies.org/mro/ont00001919
mro:ont00001919 rdf:type owl:ObjectProperty ;
                rdfs:subPropertyOf mro:mro00000001 ;
                rdfs:label "is mentioned by"@en ;
                <http://www.w3.org/2004/02/skos/core#definition> "y is_mention_by x iff x is an instance Information Bearing Entity and y is an instance Entity, such that x is used as a reference to y."@en ;
                cco:ont00001760 <https://www.commoncoreontologies.org/ModalRelationOntology> .


###  https://www.commoncoreontologies.org/mro/ont00001920
mro:ont00001920 rdf:type owl:ObjectProperty ;
                rdfs:subPropertyOf mro:ont00001801 ;
                owl:inverseOf mro:ont00001942 ;
                rdfs:range cco:ont00000965 ;
                rdfs:label "prescribed by"@en ;
                <http://www.w3.org/2004/02/skos/core#definition> "x prescribed_by y iff y is an instance of Information Content Entity and x is an instance of Entity, such that y serves as a rule or guide for x if x is an Occurrent, or y serves as a model for x if x is a Continuant."@en ;
                cco:ont00001760 <https://www.commoncoreontologies.org/ModalRelationOntology> .


###  https://www.commoncoreontologies.org/mro/ont00001921
mro:ont00001921 rdf:type owl:ObjectProperty ;
                rdfs:subPropertyOf mro:BFO_0000057 ;
                rdfs:domain obo:BFO_0000015 ;
                rdfs:range obo:BFO_0000002 ;
                rdfs:label "has input"@en ;
                <http://www.w3.org/2004/02/skos/core#definition> "y has_input x iff x is an instance of Continuant and y is an instance of Process, such that the presence of x at the beginning of y is a necessary condition for the start of y."@en ;
                cco:ont00001760 <https://www.commoncoreontologies.org/ModalRelationOntology> .


###  https://www.commoncoreontologies.org/mro/ont00001922
mro:ont00001922 rdf:type owl:ObjectProperty ;
                rdfs:subPropertyOf mro:BFO_0000057 ;
                owl:inverseOf mro:ont00001978 ;
                rdfs:range cco:ont00001017 ;
                rdfs:label "has recipient"@en ;
                <http://www.w3.org/2004/02/skos/core#definition> "x has_recipient y iff y is an instance of Agent and x is an instance of Act Of Communication, such that y is the recipient and decoder of the InformationContentEntity intended for communication in x."@en ;
                cco:ont00001760 <https://www.commoncoreontologies.org/ModalRelationOntology> .


###  https://www.commoncoreontologies.org/mro/ont00001923
mro:ont00001923 rdf:type owl:ObjectProperty ;
                rdfs:subPropertyOf mro:ont00001971 ;
                rdfs:domain obo:BFO_0000038 ;
                rdfs:range obo:BFO_0000038 ;
                rdfs:label "interval starts"@en ;
                <http://www.w3.org/2004/02/skos/core#definition> "A Temporal Interval INT1 starts some Temporal Interval INT2 iff there exist Temporal Instants inst1, inst2, and inst3 such that inst1 is the starting instant of both INT1 and INT2, inst2 is the ending instant of INT1, inst3 is the ending instant of INT2 and inst2 is before inst3."@en ;
                cco:ont00001754 "J. F. Allen and J. A. G. M. Koomen. Planning using a temporal world model. In Proceedings of the 8th International Joint Conference on Artificial Intelligence (IJCAI-1983)  pages 741–747. Available at: https://www.ijcai.org/Proceedings/83-2/Papers/036.pdf"@en ;
                cco:ont00001760 <https://www.commoncoreontologies.org/ModalRelationOntology> .


###  https://www.commoncoreontologies.org/mro/ont00001924
mro:ont00001924 rdf:type owl:ObjectProperty ;
                rdfs:subPropertyOf mro:mro00000001 ;
                owl:inverseOf mro:ont00001971 ;
                rdfs:domain obo:BFO_0000038 ;
                rdfs:range obo:BFO_0000038 ;
                rdfs:label "interval contains"@en ;
                <http://www.w3.org/2004/02/skos/core#definition> "A Temporal Interval INT2 contains some Temporal Interval INT1 iff there exist Temporal Instants inst1, inst2, inst3, and inst4 such that inst1 is the starting instant of INT1, inst2 is the ending instant of INT1, inst3 is the starting instant of INT2, inst4 is the ending instant of INT2, inst3 is before or identical to inst1, and inst2 is before or identical to inst4, but it is not the case that both inst3 is identical to inst1 and inst2 is identical to inst4."@en ;
                cco:ont00001754 "J. F. Allen and J. A. G. M. Koomen. Planning using a temporal world model. In Proceedings of the 8th International Joint Conference on Artificial Intelligence (IJCAI-1983)  pages 741–747. Available at: https://www.ijcai.org/Proceedings/83-2/Papers/036.pdf"@en ;
                cco:ont00001760 <https://www.commoncoreontologies.org/ModalRelationOntology> .


###  https://www.commoncoreontologies.org/mro/ont00001925
mro:ont00001925 rdf:type owl:ObjectProperty ;
                rdfs:subPropertyOf mro:mro00000001 ;
                rdfs:label "is used by"@en ;
                <http://www.w3.org/2004/02/skos/core#definition> "x is_used_by y iff y is an instance of an Agent and x is an instance of a Material Entity, such that both x and y participate in some instance of a Process wherein y attempts to accomplish a goal by manipulating, deploying, leveraging some attribute of y."@en ;
                cco:ont00001760 <https://www.commoncoreontologies.org/ModalRelationOntology> .


###  https://www.commoncoreontologies.org/mro/ont00001926
mro:ont00001926 rdf:type owl:ObjectProperty ;
                rdfs:subPropertyOf mro:ont00001988 ;
                rdfs:label "is paternal uncle of"@en ;
                cco:ont00001760 <https://www.commoncoreontologies.org/ModalRelationOntology> .


###  https://www.commoncoreontologies.org/mro/ont00001927
mro:ont00001927 rdf:type owl:ObjectProperty ;
                rdfs:subPropertyOf mro:ont00001975 ;
                rdfs:label "has half brother"@en ;
                cco:ont00001760 <https://www.commoncoreontologies.org/ModalRelationOntology> .


###  https://www.commoncoreontologies.org/mro/ont00001928
mro:ont00001928 rdf:type owl:ObjectProperty ;
                rdfs:subPropertyOf mro:mro00000001 ;
                rdfs:domain obo:BFO_0000004 ;
                rdfs:range obo:BFO_0000004 ;
                rdfs:label "is predecessor of"@en ;
                <http://www.w3.org/2004/02/skos/core#definition> "A continuant c1 is a predecessor of some continuant c2 iff there is some process p1 and c1 is an input to p1 and c2 is an output of p1."@en ;
                <http://www.w3.org/2004/02/skos/core#scopeNote> "More informally, c1 is a predecessor of c2 iff c1 has been followed or replaced by c2."@en ;
                cco:ont00001760 <https://www.commoncoreontologies.org/ModalRelationOntology> .


###  https://www.commoncoreontologies.org/mro/ont00001929
mro:ont00001929 rdf:type owl:ObjectProperty ;
                rdfs:subPropertyOf mro:ont00001988 ;
                rdfs:label "is maternal uncle of"@en ;
                cco:ont00001760 <https://www.commoncoreontologies.org/ModalRelationOntology> .


###  https://www.commoncoreontologies.org/mro/ont00001930
mro:ont00001930 rdf:type owl:ObjectProperty ;
                rdfs:subPropertyOf mro:ont00001865 ;
                owl:inverseOf mro:ont00001930 ;
                rdf:type owl:SymmetricProperty ;
                rdfs:label "is second cousin of"@en ;
                cco:ont00001760 <https://www.commoncoreontologies.org/ModalRelationOntology> .


###  https://www.commoncoreontologies.org/mro/ont00001931
mro:ont00001931 rdf:type owl:ObjectProperty ;
                rdfs:subPropertyOf mro:ont00001810 ;
                rdfs:domain obo:BFO_0000141 ;
                rdfs:range obo:BFO_0000141 ;
                rdfs:label "externally connects with"@en ;
                <http://www.w3.org/2004/02/skos/core#definition> "An immaterial entity im1 externally connects with some immaterial entity im2 iff im1 connects with im2 and im1 does not overlap with im2."@en ;
                <http://www.w3.org/2004/02/skos/core#scopeNote> "Given a stronger temporal interpretation, this property may be symmetric. For more info please refer to https://github.com/BFO-ontology/BFO-2020/tree/master/src/owl/temporal%20extensions."@en ;
                cco:ont00001754 "Randell, D. A., Cui, Z. and Cohn, A. G.: 1992, \"A spatial logic based on regions and connection,\" Proc. 3rd Int. Conf. on Knowledge Representation and Reasoning, Morgan Kaufmann, San Mateo, pp. 165-176. Available at: https://www.dpi.inpe.br/gilberto/references/cohn_rcc.pdf"@en ;
                cco:ont00001760 <https://www.commoncoreontologies.org/ModalRelationOntology> .


###  https://www.commoncoreontologies.org/mro/ont00001932
mro:ont00001932 rdf:type owl:ObjectProperty ;
                rdfs:subPropertyOf mro:ont00001865 ;
                rdfs:label "is niece of"@en ;
                cco:ont00001760 <https://www.commoncoreontologies.org/ModalRelationOntology> .


###  https://www.commoncoreontologies.org/mro/ont00001933
mro:ont00001933 rdf:type owl:ObjectProperty ;
                rdfs:subPropertyOf mro:ont00001803 ;
                owl:inverseOf mro:ont00001962 ;
                rdfs:label "process starts"@en ;
                <http://www.w3.org/2004/02/skos/core#definition> "x process_starts y iff x and y are instances of processes, and x is_cause_of y, and i is an instance of a temporal instant, and r is an instant of a temporal interval, and y has starting instance i, and x occurs on r, and r interval contains i."@en ;
                <http://www.w3.org/2004/02/skos/core#scopeNote> "A process x starts another process y when x causes y while x is still occurring."@en ;
                cco:ont00001760 <https://www.commoncoreontologies.org/ModalRelationOntology> .


###  https://www.commoncoreontologies.org/mro/ont00001934
mro:ont00001934 rdf:type owl:ObjectProperty ;
                rdfs:subPropertyOf mro:ont00001806 ;
                rdfs:label "has maternal first cousin"@en ;
                cco:ont00001760 <https://www.commoncoreontologies.org/ModalRelationOntology> .


###  https://www.commoncoreontologies.org/mro/ont00001935
mro:ont00001935 rdf:type owl:ObjectProperty ;
                rdfs:subPropertyOf mro:ont00001818 ;
                rdfs:label "has father in law"@en ;
                cco:ont00001760 <https://www.commoncoreontologies.org/ModalRelationOntology> .


###  https://www.commoncoreontologies.org/mro/ont00001936
mro:ont00001936 rdf:type owl:ObjectProperty ;
                rdfs:subPropertyOf mro:BFO_0000056 ;
                rdfs:label "is object of"@en ;
                <http://www.w3.org/2004/02/skos/core#definition> "If p is a process and c is a continuant, then c is object of p if and only if the c is part of the projected state that the agent intends to achieve by performing p."@en ;
                cco:ont00001760 <https://www.commoncoreontologies.org/ModalRelationOntology> .


###  https://www.commoncoreontologies.org/mro/ont00001937
mro:ont00001937 rdf:type owl:ObjectProperty ;
                rdfs:subPropertyOf mro:ont00001840 ;
                rdfs:label "has paternal grandmother"@en ;
                cco:ont00001760 <https://www.commoncoreontologies.org/ModalRelationOntology> .


###  https://www.commoncoreontologies.org/mro/ont00001938
mro:ont00001938 rdf:type owl:ObjectProperty ;
                rdfs:subPropertyOf mro:ont00001808 ;
                rdfs:domain cco:ont00001069 ;
                rdfs:comment "Isomorphism between the carrier of x and the represented entity can be via a direct similarity relation, e.g., grooves in a vinyl record corresponding to sound waves, or linguistic convention, e.g., a court stenographer's transcription of spoken words, as well as others, such as encoding processes for images."@en ;
                rdfs:label "represents"@en ;
                <http://www.w3.org/2004/02/skos/core#definition> "x represents y iff x is an instance of Information Content Entity, y is an instance of Entity, and z is carrier of x, such that x is about y in virtue of there existing an isomorphism between characteristics of z and y."@en ;
                <http://www.w3.org/2004/02/skos/core#scopeNote> "Given a stronger temporal interpretation, this property may be functional. For more info please refer to https://github.com/BFO-ontology/BFO-2020/tree/master/src/owl/temporal%20extensions."@en ,
                                                                "The relationship that is being defined here is that between the content of a photographic image and its object, between the content of a video and its objects and events, between the content of an audio recording and the sounds or events generating those sounds, or between the content of a written transcript and the verbal event that it transcribes."@en ;
                cco:ont00001760 <https://www.commoncoreontologies.org/ModalRelationOntology> .


###  https://www.commoncoreontologies.org/mro/ont00001939
mro:ont00001939 rdf:type owl:ObjectProperty ;
                rdfs:subPropertyOf mro:mro00000001 ;
                owl:inverseOf mro:ont00001977 ;
                rdfs:domain [ rdf:type owl:Class ;
                              owl:unionOf ( cco:ont00001017
                                            cco:ont00001180
                                            cco:ont00001262
                                          )
                            ] ;
                rdfs:range [ rdf:type owl:Class ;
                             owl:unionOf ( cco:ont00001017
                                           cco:ont00001180
                                           cco:ont00001262
                                         )
                           ] ;
                rdfs:label "is affiliated with"@en ;
                <http://www.w3.org/2004/02/skos/core#definition> "x is_affiliated_with y iff x and y are instances of Agent, such that they have any kind of social or business relationship."@en ;
                cco:ont00001760 <https://www.commoncoreontologies.org/ModalRelationOntology> .


###  https://www.commoncoreontologies.org/mro/ont00001940
mro:ont00001940 rdf:type owl:ObjectProperty ;
                rdfs:subPropertyOf mro:ont00001862 ;
                rdfs:domain obo:BFO_0000038 ;
                rdfs:range obo:BFO_0000038 ;
                rdfs:label "interval is before"@en ;
                <http://www.w3.org/2004/02/skos/core#definition> "A TemporalInterval INT1 is before some TemporalInterval INT2 iff there exists TemporalInstants inst1, inst2 such that inst1 is the ending instant of INT1 and inst2 is the starting instant of INT2 and inst1 is before inst2."@en ;
                cco:ont00001754 "J. F. Allen and J. A. G. M. Koomen. Planning using a temporal world model. In Proceedings of the 8th International Joint Conference on Artificial Intelligence (IJCAI-1983)  pages 741–747. Available at: https://www.ijcai.org/Proceedings/83-2/Papers/036.pdf"@en ;
                cco:ont00001760 <https://www.commoncoreontologies.org/ModalRelationOntology> .


###  https://www.commoncoreontologies.org/mro/ont00001941
mro:ont00001941 rdf:type owl:ObjectProperty ;
                rdfs:subPropertyOf mro:ont00001955 ;
                owl:inverseOf mro:ont00001958 ;
                rdfs:label "is maternal aunt of"@en ;
                cco:ont00001760 <https://www.commoncoreontologies.org/ModalRelationOntology> .


###  https://www.commoncoreontologies.org/mro/ont00001942
mro:ont00001942 rdf:type owl:ObjectProperty ;
                rdfs:subPropertyOf mro:ont00001808 ;
                rdfs:domain cco:ont00000965 ;
                rdfs:label "prescribes"@en ;
                <http://www.w3.org/2004/02/skos/core#definition> "x prescribes y iff x is an instance of Information Content Entity and y is an instance of Entity, such that x serves as a rule or guide for y if y an Occurrent, or x serves as a model for y if y is a Continuant."@en ;
                <http://www.w3.org/2004/02/skos/core#example> "A blueprint prescribes some artifact or facility by being a model for it." ,
                                                              "A professional code of conduct prescribes some realizations of a profession (role) by giving rules for how the bearer should act in those realizations." ,
                                                              "An operations plan prescribes an operation by enumerating the tasks that need to be performed in order to achieve the objectives of the operation." ;
                cco:ont00001760 <https://www.commoncoreontologies.org/ModalRelationOntology> .


###  https://www.commoncoreontologies.org/mro/ont00001943
mro:ont00001943 rdf:type owl:ObjectProperty ;
                rdfs:subPropertyOf mro:ont00001977 ;
                rdfs:domain cco:ont00001262 ;
                rdfs:range cco:ont00001262 ;
                rdfs:label "supervises"@en ;
                <http://www.w3.org/2004/02/skos/core#definition> "A person p1 supervises a person p2 by virtue of p1 directing, managing, or overseeing p2."@en ;
                cco:ont00001754 "http://en.wiktionary.org/wiki/supervise" ;
                cco:ont00001760 <https://www.commoncoreontologies.org/ModalRelationOntology> .


###  https://www.commoncoreontologies.org/mro/ont00001944
mro:ont00001944 rdf:type owl:ObjectProperty ;
                rdfs:subPropertyOf mro:BFO_0000176 ,
                                   mro:ont00001810 ;
                rdfs:domain obo:BFO_0000141 ;
                rdfs:range obo:BFO_0000141 ;
                rdfs:comment "in the sense used here, spatial part of is elsewhere referred to as proper spatial part of"@en ;
                rdfs:label "spatial part of"@en ;
                <http://www.w3.org/2004/02/skos/core#definition> "x spatial_part_of y iff x, y, z, and q are instances of Immaterial Entity, such that for any z connected with x, z is also connected with y, and q is connected with y but not connected with x."@en ;
                cco:ont00001754 "Randell, D. A., Cui, Z. and Cohn, A. G.: 1992, \"A spatial logic based on regions and connection,\" Proc. 3rd Int. Conf. on Knowledge Representation and Reasoning, Morgan Kaufmann, San Mateo, pp. 165-176. Available at: https://www.dpi.inpe.br/gilberto/references/cohn_rcc.pdf"@en ;
                cco:ont00001760 <https://www.commoncoreontologies.org/ModalRelationOntology> .


###  https://www.commoncoreontologies.org/mro/ont00001945
mro:ont00001945 rdf:type owl:ObjectProperty ;
                rdfs:subPropertyOf mro:ont00001865 ;
                rdfs:label "is grandchild of"@en ;
                cco:ont00001760 <https://www.commoncoreontologies.org/ModalRelationOntology> .


###  https://www.commoncoreontologies.org/mro/ont00001946
mro:ont00001946 rdf:type owl:ObjectProperty ;
                rdfs:subPropertyOf mro:ont00001842 ;
                owl:inverseOf mro:ont00001985 ;
                rdfs:label "has father"@en ;
                cco:ont00001760 <https://www.commoncoreontologies.org/ModalRelationOntology> .


###  https://www.commoncoreontologies.org/mro/ont00001947
mro:ont00001947 rdf:type owl:ObjectProperty ;
                rdfs:subPropertyOf mro:ont00001809 ;
                rdfs:domain obo:BFO_0000019 ;
                rdfs:range obo:BFO_0000027 ;
                rdfs:label "quality of aggregate"@en ;
                <http://www.w3.org/2004/02/skos/core#definition> "x quality_of_aggregate y iff y is an instance of Object Aggregate and x is an instance of Quality, and x inheres_in_aggregate y."@en ;
                cco:ont00001760 <https://www.commoncoreontologies.org/ModalRelationOntology> .


###  https://www.commoncoreontologies.org/mro/ont00001948
mro:ont00001948 rdf:type owl:ObjectProperty ;
                rdfs:subPropertyOf mro:ont00001975 ;
                rdfs:label "is half sister of"@en ;
                cco:ont00001760 <https://www.commoncoreontologies.org/ModalRelationOntology> .


###  https://www.commoncoreontologies.org/mro/ont00001949
mro:ont00001949 rdf:type owl:ObjectProperty ;
                rdfs:subPropertyOf mro:BFO_0000057 ;
                rdfs:domain obo:BFO_0000015 ;
                rdfs:range obo:BFO_0000040 ;
                rdfs:label "has accessory"@en ;
                <http://www.w3.org/2004/02/skos/core#definition> "x has_accessory y iff x is an instance of Process and y is an instance of Agent, such that y assists another agent in the commission of x, and y was not located at the location of x when x occurred, and y was not an agent_in x."@en ;
                cco:ont00001754 "http://en.wikipedia.org/wiki/Accessory_(legal_term)" ;
                cco:ont00001760 <https://www.commoncoreontologies.org/ModalRelationOntology> .


###  https://www.commoncoreontologies.org/mro/ont00001950
mro:ont00001950 rdf:type owl:ObjectProperty ;
                rdfs:subPropertyOf mro:ont00001865 ;
                owl:inverseOf mro:ont00001950 ;
                rdf:type owl:SymmetricProperty ;
                rdfs:label "is third cousin of"@en ;
                cco:ont00001760 <https://www.commoncoreontologies.org/ModalRelationOntology> .


###  https://www.commoncoreontologies.org/mro/ont00001951
mro:ont00001951 rdf:type owl:ObjectProperty ;
                rdfs:subPropertyOf mro:mro00000001 ;
                rdfs:domain obo:BFO_0000023 ;
                rdfs:range obo:BFO_0000023 ;
                rdfs:label "has subordinate role"@en ;
                <http://www.w3.org/2004/02/skos/core#definition> "For all x,y,t: x has subordinate role y at t iff: x is an instance of Role at time t, and y is an instance of Role at time t, and there is some z such that x is realized by z and z is an instance of Process which creates, modifies, transfers, or eliminates some u such that u is a Process Regulation at time t, and u is addressed to the bearer of y."@en ;
                cco:ont00001760 <https://www.commoncoreontologies.org/ModalRelationOntology> .


###  https://www.commoncoreontologies.org/mro/ont00001952
mro:ont00001952 rdf:type owl:ObjectProperty ;
                rdfs:subPropertyOf mro:ont00001818 ;
                rdfs:label "is brother-in-law of"@en ;
                cco:ont00001760 <https://www.commoncoreontologies.org/ModalRelationOntology> .


###  https://www.commoncoreontologies.org/mro/ont00001953
mro:ont00001953 rdf:type owl:ObjectProperty ;
                rdfs:subPropertyOf mro:ont00001865 ;
                owl:inverseOf mro:ont00001995 ;
                rdfs:label "has parent"@en ;
                cco:ont00001760 <https://www.commoncoreontologies.org/ModalRelationOntology> .


###  https://www.commoncoreontologies.org/mro/ont00001954
mro:ont00001954 rdf:type owl:ObjectProperty ;
                rdfs:subPropertyOf mro:BFO_0000196 ;
                rdfs:domain cco:ont00001017 ;
                rdfs:range cco:ont00001379 ;
                rdfs:label "has capability"@en ;
                <http://www.w3.org/2004/02/skos/core#definition> "x has_capability y iff x is an instance of Agent and y is an instance of Agent Capability, such that x bearer of y."@en ;
                cco:ont00001760 <https://www.commoncoreontologies.org/ModalRelationOntology> .


###  https://www.commoncoreontologies.org/mro/ont00001955
mro:ont00001955 rdf:type owl:ObjectProperty ;
                rdfs:subPropertyOf mro:ont00001865 ;
                rdfs:label "is aunt of"@en ;
                cco:ont00001760 <https://www.commoncoreontologies.org/ModalRelationOntology> .


###  https://www.commoncoreontologies.org/mro/ont00001956
mro:ont00001956 rdf:type owl:ObjectProperty ;
                rdfs:subPropertyOf mro:ont00001836 ;
                rdfs:domain obo:BFO_0000027 ;
                rdfs:range obo:BFO_0000016 ;
                rdfs:label "aggregate has disposition"@en ;
                <http://www.w3.org/2004/02/skos/core#definition> "x aggregate_has_disposition y iff x is an instance of Object Aggregate and y is an instance of Disposition, such that x aggregate_bearer_of y."@en ;
                cco:ont00001760 <https://www.commoncoreontologies.org/ModalRelationOntology> .


###  https://www.commoncoreontologies.org/mro/ont00001957
mro:ont00001957 rdf:type owl:ObjectProperty ;
                rdfs:subPropertyOf mro:ont00001804 ;
                rdfs:label "is husband of"@en ;
                cco:ont00001760 <https://www.commoncoreontologies.org/ModalRelationOntology> .


###  https://www.commoncoreontologies.org/mro/ont00001958
mro:ont00001958 rdf:type owl:ObjectProperty ;
                rdfs:subPropertyOf mro:ont00001789 ;
                rdfs:label "has maternal aunt"@en ;
                cco:ont00001760 <https://www.commoncoreontologies.org/ModalRelationOntology> .


###  https://www.commoncoreontologies.org/mro/ont00001959
mro:ont00001959 rdf:type owl:ObjectProperty ;
                rdfs:subPropertyOf mro:mro00000001 ;
                owl:inverseOf mro:ont00001970 ;
                rdfs:domain obo:BFO_0000015 ;
                rdfs:range obo:BFO_0000015 ;
                rdfs:label "inhibits"@en ;
                <http://www.w3.org/2004/02/skos/core#definition> "x inhibits y iff x and y are non-identical Processes, d is a Decrease of Realizable Entity, and x is_cause_of d, and r is a Realizable Entity, and d has_participant r, and r realized_in y."@en ;
                cco:ont00001760 <https://www.commoncoreontologies.org/ModalRelationOntology> .


###  https://www.commoncoreontologies.org/mro/ont00001960
mro:ont00001960 rdf:type owl:ObjectProperty ;
                rdfs:subPropertyOf mro:ont00001840 ;
                rdfs:label "has maternal grandmother"@en ;
                cco:ont00001760 <https://www.commoncoreontologies.org/ModalRelationOntology> .


###  https://www.commoncoreontologies.org/mro/ont00001961
mro:ont00001961 rdf:type owl:ObjectProperty ;
                rdfs:subPropertyOf mro:BFO_0000084 ;
                rdfs:domain cco:ont00000120 ;
                rdfs:range cco:ont00000253 ;
                rdfs:label "is measurement unit of"@en ;
                <http://www.w3.org/2004/02/skos/core#definition> "x is_measurement_unit_of y iff y is an instance of Information Bearing Entity and x is an instance of Measurement Unit, such that x describes the magnitude of measured physical quantity mentioned in y."@en ;
                cco:ont00001760 <https://www.commoncoreontologies.org/ModalRelationOntology> .


###  https://www.commoncoreontologies.org/mro/ont00001962
mro:ont00001962 rdf:type owl:ObjectProperty ;
                rdfs:subPropertyOf mro:ont00001819 ;
                rdfs:label "process started by"@en ;
                <http://www.w3.org/2004/02/skos/core#definition> "x process_started_by y iff x and y are instances of processes, and x is caused_by y, and i is an instance of a temporal instant, and r is an instant of a temporal interval, and x has starting instance i, and y occurs on r, and r interval contains i."@en ;
                <http://www.w3.org/2004/02/skos/core#scopeNote> "A process x is started by another process y when y causes x while y is still occurring."@en ;
                cco:ont00001760 <https://www.commoncoreontologies.org/ModalRelationOntology> .


###  https://www.commoncoreontologies.org/mro/ont00001963
mro:ont00001963 rdf:type owl:ObjectProperty ;
                rdfs:subPropertyOf mro:ont00001904 ;
                rdfs:range cco:ont00001010 ;
                rdfs:label "is measured by ordinal"@en ;
                <http://www.w3.org/2004/02/skos/core#definition> "y is_measured_by_ordinal x iff x is an instance of Information Content Entity and y is an instance of Entity, such that x describes some attribute of y relative to a scale ordered by rank."@en ;
                cco:ont00001760 <https://www.commoncoreontologies.org/ModalRelationOntology> .


###  https://www.commoncoreontologies.org/mro/ont00001964
mro:ont00001964 rdf:type owl:ObjectProperty ;
                rdfs:subPropertyOf mro:ont00001904 ;
                rdfs:range cco:ont00001364 ;
                rdfs:label "is measured by interval"@en ;
                <http://www.w3.org/2004/02/skos/core#definition> "y is_measured_by_interval x iff x is an instance of Information Content Entity and y is an instance of Entity, such that x describes some attribute of y relative to a scale which has uniform intervals but has a zero value that does not correspond to an absence of the attribute being measured."@en ;
                cco:ont00001760 <https://www.commoncoreontologies.org/ModalRelationOntology> .


###  https://www.commoncoreontologies.org/mro/ont00001965
mro:ont00001965 rdf:type owl:ObjectProperty ;
                rdfs:subPropertyOf mro:ont00001904 ;
                owl:inverseOf mro:ont00001983 ;
                rdfs:range cco:ont00001022 ;
                rdfs:label "is measured by ratio"@en ;
                <http://www.w3.org/2004/02/skos/core#definition> "y is_measured_by_ratio x iff x is an instance of Information Content Entity and y is an instance of Entity, such that x describes some attribute of y relative to a scale having equal unit values and a zero value that corresponds to the absence of the attribute being measured."@en ;
                cco:ont00001760 <https://www.commoncoreontologies.org/ModalRelationOntology> .


###  https://www.commoncoreontologies.org/mro/ont00001966
mro:ont00001966 rdf:type owl:ObjectProperty ;
                rdfs:subPropertyOf mro:ont00001982 ;
                rdfs:domain cco:ont00001163 ;
                rdfs:comment "This object property, as well as all of its children are typified as functional properties. This means that for instances x, y, and z if x is a measurement of y and x is a measurement of z, then y = z."@en ;
                rdfs:label "is a measurement of"@en ;
                <http://www.w3.org/2004/02/skos/core#definition> "x is_a_measurement_of y iff x is an instance of Information Content Entity and y is an instance of Entity, such that x describes some attribute of y relative to some scale or classification scheme."@en ;
                <http://www.w3.org/2004/02/skos/core#scopeNote> "Given a stronger temporal interpretation, this property may be functional. For more info please refer to https://github.com/BFO-ontology/BFO-2020/tree/master/src/owl/temporal%20extensions."@en ;
                cco:ont00001760 <https://www.commoncoreontologies.org/ModalRelationOntology> .


###  https://www.commoncoreontologies.org/mro/ont00001967
mro:ont00001967 rdf:type owl:ObjectProperty ;
                rdfs:subPropertyOf mro:ont00001865 ;
                owl:inverseOf mro:ont00001969 ;
                rdfs:label "is nephew of"@en ;
                cco:ont00001760 <https://www.commoncoreontologies.org/ModalRelationOntology> .


###  https://www.commoncoreontologies.org/mro/ont00001968
mro:ont00001968 rdf:type owl:ObjectProperty ;
                rdfs:subPropertyOf mro:ont00001865 ;
                rdfs:label "is descendent of"@en ;
                cco:ont00001760 <https://www.commoncoreontologies.org/ModalRelationOntology> .


###  https://www.commoncoreontologies.org/mro/ont00001969
mro:ont00001969 rdf:type owl:ObjectProperty ;
                rdfs:subPropertyOf mro:ont00001865 ;
                rdfs:label "has nephew"@en ;
                cco:ont00001760 <https://www.commoncoreontologies.org/ModalRelationOntology> .


###  https://www.commoncoreontologies.org/mro/ont00001970
mro:ont00001970 rdf:type owl:ObjectProperty ;
                rdfs:subPropertyOf mro:mro00000001 ;
                rdfs:domain obo:BFO_0000015 ;
                rdfs:range obo:BFO_0000015 ;
                rdfs:label "inhibited by"@en ;
                <http://www.w3.org/2004/02/skos/core#definition> "y inhibited_by x iff x and y are non-identical Processes, d is a Decrease of Realizable Entity, and x is_cause_of d, and r is a Realizable Entity, and d has_participant r, and r realized_in y."@en ;
                cco:ont00001760 <https://www.commoncoreontologies.org/ModalRelationOntology> .


###  https://www.commoncoreontologies.org/mro/ont00001971
mro:ont00001971 rdf:type owl:ObjectProperty ;
                rdfs:subPropertyOf mro:mro00000001 ;
                rdfs:domain obo:BFO_0000038 ;
                rdfs:range obo:BFO_0000038 ;
                rdfs:label "interval contained by"@en ;
                <http://www.w3.org/2004/02/skos/core#definition> "A Temporal Interval INT1 is contained by some Temporal Interval INT2 iff there exist Temporal Instants inst1, inst2, inst3, and inst4 such that inst1 is the starting instant of INT1, inst2 is the ending instant of INT1, inst3 is the starting instant of INT2, inst4 is the ending instant of INT2, inst3 is before or identical to inst1, inst2 is before or identical to inst4, and it is not the case that both inst3 is identical to inst1 and inst2 is identical to inst4."@en ;
                cco:ont00001754 "J. F. Allen and J. A. G. M. Koomen. Planning using a temporal world model. In Proceedings of the 8th International Joint Conference on Artificial Intelligence (IJCAI-1983)  pages 741–747. Available at: https://www.ijcai.org/Proceedings/83-2/Papers/036.pdf"@en ;
                cco:ont00001760 <https://www.commoncoreontologies.org/ModalRelationOntology> .


###  https://www.commoncoreontologies.org/mro/ont00001972
mro:ont00001972 rdf:type owl:ObjectProperty ;
                rdfs:subPropertyOf mro:ont00001776 ;
                rdfs:label "has paternal grandfather"@en ;
                cco:ont00001760 <https://www.commoncoreontologies.org/ModalRelationOntology> .


###  https://www.commoncoreontologies.org/mro/ont00001973
mro:ont00001973 rdf:type owl:ObjectProperty ;
                rdfs:subPropertyOf mro:ont00001776 ;
                rdfs:label "has maternal grandfather"@en ;
                cco:ont00001760 <https://www.commoncoreontologies.org/ModalRelationOntology> .


###  https://www.commoncoreontologies.org/mro/ont00001974
mro:ont00001974 rdf:type owl:ObjectProperty ;
                rdfs:subPropertyOf mro:ont00001942 ;
                rdfs:domain cco:ont00001324 ;
                rdfs:range obo:BFO_0000015 ;
                rdfs:label "requires"@en ;
                <http://www.w3.org/2004/02/skos/core#definition> "x requires y at t iff: x is an instance of Process Regulation at time t, and y is an instance of Process at time t, and x prescribes that some y must occur."@en ;
                <http://www.w3.org/2004/02/skos/core#scopeNote> "Given a stronger temporal interpretation, this property may be asymmetric and irreflexive. For more info please refer to https://github.com/BFO-ontology/BFO-2020/tree/master/src/owl/temporal%20extensions."@en ;
                cco:ont00001760 <https://www.commoncoreontologies.org/ModalRelationOntology> .


###  https://www.commoncoreontologies.org/mro/ont00001975
mro:ont00001975 rdf:type owl:ObjectProperty ;
                rdfs:subPropertyOf mro:ont00001865 ;
                owl:inverseOf mro:ont00001975 ;
                rdf:type owl:SymmetricProperty ;
                rdfs:label "is half-sibling of"@en ;
                cco:ont00001760 <https://www.commoncoreontologies.org/ModalRelationOntology> .


###  https://www.commoncoreontologies.org/mro/ont00001976
mro:ont00001976 rdf:type owl:ObjectProperty ;
                rdfs:subPropertyOf mro:ont00001920 ;
                rdfs:domain cco:ont00000253 ;
                rdfs:range cco:ont00001175 ;
                rdfs:label "uses language"@en ;
                <http://www.w3.org/2004/02/skos/core#definition> "x uses_language y iff x is an instance of an Information Bearing Entity and y is an instance of a Language such that the literal value of x is a string that is encoded according to the syntax of y."@en ;
                cco:ont00001760 <https://www.commoncoreontologies.org/ModalRelationOntology> .


###  https://www.commoncoreontologies.org/mro/ont00001977
mro:ont00001977 rdf:type owl:ObjectProperty ;
                rdfs:subPropertyOf mro:mro00000001 ;
                rdfs:domain [ rdf:type owl:Class ;
                              owl:unionOf ( cco:ont00001017
                                            cco:ont00001180
                                            cco:ont00001262
                                          )
                            ] ;
                rdfs:range [ rdf:type owl:Class ;
                             owl:unionOf ( cco:ont00001017
                                           cco:ont00001180
                                           cco:ont00001262
                                         )
                           ] ;
                rdfs:label "has affiliate"@en ;
                <http://www.w3.org/2004/02/skos/core#definition> "x is_affiliated_with y iff x and y are instances of Agent, such that they have any kind of social or business relationship."@en ;
                cco:ont00001760 <https://www.commoncoreontologies.org/ModalRelationOntology> .


###  https://www.commoncoreontologies.org/mro/ont00001978
mro:ont00001978 rdf:type owl:ObjectProperty ;
                rdfs:subPropertyOf mro:BFO_0000056 ;
                rdfs:domain cco:ont00001017 ;
                rdfs:label "receives"@en ;
                <http://www.w3.org/2004/02/skos/core#definition> "x receives y iff x is an instance of Agent and y is an instance of Act Of Communication, such that x is the recipient and decoder of the InformationContentEntity intended for communication in y."@en ;
                cco:ont00001760 <https://www.commoncoreontologies.org/ModalRelationOntology> .


###  https://www.commoncoreontologies.org/mro/ont00001979
mro:ont00001979 rdf:type owl:ObjectProperty ;
                rdfs:subPropertyOf mro:ont00001996 ;
                rdfs:label "is step-sister of"@en ;
                cco:ont00001760 <https://www.commoncoreontologies.org/ModalRelationOntology> .


###  https://www.commoncoreontologies.org/mro/ont00001980
mro:ont00001980 rdf:type owl:ObjectProperty ;
                rdfs:subPropertyOf mro:ont00001808 ;
                owl:propertyChainAxiom ( mro:BFO_0000178
                                         mro:ont00001982
                                       ) ;
                rdfs:label "describes condition"@en ;
                <http://www.w3.org/2004/02/skos/core#definition> "p describes_condition c iff p is an instance of a Performance Specification, and p has part d, and d is an instance of a Descriptive Information Content Entity, and p prescribes an entity s, and d describes c, and c is an entity that is causally relevant to s existing as prescribed by p."@en ;
                cco:ont00001760 <https://www.commoncoreontologies.org/ModalRelationOntology> .


###  https://www.commoncoreontologies.org/mro/ont00001981
mro:ont00001981 rdf:type owl:ObjectProperty ;
                rdfs:subPropertyOf mro:ont00001850 ;
                rdfs:label "has grandson"@en ;
                cco:ont00001760 <https://www.commoncoreontologies.org/ModalRelationOntology> .


###  https://www.commoncoreontologies.org/mro/ont00001982
mro:ont00001982 rdf:type owl:ObjectProperty ;
                rdfs:subPropertyOf mro:ont00001808 ;
                rdfs:domain cco:ont00000853 ;
                rdfs:comment "It is possible that this relation should be a functional property, that is for all x, y, z if x describes y and x describes z then y = z. For example, if a financial report x describes the quarterly results of a company y and that same financial report describes the quarterly results of a company z, then it should be inferred that companies y and z are the same. We refrained from classifying the relation as a functional property on the concern that descriptions are multifaceted and so consequently it may be that the same report would contain descriptions of multiple entities."@en ;
                rdfs:label "describes"@en ;
                <http://www.w3.org/2004/02/skos/core#definition> "x describes y iff x is an instance of Information Content Entity, and y is an instance of Entity, such that x is about the characteristics by which y can be recognized or visualized."@en ;
                <http://www.w3.org/2004/02/skos/core#example> "the content of a newspaper article describes some current event" ,
                                                              "the content of a visitor's log describes some facility visit" ,
                                                              "the content of an accident report describes some accident" ;
                cco:ont00001760 <https://www.commoncoreontologies.org/ModalRelationOntology> .


###  https://www.commoncoreontologies.org/mro/ont00001983
mro:ont00001983 rdf:type owl:ObjectProperty ;
                rdfs:subPropertyOf mro:ont00001966 ;
                rdfs:domain cco:ont00001022 ;
                rdfs:label "is a ratio measurement of"@en ;
                <http://www.w3.org/2004/02/skos/core#definition> "x is_a_ratio_measurement_of y iff x is an instance of Information Content Entity and y is an instance of Entity, such that x describes some attribute of y relative to a scale having equal unit values and a zero value that corresponds to the absence of the attribute being measured."@en ;
                cco:ont00001760 <https://www.commoncoreontologies.org/ModalRelationOntology> .


###  https://www.commoncoreontologies.org/mro/ont00001984
mro:ont00001984 rdf:type owl:ObjectProperty ;
                rdfs:subPropertyOf mro:mro00000001 ;
                rdfs:domain cco:ont00001017 ;
                rdfs:range obo:BFO_0000015 ;
                <http://purl.org/dc/terms/created> "2022-12-30T21:32:27-05:00"^^xsd:dateTime ;
                <http://purl.org/dc/terms/creator> "https://cubrc.org"^^xsd:anyURI ;
                rdfs:label "has interest in"@en ;
                <http://www.w3.org/2004/02/skos/core#definition> "A relation between an entity and some process where the entity has an interest in that process."@en ;
                <http://www.w3.org/2004/02/skos/core#editorialNote> "This term is meant to be weakly normative. The only sense in which the process is of positive normative value is that it's prescribed by the entity, or historically of evolutionary benefit to the entity's ancestors, or facilitates a process the entity has an interest in for the prior two reasons. The process an entity has an interest could in many or all ways be harmful to the entity."@en ;
                <http://www.w3.org/2004/02/skos/core#prefLabel> "has interest in"@en ;
                <http://www.w3.org/2004/02/skos/core#scopeNote> "There are four conditions in which an entity has an interest in some process. 1) Biological Condition: If a part (including improper part) of an organism has a function, then that organism has an interest in the realization of that function. 2) Artifactual Condition: If a part (including improper part) of an artifact has a function, then some agent or group of agents, at some time, has an interest in the realization of that function. 3) Prescription Condition: If an agent or group of agents has a plan, then it has an interest in the realization of all the processes and process-combinations prescribed by that plan. 4) Facilitation Condition: If (a) x has an interest in the realization of a disposition y, and (b) the realization of a disposition z facilitates the realization of disposition y, then (c) x has an interest in the realization of disposition z, and by 'facilitates' we mean that the occurrence of a process w, which realizes realization of z is either (1) required for y, to realize or (2) would contribute positively to the grade of, y's realization."@en ;
                cco:ont00001760 <https://www.commoncoreontologies.org/ModalRelationOntology> .


###  https://www.commoncoreontologies.org/mro/ont00001985
mro:ont00001985 rdf:type owl:ObjectProperty ;
                rdfs:subPropertyOf mro:ont00001995 ;
                rdfs:label "is father of"@en ;
                cco:ont00001760 <https://www.commoncoreontologies.org/ModalRelationOntology> .


###  https://www.commoncoreontologies.org/mro/ont00001986
mro:ont00001986 rdf:type owl:ObjectProperty ;
                rdfs:subPropertyOf mro:BFO_0000057 ;
                rdfs:domain obo:BFO_0000015 ;
                rdfs:range obo:BFO_0000002 ;
                rdfs:label "has output"@en ;
                <http://www.w3.org/2004/02/skos/core#definition> "y has_output x iff x is an instance of Continuant and y is an instance of Process, such that the presence of x at the end of y is a necessary condition for the completion of y."@en ;
                cco:ont00001754 "https://en.wikipedia.org/w/index.php?title=IPO_model&oldid=1024398398"^^xsd:anyURI ;
                cco:ont00001760 <https://www.commoncoreontologies.org/ModalRelationOntology> .


###  https://www.commoncoreontologies.org/mro/ont00001987
mro:ont00001987 rdf:type owl:ObjectProperty ;
                rdfs:subPropertyOf mro:ont00001995 ;
                rdfs:label "has daughter"@en ;
                cco:ont00001760 <https://www.commoncoreontologies.org/ModalRelationOntology> .


###  https://www.commoncoreontologies.org/mro/ont00001988
mro:ont00001988 rdf:type owl:ObjectProperty ;
                rdfs:subPropertyOf mro:ont00001865 ;
                rdfs:label "is uncle of"@en ;
                cco:ont00001760 <https://www.commoncoreontologies.org/ModalRelationOntology> .


###  https://www.commoncoreontologies.org/mro/ont00001989
mro:ont00001989 rdf:type owl:ObjectProperty ;
                rdfs:subPropertyOf mro:ont00001855 ;
                rdfs:domain obo:BFO_0000141 ;
                rdfs:range obo:BFO_0000141 ;
                rdfs:label "has nontangential part"@en ;
                <http://www.w3.org/2004/02/skos/core#definition> "x has_nontangential_part y iff x and y are instances of Immaterial Entity, and x has_spatial_part y, such that there does not exist another instance of an Immaterial Entity which externally connects with both x and y."@en ;
                <http://www.w3.org/2004/02/skos/core#scopeNote> "Given a stronger temporal interpretation, this property may be transitive. For more info please refer to https://github.com/BFO-ontology/BFO-2020/tree/master/src/owl/temporal%20extensions."@en ;
                cco:ont00001754 "Randell, D. A., Cui, Z. and Cohn, A. G.: 1992, \"A spatial logic based on regions and connection,\" Proc. 3rd Int. Conf. on Knowledge Representation and Reasoning, Morgan Kaufmann, San Mateo, pp. 165-176. Available at: https://www.dpi.inpe.br/gilberto/references/cohn_rcc.pdf"@en ;
                cco:ont00001760 <https://www.commoncoreontologies.org/ModalRelationOntology> .


###  https://www.commoncoreontologies.org/mro/ont00001990
mro:ont00001990 rdf:type owl:ObjectProperty ;
                rdfs:subPropertyOf mro:mro00000001 ;
                rdf:type owl:TransitiveProperty ;
                rdfs:domain obo:BFO_0000148 ;
                rdfs:range obo:BFO_0000148 ;
                rdfs:label "instant is before"@en ;
                <http://www.w3.org/2004/02/skos/core#definition> "A temporal instant t1 (a instance of a zero-dimensional temporal region) is before another temporal instant t2 iff there exists some instance of a temporal interval ti1 such that t1 is the starting instant of ti1 and t2 is the ending instant of ti1."@en ;
                <http://www.w3.org/2004/02/skos/core#scopeNote> "'instant is before' is a primitive relationship. Informally, a temporal instant t1 is before some temporal instant t2 if and only if t1 precedes t2."@en ;
                cco:ont00001754 "J. F. Allen and J. A. G. M. Koomen. Planning using a temporal world model. In Proceedings of the 8th International Joint Conference on Artificial Intelligence (IJCAI-1983)  pages 741–747. Available at: https://www.ijcai.org/Proceedings/83-2/Papers/036.pdf"@en ;
                cco:ont00001760 <https://www.commoncoreontologies.org/ModalRelationOntology> .


###  https://www.commoncoreontologies.org/mro/ont00001991
mro:ont00001991 rdf:type owl:ObjectProperty ;
                rdfs:subPropertyOf mro:mro00000001 ;
                rdfs:domain obo:BFO_0000030 ;
                rdfs:range obo:BFO_0000030 ;
                rdfs:label "is made of"@en ;
                <http://www.w3.org/2004/02/skos/core#definition> "An object o is made of an object m when m is the material that o consists of and that material does not undergo a change of kind during the creation of o"@en ;
                cco:ont00001760 <https://www.commoncoreontologies.org/ModalRelationOntology> .


###  https://www.commoncoreontologies.org/mro/ont00001992
mro:ont00001992 rdf:type owl:ObjectProperty ;
                rdfs:subPropertyOf mro:mro00000001 ;
                rdfs:domain obo:BFO_0000023 ;
                rdfs:range cco:ont00001180 ;
                rdfs:label "has organizational context"@en ;
                <http://www.w3.org/2004/02/skos/core#definition> "x has_organizational_context y iff y is an instance of an Organization and x is an instance of a Role and z is an instance of a Person, such that z's affiliation with y is a prerequisite for z bearing x or y ascribes x to the bearer of x."@en ;
                cco:ont00001760 <https://www.commoncoreontologies.org/ModalRelationOntology> .


###  https://www.commoncoreontologies.org/mro/ont00001993
mro:ont00001993 rdf:type owl:ObjectProperty ;
                rdfs:subPropertyOf mro:BFO_0000056 ;
                rdfs:domain cco:ont00001017 ;
                rdfs:label "sends"@en ;
                <http://www.w3.org/2004/02/skos/core#definition> "x sends y iff x is an instance of Agent and y is an instance of Act Of Communication, such that x is the initiator and encoder of the InformationContentEntity intended for communication in y."@en ;
                cco:ont00001760 <https://www.commoncoreontologies.org/ModalRelationOntology> .


###  https://www.commoncoreontologies.org/mro/ont00001994
mro:ont00001994 rdf:type owl:ObjectProperty ;
                rdfs:subPropertyOf mro:ont00001955 ;
                rdfs:label "is paternal aunt of"@en ;
                cco:ont00001760 <https://www.commoncoreontologies.org/ModalRelationOntology> .


###  https://www.commoncoreontologies.org/mro/ont00001995
mro:ont00001995 rdf:type owl:ObjectProperty ;
                rdfs:subPropertyOf mro:ont00001865 ;
                rdfs:domain cco:ont00001262 ;
                rdfs:range cco:ont00001262 ;
                rdfs:label "is parent of"@en ;
                cco:ont00001760 <https://www.commoncoreontologies.org/ModalRelationOntology> .


###  https://www.commoncoreontologies.org/mro/ont00001996
mro:ont00001996 rdf:type owl:ObjectProperty ;
                rdfs:subPropertyOf mro:ont00001865 ;
                owl:inverseOf mro:ont00001996 ;
                rdfs:label "is step-sibling of"@en ;
                <http://www.w3.org/2004/02/skos/core#scopeNote> "Given a stronger temporal interpretation, this property may be symmetric. For more info please refer to https://github.com/BFO-ontology/BFO-2020/tree/master/src/owl/temporal%20extensions."@en ;
                cco:ont00001760 <https://www.commoncoreontologies.org/ModalRelationOntology> .


###  https://www.commoncoreontologies.org/mro/ont00001997
mro:ont00001997 rdf:type owl:ObjectProperty ;
                rdfs:subPropertyOf mro:BFO_0000084 ;
                rdfs:domain cco:ont00000398 ;
                rdfs:range cco:ont00000253 ;
                rdfs:label "is reference system of"@en ;
                <http://www.w3.org/2004/02/skos/core#definition> "x is_reference_system_of y iff y is an instance of Information Bearing Entity and x is an instance of Reference System, such that x describes the set of standards mentioned in y."@en ;
                cco:ont00001760 <https://www.commoncoreontologies.org/ModalRelationOntology> .


###  https://www.commoncoreontologies.org/mro/ont00001998
mro:ont00001998 rdf:type owl:ObjectProperty ;
                rdfs:subPropertyOf mro:ont00001920 ;
                rdfs:domain obo:BFO_0000015 ;
                rdfs:range cco:ont00001324 ;
                rdfs:label "is permitted by"@en ;
                <http://www.w3.org/2004/02/skos/core#definition> "y is_permitted_by x at t iff: x is an instance of Process Regulation at time t, and y is an instance of Process at time t, and x prescribes that y may occur."@en ;
                <http://www.w3.org/2004/02/skos/core#scopeNote> "Given a stronger temporal interpretation, this property may be asymmetric and irreflexive. For more info please refer to https://github.com/BFO-ontology/BFO-2020/tree/master/src/owl/temporal%20extensions."@en ;
                cco:ont00001760 <https://www.commoncoreontologies.org/ModalRelationOntology> .


#################################################################
#    Data properties
#################################################################

###  https://www.commoncoreontologies.org/mro/asWKT
mro:asWKT rdf:type owl:DatatypeProperty ;
          rdfs:comment "ISO 19162:2015"@en ;
          rdfs:label "as WKT"@en ;
          <http://www.w3.org/2004/02/skos/core#definition> "A Data Property that has as its range a string formated according to the Well-known text standardization for geometric objects."@en ;
          <http://www.w3.org/2004/02/skos/core#example> "Polygon ((10 10, 10 20, 20 20, 20 15, 10 10))" ;
          cco:ont00001760 <https://www.commoncoreontologies.org/ModalRelationOntology> .


###  https://www.commoncoreontologies.org/mro/ont00001763
mro:ont00001763 rdf:type owl:DatatypeProperty ;
                rdfs:comment "Altitude values typically use kilometers as the Unit of Measurement."@en ;
                rdfs:label "has altitude value"@en ;
                <http://www.w3.org/2004/02/skos/core#scopeNote> "This data property can be used along with has_latitude_value and has_longitude_value to connect three-dimensional spatial data to a single Information Bearing Entity to specify the location of an entity in a Geospatial Region."@en ;
                cco:ont00001760 <https://www.commoncoreontologies.org/ModalRelationOntology> .


###  https://www.commoncoreontologies.org/mro/ont00001764
mro:ont00001764 rdf:type owl:DatatypeProperty ;
                rdfs:range xsd:decimal ;
                rdfs:label "has longitude value"@en ;
                <http://www.w3.org/2004/02/skos/core#definition> "A Data Property that has as its range the longitude value from some Geospatial Location coordinates set expressed in decimal degrees."@en ;
                cco:ont00001760 <https://www.commoncoreontologies.org/ModalRelationOntology> .


###  https://www.commoncoreontologies.org/mro/ont00001765
mro:ont00001765 rdf:type owl:DatatypeProperty ;
                rdfs:domain cco:ont00000253 ;
                rdfs:label "has text value"@en ;
                <http://www.w3.org/2004/02/skos/core#definition> "A data property that has as its range a string value."@en ;
                cco:ont00001760 <https://www.commoncoreontologies.org/ModalRelationOntology> .


###  https://www.commoncoreontologies.org/mro/ont00001766
mro:ont00001766 rdf:type owl:DatatypeProperty ;
                rdfs:range xsd:decimal ;
                rdfs:label "has latitude value"@en ;
                <http://www.w3.org/2004/02/skos/core#definition> "A Data Property that has as its range the latitude value from some Geospatial Location coordinates set expressed in decimal degrees."@en ;
                cco:ont00001760 <https://www.commoncoreontologies.org/ModalRelationOntology> .


###  https://www.commoncoreontologies.org/mro/ont00001767
mro:ont00001767 rdf:type owl:DatatypeProperty ;
                rdfs:domain cco:ont00000253 ;
                rdfs:range xsd:dateTime ;
                rdfs:label "has datetime value"@en ;
                <http://www.w3.org/2004/02/skos/core#definition> "A data property that has as its value a datetime value."@en ;
                cco:ont00001760 <https://www.commoncoreontologies.org/ModalRelationOntology> .


###  https://www.commoncoreontologies.org/mro/ont00001768
mro:ont00001768 rdf:type owl:DatatypeProperty ;
                rdfs:domain cco:ont00000253 ;
                rdfs:range xsd:anyURI ;
                rdfs:label "has URI value"@en ;
                <http://www.w3.org/2004/02/skos/core#definition> "A data property that has as its range a URI value."@en ;
                cco:ont00001760 <https://www.commoncoreontologies.org/ModalRelationOntology> .


###  https://www.commoncoreontologies.org/mro/ont00001769
mro:ont00001769 rdf:type owl:DatatypeProperty ;
                rdfs:domain cco:ont00000253 ;
                rdfs:range xsd:decimal ;
                rdfs:label "has decimal value"@en ;
                <http://www.w3.org/2004/02/skos/core#definition> "A data property that has as its range a decimal value."@en ;
                cco:ont00001760 <https://www.commoncoreontologies.org/ModalRelationOntology> .


###  https://www.commoncoreontologies.org/mro/ont00001770
mro:ont00001770 rdf:type owl:DatatypeProperty ;
                rdfs:domain cco:ont00000253 ;
                rdfs:range xsd:double ;
                rdfs:label "has double value"@en ;
                <http://www.w3.org/2004/02/skos/core#definition> "A data property that has as its range a double value."@en ;
                cco:ont00001760 <https://www.commoncoreontologies.org/ModalRelationOntology> .


###  https://www.commoncoreontologies.org/mro/ont00001771
mro:ont00001771 rdf:type owl:DatatypeProperty ;
                rdfs:domain cco:ont00000253 ;
                rdfs:label "has date value"@en ;
                <http://www.w3.org/2004/02/skos/core#definition> "A data property that has as its range a date value."@en ;
                cco:ont00001760 <https://www.commoncoreontologies.org/ModalRelationOntology> .


###  https://www.commoncoreontologies.org/mro/ont00001772
mro:ont00001772 rdf:type owl:DatatypeProperty ;
                rdfs:domain cco:ont00000253 ;
                rdfs:range xsd:boolean ;
                rdfs:label "has boolean value"@en ;
                <http://www.w3.org/2004/02/skos/core#definition> "A data property that has as its range a boolean value."@en ;
                cco:ont00001760 <https://www.commoncoreontologies.org/ModalRelationOntology> .


###  https://www.commoncoreontologies.org/mro/ont00001773
mro:ont00001773 rdf:type owl:DatatypeProperty ;
                rdfs:domain cco:ont00000253 ;
                rdfs:range xsd:integer ;
                rdfs:label "has integer value"@en ;
                <http://www.w3.org/2004/02/skos/core#definition> "A data property that has as its range an integer value."@en ;
                cco:ont00001760 <https://www.commoncoreontologies.org/ModalRelationOntology> .


#################################################################
#    Classes
#################################################################

###  http://purl.obolibrary.org/obo/BFO_0000001
obo:BFO_0000001 rdf:type owl:Class .


###  http://purl.obolibrary.org/obo/BFO_0000002
obo:BFO_0000002 rdf:type owl:Class .


###  http://purl.obolibrary.org/obo/BFO_0000003
obo:BFO_0000003 rdf:type owl:Class .


###  http://purl.obolibrary.org/obo/BFO_0000004
obo:BFO_0000004 rdf:type owl:Class .


###  http://purl.obolibrary.org/obo/BFO_0000006
obo:BFO_0000006 rdf:type owl:Class .


###  http://purl.obolibrary.org/obo/BFO_0000008
obo:BFO_0000008 rdf:type owl:Class .


###  http://purl.obolibrary.org/obo/BFO_0000011
obo:BFO_0000011 rdf:type owl:Class .


###  http://purl.obolibrary.org/obo/BFO_0000015
obo:BFO_0000015 rdf:type owl:Class .


###  http://purl.obolibrary.org/obo/BFO_0000016
obo:BFO_0000016 rdf:type owl:Class .


###  http://purl.obolibrary.org/obo/BFO_0000017
obo:BFO_0000017 rdf:type owl:Class .


###  http://purl.obolibrary.org/obo/BFO_0000019
obo:BFO_0000019 rdf:type owl:Class .


###  http://purl.obolibrary.org/obo/BFO_0000020
obo:BFO_0000020 rdf:type owl:Class .


###  http://purl.obolibrary.org/obo/BFO_0000023
obo:BFO_0000023 rdf:type owl:Class .


###  http://purl.obolibrary.org/obo/BFO_0000027
obo:BFO_0000027 rdf:type owl:Class .


###  http://purl.obolibrary.org/obo/BFO_0000029
obo:BFO_0000029 rdf:type owl:Class .


###  http://purl.obolibrary.org/obo/BFO_0000030
obo:BFO_0000030 rdf:type owl:Class .


###  http://purl.obolibrary.org/obo/BFO_0000031
obo:BFO_0000031 rdf:type owl:Class .


###  http://purl.obolibrary.org/obo/BFO_0000035
obo:BFO_0000035 rdf:type owl:Class .


###  http://purl.obolibrary.org/obo/BFO_0000038
obo:BFO_0000038 rdf:type owl:Class .


###  http://purl.obolibrary.org/obo/BFO_0000040
obo:BFO_0000040 rdf:type owl:Class .


###  http://purl.obolibrary.org/obo/BFO_0000141
obo:BFO_0000141 rdf:type owl:Class .


###  http://purl.obolibrary.org/obo/BFO_0000148
obo:BFO_0000148 rdf:type owl:Class .


###  http://purl.obolibrary.org/obo/BFO_0000182
obo:BFO_0000182 rdf:type owl:Class .


###  http://purl.obolibrary.org/obo/BFO_0000203
obo:BFO_0000203 rdf:type owl:Class .


###  https://www.commoncoreontologies.org/ont00000120
cco:ont00000120 rdf:type owl:Class .


###  https://www.commoncoreontologies.org/ont00000253
cco:ont00000253 rdf:type owl:Class .


###  https://www.commoncoreontologies.org/ont00000293
cco:ont00000293 rdf:type owl:Class .


###  https://www.commoncoreontologies.org/ont00000300
cco:ont00000300 rdf:type owl:Class .


###  https://www.commoncoreontologies.org/ont00000398
cco:ont00000398 rdf:type owl:Class .


###  https://www.commoncoreontologies.org/ont00000469
cco:ont00000469 rdf:type owl:Class .


###  https://www.commoncoreontologies.org/ont00000686
cco:ont00000686 rdf:type owl:Class .


###  https://www.commoncoreontologies.org/ont00000829
cco:ont00000829 rdf:type owl:Class .


###  https://www.commoncoreontologies.org/ont00000853
cco:ont00000853 rdf:type owl:Class .


###  https://www.commoncoreontologies.org/ont00000958
cco:ont00000958 rdf:type owl:Class .


###  https://www.commoncoreontologies.org/ont00000965
cco:ont00000965 rdf:type owl:Class .


###  https://www.commoncoreontologies.org/ont00001010
cco:ont00001010 rdf:type owl:Class .


###  https://www.commoncoreontologies.org/ont00001017
cco:ont00001017 rdf:type owl:Class .


###  https://www.commoncoreontologies.org/ont00001022
cco:ont00001022 rdf:type owl:Class .


###  https://www.commoncoreontologies.org/ont00001069
cco:ont00001069 rdf:type owl:Class .


###  https://www.commoncoreontologies.org/ont00001163
cco:ont00001163 rdf:type owl:Class .


###  https://www.commoncoreontologies.org/ont00001175
cco:ont00001175 rdf:type owl:Class .


###  https://www.commoncoreontologies.org/ont00001180
cco:ont00001180 rdf:type owl:Class .


###  https://www.commoncoreontologies.org/ont00001203
cco:ont00001203 rdf:type owl:Class .


###  https://www.commoncoreontologies.org/ont00001262
cco:ont00001262 rdf:type owl:Class .


###  https://www.commoncoreontologies.org/ont00001324
cco:ont00001324 rdf:type owl:Class .


###  https://www.commoncoreontologies.org/ont00001364
cco:ont00001364 rdf:type owl:Class .


###  https://www.commoncoreontologies.org/ont00001379
cco:ont00001379 rdf:type owl:Class .


###  Generated by the OWL API (version 4.5.26.2023-07-17T20:34:13Z) https://github.com/owlcs/owlapi
